<?xml version="1.0"?>
<rdf:RDF xmlns="http://www.semanticweb.org/smarotta/ontologies/2022/4/untitled-ontology-5#"
     xml:base="http://www.semanticweb.org/smarotta/ontologies/2022/4/untitled-ontology-5"
     xmlns:owl="http://www.w3.org/2002/07/owl#"
     xmlns:rdf="http://www.w3.org/1999/02/22-rdf-syntax-ns#"
     xmlns:xml="http://www.w3.org/XML/1998/namespace"
     xmlns:xsd="http://www.w3.org/2001/XMLSchema#"
     xmlns:rdfs="http://www.w3.org/2000/01/rdf-schema#"
     xmlns:skos="http://www.w3.org/2004/02/skos/core#"
     xmlns:silvanusOntology="http://www.semanticweb.org/smarotta/ontologies/2022/4/silvanusOntology#"
     xmlns:ExtendedRelationOntology="http://www.ontologylibrary.mil/CommonCore/Upper/ExtendedRelationOntology#">
    <owl:Ontology rdf:about="http://www.semanticweb.org/smarotta/ontologies/2022/4/silvanusOntology"/>
    


    <!-- 
    ///////////////////////////////////////////////////////////////////////////////////////
    //
    // Annotation properties
    //
    ///////////////////////////////////////////////////////////////////////////////////////
     -->

    


    <!-- http://www.ontologylibrary.mil/CommonCore/Upper/ExtendedRelationOntology#definition -->

    <owl:AnnotationProperty rdf:about="http://www.ontologylibrary.mil/CommonCore/Upper/ExtendedRelationOntology#definition"/>
    


    <!-- http://www.semanticweb.org/smarotta/ontologies/2022/4/silvanusOntology#input -->

    <owl:AnnotationProperty rdf:about="http://www.semanticweb.org/smarotta/ontologies/2022/4/silvanusOntology#input">
        <rdfs:subPropertyOf rdf:resource="http://www.w3.org/2000/01/rdf-schema#comment"/>
    </owl:AnnotationProperty>
    


    <!-- http://www.semanticweb.org/smarotta/ontologies/2022/4/silvanusOntology#output -->

    <owl:AnnotationProperty rdf:about="http://www.semanticweb.org/smarotta/ontologies/2022/4/silvanusOntology#output">
        <rdfs:subPropertyOf rdf:resource="http://www.w3.org/2000/01/rdf-schema#comment"/>
    </owl:AnnotationProperty>
    


    <!-- http://www.semanticweb.org/smarotta/ontologies/2022/4/silvanusOntology#source -->

    <owl:AnnotationProperty rdf:about="http://www.semanticweb.org/smarotta/ontologies/2022/4/silvanusOntology#source"/>
    


    <!-- http://www.w3.org/2004/02/skos/core#definition -->

    <owl:AnnotationProperty rdf:about="http://www.w3.org/2004/02/skos/core#definition"/>
    


    <!-- 
    ///////////////////////////////////////////////////////////////////////////////////////
    //
    // Object Properties
    //
    ///////////////////////////////////////////////////////////////////////////////////////
     -->

    


    <!-- http://www.semanticweb.org/smarotta/ontologies/2022/4/silvanusOntology#affects -->

    <owl:ObjectProperty rdf:about="http://www.semanticweb.org/smarotta/ontologies/2022/4/silvanusOntology#affects">
        <rdfs:subPropertyOf rdf:resource="http://www.w3.org/2002/07/owl#topObjectProperty"/>
        <rdfs:domain rdf:resource="http://www.semanticweb.org/smarotta/ontologies/2022/4/silvanusOntology#Impact"/>
        <rdfs:range rdf:resource="http://www.semanticweb.org/smarotta/ontologies/2022/4/silvanusOntology#Vulnerable_object"/>
    </owl:ObjectProperty>
    


    <!-- http://www.semanticweb.org/smarotta/ontologies/2022/4/silvanusOntology#affects_fire_characteristic -->

    <owl:ObjectProperty rdf:about="http://www.semanticweb.org/smarotta/ontologies/2022/4/silvanusOntology#affects_fire_characteristic">
        <rdfs:subPropertyOf rdf:resource="http://www.semanticweb.org/smarotta/ontologies/2022/4/silvanusOntology#affects"/>
        <rdfs:domain rdf:resource="http://www.semanticweb.org/smarotta/ontologies/2022/4/silvanusOntology#Climate_parameter"/>
        <rdfs:range rdf:resource="http://www.semanticweb.org/smarotta/ontologies/2022/4/silvanusOntology#Area_burned"/>
        <rdfs:range rdf:resource="http://www.semanticweb.org/smarotta/ontologies/2022/4/silvanusOntology#Fire_intensity"/>
        <rdfs:range rdf:resource="http://www.semanticweb.org/smarotta/ontologies/2022/4/silvanusOntology#Fire_severity"/>
        <rdfs:range rdf:resource="http://www.semanticweb.org/smarotta/ontologies/2022/4/silvanusOntology#Fire_speed"/>
        <rdfs:range rdf:resource="http://www.semanticweb.org/smarotta/ontologies/2022/4/silvanusOntology#Fire_spread_direction"/>
        <rdfs:range rdf:resource="http://www.semanticweb.org/smarotta/ontologies/2022/4/silvanusOntology#Flame_height"/>
    </owl:ObjectProperty>
    


    <!-- http://www.semanticweb.org/smarotta/ontologies/2022/4/silvanusOntology#causes_fire -->

    <owl:ObjectProperty rdf:about="http://www.semanticweb.org/smarotta/ontologies/2022/4/silvanusOntology#causes_fire">
        <rdfs:subPropertyOf rdf:resource="http://www.w3.org/2002/07/owl#topObjectProperty"/>
        <owl:inverseOf rdf:resource="http://www.semanticweb.org/smarotta/ontologies/2022/4/silvanusOntology#fire_caused_by"/>
    </owl:ObjectProperty>
    


    <!-- http://www.semanticweb.org/smarotta/ontologies/2022/4/silvanusOntology#causes_incident -->

    <owl:ObjectProperty rdf:about="http://www.semanticweb.org/smarotta/ontologies/2022/4/silvanusOntology#causes_incident">
        <rdfs:subPropertyOf rdf:resource="http://www.w3.org/2002/07/owl#topObjectProperty"/>
        <rdfs:domain rdf:resource="http://www.semanticweb.org/smarotta/ontologies/2022/4/silvanusOntology#Fire"/>
        <rdfs:range rdf:resource="http://www.semanticweb.org/smarotta/ontologies/2022/4/silvanusOntology#Incident"/>
    </owl:ObjectProperty>
    


    <!-- http://www.semanticweb.org/smarotta/ontologies/2022/4/silvanusOntology#contains -->

    <owl:ObjectProperty rdf:about="http://www.semanticweb.org/smarotta/ontologies/2022/4/silvanusOntology#contains">
        <rdfs:domain rdf:resource="http://www.semanticweb.org/smarotta/ontologies/2022/4/silvanusOntology#Dataset"/>
        <rdfs:range rdf:resource="http://www.semanticweb.org/smarotta/ontologies/2022/4/silvanusOntology#Detection"/>
    </owl:ObjectProperty>
    


    <!-- http://www.semanticweb.org/smarotta/ontologies/2022/4/silvanusOntology#detects -->

    <owl:ObjectProperty rdf:about="http://www.semanticweb.org/smarotta/ontologies/2022/4/silvanusOntology#detects">
        <rdfs:subPropertyOf rdf:resource="http://www.w3.org/2002/07/owl#topObjectProperty"/>
        <rdfs:domain rdf:resource="http://www.semanticweb.org/smarotta/ontologies/2022/4/silvanusOntology#Detection"/>
        <rdfs:range rdf:resource="http://www.semanticweb.org/smarotta/ontologies/2022/4/silvanusOntology#Incident"/>
        <rdfs:range rdf:resource="http://www.semanticweb.org/smarotta/ontologies/2022/4/silvanusOntology#Vulnerable_object"/>
    </owl:ObjectProperty>
    


    <!-- http://www.semanticweb.org/smarotta/ontologies/2022/4/silvanusOntology#fire_caused_by -->

    <owl:ObjectProperty rdf:about="http://www.semanticweb.org/smarotta/ontologies/2022/4/silvanusOntology#fire_caused_by"/>
    


    <!-- http://www.semanticweb.org/smarotta/ontologies/2022/4/silvanusOntology#hasConstructionMaterial -->

    <owl:ObjectProperty rdf:about="http://www.semanticweb.org/smarotta/ontologies/2022/4/silvanusOntology#hasConstructionMaterial">
        <rdfs:domain rdf:resource="http://www.semanticweb.org/smarotta/ontologies/2022/4/silvanusOntology#Asset"/>
    </owl:ObjectProperty>
    


    <!-- http://www.semanticweb.org/smarotta/ontologies/2022/4/silvanusOntology#has_assigned_responder -->

    <owl:ObjectProperty rdf:about="http://www.semanticweb.org/smarotta/ontologies/2022/4/silvanusOntology#has_assigned_responder">
        <rdfs:subPropertyOf rdf:resource="http://www.w3.org/2002/07/owl#topObjectProperty"/>
        <rdfs:domain rdf:resource="http://www.semanticweb.org/smarotta/ontologies/2022/4/silvanusOntology#Mission"/>
        <rdfs:range rdf:resource="http://www.semanticweb.org/smarotta/ontologies/2022/4/silvanusOntology#Responder"/>
    </owl:ObjectProperty>
    


    <!-- http://www.semanticweb.org/smarotta/ontologies/2022/4/silvanusOntology#has_biodiversity_index -->

    <owl:ObjectProperty rdf:about="http://www.semanticweb.org/smarotta/ontologies/2022/4/silvanusOntology#has_biodiversity_index">
        <rdfs:domain rdf:resource="http://www.semanticweb.org/smarotta/ontologies/2022/4/silvanusOntology#Area_burned"/>
        <rdfs:domain rdf:resource="http://www.semanticweb.org/smarotta/ontologies/2022/4/silvanusOntology#Monitored_area"/>
        <rdfs:range rdf:resource="http://www.semanticweb.org/smarotta/ontologies/2022/4/silvanusOntology#Biodiversity_index"/>
    </owl:ObjectProperty>
    


    <!-- http://www.semanticweb.org/smarotta/ontologies/2022/4/silvanusOntology#has_construction_material -->

    <owl:ObjectProperty rdf:about="http://www.semanticweb.org/smarotta/ontologies/2022/4/silvanusOntology#has_construction_material">
        <rdfs:domain rdf:resource="http://www.semanticweb.org/smarotta/ontologies/2022/4/silvanusOntology#Structure"/>
        <rdfs:range rdf:resource="http://www.semanticweb.org/smarotta/ontologies/2022/4/silvanusOntology#Construction_material"/>
    </owl:ObjectProperty>
    


    <!-- http://www.semanticweb.org/smarotta/ontologies/2022/4/silvanusOntology#has_fire_characteristic -->

    <owl:ObjectProperty rdf:about="http://www.semanticweb.org/smarotta/ontologies/2022/4/silvanusOntology#has_fire_characteristic">
        <rdfs:subPropertyOf rdf:resource="http://www.w3.org/2002/07/owl#topObjectProperty"/>
        <rdfs:domain rdf:resource="http://www.semanticweb.org/smarotta/ontologies/2022/4/silvanusOntology#Fire"/>
        <rdfs:range rdf:resource="http://www.semanticweb.org/smarotta/ontologies/2022/4/silvanusOntology#Fire_characteristic"/>
    </owl:ObjectProperty>
    


    <!-- http://www.semanticweb.org/smarotta/ontologies/2022/4/silvanusOntology#has_fire_risk -->

    <owl:ObjectProperty rdf:about="http://www.semanticweb.org/smarotta/ontologies/2022/4/silvanusOntology#has_fire_risk">
        <rdfs:subPropertyOf rdf:resource="http://www.w3.org/2002/07/owl#topObjectProperty"/>
        <rdfs:domain rdf:resource="http://www.semanticweb.org/smarotta/ontologies/2022/4/silvanusOntology#Monitored_area"/>
        <rdfs:range rdf:resource="http://www.semanticweb.org/smarotta/ontologies/2022/4/silvanusOntology#Fire_risk"/>
    </owl:ObjectProperty>
    


    <!-- http://www.semanticweb.org/smarotta/ontologies/2022/4/silvanusOntology#has_geolocation -->

    <owl:ObjectProperty rdf:about="http://www.semanticweb.org/smarotta/ontologies/2022/4/silvanusOntology#has_geolocation">
        <rdfs:subPropertyOf rdf:resource="http://www.w3.org/2002/07/owl#topObjectProperty"/>
        <rdfs:domain rdf:resource="http://www.semanticweb.org/smarotta/ontologies/2022/4/silvanusOntology#Animal"/>
        <rdfs:domain rdf:resource="http://www.semanticweb.org/smarotta/ontologies/2022/4/silvanusOntology#Area_burned"/>
        <rdfs:domain rdf:resource="http://www.semanticweb.org/smarotta/ontologies/2022/4/silvanusOntology#Climate_parameter"/>
        <rdfs:domain rdf:resource="http://www.semanticweb.org/smarotta/ontologies/2022/4/silvanusOntology#Fire"/>
        <rdfs:domain rdf:resource="http://www.semanticweb.org/smarotta/ontologies/2022/4/silvanusOntology#Incident"/>
        <rdfs:domain rdf:resource="http://www.semanticweb.org/smarotta/ontologies/2022/4/silvanusOntology#Media_item"/>
        <rdfs:domain rdf:resource="http://www.semanticweb.org/smarotta/ontologies/2022/4/silvanusOntology#Monitored_area"/>
        <rdfs:domain rdf:resource="http://www.semanticweb.org/smarotta/ontologies/2022/4/silvanusOntology#Responder"/>
        <rdfs:domain rdf:resource="http://www.semanticweb.org/smarotta/ontologies/2022/4/silvanusOntology#Response_resource"/>
        <rdfs:domain rdf:resource="http://www.semanticweb.org/smarotta/ontologies/2022/4/silvanusOntology#Sensor"/>
        <rdfs:domain rdf:resource="http://www.semanticweb.org/smarotta/ontologies/2022/4/silvanusOntology#Vulnerable_object"/>
        <rdfs:range rdf:resource="http://www.semanticweb.org/smarotta/ontologies/2022/4/silvanusOntology#Location"/>
    </owl:ObjectProperty>
    


    <!-- http://www.semanticweb.org/smarotta/ontologies/2022/4/silvanusOntology#has_government_policy -->

    <owl:ObjectProperty rdf:about="http://www.semanticweb.org/smarotta/ontologies/2022/4/silvanusOntology#has_government_policy">
        <rdfs:subPropertyOf rdf:resource="http://www.w3.org/2002/07/owl#topObjectProperty"/>
        <rdfs:domain rdf:resource="http://www.semanticweb.org/smarotta/ontologies/2022/4/silvanusOntology#Community"/>
        <rdfs:range rdf:resource="http://www.semanticweb.org/smarotta/ontologies/2022/4/silvanusOntology#Government_policy"/>
    </owl:ObjectProperty>
    


    <!-- http://www.semanticweb.org/smarotta/ontologies/2022/4/silvanusOntology#has_high_priority_area -->

    <owl:ObjectProperty rdf:about="http://www.semanticweb.org/smarotta/ontologies/2022/4/silvanusOntology#has_high_priority_area">
        <rdfs:domain rdf:resource="http://www.semanticweb.org/smarotta/ontologies/2022/4/silvanusOntology#Community"/>
        <rdfs:range rdf:resource="http://www.semanticweb.org/smarotta/ontologies/2022/4/silvanusOntology#High_priority_area"/>
    </owl:ObjectProperty>
    


    <!-- http://www.semanticweb.org/smarotta/ontologies/2022/4/silvanusOntology#has_impact -->

    <owl:ObjectProperty rdf:about="http://www.semanticweb.org/smarotta/ontologies/2022/4/silvanusOntology#has_impact">
        <rdfs:domain rdf:resource="http://www.semanticweb.org/smarotta/ontologies/2022/4/silvanusOntology#Fire"/>
        <rdfs:domain rdf:resource="http://www.semanticweb.org/smarotta/ontologies/2022/4/silvanusOntology#Incident"/>
        <rdfs:range rdf:resource="http://www.semanticweb.org/smarotta/ontologies/2022/4/silvanusOntology#Impact"/>
    </owl:ObjectProperty>
    


    <!-- http://www.semanticweb.org/smarotta/ontologies/2022/4/silvanusOntology#has_infrastructure_development -->

    <owl:ObjectProperty rdf:about="http://www.semanticweb.org/smarotta/ontologies/2022/4/silvanusOntology#has_infrastructure_development">
        <rdfs:domain rdf:resource="http://www.semanticweb.org/smarotta/ontologies/2022/4/silvanusOntology#Community"/>
    </owl:ObjectProperty>
    


    <!-- http://www.semanticweb.org/smarotta/ontologies/2022/4/silvanusOntology#has_living_being_stats -->

    <owl:ObjectProperty rdf:about="http://www.semanticweb.org/smarotta/ontologies/2022/4/silvanusOntology#has_living_being_stats">
        <rdfs:domain rdf:resource="http://www.semanticweb.org/smarotta/ontologies/2022/4/silvanusOntology#Animal"/>
        <rdfs:domain rdf:resource="http://www.semanticweb.org/smarotta/ontologies/2022/4/silvanusOntology#Fuel"/>
        <rdfs:range rdf:resource="http://www.semanticweb.org/smarotta/ontologies/2022/4/silvanusOntology#Living_being_stat"/>
    </owl:ObjectProperty>
    


    <!-- http://www.semanticweb.org/smarotta/ontologies/2022/4/silvanusOntology#has_measure -->

    <owl:ObjectProperty rdf:about="http://www.semanticweb.org/smarotta/ontologies/2022/4/silvanusOntology#has_measure"/>
    


    <!-- http://www.semanticweb.org/smarotta/ontologies/2022/4/silvanusOntology#has_moisture -->

    <owl:ObjectProperty rdf:about="http://www.semanticweb.org/smarotta/ontologies/2022/4/silvanusOntology#has_moisture">
        <rdfs:subPropertyOf rdf:resource="http://www.semanticweb.org/smarotta/ontologies/2022/4/silvanusOntology#has_vegetation_stat"/>
        <rdfs:domain rdf:resource="http://www.semanticweb.org/smarotta/ontologies/2022/4/silvanusOntology#Fuel"/>
        <rdfs:range rdf:resource="http://www.semanticweb.org/smarotta/ontologies/2022/4/silvanusOntology#Moisture"/>
    </owl:ObjectProperty>
    


    <!-- http://www.semanticweb.org/smarotta/ontologies/2022/4/silvanusOntology#has_rea_under_pressure -->

    <owl:ObjectProperty rdf:about="http://www.semanticweb.org/smarotta/ontologies/2022/4/silvanusOntology#has_rea_under_pressure">
        <rdfs:domain rdf:resource="http://www.semanticweb.org/smarotta/ontologies/2022/4/silvanusOntology#Community"/>
        <rdfs:range rdf:resource="http://www.semanticweb.org/smarotta/ontologies/2022/4/silvanusOntology#Area_under_pressure"/>
    </owl:ObjectProperty>
    


    <!-- http://www.semanticweb.org/smarotta/ontologies/2022/4/silvanusOntology#has_report -->

    <owl:ObjectProperty rdf:about="http://www.semanticweb.org/smarotta/ontologies/2022/4/silvanusOntology#has_report">
        <rdfs:subPropertyOf rdf:resource="http://www.w3.org/2002/07/owl#topObjectProperty"/>
        <rdfs:domain rdf:resource="http://www.semanticweb.org/smarotta/ontologies/2022/4/silvanusOntology#Incident"/>
        <rdfs:range rdf:resource="http://www.semanticweb.org/smarotta/ontologies/2022/4/silvanusOntology#Incident_report"/>
    </owl:ObjectProperty>
    


    <!-- http://www.semanticweb.org/smarotta/ontologies/2022/4/silvanusOntology#has_space_time -->

    <owl:ObjectProperty rdf:about="http://www.semanticweb.org/smarotta/ontologies/2022/4/silvanusOntology#has_space_time">
        <rdfs:domain rdf:resource="http://www.semanticweb.org/smarotta/ontologies/2022/4/silvanusOntology#Fire"/>
        <rdfs:range rdf:resource="http://www.semanticweb.org/smarotta/ontologies/2022/4/silvanusOntology#Spatial_entity"/>
        <rdfs:range rdf:resource="http://www.semanticweb.org/smarotta/ontologies/2022/4/silvanusOntology#Temporal_entity"/>
    </owl:ObjectProperty>
    


    <!-- http://www.semanticweb.org/smarotta/ontologies/2022/4/silvanusOntology#has_unit -->

    <owl:ObjectProperty rdf:about="http://www.semanticweb.org/smarotta/ontologies/2022/4/silvanusOntology#has_unit">
        <rdfs:domain rdf:resource="http://www.semanticweb.org/smarotta/ontologies/2022/4/silvanusOntology#Measure"/>
        <rdfs:range rdf:resource="http://www.semanticweb.org/smarotta/ontologies/2022/4/silvanusOntology#Unit"/>
    </owl:ObjectProperty>
    


    <!-- http://www.semanticweb.org/smarotta/ontologies/2022/4/silvanusOntology#has_vegetation_stat -->

    <owl:ObjectProperty rdf:about="http://www.semanticweb.org/smarotta/ontologies/2022/4/silvanusOntology#has_vegetation_stat">
        <rdfs:subPropertyOf rdf:resource="http://www.semanticweb.org/smarotta/ontologies/2022/4/silvanusOntology#has_living_being_stats"/>
        <rdfs:domain rdf:resource="http://www.semanticweb.org/smarotta/ontologies/2022/4/silvanusOntology#Fuel"/>
        <rdfs:range rdf:resource="http://www.semanticweb.org/smarotta/ontologies/2022/4/silvanusOntology#Vegetation_stat"/>
    </owl:ObjectProperty>
    


    <!-- http://www.semanticweb.org/smarotta/ontologies/2022/4/silvanusOntology#involves -->

    <owl:ObjectProperty rdf:about="http://www.semanticweb.org/smarotta/ontologies/2022/4/silvanusOntology#involves">
        <rdfs:subPropertyOf rdf:resource="http://www.w3.org/2002/07/owl#topObjectProperty"/>
        <rdfs:domain rdf:resource="http://www.semanticweb.org/smarotta/ontologies/2022/4/silvanusOntology#Incident"/>
        <rdfs:range rdf:resource="http://www.semanticweb.org/smarotta/ontologies/2022/4/silvanusOntology#Vulnerable_object"/>
    </owl:ObjectProperty>
    


    <!-- http://www.semanticweb.org/smarotta/ontologies/2022/4/silvanusOntology#observes -->

    <owl:ObjectProperty rdf:about="http://www.semanticweb.org/smarotta/ontologies/2022/4/silvanusOntology#observes">
        <rdfs:subPropertyOf rdf:resource="http://www.w3.org/2002/07/owl#topObjectProperty"/>
        <rdfs:domain rdf:resource="http://www.semanticweb.org/smarotta/ontologies/2022/4/silvanusOntology#Sensor"/>
        <rdfs:range rdf:resource="http://www.semanticweb.org/smarotta/ontologies/2022/4/silvanusOntology#Climate_parameter"/>
    </owl:ObjectProperty>
    


    <!-- http://www.semanticweb.org/smarotta/ontologies/2022/4/silvanusOntology#produces -->

    <owl:ObjectProperty rdf:about="http://www.semanticweb.org/smarotta/ontologies/2022/4/silvanusOntology#produces">
        <rdfs:subPropertyOf rdf:resource="http://www.w3.org/2002/07/owl#topObjectProperty"/>
        <rdfs:domain rdf:resource="http://www.semanticweb.org/smarotta/ontologies/2022/4/silvanusOntology#Silvanus_module"/>
        <rdfs:range rdf:resource="http://www.semanticweb.org/smarotta/ontologies/2022/4/silvanusOntology#Dataset"/>
    </owl:ObjectProperty>
    


    <!-- http://www.semanticweb.org/smarotta/ontologies/2022/4/silvanusOntology#relates_to_mission -->

    <owl:ObjectProperty rdf:about="http://www.semanticweb.org/smarotta/ontologies/2022/4/silvanusOntology#relates_to_mission">
        <rdfs:domain rdf:resource="http://www.semanticweb.org/smarotta/ontologies/2022/4/silvanusOntology#Incident"/>
        <rdfs:range rdf:resource="http://www.semanticweb.org/smarotta/ontologies/2022/4/silvanusOntology#Mission"/>
    </owl:ObjectProperty>
    


    <!-- http://www.semanticweb.org/smarotta/ontologies/2022/4/silvanusOntology#relates_to_silvanus_module -->

    <owl:ObjectProperty rdf:about="http://www.semanticweb.org/smarotta/ontologies/2022/4/silvanusOntology#relates_to_silvanus_module">
        <rdfs:domain rdf:resource="http://www.semanticweb.org/smarotta/ontologies/2022/4/silvanusOntology#Media_item"/>
        <rdfs:range rdf:resource="http://www.semanticweb.org/smarotta/ontologies/2022/4/silvanusOntology#Silvanus_module"/>
    </owl:ObjectProperty>
    


    <!-- 
    ///////////////////////////////////////////////////////////////////////////////////////
    //
    // Classes
    //
    ///////////////////////////////////////////////////////////////////////////////////////
     -->

    


    <!-- http://www.semanticweb.org/smarotta/ontologies/2022/4/silvanusOntology#Accident -->

    <owl:Class rdf:about="http://www.semanticweb.org/smarotta/ontologies/2022/4/silvanusOntology#Accident">
        <rdfs:subClassOf rdf:resource="http://www.semanticweb.org/smarotta/ontologies/2022/4/silvanusOntology#Cause"/>
        <silvanusOntology:source>https://effis-gwis-cms.s3-eu-west-1.amazonaws.com/effis/reports-and-publications/effis-related-publications/lb-na-25-923-en-n.pdf (page 10)</silvanusOntology:source>
        <rdfs:comment>Wildfire unintentionally and indirectly caused by human without use of fire, connected neither to will nor to negligence rather to fatality.</rdfs:comment>
    </owl:Class>
    


    <!-- http://www.semanticweb.org/smarotta/ontologies/2022/4/silvanusOntology#Accomodation -->

    <owl:Class rdf:about="http://www.semanticweb.org/smarotta/ontologies/2022/4/silvanusOntology#Accomodation">
        <rdfs:subClassOf rdf:resource="http://www.semanticweb.org/smarotta/ontologies/2022/4/silvanusOntology#Building"/>
        <rdfs:comment>Settlement</rdfs:comment>
        <rdfs:seeAlso>http://www.semanticweb.org/earthquake#Accomodation</rdfs:seeAlso>
    </owl:Class>
    


    <!-- http://www.semanticweb.org/smarotta/ontologies/2022/4/silvanusOntology#Active_crown_fire -->

    <owl:Class rdf:about="http://www.semanticweb.org/smarotta/ontologies/2022/4/silvanusOntology#Active_crown_fire">
        <rdfs:subClassOf rdf:resource="http://www.semanticweb.org/smarotta/ontologies/2022/4/silvanusOntology#Crown_fire"/>
        <silvanusOntology:source>https://www.fs.fed.us/database/feis/glossary2.html</silvanusOntology:source>
        <rdfs:comment>A crown fire in which the entire fuel complex is involved in flame, but the crowning phase remains dependent on heat released from surface fuel for continued spread. An active crown fire may also be also called a running crown fire or continuous crown fire. An active crown fire presents a solid wall of flame from the surface through the canopy fuel layers. Flames appear to emanate from the canopy as a whole rather than from individual trees within the canopy. Active crown fire is one of several types of crown fire and is contrasted with passive crown fires which are less vigorous types of crown fire that do not emit continuous, solid flames from the canopy</rdfs:comment>
    </owl:Class>
    


    <!-- http://www.semanticweb.org/smarotta/ontologies/2022/4/silvanusOntology#Active_fronts_number -->

    <owl:Class rdf:about="http://www.semanticweb.org/smarotta/ontologies/2022/4/silvanusOntology#Active_fronts_number">
        <rdfs:subClassOf rdf:resource="http://www.semanticweb.org/smarotta/ontologies/2022/4/silvanusOntology#Fire_characteristic"/>
        <silvanusOntology:source>French pilot</silvanusOntology:source>
        <rdfs:comment>Number of active fire fronts</rdfs:comment>
    </owl:Class>
    


    <!-- http://www.semanticweb.org/smarotta/ontologies/2022/4/silvanusOntology#Adolescent -->

    <owl:Class rdf:about="http://www.semanticweb.org/smarotta/ontologies/2022/4/silvanusOntology#Adolescent">
        <rdfs:subClassOf rdf:resource="http://www.semanticweb.org/smarotta/ontologies/2022/4/silvanusOntology#Age_group"/>
        <rdfs:comment xml:lang="en">An adolescent is a person aged 10 to 19 years inclusive</rdfs:comment>
        <rdfs:seeAlso>https://w3id.org/empathi/adolescent</rdfs:seeAlso>
    </owl:Class>
    


    <!-- http://www.semanticweb.org/smarotta/ontologies/2022/4/silvanusOntology#Adult -->

    <owl:Class rdf:about="http://www.semanticweb.org/smarotta/ontologies/2022/4/silvanusOntology#Adult">
        <rdfs:subClassOf rdf:resource="http://www.semanticweb.org/smarotta/ontologies/2022/4/silvanusOntology#Age_group"/>
        <rdfs:comment xml:lang="en">An adult is a person older than 19 years of age unless national law defines a person as being an adult at an earlier age</rdfs:comment>
        <rdfs:seeAlso>https://w3id.org/empathi/adult</rdfs:seeAlso>
    </owl:Class>
    


    <!-- http://www.semanticweb.org/smarotta/ontologies/2022/4/silvanusOntology#Age_group -->

    <owl:Class rdf:about="http://www.semanticweb.org/smarotta/ontologies/2022/4/silvanusOntology#Age_group">
        <rdfs:comment rdf:datatype="http://www.w3.org/2001/XMLSchema#string">a number of people or things classed together as being of similar age.</rdfs:comment>
        <rdfs:seeAlso>https://w3id.org/empathi/Age_Group</rdfs:seeAlso>
    </owl:Class>
    


    <!-- http://www.semanticweb.org/smarotta/ontologies/2022/4/silvanusOntology#Agricultural_management -->

    <owl:Class rdf:about="http://www.semanticweb.org/smarotta/ontologies/2022/4/silvanusOntology#Agricultural_management">
        <rdfs:subClassOf rdf:resource="http://www.semanticweb.org/smarotta/ontologies/2022/4/silvanusOntology#Use_of_fire"/>
        <silvanusOntology:source>https://effis-gwis-cms.s3-eu-west-1.amazonaws.com/effis/reports-and-publications/effis-related-publications/lb-na-25-923-en-n.pdf (page 10)</silvanusOntology:source>
        <rdfs:comment>Wildfire caused by all types of agricultural burnings (stubble burnings, etc.).</rdfs:comment>
    </owl:Class>
    


    <!-- http://www.semanticweb.org/smarotta/ontologies/2022/4/silvanusOntology#Agriculture -->

    <owl:Class rdf:about="http://www.semanticweb.org/smarotta/ontologies/2022/4/silvanusOntology#Agriculture">
        <rdfs:subClassOf rdf:resource="http://www.semanticweb.org/smarotta/ontologies/2022/4/silvanusOntology#Ecological_asset"/>
        <rdfs:comment>Agricultural used spaces.</rdfs:comment>
        <rdfs:seeAlso>https://raw.githubusercontent.com/beAWARE-project/ontology/master/beAWARE_ontology#Agriculture</rdfs:seeAlso>
    </owl:Class>
    


    <!-- http://www.semanticweb.org/smarotta/ontologies/2022/4/silvanusOntology#Aircraft -->

    <owl:Class rdf:about="http://www.semanticweb.org/smarotta/ontologies/2022/4/silvanusOntology#Aircraft">
        <rdfs:subClassOf rdf:resource="http://www.semanticweb.org/smarotta/ontologies/2022/4/silvanusOntology#Response_vehicle"/>
        <rdfs:comment>Aircraft</rdfs:comment>
        <rdfs:seeAlso>http://www.ontologylibrary.mil/CommonCore/Mid/ArtifactOntology#Aircraft</rdfs:seeAlso>
    </owl:Class>
    


    <!-- http://www.semanticweb.org/smarotta/ontologies/2022/4/silvanusOntology#Airport -->

    <owl:Class rdf:about="http://www.semanticweb.org/smarotta/ontologies/2022/4/silvanusOntology#Airport">
        <rdfs:subClassOf rdf:resource="http://www.semanticweb.org/smarotta/ontologies/2022/4/silvanusOntology#Transportation_Facility"/>
        <rdfs:comment rdf:datatype="http://www.w3.org/2001/XMLSchema#string">A Transportation Facility that is designed for launching, receiving, and housing Aircraft.</rdfs:comment>
        <rdfs:seeAlso>http://www.ontologylibrary.mil/CommonCore/Mid/ArtifactOntology#Airport</rdfs:seeAlso>
        <rdfs:seeAlso>http://www.semanticweb.org/earthquake#AirportLoss</rdfs:seeAlso>
    </owl:Class>
    


    <!-- http://www.semanticweb.org/smarotta/ontologies/2022/4/silvanusOntology#All_season_road -->

    <owl:Class rdf:about="http://www.semanticweb.org/smarotta/ontologies/2022/4/silvanusOntology#All_season_road">
        <rdfs:subClassOf rdf:resource="http://www.semanticweb.org/smarotta/ontologies/2022/4/silvanusOntology#Street"/>
        <rdfs:comment>A road which is usable across all seasons.</rdfs:comment>
        <rdfs:seeAlso>http://purl.obolibrary.org/obo/ENVO_01000771</rdfs:seeAlso>
    </owl:Class>
    


    <!-- http://www.semanticweb.org/smarotta/ontologies/2022/4/silvanusOntology#Allocentric_Position -->

    <owl:Class rdf:about="http://www.semanticweb.org/smarotta/ontologies/2022/4/silvanusOntology#Allocentric_Position">
        <rdfs:subClassOf rdf:resource="http://www.semanticweb.org/smarotta/ontologies/2022/4/silvanusOntology#Position"/>
        <rdfs:comment>Position from a set of points</rdfs:comment>
        <rdfs:seeAlso>http://crossforest.eu/position/ontology/AllocentricPosition</rdfs:seeAlso>
    </owl:Class>
    


    <!-- http://www.semanticweb.org/smarotta/ontologies/2022/4/silvanusOntology#Alpine_Biome -->

    <owl:Class rdf:about="http://www.semanticweb.org/smarotta/ontologies/2022/4/silvanusOntology#Alpine_Biome">
        <rdfs:subClassOf rdf:resource="http://www.semanticweb.org/smarotta/ontologies/2022/4/silvanusOntology#Biome"/>
        <rdfs:comment>A biome which is subject to alpine altitudinal conditions.</rdfs:comment>
        <rdfs:seeAlso>http://purl.obolibrary.org/obo/ENVO_01001835</rdfs:seeAlso>
    </owl:Class>
    


    <!-- http://www.semanticweb.org/smarotta/ontologies/2022/4/silvanusOntology#Altitude -->

    <owl:Class rdf:about="http://www.semanticweb.org/smarotta/ontologies/2022/4/silvanusOntology#Altitude">
        <rdfs:subClassOf rdf:resource="http://www.semanticweb.org/smarotta/ontologies/2022/4/silvanusOntology#Spatial_entity"/>
        <rdfs:comment>Altitude from sea level</rdfs:comment>
        <rdfs:seeAlso>http://crossforest.eu/ifi/ontology/Altitude</rdfs:seeAlso>
    </owl:Class>
    


    <!-- http://www.semanticweb.org/smarotta/ontologies/2022/4/silvanusOntology#Anemometer -->

    <owl:Class rdf:about="http://www.semanticweb.org/smarotta/ontologies/2022/4/silvanusOntology#Anemometer">
        <rdfs:subClassOf rdf:resource="http://www.semanticweb.org/smarotta/ontologies/2022/4/silvanusOntology#IoT_sensor"/>
        <silvanusOntology:source>Most pilots</silvanusOntology:source>
        <rdfs:comment>An anemometer is a device that measures wind speed and direction. It is a common weather station instrument.</rdfs:comment>
    </owl:Class>
    


    <!-- http://www.semanticweb.org/smarotta/ontologies/2022/4/silvanusOntology#Animal -->

    <owl:Class rdf:about="http://www.semanticweb.org/smarotta/ontologies/2022/4/silvanusOntology#Animal">
        <rdfs:subClassOf rdf:resource="http://www.semanticweb.org/smarotta/ontologies/2022/4/silvanusOntology#Biodiversity_index"/>
        <rdfs:subClassOf rdf:resource="http://www.semanticweb.org/smarotta/ontologies/2022/4/silvanusOntology#Living_being"/>
        <silvanusOntology:input>Spatial locations (spatial resolution variable) of wild life specie occurances retrieved from public atlas and repositories (GBIF, iNaturalist; locations uploaded by stakeholders)</silvanusOntology:input>
        <silvanusOntology:output>List of wildlife species potentially present in an area of interest; information on species conservation status (and other relevant information)</silvanusOntology:output>
        <rdfs:comment>List and map of wildlife known to be present in the area of interest</rdfs:comment>
        <rdfs:seeAlso>https://raw.githubusercontent.com/beAWARE-project/ontology/master/beAWARE_ontology#Animal</rdfs:seeAlso>
    </owl:Class>
    


    <!-- http://www.semanticweb.org/smarotta/ontologies/2022/4/silvanusOntology#Animal_tracker -->

    <owl:Class rdf:about="http://www.semanticweb.org/smarotta/ontologies/2022/4/silvanusOntology#Animal_tracker">
        <rdfs:subClassOf rdf:resource="http://www.semanticweb.org/smarotta/ontologies/2022/4/silvanusOntology#Biodiversity_sensor"/>
        <silvanusOntology:source>Portuguese pilot</silvanusOntology:source>
        <rdfs:comment>Device for tracking animal position</rdfs:comment>
    </owl:Class>
    


    <!-- http://www.semanticweb.org/smarotta/ontologies/2022/4/silvanusOntology#Annual_precipitation -->

    <owl:Class rdf:about="http://www.semanticweb.org/smarotta/ontologies/2022/4/silvanusOntology#Annual_precipitation">
        <rdfs:subClassOf rdf:resource="http://www.semanticweb.org/smarotta/ontologies/2022/4/silvanusOntology#Precipitation"/>
        <silvanusOntology:source>Brazilian pilot</silvanusOntology:source>
        <rdfs:comment>Precipitations in the span of 1 year</rdfs:comment>
    </owl:Class>
    


    <!-- http://www.semanticweb.org/smarotta/ontologies/2022/4/silvanusOntology#Anthropogenic_Terrestrial_Biome -->

    <owl:Class rdf:about="http://www.semanticweb.org/smarotta/ontologies/2022/4/silvanusOntology#Anthropogenic_Terrestrial_Biome">
        <rdfs:subClassOf rdf:resource="http://www.semanticweb.org/smarotta/ontologies/2022/4/silvanusOntology#Terrestrial_Biome"/>
        <rdfs:comment>An anthropogenic terrestrial biome is a terrestrial biome which has community structures determined by human activity.</rdfs:comment>
        <rdfs:seeAlso>http://purl.obolibrary.org/obo/ENVO_01000219</rdfs:seeAlso>
    </owl:Class>
    


    <!-- http://www.semanticweb.org/smarotta/ontologies/2022/4/silvanusOntology#Aquatic_Biome -->

    <owl:Class rdf:about="http://www.semanticweb.org/smarotta/ontologies/2022/4/silvanusOntology#Aquatic_Biome">
        <rdfs:subClassOf rdf:resource="http://www.semanticweb.org/smarotta/ontologies/2022/4/silvanusOntology#Biome"/>
        <rdfs:comment>A biome which is determined by a water body and which has ecological climax communities adapted to life in or on water.</rdfs:comment>
        <rdfs:seeAlso>http://purl.obolibrary.org/obo/ENVO_00002030</rdfs:seeAlso>
    </owl:Class>
    


    <!-- http://www.semanticweb.org/smarotta/ontologies/2022/4/silvanusOntology#Area_Of_Cropland -->

    <owl:Class rdf:about="http://www.semanticweb.org/smarotta/ontologies/2022/4/silvanusOntology#Area_Of_Cropland">
        <rdfs:subClassOf rdf:resource="http://www.semanticweb.org/smarotta/ontologies/2022/4/silvanusOntology#Vegetated_area"/>
        <rdfs:comment>An area of a planet&apos;s surface which is partly covered either by annual crops and perennial woody crops or by actively tilled land. This area is in contact with an atmospheric column extending from the planetary boundary layer to the planet&apos;s exosphere with little to no physical obstruction.</rdfs:comment>
        <rdfs:seeAlso>http://purl.obolibrary.org/obo/ENVO_01000892</rdfs:seeAlso>
    </owl:Class>
    


    <!-- http://www.semanticweb.org/smarotta/ontologies/2022/4/silvanusOntology#Area_Of_Evergreen_Forest -->

    <owl:Class rdf:about="http://www.semanticweb.org/smarotta/ontologies/2022/4/silvanusOntology#Area_Of_Evergreen_Forest">
        <rdfs:subClassOf rdf:resource="http://www.semanticweb.org/smarotta/ontologies/2022/4/silvanusOntology#Vegetated_area"/>
        <rdfs:comment>An area of a planet&apos;s surface which is primarily covered by a forest in which the majority of trees maintain their foliage despite seasonal change. The surfaces of this area (including the surface of the forest canopy) are in contact with an atmospheric column extending from the planetary boundary layer to the planet&apos;s exosphere with little to no physical obstruction.</rdfs:comment>
        <rdfs:seeAlso>http://purl.obolibrary.org/obo/ENVO_01000843</rdfs:seeAlso>
    </owl:Class>
    


    <!-- http://www.semanticweb.org/smarotta/ontologies/2022/4/silvanusOntology#Area_Of_Lichen-dominated_Vegetation -->

    <owl:Class rdf:about="http://www.semanticweb.org/smarotta/ontologies/2022/4/silvanusOntology#Area_Of_Lichen-dominated_Vegetation">
        <rdfs:subClassOf rdf:resource="http://www.semanticweb.org/smarotta/ontologies/2022/4/silvanusOntology#Vegetated_area"/>
        <rdfs:comment>An area of a planet&apos;s surface which is primarily covered by fruticose or foliose lichens and which is in contact with an atmospheric column extending from the planetary boundary layer to the planet&apos;s exosphere with little to no physical obstruction.</rdfs:comment>
        <rdfs:seeAlso>http://purl.obolibrary.org/obo/ENVO_01000889</rdfs:seeAlso>
    </owl:Class>
    


    <!-- http://www.semanticweb.org/smarotta/ontologies/2022/4/silvanusOntology#Area_Of_Mixed_Forest -->

    <owl:Class rdf:about="http://www.semanticweb.org/smarotta/ontologies/2022/4/silvanusOntology#Area_Of_Mixed_Forest">
        <rdfs:subClassOf rdf:resource="http://www.semanticweb.org/smarotta/ontologies/2022/4/silvanusOntology#Vegetated_area"/>
        <rdfs:comment>An area of a planet&apos;s surface which is primarily covered by a forest in which the trees are a mixture between those that lose and retain their foliage despite seasonal change. The surfaces of this area (including the surface of the forest canopy) are in contact with an atmospheric column extending from the planetary boundary layer to the planet&apos;s exosphere with little to no physical obstruction.</rdfs:comment>
        <rdfs:seeAlso>http://purl.obolibrary.org/obo/ENVO_01000855</rdfs:seeAlso>
    </owl:Class>
    


    <!-- http://www.semanticweb.org/smarotta/ontologies/2022/4/silvanusOntology#Area_Of_Moss-dominated_Vegetation -->

    <owl:Class rdf:about="http://www.semanticweb.org/smarotta/ontologies/2022/4/silvanusOntology#Area_Of_Moss-dominated_Vegetation">
        <rdfs:subClassOf rdf:resource="http://www.semanticweb.org/smarotta/ontologies/2022/4/silvanusOntology#Vegetated_area"/>
        <rdfs:comment>An area of a planet&apos;s surface which is primarily covered by mosses and which is in contact with an atmospheric column extending from the planetary boundary layer to the planet&apos;s exosphere with little to no physical obstruction.</rdfs:comment>
        <rdfs:seeAlso>http://purl.obolibrary.org/obo/ENVO_01000890</rdfs:seeAlso>
    </owl:Class>
    


    <!-- http://www.semanticweb.org/smarotta/ontologies/2022/4/silvanusOntology#Area_Of_Sedge-_And_Forb-dominated_Herbaceous_Vegetation -->

    <owl:Class rdf:about="http://www.semanticweb.org/smarotta/ontologies/2022/4/silvanusOntology#Area_Of_Sedge-_And_Forb-dominated_Herbaceous_Vegetation">
        <rdfs:subClassOf rdf:resource="http://www.semanticweb.org/smarotta/ontologies/2022/4/silvanusOntology#Vegetated_area"/>
        <rdfs:comment>An area of a planet&apos;s surface which is primarily covered by sedges or forbs, possibly interpersed with grasses or grass-like plants. This area is in contact with an atmospheric column extending from the planetary boundary layer to the planet&apos;s exosphere with little to no physical obstruction.</rdfs:comment>
        <rdfs:seeAlso>http://purl.obolibrary.org/obo/ENVO_01000887</rdfs:seeAlso>
    </owl:Class>
    


    <!-- http://www.semanticweb.org/smarotta/ontologies/2022/4/silvanusOntology#Area_Of_Tundra -->

    <owl:Class rdf:about="http://www.semanticweb.org/smarotta/ontologies/2022/4/silvanusOntology#Area_Of_Tundra">
        <rdfs:subClassOf rdf:resource="http://www.semanticweb.org/smarotta/ontologies/2022/4/silvanusOntology#Vegetated_area"/>
        <rdfs:comment>A vegetated area which is part of a tundra ecosystem.</rdfs:comment>
        <rdfs:seeAlso>http://purl.obolibrary.org/obo/ENVO_00000112</rdfs:seeAlso>
    </owl:Class>
    


    <!-- http://www.semanticweb.org/smarotta/ontologies/2022/4/silvanusOntology#Area_Of_Woody_Wetland -->

    <owl:Class rdf:about="http://www.semanticweb.org/smarotta/ontologies/2022/4/silvanusOntology#Area_Of_Woody_Wetland">
        <rdfs:subClassOf rdf:resource="http://www.semanticweb.org/smarotta/ontologies/2022/4/silvanusOntology#Vegetated_area"/>
        <rdfs:comment>An area of a planet&apos;s surface which is partly covered by forest or shrubland vegetation and where the underlying soil or substrate is periodically saturated with or covered by water. This area is in contact with an atmospheric column extending from the planetary boundary layer to the planet&apos;s exosphere with little to no physical obstruction.</rdfs:comment>
        <rdfs:seeAlso>http://purl.obolibrary.org/obo/ENVO_01000893</rdfs:seeAlso>
    </owl:Class>
    


    <!-- http://www.semanticweb.org/smarotta/ontologies/2022/4/silvanusOntology#Area_burned -->

    <owl:Class rdf:about="http://www.semanticweb.org/smarotta/ontologies/2022/4/silvanusOntology#Area_burned">
        <rdfs:subClassOf rdf:resource="http://www.semanticweb.org/smarotta/ontologies/2022/4/silvanusOntology#Fire_characteristic"/>
        <rdfs:comment>It&apos;s the total area affected by fire in a burn event.</rdfs:comment>
        <rdfs:seeAlso>http://cerrado.linkeddata.es/ecology/fire#AreaBurned</rdfs:seeAlso>
    </owl:Class>
    


    <!-- http://www.semanticweb.org/smarotta/ontologies/2022/4/silvanusOntology#Area_under_pressure -->

    <owl:Class rdf:about="http://www.semanticweb.org/smarotta/ontologies/2022/4/silvanusOntology#Area_under_pressure">
        <rdfs:comment>Areas under pressure, meaning with negative impacts on biodiversity, due to human causes</rdfs:comment>
    </owl:Class>
    


    <!-- http://www.semanticweb.org/smarotta/ontologies/2022/4/silvanusOntology#Arid_Biome -->

    <owl:Class rdf:about="http://www.semanticweb.org/smarotta/ontologies/2022/4/silvanusOntology#Arid_Biome">
        <rdfs:subClassOf rdf:resource="http://www.semanticweb.org/smarotta/ontologies/2022/4/silvanusOntology#Biome"/>
        <rdfs:comment>A biome which is subject to arid environmental conditions.</rdfs:comment>
        <rdfs:seeAlso>http://purl.obolibrary.org/obo/ENVO_01001838</rdfs:seeAlso>
    </owl:Class>
    


    <!-- http://www.semanticweb.org/smarotta/ontologies/2022/4/silvanusOntology#Armored_Personnel_Carrier -->

    <owl:Class rdf:about="http://www.semanticweb.org/smarotta/ontologies/2022/4/silvanusOntology#Armored_Personnel_Carrier">
        <rdfs:subClassOf rdf:resource="http://www.semanticweb.org/smarotta/ontologies/2022/4/silvanusOntology#Ground_Motor_Vehicle"/>
        <rdfs:comment>An armoured personnel carrier (APC) is a broad type of armoured military vehicle designed to transport personnel and equipment in combat zones.</rdfs:comment>
        <rdfs:seeAlso>http://www.ontologylibrary.mil/CommonCore/Mid/ArtifactOntology#ArmoredPersonnelCarrier</rdfs:seeAlso>
    </owl:Class>
    


    <!-- http://www.semanticweb.org/smarotta/ontologies/2022/4/silvanusOntology#Asphalt_road -->

    <owl:Class rdf:about="http://www.semanticweb.org/smarotta/ontologies/2022/4/silvanusOntology#Asphalt_road">
        <rdfs:subClassOf rdf:resource="http://www.semanticweb.org/smarotta/ontologies/2022/4/silvanusOntology#Street"/>
        <rdfs:comment>A road which is primarily composed of asphalt.</rdfs:comment>
        <rdfs:seeAlso>http://purl.obolibrary.org/obo/ENVO_01001277</rdfs:seeAlso>
    </owl:Class>
    


    <!-- http://www.semanticweb.org/smarotta/ontologies/2022/4/silvanusOntology#Asset -->

    <owl:Class rdf:about="http://www.semanticweb.org/smarotta/ontologies/2022/4/silvanusOntology#Asset">
        <rdfs:subClassOf rdf:resource="http://www.semanticweb.org/smarotta/ontologies/2022/4/silvanusOntology#Vulnerable_object"/>
        <rdfs:comment>Any non-living item of interest.</rdfs:comment>
        <rdfs:seeAlso>https://raw.githubusercontent.com/beAWARE-project/ontology/master/beAWARE_ontology#Asset</rdfs:seeAlso>
    </owl:Class>
    


    <!-- http://www.semanticweb.org/smarotta/ontologies/2022/4/silvanusOntology#Atmospheric_pressure -->

    <owl:Class rdf:about="http://www.semanticweb.org/smarotta/ontologies/2022/4/silvanusOntology#Atmospheric_pressure">
        <rdfs:subClassOf rdf:resource="http://www.semanticweb.org/smarotta/ontologies/2022/4/silvanusOntology#Climate_parameter"/>
        <silvanusOntology:source>Romanian pilot</silvanusOntology:source>
        <rdfs:comment>The force exerted over a given area or object, either because of gravity pulling on it or other motion the object has. Molecules in the air produce pressure through both their weight and movement, and this pressure is connected to other properties of the atmosphere.</rdfs:comment>
        <rdfs:seeAlso>https://bimerr.iot.linkeddata.es/def/weather#Pressure</rdfs:seeAlso>
    </owl:Class>
    


    <!-- http://www.semanticweb.org/smarotta/ontologies/2022/4/silvanusOntology#Audio_item -->

    <owl:Class rdf:about="http://www.semanticweb.org/smarotta/ontologies/2022/4/silvanusOntology#Audio_item">
        <rdfs:subClassOf rdf:resource="http://www.semanticweb.org/smarotta/ontologies/2022/4/silvanusOntology#Media_item"/>
        <rdfs:comment>Represents an audio item</rdfs:comment>
        <rdfs:seeAlso>https://raw.githubusercontent.com/beAWARE-project/ontology/master/beAWARE_ontology#AudioItem</rdfs:seeAlso>
    </owl:Class>
    


    <!-- http://www.semanticweb.org/smarotta/ontologies/2022/4/silvanusOntology#Automobile -->

    <owl:Class rdf:about="http://www.semanticweb.org/smarotta/ontologies/2022/4/silvanusOntology#Automobile">
        <rdfs:subClassOf rdf:resource="http://www.semanticweb.org/smarotta/ontologies/2022/4/silvanusOntology#Ground_Motor_Vehicle"/>
        <rdfs:comment>A four-wheeled road vehicle that is powered by an engine and is able to carry a small number of people</rdfs:comment>
        <rdfs:seeAlso>http://www.ontologylibrary.mil/CommonCore/Mid/ArtifactOntology#Automobile</rdfs:seeAlso>
    </owl:Class>
    


    <!-- http://www.semanticweb.org/smarotta/ontologies/2022/4/silvanusOntology#Average_annual_precipitation -->

    <owl:Class rdf:about="http://www.semanticweb.org/smarotta/ontologies/2022/4/silvanusOntology#Average_annual_precipitation">
        <rdfs:subClassOf rdf:resource="http://www.semanticweb.org/smarotta/ontologies/2022/4/silvanusOntology#Precipitation"/>
        <silvanusOntology:source>Brazilian pilot</silvanusOntology:source>
        <rdfs:comment>Average annual precipitation for a given area</rdfs:comment>
    </owl:Class>
    


    <!-- http://www.semanticweb.org/smarotta/ontologies/2022/4/silvanusOntology#Average_annual_temperature -->

    <owl:Class rdf:about="http://www.semanticweb.org/smarotta/ontologies/2022/4/silvanusOntology#Average_annual_temperature">
        <rdfs:subClassOf rdf:resource="http://www.semanticweb.org/smarotta/ontologies/2022/4/silvanusOntology#Temperature"/>
        <silvanusOntology:source>Brazilian pilot</silvanusOntology:source>
        <rdfs:comment>Average annual temperature for a given area</rdfs:comment>
    </owl:Class>
    


    <!-- http://www.semanticweb.org/smarotta/ontologies/2022/4/silvanusOntology#Backfire -->

    <owl:Class rdf:about="http://www.semanticweb.org/smarotta/ontologies/2022/4/silvanusOntology#Backfire">
        <rdfs:subClassOf rdf:resource="http://www.semanticweb.org/smarotta/ontologies/2022/4/silvanusOntology#Controlled_fire"/>
        <silvanusOntology:source>https://www.fs.fed.us/database/feis/glossary2.html</silvanusOntology:source>
        <rdfs:comment>A fire set along the inner edge of a fireline to consume the fuel in the path of a fire or to change the fire&apos;s convection column [92]. Backfires are often set during the course of wildland firefighting, with the prescribed fire advancing aginast the wind [79].</rdfs:comment>
    </owl:Class>
    


    <!-- http://www.semanticweb.org/smarotta/ontologies/2022/4/silvanusOntology#Basal_Area -->

    <owl:Class rdf:about="http://www.semanticweb.org/smarotta/ontologies/2022/4/silvanusOntology#Basal_Area">
        <rdfs:subClassOf rdf:resource="http://www.semanticweb.org/smarotta/ontologies/2022/4/silvanusOntology#Measure"/>
        <owl:disjointWith rdf:resource="http://www.semanticweb.org/smarotta/ontologies/2022/4/silvanusOntology#Volume_with_bark"/>
        <rdfs:comment>Sum of the sectional areas of the trees at 1.30 m from the ground.</rdfs:comment>
        <rdfs:seeAlso>http://crossforest.eu/ifi/ontology/BasalArea</rdfs:seeAlso>
    </owl:Class>
    


    <!-- http://www.semanticweb.org/smarotta/ontologies/2022/4/silvanusOntology#Basic_region_for_the_application_of_regional_policies -->

    <owl:Class rdf:about="http://www.semanticweb.org/smarotta/ontologies/2022/4/silvanusOntology#Basic_region_for_the_application_of_regional_policies">
        <rdfs:subClassOf rdf:resource="http://www.semanticweb.org/smarotta/ontologies/2022/4/silvanusOntology#NUTS_unit"/>
        <rdfs:comment>NUTS 2: basic regions for the application of regional policies</rdfs:comment>
        <rdfs:seeAlso>http://crossforest.eu/ifi/ontology/NUTS2</rdfs:seeAlso>
    </owl:Class>
    


    <!-- http://www.semanticweb.org/smarotta/ontologies/2022/4/silvanusOntology#Bicycle -->

    <owl:Class rdf:about="http://www.semanticweb.org/smarotta/ontologies/2022/4/silvanusOntology#Bicycle">
        <rdfs:subClassOf rdf:resource="http://www.semanticweb.org/smarotta/ontologies/2022/4/silvanusOntology#Ground_Vehicle"/>
        <rdfs:comment>A vehicle consisting of two wheels held in a frame one behind the other, propelled by pedals and steered with handlebars attached to the front wheel.</rdfs:comment>
        <rdfs:seeAlso>http://www.ontologylibrary.mil/CommonCore/Mid/ArtifactOntology#Bicycle</rdfs:seeAlso>
    </owl:Class>
    


    <!-- http://www.semanticweb.org/smarotta/ontologies/2022/4/silvanusOntology#Biodiversity_index -->

    <owl:Class rdf:about="http://www.semanticweb.org/smarotta/ontologies/2022/4/silvanusOntology#Biodiversity_index">
        <rdfs:comment>Scientists use a formula called the biodiversity index to describe the amount of species diversity in a given area. A simple biodiversity index is calculated as follows: number of species in the area ÷ total number of individuals in the area = biodiversity index</rdfs:comment>
    </owl:Class>
    


    <!-- http://www.semanticweb.org/smarotta/ontologies/2022/4/silvanusOntology#Biodiversity_sensor -->

    <owl:Class rdf:about="http://www.semanticweb.org/smarotta/ontologies/2022/4/silvanusOntology#Biodiversity_sensor">
        <rdfs:subClassOf rdf:resource="http://www.semanticweb.org/smarotta/ontologies/2022/4/silvanusOntology#Sensor"/>
        <silvanusOntology:source>Portugues pilot</silvanusOntology:source>
        <rdfs:comment>Sensor for detecting biodiversity features</rdfs:comment>
    </owl:Class>
    


    <!-- http://www.semanticweb.org/smarotta/ontologies/2022/4/silvanusOntology#Biome -->

    <owl:Class rdf:about="http://www.semanticweb.org/smarotta/ontologies/2022/4/silvanusOntology#Biome">
        <rdfs:subClassOf rdf:resource="http://www.semanticweb.org/smarotta/ontologies/2022/4/silvanusOntology#Biodiversity_index"/>
        <rdfs:comment>A biome is an ecosystem to which resident ecological communities have evolved adaptations.</rdfs:comment>
        <rdfs:seeAlso>http://purl.obolibrary.org/obo/ENVO_00000428</rdfs:seeAlso>
    </owl:Class>
    


    <!-- http://www.semanticweb.org/smarotta/ontologies/2022/4/silvanusOntology#Boundary_wall -->

    <owl:Class rdf:about="http://www.semanticweb.org/smarotta/ontologies/2022/4/silvanusOntology#Boundary_wall">
        <rdfs:subClassOf rdf:resource="http://www.semanticweb.org/smarotta/ontologies/2022/4/silvanusOntology#Constructed_barrier"/>
        <rdfs:comment>A boundary wall is a constructed barrier which is usually opaque, constructed from masonry, and of greater structural strength than a fence.</rdfs:comment>
        <rdfs:seeAlso>http://purl.obolibrary.org/obo/ENVO_01000466</rdfs:seeAlso>
    </owl:Class>
    


    <!-- http://www.semanticweb.org/smarotta/ontologies/2022/4/silvanusOntology#Bridge -->

    <owl:Class rdf:about="http://www.semanticweb.org/smarotta/ontologies/2022/4/silvanusOntology#Bridge">
        <rdfs:subClassOf rdf:resource="http://www.semanticweb.org/smarotta/ontologies/2022/4/silvanusOntology#Structure"/>
        <rdfs:subClassOf rdf:resource="http://www.semanticweb.org/smarotta/ontologies/2022/4/silvanusOntology#Transportation"/>
        <rdfs:comment>Represents subway infrastructure.</rdfs:comment>
        <rdfs:seeAlso>http://purl.obolibrary.org/obo/ENVO_00000075</rdfs:seeAlso>
        <rdfs:seeAlso>http://www.semanticweb.org/earthquake#BridgeLoss</rdfs:seeAlso>
        <rdfs:seeAlso>https://raw.githubusercontent.com/beAWARE-project/ontology/master/beAWARE_ontology#Bridge</rdfs:seeAlso>
    </owl:Class>
    


    <!-- http://www.semanticweb.org/smarotta/ontologies/2022/4/silvanusOntology#Bronchodilator -->

    <owl:Class rdf:about="http://www.semanticweb.org/smarotta/ontologies/2022/4/silvanusOntology#Bronchodilator">
        <rdfs:subClassOf rdf:resource="http://www.semanticweb.org/smarotta/ontologies/2022/4/silvanusOntology#MedicalItem"/>
        <silvanusOntology:source>Greek pilot</silvanusOntology:source>
        <rdfs:comment>Bronchodilators are a type of medication that make breathing easier by relaxing the muscles in the lungs and widening the airways</rdfs:comment>
    </owl:Class>
    


    <!-- http://www.semanticweb.org/smarotta/ontologies/2022/4/silvanusOntology#Brush_fire -->

    <owl:Class rdf:about="http://www.semanticweb.org/smarotta/ontologies/2022/4/silvanusOntology#Brush_fire">
        <rdfs:subClassOf rdf:resource="http://www.semanticweb.org/smarotta/ontologies/2022/4/silvanusOntology#Fire"/>
        <rdfs:subClassOf>
            <owl:Restriction>
                <owl:onProperty rdf:resource="http://www.semanticweb.org/smarotta/ontologies/2022/4/silvanusOntology#fire_caused_by"/>
                <owl:someValuesFrom rdf:resource="http://www.semanticweb.org/smarotta/ontologies/2022/4/silvanusOntology#Negligence"/>
            </owl:Restriction>
        </rdfs:subClassOf>
        <rdfs:comment>A fire in low-growing and brush</rdfs:comment>
        <rdfs:seeAlso>http://cerrado.linkeddata.es/ecology/fire#BrushFire</rdfs:seeAlso>
    </owl:Class>
    


    <!-- http://www.semanticweb.org/smarotta/ontologies/2022/4/silvanusOntology#Building -->

    <owl:Class rdf:about="http://www.semanticweb.org/smarotta/ontologies/2022/4/silvanusOntology#Building">
        <rdfs:subClassOf rdf:resource="http://www.semanticweb.org/smarotta/ontologies/2022/4/silvanusOntology#Structure"/>
        <rdfs:comment rdf:datatype="http://www.w3.org/2001/XMLSchema#string">An Artifact that is designed as a building or campus dedicated to some specific purpose.</rdfs:comment>
        <rdfs:seeAlso>http://www.ontologylibrary.mil/CommonCore/Mid/ArtifactOntology#Facility</rdfs:seeAlso>
        <rdfs:seeAlso>http://www.semanticweb.org/earthquake#Building</rdfs:seeAlso>
        <rdfs:seeAlso>https://raw.githubusercontent.com/beAWARE-project/ontology/master/beAWARE_ontology#Building</rdfs:seeAlso>
    </owl:Class>
    


    <!-- http://www.semanticweb.org/smarotta/ontologies/2022/4/silvanusOntology#Buildup_index -->

    <owl:Class rdf:about="http://www.semanticweb.org/smarotta/ontologies/2022/4/silvanusOntology#Buildup_index">
        <rdfs:subClassOf rdf:resource="http://www.semanticweb.org/smarotta/ontologies/2022/4/silvanusOntology#Fire_weather_index"/>
        <silvanusOntology:source>https://cwfis.cfs.nrcan.gc.ca/background/summary/fwi</silvanusOntology:source>
        <rdfs:comment>The Buildup Index (BUI) is a numeric rating of the total amount of fuel available for combustion. It is based on the DMC and the DC. The BUI is generally less than twice the DMC value, and moisture in the DMC layer is expected to help prevent burning in material deeper down in the available fuel.</rdfs:comment>
    </owl:Class>
    


    <!-- http://www.semanticweb.org/smarotta/ontologies/2022/4/silvanusOntology#Bus -->

    <owl:Class rdf:about="http://www.semanticweb.org/smarotta/ontologies/2022/4/silvanusOntology#Bus">
        <rdfs:subClassOf rdf:resource="http://www.semanticweb.org/smarotta/ontologies/2022/4/silvanusOntology#Ground_Motor_Vehicle"/>
        <rdfs:comment>A large motor vehicle, having a long body, equipped with seats or benches for passengers, usually operating as part of a scheduled service</rdfs:comment>
        <rdfs:seeAlso>http://www.ontologylibrary.mil/CommonCore/Mid/ArtifactOntology#Bus</rdfs:seeAlso>
    </owl:Class>
    


    <!-- http://www.semanticweb.org/smarotta/ontologies/2022/4/silvanusOntology#Bush_Area -->

    <owl:Class rdf:about="http://www.semanticweb.org/smarotta/ontologies/2022/4/silvanusOntology#Bush_Area">
        <rdfs:subClassOf rdf:resource="http://www.semanticweb.org/smarotta/ontologies/2022/4/silvanusOntology#Vegetated_area"/>
        <rdfs:comment>A vegetated area which has not been cleared or is sparsely settled, usually scrub-covered or forested</rdfs:comment>
        <rdfs:seeAlso>http://purl.obolibrary.org/obo/ENVO_01001293</rdfs:seeAlso>
    </owl:Class>
    


    <!-- http://www.semanticweb.org/smarotta/ontologies/2022/4/silvanusOntology#CCTV -->

    <owl:Class rdf:about="http://www.semanticweb.org/smarotta/ontologies/2022/4/silvanusOntology#CCTV">
        <rdfs:subClassOf rdf:resource="http://www.semanticweb.org/smarotta/ontologies/2022/4/silvanusOntology#Camera"/>
        <silvanusOntology:source>Slovak pilot</silvanusOntology:source>
        <rdfs:comment>CCTV stands for closed-circuit television and is commonly known as video surveillance. “Closed-circuit” means broadcasts are usually transmitted to a limited (closed) number of monitors, unlike “regular” TV, which is broadcast to the public at large. CCTV networks are commonly used to detect and deter criminal activities, and record traffic infractions, but they have other uses.</rdfs:comment>
    </owl:Class>
    


    <!-- http://www.semanticweb.org/smarotta/ontologies/2022/4/silvanusOntology#Camera -->

    <owl:Class rdf:about="http://www.semanticweb.org/smarotta/ontologies/2022/4/silvanusOntology#Camera">
        <rdfs:subClassOf rdf:resource="http://www.semanticweb.org/smarotta/ontologies/2022/4/silvanusOntology#Sensor"/>
        <silvanusOntology:source>Croatian pilot</silvanusOntology:source>
        <silvanusOntology:source>Czech pilot</silvanusOntology:source>
        <silvanusOntology:source>Italian pilot</silvanusOntology:source>
        <silvanusOntology:source>Portuguese pilot</silvanusOntology:source>
        <silvanusOntology:source>Romanian pilot</silvanusOntology:source>
        <rdfs:comment>Device for capturing images</rdfs:comment>
    </owl:Class>
    


    <!-- http://www.semanticweb.org/smarotta/ontologies/2022/4/silvanusOntology#CanopyCover -->

    <owl:Class rdf:about="http://www.semanticweb.org/smarotta/ontologies/2022/4/silvanusOntology#CanopyCover">
        <rdfs:subClassOf rdf:resource="http://www.semanticweb.org/smarotta/ontologies/2022/4/silvanusOntology#Biodiversity_index"/>
        <rdfs:comment>Forest canopy cover, also known as canopy coverage or crown cover, is defined as the proportion of the forest covered by the vertical projection of the tree crowns</rdfs:comment>
        <rdfs:seeAlso>http://crossforest.eu/ilu/ontology/CanopyCover</rdfs:seeAlso>
    </owl:Class>
    


    <!-- http://www.semanticweb.org/smarotta/ontologies/2022/4/silvanusOntology#Car -->

    <owl:Class rdf:about="http://www.semanticweb.org/smarotta/ontologies/2022/4/silvanusOntology#Car">
        <rdfs:subClassOf rdf:resource="http://www.semanticweb.org/smarotta/ontologies/2022/4/silvanusOntology#Vehicle"/>
        <rdfs:comment>Represents any type of car.</rdfs:comment>
        <rdfs:seeAlso>https://raw.githubusercontent.com/beAWARE-project/ontology/master/beAWARE_ontology#Car</rdfs:seeAlso>
    </owl:Class>
    


    <!-- http://www.semanticweb.org/smarotta/ontologies/2022/4/silvanusOntology#Cause -->

    <owl:Class rdf:about="http://www.semanticweb.org/smarotta/ontologies/2022/4/silvanusOntology#Cause">
        <silvanusOntology:source>https://effis-gwis-cms.s3-eu-west-1.amazonaws.com/effis/reports-and-publications/effis-related-publications/lb-na-25-923-en-n.pdf (page 10)</silvanusOntology:source>
        <rdfs:comment>Cause that started the fire</rdfs:comment>
    </owl:Class>
    


    <!-- http://www.semanticweb.org/smarotta/ontologies/2022/4/silvanusOntology#Causeway -->

    <owl:Class rdf:about="http://www.semanticweb.org/smarotta/ontologies/2022/4/silvanusOntology#Causeway">
        <rdfs:subClassOf rdf:resource="http://www.semanticweb.org/smarotta/ontologies/2022/4/silvanusOntology#Transportation"/>
        <rdfs:comment>Represents subway infrastructure.</rdfs:comment>
        <rdfs:seeAlso>http://purl.obolibrary.org/obo/ENVO_00000158</rdfs:seeAlso>
    </owl:Class>
    


    <!-- http://www.semanticweb.org/smarotta/ontologies/2022/4/silvanusOntology#Chemical_composition_sensor -->

    <owl:Class rdf:about="http://www.semanticweb.org/smarotta/ontologies/2022/4/silvanusOntology#Chemical_composition_sensor">
        <rdfs:subClassOf rdf:resource="http://www.semanticweb.org/smarotta/ontologies/2022/4/silvanusOntology#Chemical_sensor"/>
        <silvanusOntology:source>French pilot</silvanusOntology:source>
        <rdfs:comment>Sensor to elicit the composition of the combustion gases</rdfs:comment>
    </owl:Class>
    


    <!-- http://www.semanticweb.org/smarotta/ontologies/2022/4/silvanusOntology#Chemical_sensor -->

    <owl:Class rdf:about="http://www.semanticweb.org/smarotta/ontologies/2022/4/silvanusOntology#Chemical_sensor">
        <rdfs:subClassOf rdf:resource="http://www.semanticweb.org/smarotta/ontologies/2022/4/silvanusOntology#Sensor"/>
        <silvanusOntology:source>French pilot</silvanusOntology:source>
        <rdfs:comment>A chemical sensor is a device that converts a property (physical or chemical) of a particular analyte into a measurable signal that is proportional to the analyte concentration. It recognizes the analyte molecule in a selective way by transforming the response into an analytical electrical signal.</rdfs:comment>
    </owl:Class>
    


    <!-- http://www.semanticweb.org/smarotta/ontologies/2022/4/silvanusOntology#Child -->

    <owl:Class rdf:about="http://www.semanticweb.org/smarotta/ontologies/2022/4/silvanusOntology#Child">
        <rdfs:subClassOf rdf:resource="http://www.semanticweb.org/smarotta/ontologies/2022/4/silvanusOntology#Age_group"/>
        <rdfs:comment xml:lang="en">A child is a person 19 years or younger unless national law defines a person to be an adult at an earlier age</rdfs:comment>
        <rdfs:seeAlso>https://w3id.org/empathi/child</rdfs:seeAlso>
    </owl:Class>
    


    <!-- http://www.semanticweb.org/smarotta/ontologies/2022/4/silvanusOntology#Children -->

    <owl:Class rdf:about="http://www.semanticweb.org/smarotta/ontologies/2022/4/silvanusOntology#Children">
        <rdfs:subClassOf rdf:resource="http://www.semanticweb.org/smarotta/ontologies/2022/4/silvanusOntology#Irresponsible"/>
        <owl:disjointWith rdf:resource="http://www.semanticweb.org/smarotta/ontologies/2022/4/silvanusOntology#Mental_illness"/>
        <silvanusOntology:source>https://effis-gwis-cms.s3-eu-west-1.amazonaws.com/effis/reports-and-publications/effis-related-publications/lb-na-25-923-en-n.pdf (page 10)</silvanusOntology:source>
        <rdfs:comment>Wildfire set by children (under legal age) for game or entertainment.</rdfs:comment>
    </owl:Class>
    


    <!-- http://www.semanticweb.org/smarotta/ontologies/2022/4/silvanusOntology#Church -->

    <owl:Class rdf:about="http://www.semanticweb.org/smarotta/ontologies/2022/4/silvanusOntology#Church">
        <rdfs:subClassOf rdf:resource="http://www.semanticweb.org/smarotta/ontologies/2022/4/silvanusOntology#Building"/>
        <silvanusOntology:source>Greek pilot</silvanusOntology:source>
        <rdfs:comment>Represents any type of religious building</rdfs:comment>
    </owl:Class>
    


    <!-- http://www.semanticweb.org/smarotta/ontologies/2022/4/silvanusOntology#Cigarettes -->

    <owl:Class rdf:about="http://www.semanticweb.org/smarotta/ontologies/2022/4/silvanusOntology#Cigarettes">
        <rdfs:subClassOf rdf:resource="http://www.semanticweb.org/smarotta/ontologies/2022/4/silvanusOntology#Use_of_glowing_objects"/>
        <silvanusOntology:source>https://effis-gwis-cms.s3-eu-west-1.amazonaws.com/effis/reports-and-publications/effis-related-publications/lb-na-25-923-en-n.pdf (page 10)</silvanusOntology:source>
        <rdfs:comment>Wildfire caused by cigarettes and tobacco pipe regardless of the activity or the location of the smoker. It includes the fires set by the match used for lighting the cigarette and negligently thrown away by the smoker, but not cases where a cigarette or matches have been used to set an arson fire.</rdfs:comment>
    </owl:Class>
    


    <!-- http://www.semanticweb.org/smarotta/ontologies/2022/4/silvanusOntology#City -->

    <owl:Class rdf:about="http://www.semanticweb.org/smarotta/ontologies/2022/4/silvanusOntology#City">
        <rdfs:subClassOf rdf:resource="http://www.semanticweb.org/smarotta/ontologies/2022/4/silvanusOntology#Spatial_entity"/>
        <rdfs:comment>A city is a large human settlement. A city is distinguished from other human settlements by its relatively great size, but also by its functions and its special symbolic status, which may be conferred by a central authority.</rdfs:comment>
        <rdfs:seeAlso>https://w3id.org/def/saref4city#City</rdfs:seeAlso>
    </owl:Class>
    


    <!-- http://www.semanticweb.org/smarotta/ontologies/2022/4/silvanusOntology#ClarificationOfSituation -->

    <owl:Class rdf:about="http://www.semanticweb.org/smarotta/ontologies/2022/4/silvanusOntology#ClarificationOfSituation">
        <rdfs:subClassOf rdf:resource="http://www.semanticweb.org/smarotta/ontologies/2022/4/silvanusOntology#Response_procedure"/>
        <rdfs:comment>Clarification of the situation</rdfs:comment>
        <rdfs:seeAlso>http://www.semanticweb.org/earthquake#ClarificationOfSituation</rdfs:seeAlso>
    </owl:Class>
    


    <!-- http://www.semanticweb.org/smarotta/ontologies/2022/4/silvanusOntology#ClearingWork -->

    <owl:Class rdf:about="http://www.semanticweb.org/smarotta/ontologies/2022/4/silvanusOntology#ClearingWork">
        <rdfs:subClassOf rdf:resource="http://www.semanticweb.org/smarotta/ontologies/2022/4/silvanusOntology#Response_procedure"/>
        <rdfs:comment>Clearing of rubble and obstacles</rdfs:comment>
        <rdfs:seeAlso>http://www.semanticweb.org/earthquake#ClearingWork</rdfs:seeAlso>
    </owl:Class>
    


    <!-- http://www.semanticweb.org/smarotta/ontologies/2022/4/silvanusOntology#Climate_parameter -->

    <owl:Class rdf:about="http://www.semanticweb.org/smarotta/ontologies/2022/4/silvanusOntology#Climate_parameter">
        <rdfs:comment>Parameters based on the Canadian Fire Weather Index System
https://www.nwcg.gov/publications/pms437/cffdrs/fire-weather-index-system</rdfs:comment>
        <rdfs:seeAlso>http://www.semanticweb.org/smarotta/ontologies/2022/4/silvanusOntology#ClimateParameter</rdfs:seeAlso>
    </owl:Class>
    


    <!-- http://www.semanticweb.org/smarotta/ontologies/2022/4/silvanusOntology#Clothing -->

    <owl:Class rdf:about="http://www.semanticweb.org/smarotta/ontologies/2022/4/silvanusOntology#Clothing">
        <rdfs:subClassOf rdf:resource="http://www.semanticweb.org/smarotta/ontologies/2022/4/silvanusOntology#ReliefItem"/>
        <rdfs:comment>Clothing items</rdfs:comment>
        <rdfs:seeAlso>http://www.semanticweb.org/earthquake#Clothing</rdfs:seeAlso>
    </owl:Class>
    


    <!-- http://www.semanticweb.org/smarotta/ontologies/2022/4/silvanusOntology#Collection_point -->

    <owl:Class rdf:about="http://www.semanticweb.org/smarotta/ontologies/2022/4/silvanusOntology#Collection_point">
        <rdfs:subClassOf rdf:resource="http://www.semanticweb.org/smarotta/ontologies/2022/4/silvanusOntology#Structure"/>
        <silvanusOntology:source>Italian piliot</silvanusOntology:source>
        <rdfs:comment>A geographically defined place where people meet in case of emergency.</rdfs:comment>
    </owl:Class>
    


    <!-- http://www.semanticweb.org/smarotta/ontologies/2022/4/silvanusOntology#Communication -->

    <owl:Class rdf:about="http://www.semanticweb.org/smarotta/ontologies/2022/4/silvanusOntology#Communication">
        <rdfs:subClassOf rdf:resource="http://www.semanticweb.org/smarotta/ontologies/2022/4/silvanusOntology#Infrastructure"/>
        <rdfs:comment>Represents any type of (tele)communication infrastructure.</rdfs:comment>
        <rdfs:seeAlso>http://www.semanticweb.org/earthquake#Communication</rdfs:seeAlso>
        <rdfs:seeAlso>https://raw.githubusercontent.com/beAWARE-project/ontology/master/beAWARE_ontology#Communication</rdfs:seeAlso>
    </owl:Class>
    


    <!-- http://www.semanticweb.org/smarotta/ontologies/2022/4/silvanusOntology#CommunicationChannel -->

    <owl:Class rdf:about="http://www.semanticweb.org/smarotta/ontologies/2022/4/silvanusOntology#CommunicationChannel">
        <rdfs:subClassOf rdf:resource="http://www.semanticweb.org/smarotta/ontologies/2022/4/silvanusOntology#Response_resource"/>
        <rdfs:comment>Transmission medium</rdfs:comment>
        <rdfs:seeAlso>http://www.semanticweb.org/earthquake#CommunicationChannel</rdfs:seeAlso>
    </owl:Class>
    


    <!-- http://www.semanticweb.org/smarotta/ontologies/2022/4/silvanusOntology#CommunicationFacility -->

    <owl:Class rdf:about="http://www.semanticweb.org/smarotta/ontologies/2022/4/silvanusOntology#CommunicationFacility">
        <rdfs:subClassOf rdf:resource="http://www.semanticweb.org/smarotta/ontologies/2022/4/silvanusOntology#Building"/>
        <rdfs:comment>Any and all public and private instrumentalities used or useful in the transmission of writing, signs, signals, pictures, or sounds of all kinds and includes mail, telephone, wire, radio, and all other means of communication.</rdfs:comment>
        <rdfs:seeAlso>http://www.semanticweb.org/earthquake#CommunicationFacility</rdfs:seeAlso>
        <rdfs:seeAlso>https://w3id.org/empathi/Communication</rdfs:seeAlso>
    </owl:Class>
    


    <!-- http://www.semanticweb.org/smarotta/ontologies/2022/4/silvanusOntology#CommunicationLeader -->

    <owl:Class rdf:about="http://www.semanticweb.org/smarotta/ontologies/2022/4/silvanusOntology#CommunicationLeader">
        <rdfs:subClassOf rdf:resource="http://www.semanticweb.org/smarotta/ontologies/2022/4/silvanusOntology#Responder"/>
        <rdfs:comment>Person in charge of the communication</rdfs:comment>
        <rdfs:seeAlso>http://www.semanticweb.org/earthquake#CommunicationLeader</rdfs:seeAlso>
    </owl:Class>
    


    <!-- http://www.semanticweb.org/smarotta/ontologies/2022/4/silvanusOntology#Communication_tower -->

    <owl:Class rdf:about="http://www.semanticweb.org/smarotta/ontologies/2022/4/silvanusOntology#Communication_tower">
        <rdfs:subClassOf rdf:resource="http://www.semanticweb.org/smarotta/ontologies/2022/4/silvanusOntology#Communication"/>
        <silvanusOntology:source>Italian pilot</silvanusOntology:source>
        <rdfs:comment>Telecommunications tower, a mast or tower built primarily to hold telecommunications antennas</rdfs:comment>
    </owl:Class>
    


    <!-- http://www.semanticweb.org/smarotta/ontologies/2022/4/silvanusOntology#Community -->

    <owl:Class rdf:about="http://www.semanticweb.org/smarotta/ontologies/2022/4/silvanusOntology#Community">
        <rdfs:subClassOf rdf:resource="http://www.semanticweb.org/smarotta/ontologies/2022/4/silvanusOntology#Asset"/>
        <silvanusOntology:source>Indonesian pilot</silvanusOntology:source>
        <rdfs:comment>The people with common interests living in a particular area</rdfs:comment>
    </owl:Class>
    


    <!-- http://www.semanticweb.org/smarotta/ontologies/2022/4/silvanusOntology#Concrete_road -->

    <owl:Class rdf:about="http://www.semanticweb.org/smarotta/ontologies/2022/4/silvanusOntology#Concrete_road">
        <rdfs:subClassOf rdf:resource="http://www.semanticweb.org/smarotta/ontologies/2022/4/silvanusOntology#Street"/>
        <rdfs:comment>A road which is primarily composed of concrete.</rdfs:comment>
        <rdfs:seeAlso>http://purl.obolibrary.org/obo/ENVO_01001278</rdfs:seeAlso>
    </owl:Class>
    


    <!-- http://www.semanticweb.org/smarotta/ontologies/2022/4/silvanusOntology#Conflict -->

    <owl:Class rdf:about="http://www.semanticweb.org/smarotta/ontologies/2022/4/silvanusOntology#Conflict">
        <rdfs:subClassOf rdf:resource="http://www.semanticweb.org/smarotta/ontologies/2022/4/silvanusOntology#Responsible"/>
        <silvanusOntology:source>https://effis-gwis-cms.s3-eu-west-1.amazonaws.com/effis/reports-and-publications/effis-related-publications/lb-na-25-923-en-n.pdf (page 10)</silvanusOntology:source>
        <rdfs:comment>Wildfire set in retaliation for real or perceived injustice or wrong:
- Personal revenge: (to retaliate for a one-to one or personal grievance, argument,
fight, personal affront or any of infinite arrays of events perceived by the offender
to warrant retaliation).
- Societal retaliation: (in revenge against the society that the author perceives has
wronged him).
- Institutional: (fire against institutions or use of fire to settle grievances with the
institution and to intimidate those associated with the institution).
- Group retaliation: (fire as expression of anger towards the group or its members
rather than anger at a specific individual within the group).
- Intimidation.</rdfs:comment>
    </owl:Class>
    


    <!-- http://www.semanticweb.org/smarotta/ontologies/2022/4/silvanusOntology#Constructed_barrier -->

    <owl:Class rdf:about="http://www.semanticweb.org/smarotta/ontologies/2022/4/silvanusOntology#Constructed_barrier">
        <rdfs:subClassOf rdf:resource="http://www.semanticweb.org/smarotta/ontologies/2022/4/silvanusOntology#Structure"/>
        <rdfs:comment>A constructed barrier is a freestanding wall, berm, or fence built to limit movement of entities across a boundary.</rdfs:comment>
        <rdfs:seeAlso>http://purl.obolibrary.org/obo/ENVO_01000467</rdfs:seeAlso>
    </owl:Class>
    


    <!-- http://www.semanticweb.org/smarotta/ontologies/2022/4/silvanusOntology#Construction_material -->

    <owl:Class rdf:about="http://www.semanticweb.org/smarotta/ontologies/2022/4/silvanusOntology#Construction_material">
        <silvanusOntology:source>Portuguese pilot</silvanusOntology:source>
        <rdfs:comment>Construction materials of a building</rdfs:comment>
    </owl:Class>
    


    <!-- http://www.semanticweb.org/smarotta/ontologies/2022/4/silvanusOntology#Containment -->

    <owl:Class rdf:about="http://www.semanticweb.org/smarotta/ontologies/2022/4/silvanusOntology#Containment">
        <rdfs:subClassOf rdf:resource="http://www.semanticweb.org/smarotta/ontologies/2022/4/silvanusOntology#Response_procedure"/>
        <rdfs:comment>Containment of the interested area</rdfs:comment>
        <rdfs:seeAlso>http://www.semanticweb.org/earthquake#Containment</rdfs:seeAlso>
    </owl:Class>
    


    <!-- http://www.semanticweb.org/smarotta/ontologies/2022/4/silvanusOntology#Controlled_fire -->

    <owl:Class rdf:about="http://www.semanticweb.org/smarotta/ontologies/2022/4/silvanusOntology#Controlled_fire">
        <rdfs:subClassOf rdf:resource="http://www.semanticweb.org/smarotta/ontologies/2022/4/silvanusOntology#Fire"/>
        <silvanusOntology:source>https://www.fs.fed.us/database/feis/glossary2.html#PrescribedFire</silvanusOntology:source>
        <rdfs:comment>Any fire intentionally ignited by management in accordance with applicable laws, policies, and regulations to meet specific objectives. Also called a controlled burn or prescribed burn [91,147]. An escaped prescribed fire is considered a wildfire [91]. A fire set under controlled and planned situation.</rdfs:comment>
        <rdfs:seeAlso>http://cerrado.linkeddata.es/ecology/fire#PrescriptionFire</rdfs:seeAlso>
    </owl:Class>
    


    <!-- http://www.semanticweb.org/smarotta/ontologies/2022/4/silvanusOntology#Cool-season_fire -->

    <owl:Class rdf:about="http://www.semanticweb.org/smarotta/ontologies/2022/4/silvanusOntology#Cool-season_fire">
        <rdfs:subClassOf rdf:resource="http://www.semanticweb.org/smarotta/ontologies/2022/4/silvanusOntology#Hazard-reduction_fire"/>
        <rdfs:comment>It&apos;s a fire set during the cool season, to avoid the fire to achieve very high temperatures or to make it easy to stop it.</rdfs:comment>
        <rdfs:seeAlso>http://cerrado.linkeddata.es/ecology/fire#CoolSeasonFire</rdfs:seeAlso>
    </owl:Class>
    


    <!-- http://www.semanticweb.org/smarotta/ontologies/2022/4/silvanusOntology#Coordinate -->

    <owl:Class rdf:about="http://www.semanticweb.org/smarotta/ontologies/2022/4/silvanusOntology#Coordinate">
        <rdfs:subClassOf rdf:resource="http://www.semanticweb.org/smarotta/ontologies/2022/4/silvanusOntology#Spatial_entity"/>
        <rdfs:comment>Any of a set of numbers used in specifying the location of a point on a line, on a surface, or in space</rdfs:comment>
        <rdfs:seeAlso>http://crossforest.eu/position/ontology/Coordinate</rdfs:seeAlso>
        <rdfs:seeAlso>http://www.w3.org/2003/01/geo/wgs84_pos#Point</rdfs:seeAlso>
    </owl:Class>
    


    <!-- http://www.semanticweb.org/smarotta/ontologies/2022/4/silvanusOntology#Country -->

    <owl:Class rdf:about="http://www.semanticweb.org/smarotta/ontologies/2022/4/silvanusOntology#Country">
        <rdfs:subClassOf rdf:resource="http://www.semanticweb.org/smarotta/ontologies/2022/4/silvanusOntology#Spatial_entity"/>
        <rdfs:comment>A country is a region that is identified as a distinct national entity in political geography.</rdfs:comment>
        <rdfs:seeAlso>http://crossforest.eu/ifi/ontology/Country</rdfs:seeAlso>
        <rdfs:seeAlso>https://w3id.org/def/saref4city#Country</rdfs:seeAlso>
    </owl:Class>
    


    <!-- http://www.semanticweb.org/smarotta/ontologies/2022/4/silvanusOntology#Crime_concealment -->

    <owl:Class rdf:about="http://www.semanticweb.org/smarotta/ontologies/2022/4/silvanusOntology#Crime_concealment">
        <rdfs:subClassOf rdf:resource="http://www.semanticweb.org/smarotta/ontologies/2022/4/silvanusOntology#Responsible"/>
        <silvanusOntology:source>https://effis-gwis-cms.s3-eu-west-1.amazonaws.com/effis/reports-and-publications/effis-related-publications/lb-na-25-923-en-n.pdf (page 10)</silvanusOntology:source>
        <rdfs:comment>Wildfire set to hide or conceal the primary crime activity: murder, suicide, breaking and entering, embezzlement, larceny, destroying records. Fires set as diversionary tactic fall into this category.</rdfs:comment>
    </owl:Class>
    


    <!-- http://www.semanticweb.org/smarotta/ontologies/2022/4/silvanusOntology#Critical_infrastructure -->

    <owl:Class rdf:about="http://www.semanticweb.org/smarotta/ontologies/2022/4/silvanusOntology#Critical_infrastructure">
        <rdfs:subClassOf rdf:resource="http://www.semanticweb.org/smarotta/ontologies/2022/4/silvanusOntology#Infrastructure"/>
        <silvanusOntology:input>CI location, perimeter and vegetation characterization.</silvanusOntology:input>
        <silvanusOntology:output>Critical Infrastructure Protection Areas displayed on map.</silvanusOntology:output>
        <silvanusOntology:source>Portuguese pilot</silvanusOntology:source>
        <rdfs:comment>Areas around critical infrastructure need to be kept clear of combustible biomass. Identification and monitoring of these areas is therefore necessary. They are defined by a perimeter around the critical infrastructure.</rdfs:comment>
    </owl:Class>
    


    <!-- http://www.semanticweb.org/smarotta/ontologies/2022/4/silvanusOntology#Crown_class -->

    <owl:Class rdf:about="http://www.semanticweb.org/smarotta/ontologies/2022/4/silvanusOntology#Crown_class">
        <silvanusOntology:source>https://www.fs.fed.us/database/feis/glossary2.html</silvanusOntology:source>
        <rdfs:comment>Measure of stand structure classifying trees within a stand as dominant (crowns rise through or above general canopy and receive full light from above and partial light from the sides), codominant (crowns in upper canopy but are blocked from receiving light from the sides by neighboring crowns), emergent (crowns completely above main canopy), intermediate (crowns receive little light from above and none from the side), overtopped or suppressed (one or more neighboring trees completely overtop crowns), and seedlings</rdfs:comment>
    </owl:Class>
    


    <!-- http://www.semanticweb.org/smarotta/ontologies/2022/4/silvanusOntology#Crown_fire -->

    <owl:Class rdf:about="http://www.semanticweb.org/smarotta/ontologies/2022/4/silvanusOntology#Crown_fire">
        <rdfs:subClassOf rdf:resource="http://www.semanticweb.org/smarotta/ontologies/2022/4/silvanusOntology#Fire"/>
        <silvanusOntology:source>https://www.fs.fed.us/database/feis/glossary2.html#CrownFire</silvanusOntology:source>
        <rdfs:comment>Fire that burns in the crowns of trees and shrubs. Usually ignited by a surface fire. Crown fires are common in coniferous forests and chaparral-type shrublands [20]. Also see active crown fire and passive crown fire.</rdfs:comment>
    </owl:Class>
    


    <!-- http://www.semanticweb.org/smarotta/ontologies/2022/4/silvanusOntology#Cycling_route -->

    <owl:Class rdf:about="http://www.semanticweb.org/smarotta/ontologies/2022/4/silvanusOntology#Cycling_route">
        <rdfs:subClassOf rdf:resource="http://www.semanticweb.org/smarotta/ontologies/2022/4/silvanusOntology#Transportation"/>
        <silvanusOntology:source>Slovak pilot</silvanusOntology:source>
        <rdfs:comment>A cycling route is a bikeway separated from motorized traffic and dedicated to cycling or shared with pedestrians or other non-motorized users.</rdfs:comment>
    </owl:Class>
    


    <!-- http://www.semanticweb.org/smarotta/ontologies/2022/4/silvanusOntology#Dairy -->

    <owl:Class rdf:about="http://www.semanticweb.org/smarotta/ontologies/2022/4/silvanusOntology#Dairy">
        <rdfs:subClassOf rdf:resource="http://www.semanticweb.org/smarotta/ontologies/2022/4/silvanusOntology#Industrial_building"/>
        <rdfs:comment>A dairy is a building in which animal milk is harvested and, optionally, processed for human consumption</rdfs:comment>
        <rdfs:seeAlso>http://purl.obolibrary.org/obo/ENVO_00003862</rdfs:seeAlso>
    </owl:Class>
    


    <!-- http://www.semanticweb.org/smarotta/ontologies/2022/4/silvanusOntology#Dam -->

    <owl:Class rdf:about="http://www.semanticweb.org/smarotta/ontologies/2022/4/silvanusOntology#Dam">
        <rdfs:subClassOf rdf:resource="http://www.semanticweb.org/smarotta/ontologies/2022/4/silvanusOntology#Constructed_barrier"/>
        <rdfs:comment>A barrier constructed across a watercourse to control the flow or raise the level of water.</rdfs:comment>
        <rdfs:seeAlso>http://purl.obolibrary.org/obo/ENVO_00000074</rdfs:seeAlso>
    </owl:Class>
    


    <!-- http://www.semanticweb.org/smarotta/ontologies/2022/4/silvanusOntology#Damage_quantification -->

    <owl:Class rdf:about="http://www.semanticweb.org/smarotta/ontologies/2022/4/silvanusOntology#Damage_quantification">
        <rdfs:subClassOf rdf:resource="http://www.semanticweb.org/smarotta/ontologies/2022/4/silvanusOntology#Biodiversity_index"/>
        <silvanusOntology:source>French pilot</silvanusOntology:source>
        <rdfs:comment>Quantifying the damage of forest fire (loss of XX cubic tons of oxygen, etc.)</rdfs:comment>
    </owl:Class>
    


    <!-- http://www.semanticweb.org/smarotta/ontologies/2022/4/silvanusOntology#Data_analysis -->

    <owl:Class rdf:about="http://www.semanticweb.org/smarotta/ontologies/2022/4/silvanusOntology#Data_analysis">
        <rdfs:subClassOf rdf:resource="http://www.semanticweb.org/smarotta/ontologies/2022/4/silvanusOntology#Silvanus_module"/>
        <rdfs:comment>A type of task carried out by a silvanus module involving data analysis.</rdfs:comment>
        <rdfs:seeAlso>https://raw.githubusercontent.com/beAWARE-project/ontology/master/beAWARE_ontology#DataAnalysis</rdfs:seeAlso>
    </owl:Class>
    


    <!-- http://www.semanticweb.org/smarotta/ontologies/2022/4/silvanusOntology#Dataset -->

    <owl:Class rdf:about="http://www.semanticweb.org/smarotta/ontologies/2022/4/silvanusOntology#Dataset">
        <rdfs:comment>Represents the dataset produced by a silvanus module.</rdfs:comment>
        <rdfs:seeAlso>https://raw.githubusercontent.com/beAWARE-project/ontology/master/beAWARE_ontology#Dataset</rdfs:seeAlso>
    </owl:Class>
    


    <!-- http://www.semanticweb.org/smarotta/ontologies/2022/4/silvanusOntology#Deliberate -->

    <owl:Class rdf:about="http://www.semanticweb.org/smarotta/ontologies/2022/4/silvanusOntology#Deliberate">
        <rdfs:subClassOf rdf:resource="http://www.semanticweb.org/smarotta/ontologies/2022/4/silvanusOntology#Cause"/>
        <silvanusOntology:source>https://effis-gwis-cms.s3-eu-west-1.amazonaws.com/effis/reports-and-publications/effis-related-publications/lb-na-25-923-en-n.pdf (page 10)</silvanusOntology:source>
        <rdfs:comment>Wildfire intentionally caused by human with the use of fire.</rdfs:comment>
    </owl:Class>
    


    <!-- http://www.semanticweb.org/smarotta/ontologies/2022/4/silvanusOntology#Dense_Settlement_Biome -->

    <owl:Class rdf:about="http://www.semanticweb.org/smarotta/ontologies/2022/4/silvanusOntology#Dense_Settlement_Biome">
        <rdfs:subClassOf rdf:resource="http://www.semanticweb.org/smarotta/ontologies/2022/4/silvanusOntology#Anthropogenic_Terrestrial_Biome"/>
        <rdfs:comment>A dense settlement biome is an anthropogenic terrestrial biome which is primarily used for human habitation, recreation, and industry within built structures with little other land use.</rdfs:comment>
        <rdfs:seeAlso>http://purl.obolibrary.org/obo/ENVO_01000248</rdfs:seeAlso>
    </owl:Class>
    


    <!-- http://www.semanticweb.org/smarotta/ontologies/2022/4/silvanusOntology#Density -->

    <owl:Class rdf:about="http://www.semanticweb.org/smarotta/ontologies/2022/4/silvanusOntology#Density">
        <rdfs:subClassOf rdf:resource="http://www.semanticweb.org/smarotta/ontologies/2022/4/silvanusOntology#Living_being_stat"/>
        <silvanusOntology:source>https://www.fs.fed.us/database/feis/glossary2.html</silvanusOntology:source>
        <rdfs:comment>1) In plant ecology, density = (Total number of individuals)/(total number of quadrats)[45]. Sometimes called abundance [87], a term usually not used in FEIS because of its ambiguity.
2) In range and wildlife ecology, the number of animals per unit area at a given time; stocking [43]</rdfs:comment>
    </owl:Class>
    


    <!-- http://www.semanticweb.org/smarotta/ontologies/2022/4/silvanusOntology#Detection -->

    <owl:Class rdf:about="http://www.semanticweb.org/smarotta/ontologies/2022/4/silvanusOntology#Detection">
        <rdfs:comment>Represents detections in a dataset.</rdfs:comment>
        <rdfs:seeAlso>https://raw.githubusercontent.com/beAWARE-project/ontology/master/beAWARE_ontology#Detection</rdfs:seeAlso>
    </owl:Class>
    


    <!-- http://www.semanticweb.org/smarotta/ontologies/2022/4/silvanusOntology#Diametric_class -->

    <owl:Class rdf:about="http://www.semanticweb.org/smarotta/ontologies/2022/4/silvanusOntology#Diametric_class">
        <rdfs:subClassOf rdf:resource="http://www.semanticweb.org/smarotta/ontologies/2022/4/silvanusOntology#Biodiversity_index"/>
        <rdfs:comment>Set of trees in a given forest having a diameter at the height of human breast between the two extremes of the class, e.g. class 41 to 45 cm</rdfs:comment>
        <rdfs:seeAlso>http://crossforest.eu/ifi/ontology/DiametricClass</rdfs:seeAlso>
    </owl:Class>
    


    <!-- http://www.semanticweb.org/smarotta/ontologies/2022/4/silvanusOntology#Direction -->

    <owl:Class rdf:about="http://www.semanticweb.org/smarotta/ontologies/2022/4/silvanusOntology#Direction">
        <rdfs:subClassOf rdf:resource="http://www.semanticweb.org/smarotta/ontologies/2022/4/silvanusOntology#Spatial_entity"/>
        <rdfs:comment>A course along which someone or something moves.</rdfs:comment>
        <rdfs:seeAlso>http://crossforest.eu/position/ontology/Direction</rdfs:seeAlso>
    </owl:Class>
    


    <!-- http://www.semanticweb.org/smarotta/ontologies/2022/4/silvanusOntology#Distance -->

    <owl:Class rdf:about="http://www.semanticweb.org/smarotta/ontologies/2022/4/silvanusOntology#Distance">
        <rdfs:subClassOf rdf:resource="http://www.semanticweb.org/smarotta/ontologies/2022/4/silvanusOntology#Spatial_entity"/>
        <rdfs:comment>The length of the space between two points.</rdfs:comment>
        <rdfs:seeAlso>http://crossforest.eu/position/ontology/Distance</rdfs:seeAlso>
    </owl:Class>
    


    <!-- http://www.semanticweb.org/smarotta/ontologies/2022/4/silvanusOntology#District -->

    <owl:Class rdf:about="http://www.semanticweb.org/smarotta/ontologies/2022/4/silvanusOntology#District">
        <rdfs:subClassOf rdf:resource="http://www.semanticweb.org/smarotta/ontologies/2022/4/silvanusOntology#Spatial_entity"/>
        <rdfs:comment>A district is a type of administrative division that, in some countries, is managed by local government. Across the world, areas known as &quot;districts&quot; vary greatly in size, spanning regions or counties, several municipalities, subdivisions of municipalities, school district, or political district.</rdfs:comment>
        <rdfs:seeAlso>https://saref.etsi.org/saref4city/District</rdfs:seeAlso>
    </owl:Class>
    


    <!-- http://www.semanticweb.org/smarotta/ontologies/2022/4/silvanusOntology#Dominant_formation -->

    <owl:Class rdf:about="http://www.semanticweb.org/smarotta/ontologies/2022/4/silvanusOntology#Dominant_formation">
        <rdfs:subClassOf rdf:resource="http://www.semanticweb.org/smarotta/ontologies/2022/4/silvanusOntology#Biodiversity_index"/>
        <silvanusOntology:source>https://www.fs.fed.us/database/feis/glossary2.html#dominance</silvanusOntology:source>
        <rdfs:comment>The extent to which a given species predominates in a community because of its size, abundance, or coverage [78].</rdfs:comment>
        <rdfs:seeAlso>http://crossforest.eu/ifi/ontology/DominantFormation</rdfs:seeAlso>
    </owl:Class>
    


    <!-- http://www.semanticweb.org/smarotta/ontologies/2022/4/silvanusOntology#Dominant_species -->

    <owl:Class rdf:about="http://www.semanticweb.org/smarotta/ontologies/2022/4/silvanusOntology#Dominant_species">
        <rdfs:subClassOf rdf:resource="http://www.semanticweb.org/smarotta/ontologies/2022/4/silvanusOntology#Living_being_stat"/>
        <silvanusOntology:source>Indonesian pilot</silvanusOntology:source>
        <silvanusOntology:source>https://www.fs.fed.us/database/feis/glossary2.html#dominance</silvanusOntology:source>
        <rdfs:comment>The dominant species  in a community based on its size, abundance, or coverage</rdfs:comment>
    </owl:Class>
    


    <!-- http://www.semanticweb.org/smarotta/ontologies/2022/4/silvanusOntology#Drinking_water_pipeline_network -->

    <owl:Class rdf:about="http://www.semanticweb.org/smarotta/ontologies/2022/4/silvanusOntology#Drinking_water_pipeline_network">
        <rdfs:subClassOf rdf:resource="http://www.semanticweb.org/smarotta/ontologies/2022/4/silvanusOntology#Pipeline_network"/>
        <rdfs:comment>A pipeline network which is used to transport drinking water to consumers.</rdfs:comment>
        <rdfs:seeAlso>http://purl.obolibrary.org/obo/ENVO_03600012</rdfs:seeAlso>
    </owl:Class>
    


    <!-- http://www.semanticweb.org/smarotta/ontologies/2022/4/silvanusOntology#Drinking_water_treatment_plant -->

    <owl:Class rdf:about="http://www.semanticweb.org/smarotta/ontologies/2022/4/silvanusOntology#Drinking_water_treatment_plant">
        <rdfs:subClassOf rdf:resource="http://www.semanticweb.org/smarotta/ontologies/2022/4/silvanusOntology#Waste_treatment_plant"/>
        <rdfs:subClassOf rdf:resource="http://www.semanticweb.org/smarotta/ontologies/2022/4/silvanusOntology#Water_supply"/>
        <rdfs:comment>An industrial building in which water undergoes a purification process to make it fit for human consumption.</rdfs:comment>
        <rdfs:seeAlso>http://purl.obolibrary.org/obo/ENVO_03600004</rdfs:seeAlso>
    </owl:Class>
    


    <!-- http://www.semanticweb.org/smarotta/ontologies/2022/4/silvanusOntology#Driveway -->

    <owl:Class rdf:about="http://www.semanticweb.org/smarotta/ontologies/2022/4/silvanusOntology#Driveway">
        <rdfs:subClassOf rdf:resource="http://www.semanticweb.org/smarotta/ontologies/2022/4/silvanusOntology#Street"/>
        <rdfs:comment>A road which is used for local access to one or more structures, and is privately owned and maintained by an individual or group.</rdfs:comment>
        <rdfs:seeAlso>http://purl.obolibrary.org/obo/ENVO_01001280</rdfs:seeAlso>
    </owl:Class>
    


    <!-- http://www.semanticweb.org/smarotta/ontologies/2022/4/silvanusOntology#Drought_fuel_moisture -->

    <owl:Class rdf:about="http://www.semanticweb.org/smarotta/ontologies/2022/4/silvanusOntology#Drought_fuel_moisture">
        <rdfs:subClassOf rdf:resource="http://www.semanticweb.org/smarotta/ontologies/2022/4/silvanusOntology#Moisture"/>
        <silvanusOntology:source>https://cwfis.cfs.nrcan.gc.ca/background/summary/fwi</silvanusOntology:source>
        <rdfs:comment>The Drought Code (DC) is a numeric rating of the average moisture content of deep, compact organic layers. This code is a useful indicator of seasonal drought effects on forest fuels and the amount of smoldering in deep duff layers and large logs.</rdfs:comment>
    </owl:Class>
    


    <!-- http://www.semanticweb.org/smarotta/ontologies/2022/4/silvanusOntology#DryFood -->

    <owl:Class rdf:about="http://www.semanticweb.org/smarotta/ontologies/2022/4/silvanusOntology#DryFood">
        <rdfs:subClassOf rdf:resource="http://www.semanticweb.org/smarotta/ontologies/2022/4/silvanusOntology#ReliefItem"/>
        <rdfs:comment>Dryfood items</rdfs:comment>
        <rdfs:seeAlso>http://www.semanticweb.org/earthquake#DryFood</rdfs:seeAlso>
    </owl:Class>
    


    <!-- http://www.semanticweb.org/smarotta/ontologies/2022/4/silvanusOntology#Duff -->

    <owl:Class rdf:about="http://www.semanticweb.org/smarotta/ontologies/2022/4/silvanusOntology#Duff">
        <rdfs:subClassOf rdf:resource="http://www.semanticweb.org/smarotta/ontologies/2022/4/silvanusOntology#Evnironment_index"/>
        <silvanusOntology:source>https://www.fs.fed.us/database/feis/glossary2.html</silvanusOntology:source>
        <rdfs:comment>Partially decomposed organic matter lying beneath the litter layer and above the mineral soil. Includes the fermentation and humus layers of the forest floor (Oa and Oe soil horizons) [20,125]. Also see litter.</rdfs:comment>
    </owl:Class>
    


    <!-- http://www.semanticweb.org/smarotta/ontologies/2022/4/silvanusOntology#Duff_fuel_moisture -->

    <owl:Class rdf:about="http://www.semanticweb.org/smarotta/ontologies/2022/4/silvanusOntology#Duff_fuel_moisture">
        <rdfs:subClassOf rdf:resource="http://www.semanticweb.org/smarotta/ontologies/2022/4/silvanusOntology#Moisture"/>
        <silvanusOntology:source>https://cwfis.cfs.nrcan.gc.ca/background/summary/fwi</silvanusOntology:source>
        <silvanusOntology:source>https://www.fs.fed.us/database/feis/glossary2.html</silvanusOntology:source>
        <rdfs:comment>The moisture in the 2.8-inch-deep (7 cm) layer below the fine fuel layer, assumed to be a layer of loosely compacted organic material. The duff moisture code has a time lag of approximately 12 days. It is an indicator for the fire consumption of a moderate duff layer or medium-diameter woody debris. The duff moisture code is always positive, but has no maximum, and high values indicate drier litter and higher fire spread/danger than low values.

The Duff Moisture Code (DMC) is a numeric rating of the average moisture content of loosely compacted organic layers of moderate depth. This code gives an indication of fuel consumption in moderate duff layers and medium-size woody material.</rdfs:comment>
    </owl:Class>
    


    <!-- http://www.semanticweb.org/smarotta/ontologies/2022/4/silvanusOntology#Dunes -->

    <owl:Class rdf:about="http://www.semanticweb.org/smarotta/ontologies/2022/4/silvanusOntology#Dunes">
        <rdfs:subClassOf rdf:resource="http://www.semanticweb.org/smarotta/ontologies/2022/4/silvanusOntology#Ecological_asset"/>
        <rdfs:comment>Represents dunes.</rdfs:comment>
        <rdfs:seeAlso>https://raw.githubusercontent.com/beAWARE-project/ontology/master/beAWARE_ontology#Dunes</rdfs:seeAlso>
    </owl:Class>
    


    <!-- http://www.semanticweb.org/smarotta/ontologies/2022/4/silvanusOntology#Duration -->

    <owl:Class rdf:about="http://www.semanticweb.org/smarotta/ontologies/2022/4/silvanusOntology#Duration">
        <rdfs:subClassOf rdf:resource="http://www.semanticweb.org/smarotta/ontologies/2022/4/silvanusOntology#Temporal_entity"/>
        <silvanusOntology:source>https://www.fs.fed.us/database/feis/glossary2.htmlhttp://cerrado.linkeddata.es/ecology/fire#Duration</silvanusOntology:source>
        <rdfs:comment>The length of time that combustion occurs at a given point [83]. Fire duration relates closely to downward heating and fire effects below the fuel surface as well as heating of tree boles above the surface.</rdfs:comment>
        <rdfs:seeAlso>http://cerrado.linkeddata.es/ecology/fire#Duration</rdfs:seeAlso>
    </owl:Class>
    


    <!-- http://www.semanticweb.org/smarotta/ontologies/2022/4/silvanusOntology#Ecological_asset -->

    <owl:Class rdf:about="http://www.semanticweb.org/smarotta/ontologies/2022/4/silvanusOntology#Ecological_asset">
        <rdfs:subClassOf rdf:resource="http://www.semanticweb.org/smarotta/ontologies/2022/4/silvanusOntology#Asset"/>
        <rdfs:comment>Ecological assets of various types.</rdfs:comment>
        <rdfs:seeAlso>https://raw.githubusercontent.com/beAWARE-project/ontology/master/beAWARE_ontology#EcologicalAsset</rdfs:seeAlso>
    </owl:Class>
    


    <!-- http://www.semanticweb.org/smarotta/ontologies/2022/4/silvanusOntology#EducationFacility -->

    <owl:Class rdf:about="http://www.semanticweb.org/smarotta/ontologies/2022/4/silvanusOntology#EducationFacility">
        <rdfs:subClassOf rdf:resource="http://www.semanticweb.org/smarotta/ontologies/2022/4/silvanusOntology#Building"/>
        <rdfs:comment>Represents any type of educational facility.</rdfs:comment>
        <rdfs:seeAlso>http://www.semanticweb.org/earthquake#EducationalInstitute</rdfs:seeAlso>
        <rdfs:seeAlso>https://raw.githubusercontent.com/beAWARE-project/ontology/master/beAWARE_ontology#EducationalFacility</rdfs:seeAlso>
        <rdfs:seeAlso>https://w3id.org/empathi/#Education_Resource</rdfs:seeAlso>
    </owl:Class>
    


    <!-- http://www.semanticweb.org/smarotta/ontologies/2022/4/silvanusOntology#Educational_facility -->

    <owl:Class rdf:about="http://www.semanticweb.org/smarotta/ontologies/2022/4/silvanusOntology#Educational_facility">
        <rdfs:subClassOf rdf:resource="http://www.semanticweb.org/smarotta/ontologies/2022/4/silvanusOntology#Infrastructure"/>
        <rdfs:comment>Represents any type of educational facility.</rdfs:comment>
        <rdfs:seeAlso>https://raw.githubusercontent.com/beAWARE-project/ontology/master/beAWARE_ontology#EducationalFacility</rdfs:seeAlso>
    </owl:Class>
    


    <!-- http://www.semanticweb.org/smarotta/ontologies/2022/4/silvanusOntology#Egocentric_Position -->

    <owl:Class rdf:about="http://www.semanticweb.org/smarotta/ontologies/2022/4/silvanusOntology#Egocentric_Position">
        <rdfs:subClassOf rdf:resource="http://www.semanticweb.org/smarotta/ontologies/2022/4/silvanusOntology#Position"/>
        <rdfs:comment xml:lang="en">Position from a point of reference</rdfs:comment>
        <rdfs:seeAlso>http://crossforest.eu/position/ontology/EgocentricPosition</rdfs:seeAlso>
    </owl:Class>
    


    <!-- http://www.semanticweb.org/smarotta/ontologies/2022/4/silvanusOntology#Electric_energy_supply -->

    <owl:Class rdf:about="http://www.semanticweb.org/smarotta/ontologies/2022/4/silvanusOntology#Electric_energy_supply">
        <rdfs:subClassOf rdf:resource="http://www.semanticweb.org/smarotta/ontologies/2022/4/silvanusOntology#Energy"/>
        <rdfs:comment>Represents electric energy supply infrastructure.</rdfs:comment>
        <rdfs:seeAlso>https://raw.githubusercontent.com/beAWARE-project/ontology/master/beAWARE_ontology#ElectricEnergySupply</rdfs:seeAlso>
    </owl:Class>
    


    <!-- http://www.semanticweb.org/smarotta/ontologies/2022/4/silvanusOntology#Electrical_infrastructure_criticallity -->

    <owl:Class rdf:about="http://www.semanticweb.org/smarotta/ontologies/2022/4/silvanusOntology#Electrical_infrastructure_criticallity">
        <rdfs:subClassOf rdf:resource="http://www.semanticweb.org/smarotta/ontologies/2022/4/silvanusOntology#Infrastructure"/>
        <silvanusOntology:source>Portuguese pilot</silvanusOntology:source>
        <rdfs:comment>Criticallity, based on grid redundancy and voltage characteristics.</rdfs:comment>
    </owl:Class>
    


    <!-- http://www.semanticweb.org/smarotta/ontologies/2022/4/silvanusOntology#Electrical_power -->

    <owl:Class rdf:about="http://www.semanticweb.org/smarotta/ontologies/2022/4/silvanusOntology#Electrical_power">
        <rdfs:subClassOf rdf:resource="http://www.semanticweb.org/smarotta/ontologies/2022/4/silvanusOntology#Accident"/>
        <silvanusOntology:source>https://effis-gwis-cms.s3-eu-west-1.amazonaws.com/effis/reports-and-publications/effis-related-publications/lb-na-25-923-en-n.pdf (page 10)</silvanusOntology:source>
        <rdfs:comment>Wildfire caused by sparks due to failure of electric lines or other electric wirings:
short-circuits due to contact between two lines or between line and vegetation or
bird, fall of the line, etc.</rdfs:comment>
    </owl:Class>
    


    <!-- http://www.semanticweb.org/smarotta/ontologies/2022/4/silvanusOntology#Ending_point -->

    <owl:Class rdf:about="http://www.semanticweb.org/smarotta/ontologies/2022/4/silvanusOntology#Ending_point">
        <rdfs:subClassOf rdf:resource="http://www.semanticweb.org/smarotta/ontologies/2022/4/silvanusOntology#Spatial_entity"/>
        <rdfs:comment>Ending point of a space</rdfs:comment>
        <rdfs:seeAlso>http://cerrado.linkeddata.es/ecology/fire#EndingPoint</rdfs:seeAlso>
    </owl:Class>
    


    <!-- http://www.semanticweb.org/smarotta/ontologies/2022/4/silvanusOntology#Ending_time -->

    <owl:Class rdf:about="http://www.semanticweb.org/smarotta/ontologies/2022/4/silvanusOntology#Ending_time">
        <rdfs:subClassOf rdf:resource="http://www.semanticweb.org/smarotta/ontologies/2022/4/silvanusOntology#Temporal_entity"/>
        <rdfs:comment>Ending timestamp of an event</rdfs:comment>
        <rdfs:seeAlso>http://cerrado.linkeddata.es/ecology/fire#EndingTime</rdfs:seeAlso>
    </owl:Class>
    


    <!-- http://www.semanticweb.org/smarotta/ontologies/2022/4/silvanusOntology#Energy -->

    <owl:Class rdf:about="http://www.semanticweb.org/smarotta/ontologies/2022/4/silvanusOntology#Energy">
        <rdfs:subClassOf rdf:resource="http://www.semanticweb.org/smarotta/ontologies/2022/4/silvanusOntology#Infrastructure"/>
        <silvanusOntology:output>Electrical Infrastructure characterized and displayed on map</silvanusOntology:output>
        <silvanusOntology:source>Portuguese pilot</silvanusOntology:source>
        <rdfs:comment>Represents any type of energy-generating infrastructure.</rdfs:comment>
        <rdfs:seeAlso>http://www.semanticweb.org/earthquake#Electricity</rdfs:seeAlso>
        <rdfs:seeAlso>https://raw.githubusercontent.com/beAWARE-project/ontology/master/beAWARE_ontology#Energy</rdfs:seeAlso>
    </owl:Class>
    


    <!-- http://www.semanticweb.org/smarotta/ontologies/2022/4/silvanusOntology#EnlightenmentOfPopulation -->

    <owl:Class rdf:about="http://www.semanticweb.org/smarotta/ontologies/2022/4/silvanusOntology#EnlightenmentOfPopulation">
        <rdfs:subClassOf rdf:resource="http://www.semanticweb.org/smarotta/ontologies/2022/4/silvanusOntology#Response_procedure"/>
        <rdfs:comment>Updating the communities on the state of the incident</rdfs:comment>
        <rdfs:seeAlso>http://www.semanticweb.org/earthquake#EnlightenmentOfPopulation</rdfs:seeAlso>
    </owl:Class>
    


    <!-- http://www.semanticweb.org/smarotta/ontologies/2022/4/silvanusOntology#Erosion -->

    <owl:Class rdf:about="http://www.semanticweb.org/smarotta/ontologies/2022/4/silvanusOntology#Erosion">
        <rdfs:subClassOf rdf:resource="http://www.semanticweb.org/smarotta/ontologies/2022/4/silvanusOntology#Biodiversity_index"/>
        <rdfs:comment>Erosion is the geological process in which earthen materials are worn away and transported by natural forces such as wind or water.</rdfs:comment>
        <rdfs:seeAlso>http://crossforest.eu/ifi/ontology/Erosion</rdfs:seeAlso>
    </owl:Class>
    


    <!-- http://www.semanticweb.org/smarotta/ontologies/2022/4/silvanusOntology#Escaped_prescribed_fire -->

    <owl:Class rdf:about="http://www.semanticweb.org/smarotta/ontologies/2022/4/silvanusOntology#Escaped_prescribed_fire">
        <rdfs:subClassOf rdf:resource="http://www.semanticweb.org/smarotta/ontologies/2022/4/silvanusOntology#Uncontrolled_fire"/>
        <silvanusOntology:source>https://www.fs.fed.us/database/feis/glossary2.html</silvanusOntology:source>
        <rdfs:comment>Prescribed fire that has exceeded prescription or is expected to exceed prescription or, for some other reason, meets criteria for conversion to wildfire. An escaped prescribed fire is considered a wildfire [91].</rdfs:comment>
    </owl:Class>
    


    <!-- http://www.semanticweb.org/smarotta/ontologies/2022/4/silvanusOntology#Evacuation -->

    <owl:Class rdf:about="http://www.semanticweb.org/smarotta/ontologies/2022/4/silvanusOntology#Evacuation">
        <rdfs:subClassOf rdf:resource="http://www.semanticweb.org/smarotta/ontologies/2022/4/silvanusOntology#Response_procedure"/>
        <rdfs:comment>Evacuation of the interested area</rdfs:comment>
        <rdfs:seeAlso>http://www.semanticweb.org/earthquake#Evacuation</rdfs:seeAlso>
    </owl:Class>
    


    <!-- http://www.semanticweb.org/smarotta/ontologies/2022/4/silvanusOntology#Evnironment_index -->

    <owl:Class rdf:about="http://www.semanticweb.org/smarotta/ontologies/2022/4/silvanusOntology#Evnironment_index">
        <rdfs:subClassOf rdf:resource="http://www.semanticweb.org/smarotta/ontologies/2022/4/silvanusOntology#Biodiversity_index"/>
    </owl:Class>
    


    <!-- http://www.semanticweb.org/smarotta/ontologies/2022/4/silvanusOntology#Excitement -->

    <owl:Class rdf:about="http://www.semanticweb.org/smarotta/ontologies/2022/4/silvanusOntology#Excitement">
        <rdfs:subClassOf rdf:resource="http://www.semanticweb.org/smarotta/ontologies/2022/4/silvanusOntology#Responsible"/>
        <silvanusOntology:source>https://effis-gwis-cms.s3-eu-west-1.amazonaws.com/effis/reports-and-publications/effis-related-publications/lb-na-25-923-en-n.pdf (page 10)</silvanusOntology:source>
        <rdfs:comment>Wildfires set to gain attention and to meet the needs of being important. Seeking of thrill, attention, recognition, relief of boredom. Includes fires lit in order to admire the spectacle of extinguishing means.</rdfs:comment>
    </owl:Class>
    


    <!-- http://www.semanticweb.org/smarotta/ontologies/2022/4/silvanusOntology#Extension -->

    <owl:Class rdf:about="http://www.semanticweb.org/smarotta/ontologies/2022/4/silvanusOntology#Extension">
        <rdfs:subClassOf rdf:resource="http://www.semanticweb.org/smarotta/ontologies/2022/4/silvanusOntology#Spatial_entity"/>
        <rdfs:comment>Extension in space</rdfs:comment>
        <rdfs:seeAlso>http://cerrado.linkeddata.es/ecology/fire#Extension</rdfs:seeAlso>
    </owl:Class>
    


    <!-- http://www.semanticweb.org/smarotta/ontologies/2022/4/silvanusOntology#Extreme_fire_behavior -->

    <owl:Class rdf:about="http://www.semanticweb.org/smarotta/ontologies/2022/4/silvanusOntology#Extreme_fire_behavior">
        <rdfs:subClassOf rdf:resource="http://www.semanticweb.org/smarotta/ontologies/2022/4/silvanusOntology#Fire_characteristic"/>
        <silvanusOntology:source>https://www.fs.fed.us/database/feis/glossary2.html</silvanusOntology:source>
        <rdfs:comment>Fire behavior characteristics that ordinarily preclude methods of direct control action. One or more of the following is usually involved: high rate of spread, prolific crowning and/or spotting, presence of fire whirls, strong convection column. Characteristics of such fires may change rapidly and dangerously. Terms used to describe extreme fire behavior include &quot;blowup&quot;, &quot;flare-up&quot;, and &quot;fire storm&quot; [92].</rdfs:comment>
    </owl:Class>
    


    <!-- http://www.semanticweb.org/smarotta/ontologies/2022/4/silvanusOntology#Extremist -->

    <owl:Class rdf:about="http://www.semanticweb.org/smarotta/ontologies/2022/4/silvanusOntology#Extremist">
        <rdfs:subClassOf rdf:resource="http://www.semanticweb.org/smarotta/ontologies/2022/4/silvanusOntology#Responsible"/>
        <silvanusOntology:source>https://effis-gwis-cms.s3-eu-west-1.amazonaws.com/effis/reports-and-publications/effis-related-publications/lb-na-25-923-en-n.pdf (page 10)</silvanusOntology:source>
        <rdfs:comment>Wildfire set to further social, political or religious causes: terrorism, discrimination, riots/civil disturbance.</rdfs:comment>
    </owl:Class>
    


    <!-- http://www.semanticweb.org/smarotta/ontologies/2022/4/silvanusOntology#FRCC1 -->

    <owl:Class rdf:about="http://www.semanticweb.org/smarotta/ontologies/2022/4/silvanusOntology#FRCC1">
        <rdfs:subClassOf rdf:resource="http://www.semanticweb.org/smarotta/ontologies/2022/4/silvanusOntology#Fire_regime_condition_class"/>
        <silvanusOntology:source>https://www.fs.fed.us/database/feis/glossary2.html</silvanusOntology:source>
        <rdfs:comment>ecosystems with high (&gt;66%) departure from reference conditions</rdfs:comment>
    </owl:Class>
    


    <!-- http://www.semanticweb.org/smarotta/ontologies/2022/4/silvanusOntology#FRCC2 -->

    <owl:Class rdf:about="http://www.semanticweb.org/smarotta/ontologies/2022/4/silvanusOntology#FRCC2">
        <rdfs:subClassOf rdf:resource="http://www.semanticweb.org/smarotta/ontologies/2022/4/silvanusOntology#Fire_regime_condition_class"/>
        <silvanusOntology:source>https://www.fs.fed.us/database/feis/glossary2.html</silvanusOntology:source>
        <rdfs:comment>ecosystems with moderate (33%-66%) departure</rdfs:comment>
    </owl:Class>
    


    <!-- http://www.semanticweb.org/smarotta/ontologies/2022/4/silvanusOntology#FRCC3 -->

    <owl:Class rdf:about="http://www.semanticweb.org/smarotta/ontologies/2022/4/silvanusOntology#FRCC3">
        <rdfs:subClassOf rdf:resource="http://www.semanticweb.org/smarotta/ontologies/2022/4/silvanusOntology#Fire_regime_condition_class"/>
        <silvanusOntology:source>https://www.fs.fed.us/database/feis/glossary2.html</silvanusOntology:source>
        <rdfs:comment>ecosystems with low (&lt;33%) departure from a defined reference period; i.e., landscapes still within the natural or historical range of variation</rdfs:comment>
    </owl:Class>
    


    <!-- http://www.semanticweb.org/smarotta/ontologies/2022/4/silvanusOntology#Factory -->

    <owl:Class rdf:about="http://www.semanticweb.org/smarotta/ontologies/2022/4/silvanusOntology#Factory">
        <rdfs:subClassOf rdf:resource="http://www.semanticweb.org/smarotta/ontologies/2022/4/silvanusOntology#Industrial_building"/>
        <rdfs:comment>A factory (previously manufactory) or manufacturing plant is an industrial site, usually consisting of buildings and machinery, or more commonly a complex having several buildings, where workers manufacture goods or operate machines processing one product into another.</rdfs:comment>
        <rdfs:seeAlso>http://purl.obolibrary.org/obo/ENVO_01000536</rdfs:seeAlso>
    </owl:Class>
    


    <!-- http://www.semanticweb.org/smarotta/ontologies/2022/4/silvanusOntology#Feaure_of_Interest -->

    <owl:Class rdf:about="http://www.semanticweb.org/smarotta/ontologies/2022/4/silvanusOntology#Feaure_of_Interest">
        <rdfs:comment xml:lang="en">A feature of interest represents any real world entity from which a property is measured. It is linked to the different properties it has and to its measurements.</rdfs:comment>
        <rdfs:seeAlso>https://saref.etsi.org/core/FeatureOfInterest</rdfs:seeAlso>
    </owl:Class>
    


    <!-- http://www.semanticweb.org/smarotta/ontologies/2022/4/silvanusOntology#Fence -->

    <owl:Class rdf:about="http://www.semanticweb.org/smarotta/ontologies/2022/4/silvanusOntology#Fence">
        <rdfs:subClassOf rdf:resource="http://www.semanticweb.org/smarotta/ontologies/2022/4/silvanusOntology#Constructed_barrier"/>
        <rdfs:comment>A fence is a constructed barrier which is generally of lighter construction than a wall and used to provide visual sectioning of spaces.</rdfs:comment>
        <rdfs:seeAlso>http://purl.obolibrary.org/obo/ENVO_01000468</rdfs:seeAlso>
    </owl:Class>
    


    <!-- http://www.semanticweb.org/smarotta/ontologies/2022/4/silvanusOntology#Fine_fuel_moisture -->

    <owl:Class rdf:about="http://www.semanticweb.org/smarotta/ontologies/2022/4/silvanusOntology#Fine_fuel_moisture">
        <rdfs:subClassOf rdf:resource="http://www.semanticweb.org/smarotta/ontologies/2022/4/silvanusOntology#Moisture"/>
        <silvanusOntology:source>https://cwfis.cfs.nrcan.gc.ca/background/summary/fwi</silvanusOntology:source>
        <rdfs:comment>The Fine Fuel Moisture Code (FFMC) is a numeric rating of the moisture content of litter and other cured fine fuels. This code is an indicator of the relative ease of ignition and the flammability of fine fuel.</rdfs:comment>
    </owl:Class>
    


    <!-- http://www.semanticweb.org/smarotta/ontologies/2022/4/silvanusOntology#Fire -->

    <owl:Class rdf:about="http://www.semanticweb.org/smarotta/ontologies/2022/4/silvanusOntology#Fire">
        <rdfs:comment>It&apos;s the rapid oxidation of a material in the exothermic chemical process of combustion, releasing heat, light, and various reaction products.</rdfs:comment>
        <rdfs:seeAlso>http://cerrado.linkeddata.es/ecology/fire#Fire</rdfs:seeAlso>
    </owl:Class>
    


    <!-- http://www.semanticweb.org/smarotta/ontologies/2022/4/silvanusOntology#Fire-prone_invasive_specie -->

    <owl:Class rdf:about="http://www.semanticweb.org/smarotta/ontologies/2022/4/silvanusOntology#Fire-prone_invasive_specie">
        <rdfs:subClassOf rdf:resource="http://www.semanticweb.org/smarotta/ontologies/2022/4/silvanusOntology#Vegetation_type"/>
        <silvanusOntology:input>Known locations (from land cover maps, citizen science data repositories and location uploaded by stakeholders); topography and infrastructures to further assess risk of invasion</silvanusOntology:input>
        <silvanusOntology:output>Map of distribution of invasive species and list of locations requiring preventive action</silvanusOntology:output>
        <silvanusOntology:source>Portuguese pilot</silvanusOntology:source>
        <rdfs:comment>Location of patches or individuals of fire-prone invasive species; their presence in the landscape aggravates the potential ecological and socio-economic effects of wildfires, thus requiring preventive measures to remove or control their expansion.</rdfs:comment>
    </owl:Class>
    


    <!-- http://www.semanticweb.org/smarotta/ontologies/2022/4/silvanusOntology#Fire-resistant_species -->

    <owl:Class rdf:about="http://www.semanticweb.org/smarotta/ontologies/2022/4/silvanusOntology#Fire-resistant_species">
        <rdfs:subClassOf rdf:resource="http://www.semanticweb.org/smarotta/ontologies/2022/4/silvanusOntology#Vegetation_type"/>
        <silvanusOntology:source>https://www.fs.fed.us/database/feis/glossary2.html</silvanusOntology:source>
        <rdfs:comment>Species with morphological characteristics that give it a lower probability of being injured or killed by fire than a fire-sensitive species</rdfs:comment>
    </owl:Class>
    


    <!-- http://www.semanticweb.org/smarotta/ontologies/2022/4/silvanusOntology#Fire-sensitive_species -->

    <owl:Class rdf:about="http://www.semanticweb.org/smarotta/ontologies/2022/4/silvanusOntology#Fire-sensitive_species">
        <rdfs:subClassOf rdf:resource="http://www.semanticweb.org/smarotta/ontologies/2022/4/silvanusOntology#Vegetation_type"/>
        <silvanusOntology:source>https://www.fs.fed.us/database/feis/glossary2.html</silvanusOntology:source>
        <rdfs:comment>A species with a &quot;relatively high&quot; probability of being injured or killed by fire [83]. Compare with fire-resistant species</rdfs:comment>
    </owl:Class>
    


    <!-- http://www.semanticweb.org/smarotta/ontologies/2022/4/silvanusOntology#Fire_Frequency -->

    <owl:Class rdf:about="http://www.semanticweb.org/smarotta/ontologies/2022/4/silvanusOntology#Fire_Frequency">
        <rdfs:subClassOf rdf:resource="http://www.semanticweb.org/smarotta/ontologies/2022/4/silvanusOntology#Fire_characteristic"/>
        <rdfs:comment>The average time interval between successive fires or the number of fires within a specific period of time.</rdfs:comment>
        <rdfs:seeAlso>http://cerrado.linkeddata.es/ecology/fire#FireFrequency</rdfs:seeAlso>
    </owl:Class>
    


    <!-- http://www.semanticweb.org/smarotta/ontologies/2022/4/silvanusOntology#Fire_Station -->

    <owl:Class rdf:about="http://www.semanticweb.org/smarotta/ontologies/2022/4/silvanusOntology#Fire_Station">
        <rdfs:subClassOf rdf:resource="http://www.semanticweb.org/smarotta/ontologies/2022/4/silvanusOntology#Public_Safety_Facility"/>
        <owl:disjointWith rdf:resource="http://www.semanticweb.org/smarotta/ontologies/2022/4/silvanusOntology#Police_Station"/>
        <rdfs:comment rdf:datatype="http://www.w3.org/2001/XMLSchema#string">A Public Safety Facility that is designed for the storage of firefighting apparatus.</rdfs:comment>
        <rdfs:seeAlso>http://www.ontologylibrary.mil/CommonCore/Mid/ArtifactOntology#FireStation</rdfs:seeAlso>
    </owl:Class>
    


    <!-- http://www.semanticweb.org/smarotta/ontologies/2022/4/silvanusOntology#Fire_access_path -->

    <owl:Class rdf:about="http://www.semanticweb.org/smarotta/ontologies/2022/4/silvanusOntology#Fire_access_path">
        <rdfs:subClassOf rdf:resource="http://www.semanticweb.org/smarotta/ontologies/2022/4/silvanusOntology#Fire_characteristic"/>
        <silvanusOntology:source>French pilot</silvanusOntology:source>
        <rdfs:comment>Identification of fire access paths for fireghting apparatus</rdfs:comment>
    </owl:Class>
    


    <!-- http://www.semanticweb.org/smarotta/ontologies/2022/4/silvanusOntology#Fire_characteristic -->

    <owl:Class rdf:about="http://www.semanticweb.org/smarotta/ontologies/2022/4/silvanusOntology#Fire_characteristic">
        <rdfs:comment>Represents parameters used to describe the characteristics or behavior of a fire event.</rdfs:comment>
        <rdfs:seeAlso>http://cerrado.linkeddata.es/ecology/fire#FireCharacteristic</rdfs:seeAlso>
    </owl:Class>
    


    <!-- http://www.semanticweb.org/smarotta/ontologies/2022/4/silvanusOntology#Fire_critical_point -->

    <owl:Class rdf:about="http://www.semanticweb.org/smarotta/ontologies/2022/4/silvanusOntology#Fire_critical_point">
        <rdfs:subClassOf rdf:resource="http://www.semanticweb.org/smarotta/ontologies/2022/4/silvanusOntology#Fire_characteristic"/>
        <silvanusOntology:source>Italian pilot</silvanusOntology:source>
        <rdfs:comment>The point where the fire increases intensity and / or speed</rdfs:comment>
    </owl:Class>
    


    <!-- http://www.semanticweb.org/smarotta/ontologies/2022/4/silvanusOntology#Fire_department -->

    <owl:Class rdf:about="http://www.semanticweb.org/smarotta/ontologies/2022/4/silvanusOntology#Fire_department">
        <rdfs:subClassOf rdf:resource="http://www.semanticweb.org/smarotta/ontologies/2022/4/silvanusOntology#Infrastructure"/>
        <rdfs:comment>Represents fire departments.</rdfs:comment>
        <rdfs:seeAlso>https://raw.githubusercontent.com/beAWARE-project/ontology/master/beAWARE_ontology#FireDepartment</rdfs:seeAlso>
    </owl:Class>
    


    <!-- http://www.semanticweb.org/smarotta/ontologies/2022/4/silvanusOntology#Fire_distance -->

    <owl:Class rdf:about="http://www.semanticweb.org/smarotta/ontologies/2022/4/silvanusOntology#Fire_distance">
        <rdfs:subClassOf rdf:resource="http://www.semanticweb.org/smarotta/ontologies/2022/4/silvanusOntology#Fire_characteristic"/>
        <silvanusOntology:source>Greek pilot</silvanusOntology:source>
        <rdfs:comment>Distance of fire front from an individual</rdfs:comment>
    </owl:Class>
    


    <!-- http://www.semanticweb.org/smarotta/ontologies/2022/4/silvanusOntology#Fire_intensity -->

    <owl:Class rdf:about="http://www.semanticweb.org/smarotta/ontologies/2022/4/silvanusOntology#Fire_intensity">
        <rdfs:subClassOf rdf:resource="http://www.semanticweb.org/smarotta/ontologies/2022/4/silvanusOntology#Fire_characteristic"/>
        <silvanusOntology:source>https://www.fs.fed.us/database/feis/glossary2.html#FireIntensity</silvanusOntology:source>
        <rdfs:comment>A general term relating to the heat energy released in a fire [63,83]. Wherever possible, FEIS uses more specific terms to describe rate of heat release. See fireline intensity below. Energy output from fire.</rdfs:comment>
        <rdfs:seeAlso>http://cerrado.linkeddata.es/ecology/fire#FireIntensity</rdfs:seeAlso>
    </owl:Class>
    


    <!-- http://www.semanticweb.org/smarotta/ontologies/2022/4/silvanusOntology#Fire_interval -->

    <owl:Class rdf:about="http://www.semanticweb.org/smarotta/ontologies/2022/4/silvanusOntology#Fire_interval">
        <rdfs:subClassOf rdf:resource="http://www.semanticweb.org/smarotta/ontologies/2022/4/silvanusOntology#Temporal_entity"/>
        <silvanusOntology:source>https://www.fs.fed.us/database/feis/glossary2.html</silvanusOntology:source>
        <rdfs:comment>Number of years between two successive fires in a specified area. The size of the area must be clearly specified [83,91]. Often used to designate an average of intervals (i.e., mean fire interval).</rdfs:comment>
    </owl:Class>
    


    <!-- http://www.semanticweb.org/smarotta/ontologies/2022/4/silvanusOntology#Fire_prediction -->

    <owl:Class rdf:about="http://www.semanticweb.org/smarotta/ontologies/2022/4/silvanusOntology#Fire_prediction">
        <rdfs:subClassOf rdf:resource="http://www.semanticweb.org/smarotta/ontologies/2022/4/silvanusOntology#Fire_characteristic"/>
        <silvanusOntology:source>French pilot</silvanusOntology:source>
        <rdfs:comment>Anticipation of fire development and development axes</rdfs:comment>
    </owl:Class>
    


    <!-- http://www.semanticweb.org/smarotta/ontologies/2022/4/silvanusOntology#Fire_regime_condition_class -->

    <owl:Class rdf:about="http://www.semanticweb.org/smarotta/ontologies/2022/4/silvanusOntology#Fire_regime_condition_class">
        <rdfs:subClassOf rdf:resource="http://www.semanticweb.org/smarotta/ontologies/2022/4/silvanusOntology#Biodiversity_index"/>
        <silvanusOntology:source>https://www.fs.fed.us/database/feis/glossary2.html</silvanusOntology:source>
        <rdfs:comment>A standardized, interagency index to measure the departure of current conditions from reference or historical conditions [74]. The fire regime condition classes are [9]:</rdfs:comment>
    </owl:Class>
    


    <!-- http://www.semanticweb.org/smarotta/ontologies/2022/4/silvanusOntology#Fire_risk -->

    <owl:Class rdf:about="http://www.semanticweb.org/smarotta/ontologies/2022/4/silvanusOntology#Fire_risk">
        <silvanusOntology:input>Updated land cover from UAV or satellite (resolution adapted to mapping scale), topography, infrastructures (to protect) and road accessibility.</silvanusOntology:input>
        <silvanusOntology:output>Map of fire hazard risk</silvanusOntology:output>
        <silvanusOntology:source>Portuguese pilot</silvanusOntology:source>
        <rdfs:comment>&quot;Map of fire hazard risk at the landscape and farm/local scale (resolution to be adapted to scale requirements). Relevant to identify priority areas for preventive biomass management
(portugese fire hazard risk reference - https://florestas.pt/saiba-mais/como-se-calcula-o-indice-de-risco-de-incendio-florestal/)&quot;</rdfs:comment>
        <rdfs:seeAlso>http://cerrado.linkeddata.es/ecology/fire#FireRisk</rdfs:seeAlso>
    </owl:Class>
    


    <!-- http://www.semanticweb.org/smarotta/ontologies/2022/4/silvanusOntology#Fire_severity -->

    <owl:Class rdf:about="http://www.semanticweb.org/smarotta/ontologies/2022/4/silvanusOntology#Fire_severity">
        <rdfs:subClassOf rdf:resource="http://www.semanticweb.org/smarotta/ontologies/2022/4/silvanusOntology#Fire_characteristic"/>
        <silvanusOntology:source>https://www.fs.fed.us/database/feis/glossary2.html</silvanusOntology:source>
        <rdfs:comment>Fire severity generally indicates the degree of environmental change caused by fire [92,118]. The FRCC guidebook classifies levels of fire severity as low, mixed, and replacement.</rdfs:comment>
        <rdfs:seeAlso>http://cerrado.linkeddata.es/ecology/fire#FireSeverity</rdfs:seeAlso>
    </owl:Class>
    


    <!-- http://www.semanticweb.org/smarotta/ontologies/2022/4/silvanusOntology#Fire_speed -->

    <owl:Class rdf:about="http://www.semanticweb.org/smarotta/ontologies/2022/4/silvanusOntology#Fire_speed">
        <rdfs:subClassOf rdf:resource="http://www.semanticweb.org/smarotta/ontologies/2022/4/silvanusOntology#Fire_characteristic"/>
        <rdfs:comment>it&apos;s the average speed of the fire front.</rdfs:comment>
        <rdfs:seeAlso>http://cerrado.linkeddata.es/ecology/fire#FireSpeed</rdfs:seeAlso>
    </owl:Class>
    


    <!-- http://www.semanticweb.org/smarotta/ontologies/2022/4/silvanusOntology#Fire_spread_direction -->

    <owl:Class rdf:about="http://www.semanticweb.org/smarotta/ontologies/2022/4/silvanusOntology#Fire_spread_direction">
        <rdfs:subClassOf rdf:resource="http://www.semanticweb.org/smarotta/ontologies/2022/4/silvanusOntology#Fire_characteristic"/>
        <rdfs:comment>It&apos;s how the fire event is spreading, the directions.</rdfs:comment>
        <rdfs:seeAlso>http://cerrado.linkeddata.es/ecology/fire#FireSpread</rdfs:seeAlso>
    </owl:Class>
    


    <!-- http://www.semanticweb.org/smarotta/ontologies/2022/4/silvanusOntology#Fire_strategy -->

    <owl:Class rdf:about="http://www.semanticweb.org/smarotta/ontologies/2022/4/silvanusOntology#Fire_strategy">
        <rdfs:subClassOf rdf:resource="http://www.semanticweb.org/smarotta/ontologies/2022/4/silvanusOntology#Vegetation_stat"/>
        <silvanusOntology:source>https://botany.one/2020/10/four-plant-strategies-to-deal-with-fire/</silvanusOntology:source>
        <rdfs:comment>Plant species and populations have different strategies of  responding to fires. Some species can survive fires (resprouters), disperse their seeds in the soil before fires (geosporous), others die (non-sprouters) or disperse seeds postfires (serotinous).</rdfs:comment>
    </owl:Class>
    


    <!-- http://www.semanticweb.org/smarotta/ontologies/2022/4/silvanusOntology#Fire_weather_index -->

    <owl:Class rdf:about="http://www.semanticweb.org/smarotta/ontologies/2022/4/silvanusOntology#Fire_weather_index">
        <silvanusOntology:source>https://cwfis.cfs.nrcan.gc.ca/background/summary/fwi</silvanusOntology:source>
        <rdfs:comment>The Fire Weather Index (FWI) is a numeric rating of fire intensity. It is based on the ISI and the BUI, and is used as a general index of fire danger throughout the forested areas of Canada.</rdfs:comment>
    </owl:Class>
    


    <!-- http://www.semanticweb.org/smarotta/ontologies/2022/4/silvanusOntology#Firebreak -->

    <owl:Class rdf:about="http://www.semanticweb.org/smarotta/ontologies/2022/4/silvanusOntology#Firebreak">
        <rdfs:subClassOf rdf:resource="http://www.semanticweb.org/smarotta/ontologies/2022/4/silvanusOntology#Response_resource"/>
        <rdfs:comment>An obstacle to the spread of fire, such as a strip of open space in a forest. .The location of firebreaks (natural and man-made) is important for the modelling of the fire spread behaviour, as well as for monitoring the state of the firebreak and if it needs clearing.</rdfs:comment>
    </owl:Class>
    


    <!-- http://www.semanticweb.org/smarotta/ontologies/2022/4/silvanusOntology#Firefighting_unit -->

    <owl:Class rdf:about="http://www.semanticweb.org/smarotta/ontologies/2022/4/silvanusOntology#Firefighting_unit">
        <rdfs:subClassOf rdf:resource="http://www.semanticweb.org/smarotta/ontologies/2022/4/silvanusOntology#Responder"/>
        <rdfs:comment>Individual firefighter</rdfs:comment>
        <rdfs:seeAlso>http://www.semanticweb.org/earthquake#FireBrigade</rdfs:seeAlso>
    </owl:Class>
    


    <!-- http://www.semanticweb.org/smarotta/ontologies/2022/4/silvanusOntology#Fireline_intensity -->

    <owl:Class rdf:about="http://www.semanticweb.org/smarotta/ontologies/2022/4/silvanusOntology#Fireline_intensity">
        <rdfs:subClassOf rdf:resource="http://www.semanticweb.org/smarotta/ontologies/2022/4/silvanusOntology#Fire_intensity"/>
        <silvanusOntology:source>https://www.fs.fed.us/database/feis/glossary2.html#FirelineIntensity</silvanusOntology:source>
        <rdfs:comment>The rate of heat release per unit time per unit length of fire front. Numerically, the product of the heat of combustion, quantity of fuel consumed per unit area in the fire front, and the rate of spread of a fire, expressed in kW/m [83]. Not synonymous with fire severity, which refers to the degree of environmental change caused by fire.</rdfs:comment>
    </owl:Class>
    


    <!-- http://www.semanticweb.org/smarotta/ontologies/2022/4/silvanusOntology#First_Aid_Kit -->

    <owl:Class rdf:about="http://www.semanticweb.org/smarotta/ontologies/2022/4/silvanusOntology#First_Aid_Kit">
        <rdfs:subClassOf rdf:resource="http://www.semanticweb.org/smarotta/ontologies/2022/4/silvanusOntology#ReliefItem"/>
        <rdfs:comment>First-aid kit items</rdfs:comment>
        <rdfs:seeAlso>http://www.semanticweb.org/earthquake#First_Aid_Kit</rdfs:seeAlso>
    </owl:Class>
    


    <!-- http://www.semanticweb.org/smarotta/ontologies/2022/4/silvanusOntology#Flame_ground_temperature -->

    <owl:Class rdf:about="http://www.semanticweb.org/smarotta/ontologies/2022/4/silvanusOntology#Flame_ground_temperature">
        <rdfs:subClassOf rdf:resource="http://www.semanticweb.org/smarotta/ontologies/2022/4/silvanusOntology#Fire_characteristic"/>
        <silvanusOntology:source>French pilot</silvanusOntology:source>
        <rdfs:comment>Ground temperature of the flames</rdfs:comment>
    </owl:Class>
    


    <!-- http://www.semanticweb.org/smarotta/ontologies/2022/4/silvanusOntology#Flame_height -->

    <owl:Class rdf:about="http://www.semanticweb.org/smarotta/ontologies/2022/4/silvanusOntology#Flame_height">
        <rdfs:subClassOf rdf:resource="http://www.semanticweb.org/smarotta/ontologies/2022/4/silvanusOntology#Fire_characteristic"/>
        <silvanusOntology:source>https://www.fs.fed.us/database/feis/glossary2.html</silvanusOntology:source>
        <rdfs:comment>The length of flames in a fire front measured along the slant of the flame, from the midpoint of its base to its tip. Flame length is mathematically related to fireline intensity and tree crown scorch height.
Its the maximum height a flame achieve in a fire event.</rdfs:comment>
        <rdfs:seeAlso>http://cerrado.linkeddata.es/ecology/fire#FlameHeight</rdfs:seeAlso>
    </owl:Class>
    


    <!-- http://www.semanticweb.org/smarotta/ontologies/2022/4/silvanusOntology#Flower_Strip -->

    <owl:Class rdf:about="http://www.semanticweb.org/smarotta/ontologies/2022/4/silvanusOntology#Flower_Strip">
        <rdfs:subClassOf rdf:resource="http://www.semanticweb.org/smarotta/ontologies/2022/4/silvanusOntology#Vegetated_area"/>
        <rdfs:comment>A vegetated area which includes a community of flowering plants that provide food for local pollinators.</rdfs:comment>
        <rdfs:seeAlso>http://purl.obolibrary.org/obo/ENVO_01000848</rdfs:seeAlso>
    </owl:Class>
    


    <!-- http://www.semanticweb.org/smarotta/ontologies/2022/4/silvanusOntology#FoodAndShelter -->

    <owl:Class rdf:about="http://www.semanticweb.org/smarotta/ontologies/2022/4/silvanusOntology#FoodAndShelter">
        <rdfs:subClassOf rdf:resource="http://www.semanticweb.org/smarotta/ontologies/2022/4/silvanusOntology#Response_resource"/>
        <rdfs:comment>Sustainment for those affected by a fire</rdfs:comment>
        <rdfs:seeAlso>http://www.semanticweb.org/earthquake#FoodAndShelter</rdfs:seeAlso>
    </owl:Class>
    


    <!-- http://www.semanticweb.org/smarotta/ontologies/2022/4/silvanusOntology#Forest -->

    <owl:Class rdf:about="http://www.semanticweb.org/smarotta/ontologies/2022/4/silvanusOntology#Forest">
        <rdfs:subClassOf rdf:resource="http://www.semanticweb.org/smarotta/ontologies/2022/4/silvanusOntology#Biodiversity_index"/>
        <silvanusOntology:source>https://www.fs.fed.us/database/feis/glossary2.html</silvanusOntology:source>
        <rdfs:comment>A formation dominated by trees, in which the canopy is more closed than open [112]. Generally, overstory trees are &gt;16 feet (5 m) tall and have 60% to 100% cover [75]. When describing forests, use of a dash indicates an overstory/understory relationship (e.g., northern red oak/America witch-hazel forest). Compare with grassland, shrubland, wooded shrubland, woodland, savanna.</rdfs:comment>
    </owl:Class>
    


    <!-- http://www.semanticweb.org/smarotta/ontologies/2022/4/silvanusOntology#Forest_fire -->

    <owl:Class rdf:about="http://www.semanticweb.org/smarotta/ontologies/2022/4/silvanusOntology#Forest_fire">
        <rdfs:subClassOf rdf:resource="http://www.semanticweb.org/smarotta/ontologies/2022/4/silvanusOntology#Fire"/>
        <rdfs:comment>A fire that occurs in a wooded area.</rdfs:comment>
        <rdfs:seeAlso>http://cerrado.linkeddata.es/ecology/fire#ForestFire</rdfs:seeAlso>
    </owl:Class>
    


    <!-- http://www.semanticweb.org/smarotta/ontologies/2022/4/silvanusOntology#Forest_type -->

    <owl:Class rdf:about="http://www.semanticweb.org/smarotta/ontologies/2022/4/silvanusOntology#Forest_type">
        <rdfs:subClassOf rdf:resource="http://www.semanticweb.org/smarotta/ontologies/2022/4/silvanusOntology#Vegetation_type"/>
        <rdfs:comment>Type of Forest</rdfs:comment>
        <rdfs:seeAlso>http://crossforest.eu/ilu/ontology/ForestType</rdfs:seeAlso>
    </owl:Class>
    


    <!-- http://www.semanticweb.org/smarotta/ontologies/2022/4/silvanusOntology#Fuel -->

    <owl:Class rdf:about="http://www.semanticweb.org/smarotta/ontologies/2022/4/silvanusOntology#Fuel">
        <rdfs:subClassOf rdf:resource="http://www.semanticweb.org/smarotta/ontologies/2022/4/silvanusOntology#Biodiversity_index"/>
        <silvanusOntology:input>Updated land cover from UAV or satellite (resolution adapted to mapping scale), LIDAR data, in-situ data or estimated volume of fuel classes per land cover type</silvanusOntology:input>
        <silvanusOntology:output>Map of fuel distribution</silvanusOntology:output>
        <silvanusOntology:source>https://www.fs.fed.us/database/feis/glossary2.html#fuel</silvanusOntology:source>
        <rdfs:comment>Fuel is comprised of living and dead vegetation that can be ignited. It is often classified as dead or alive and as natural fuels or those from logging operations. Fuel components refer to such items as downed dead woody material in various size classes, litter, duff, herbaceous vegetation, live foliage, etc. [20].</rdfs:comment>
    </owl:Class>
    


    <!-- http://www.semanticweb.org/smarotta/ontologies/2022/4/silvanusOntology#Fuel_class -->

    <owl:Class rdf:about="http://www.semanticweb.org/smarotta/ontologies/2022/4/silvanusOntology#Fuel_class">
        <rdfs:subClassOf rdf:resource="http://www.semanticweb.org/smarotta/ontologies/2022/4/silvanusOntology#Biodiversity_index"/>
        <silvanusOntology:source>https://www.fs.fed.us/database/feis/glossary2.html#FuelClass</silvanusOntology:source>
        <rdfs:comment>A set of fuels with similar traits. Fuels are categorized as herbaceous or woody and live or dead. Dead fuels are classed as 1-, 10-, 100-, or 1,000-hour timelag fuels, based on the time needed for fuel moisture to come into equilibrium with the environment [92]:</rdfs:comment>
    </owl:Class>
    


    <!-- http://www.semanticweb.org/smarotta/ontologies/2022/4/silvanusOntology#Fuel_continuity -->

    <owl:Class rdf:about="http://www.semanticweb.org/smarotta/ontologies/2022/4/silvanusOntology#Fuel_continuity">
        <rdfs:subClassOf rdf:resource="http://www.semanticweb.org/smarotta/ontologies/2022/4/silvanusOntology#Biodiversity_index"/>
        <silvanusOntology:source>https://www.fs.fed.us/database/feis/glossary2.html#FuelContinuity</silvanusOntology:source>
        <rdfs:comment>A qualitative description of the distribution of fuels both horizontally and vertically. Continuous fuels readily support fire spread. The larger the fuel discontinuity, the greater the fire intensity required for fire spread [20].</rdfs:comment>
    </owl:Class>
    


    <!-- http://www.semanticweb.org/smarotta/ontologies/2022/4/silvanusOntology#Fuel_loading -->

    <owl:Class rdf:about="http://www.semanticweb.org/smarotta/ontologies/2022/4/silvanusOntology#Fuel_loading">
        <rdfs:subClassOf rdf:resource="http://www.semanticweb.org/smarotta/ontologies/2022/4/silvanusOntology#Biodiversity_index"/>
        <silvanusOntology:source>https://www.fs.fed.us/database/feis/glossary2.html#FuelLoading</silvanusOntology:source>
        <rdfs:comment>The weight per unit area of fuel, often expressed in tons/acre or tonnes/hectare. Dead woody fuel loadings are commonly described for small material in diameter classes of 0 to 1/4, 1/4 to 1, and 1 to 3 inches and for large material in one class greater than 3 inches [20].</rdfs:comment>
    </owl:Class>
    


    <!-- http://www.semanticweb.org/smarotta/ontologies/2022/4/silvanusOntology#Garbage_collection -->

    <owl:Class rdf:about="http://www.semanticweb.org/smarotta/ontologies/2022/4/silvanusOntology#Garbage_collection">
        <rdfs:subClassOf rdf:resource="http://www.semanticweb.org/smarotta/ontologies/2022/4/silvanusOntology#Infrastructure"/>
        <rdfs:comment>Represents garbage collection infrastructure and services.</rdfs:comment>
        <rdfs:seeAlso>https://raw.githubusercontent.com/beAWARE-project/ontology/master/beAWARE_ontology#GarbageCollection</rdfs:seeAlso>
    </owl:Class>
    


    <!-- http://www.semanticweb.org/smarotta/ontologies/2022/4/silvanusOntology#Gas_emission -->

    <owl:Class rdf:about="http://www.semanticweb.org/smarotta/ontologies/2022/4/silvanusOntology#Gas_emission">
        <rdfs:subClassOf rdf:resource="http://www.semanticweb.org/smarotta/ontologies/2022/4/silvanusOntology#Natural"/>
        <silvanusOntology:source>https://effis-gwis-cms.s3-eu-west-1.amazonaws.com/effis/reports-and-publications/effis-related-publications/lb-na-25-923-en-n.pdf (page 10)</silvanusOntology:source>
        <rdfs:comment>Wildfire caused by natural emissions of gas (e.g. coming from peat bog) that can</rdfs:comment>
    </owl:Class>
    


    <!-- http://www.semanticweb.org/smarotta/ontologies/2022/4/silvanusOntology#Gas_sensor -->

    <owl:Class rdf:about="http://www.semanticweb.org/smarotta/ontologies/2022/4/silvanusOntology#Gas_sensor">
        <rdfs:subClassOf rdf:resource="http://www.semanticweb.org/smarotta/ontologies/2022/4/silvanusOntology#Chemical_sensor"/>
        <silvanusOntology:source>French pilot</silvanusOntology:source>
        <rdfs:comment>Gas sensors are devices that can detect the presence and concentration of various hazardous gases and vapors, such as toxic or explosive gases, volatile organic compounds (VOCs), humidity, and odors</rdfs:comment>
    </owl:Class>
    


    <!-- http://www.semanticweb.org/smarotta/ontologies/2022/4/silvanusOntology#Geocentric_Position -->

    <owl:Class rdf:about="http://www.semanticweb.org/smarotta/ontologies/2022/4/silvanusOntology#Geocentric_Position">
        <rdfs:subClassOf rdf:resource="http://www.semanticweb.org/smarotta/ontologies/2022/4/silvanusOntology#Position"/>
        <rdfs:comment>Position that uses a geodetic coordinate reference system</rdfs:comment>
        <rdfs:seeAlso>http://crossforest.eu/position/ontology/GeocentricPosition</rdfs:seeAlso>
    </owl:Class>
    


    <!-- http://www.semanticweb.org/smarotta/ontologies/2022/4/silvanusOntology#Geology -->

    <owl:Class rdf:about="http://www.semanticweb.org/smarotta/ontologies/2022/4/silvanusOntology#Geology">
        <rdfs:subClassOf rdf:resource="http://www.semanticweb.org/smarotta/ontologies/2022/4/silvanusOntology#Biodiversity_index"/>
        <silvanusOntology:source>Italian pilot</silvanusOntology:source>
        <rdfs:comment>Geology describes the structure of the Earth on and beneath its surface, and the processes that have shaped that structure.</rdfs:comment>
    </owl:Class>
    


    <!-- http://www.semanticweb.org/smarotta/ontologies/2022/4/silvanusOntology#Geosporous -->

    <owl:Class rdf:about="http://www.semanticweb.org/smarotta/ontologies/2022/4/silvanusOntology#Geosporous">
        <rdfs:subClassOf rdf:resource="http://www.semanticweb.org/smarotta/ontologies/2022/4/silvanusOntology#Fire_strategy"/>
        <silvanusOntology:source>https://botany.one/2020/10/four-plant-strategies-to-deal-with-fire/</silvanusOntology:source>
        <rdfs:comment>Species disperse their seeds in the soil before fires</rdfs:comment>
    </owl:Class>
    


    <!-- http://www.semanticweb.org/smarotta/ontologies/2022/4/silvanusOntology#Government_policy -->

    <owl:Class rdf:about="http://www.semanticweb.org/smarotta/ontologies/2022/4/silvanusOntology#Government_policy">
        <silvanusOntology:source>Indonesian pilot</silvanusOntology:source>
        <rdfs:comment>Policy adopted by the local government</rdfs:comment>
    </owl:Class>
    


    <!-- http://www.semanticweb.org/smarotta/ontologies/2022/4/silvanusOntology#Grassland -->

    <owl:Class rdf:about="http://www.semanticweb.org/smarotta/ontologies/2022/4/silvanusOntology#Grassland">
        <rdfs:subClassOf rdf:resource="http://www.semanticweb.org/smarotta/ontologies/2022/4/silvanusOntology#Biodiversity_index"/>
        <silvanusOntology:source>https://www.fs.fed.us/database/feis/glossary2.html#grassland</silvanusOntology:source>
        <rdfs:comment>A formation dominated by grasses (&gt;25% cover), with shrubs and trees constituting &lt;25% of total cover [75]. Compare with shrubland, woodland, wooded shrubland, savanna, forest.</rdfs:comment>
    </owl:Class>
    


    <!-- http://www.semanticweb.org/smarotta/ontologies/2022/4/silvanusOntology#Grassland_Area -->

    <owl:Class rdf:about="http://www.semanticweb.org/smarotta/ontologies/2022/4/silvanusOntology#Grassland_Area">
        <rdfs:subClassOf rdf:resource="http://www.semanticweb.org/smarotta/ontologies/2022/4/silvanusOntology#Vegetated_area"/>
        <rdfs:comment>An area in which grasses (Graminae) are a significant component of the vegetation.</rdfs:comment>
        <rdfs:seeAlso>http://purl.obolibrary.org/obo/ENVO_00000106</rdfs:seeAlso>
    </owl:Class>
    


    <!-- http://www.semanticweb.org/smarotta/ontologies/2022/4/silvanusOntology#Grazing_activity -->

    <owl:Class rdf:about="http://www.semanticweb.org/smarotta/ontologies/2022/4/silvanusOntology#Grazing_activity">
        <rdfs:subClassOf rdf:resource="http://www.semanticweb.org/smarotta/ontologies/2022/4/silvanusOntology#Biodiversity_index"/>
        <silvanusOntology:input>GPS location points (with high temporal resolution), movement sensor data (x,y,z - to model behaviour), and land cover maps</silvanusOntology:input>
        <silvanusOntology:output>Maps of grazing activity to support grazing management</silvanusOntology:output>
        <silvanusOntology:source>Portuguese pilot</silvanusOntology:source>
        <rdfs:comment>Report on grazing activity - areas of higher activity; daily, monthly and annual patterns of habitat selection and dominant behaviour per area (resting, grazing, moving/walking)</rdfs:comment>
    </owl:Class>
    


    <!-- http://www.semanticweb.org/smarotta/ontologies/2022/4/silvanusOntology#Ground_Motor_Vehicle -->

    <owl:Class rdf:about="http://www.semanticweb.org/smarotta/ontologies/2022/4/silvanusOntology#Ground_Motor_Vehicle">
        <rdfs:subClassOf rdf:resource="http://www.semanticweb.org/smarotta/ontologies/2022/4/silvanusOntology#Ground_Vehicle"/>
        <rdfs:comment>A land-based motorized vehicle that traveled on the ground/land</rdfs:comment>
        <rdfs:seeAlso>http://www.ontologylibrary.mil/CommonCore/Mid/ArtifactOntology#GroundMotorVehicle</rdfs:seeAlso>
    </owl:Class>
    


    <!-- http://www.semanticweb.org/smarotta/ontologies/2022/4/silvanusOntology#Ground_Vehicle -->

    <owl:Class rdf:about="http://www.semanticweb.org/smarotta/ontologies/2022/4/silvanusOntology#Ground_Vehicle">
        <rdfs:subClassOf rdf:resource="http://www.semanticweb.org/smarotta/ontologies/2022/4/silvanusOntology#Response_vehicle"/>
        <rdfs:comment>A land-based vehicle that traveled on the ground/land</rdfs:comment>
        <rdfs:seeAlso>http://www.ontologylibrary.mil/CommonCore/Mid/ArtifactOntology#GroundVehicle</rdfs:seeAlso>
    </owl:Class>
    


    <!-- http://www.semanticweb.org/smarotta/ontologies/2022/4/silvanusOntology#Ground_fire -->

    <owl:Class rdf:about="http://www.semanticweb.org/smarotta/ontologies/2022/4/silvanusOntology#Ground_fire">
        <rdfs:subClassOf rdf:resource="http://www.semanticweb.org/smarotta/ontologies/2022/4/silvanusOntology#Fire"/>
        <silvanusOntology:source>https://www.fs.fed.us/database/feis/glossary2.html#GroundFire</silvanusOntology:source>
        <rdfs:comment>Fire that burns in the organic material below the litter layer, mostly by smoldering combustion. Fires in duff, peat, dry or dead moss and lichens, and/or punky wood are typically ground fires [20].</rdfs:comment>
    </owl:Class>
    


    <!-- http://www.semanticweb.org/smarotta/ontologies/2022/4/silvanusOntology#Hazard-reduction_fire -->

    <owl:Class rdf:about="http://www.semanticweb.org/smarotta/ontologies/2022/4/silvanusOntology#Hazard-reduction_fire">
        <rdfs:subClassOf rdf:resource="http://www.semanticweb.org/smarotta/ontologies/2022/4/silvanusOntology#Controlled_fire"/>
        <rdfs:comment>It&apos;s a fire set in order to prevent large and severe events of burning.</rdfs:comment>
        <rdfs:seeAlso>http://cerrado.linkeddata.es/ecology/fire#HarzardReductionFire</rdfs:seeAlso>
    </owl:Class>
    


    <!-- http://www.semanticweb.org/smarotta/ontologies/2022/4/silvanusOntology#Health_sensor -->

    <owl:Class rdf:about="http://www.semanticweb.org/smarotta/ontologies/2022/4/silvanusOntology#Health_sensor">
        <rdfs:subClassOf rdf:resource="http://www.semanticweb.org/smarotta/ontologies/2022/4/silvanusOntology#Sensor"/>
        <silvanusOntology:source>Greek pilot</silvanusOntology:source>
        <silvanusOntology:source>Slovak pilot</silvanusOntology:source>
        <rdfs:comment>A sensor capable of collecting health-related parameters</rdfs:comment>
    </owl:Class>
    


    <!-- http://www.semanticweb.org/smarotta/ontologies/2022/4/silvanusOntology#Heart_rate_monitor -->

    <owl:Class rdf:about="http://www.semanticweb.org/smarotta/ontologies/2022/4/silvanusOntology#Heart_rate_monitor">
        <rdfs:subClassOf rdf:resource="http://www.semanticweb.org/smarotta/ontologies/2022/4/silvanusOntology#Health_sensor"/>
        <silvanusOntology:source>AHEPA</silvanusOntology:source>
        <rdfs:comment>A heart rate monitor (HRM) is a personal monitoring device that allows one to measure/display heart rate in real time or record the heart rate for later study.</rdfs:comment>
    </owl:Class>
    


    <!-- http://www.semanticweb.org/smarotta/ontologies/2022/4/silvanusOntology#Heath -->

    <owl:Class rdf:about="http://www.semanticweb.org/smarotta/ontologies/2022/4/silvanusOntology#Heath">
        <rdfs:subClassOf rdf:resource="http://www.semanticweb.org/smarotta/ontologies/2022/4/silvanusOntology#Vegetated_area"/>
        <rdfs:comment>An upland moor or sandy area dominated by low shrubby vegetation including heather.</rdfs:comment>
        <rdfs:seeAlso>http://purl.obolibrary.org/obo/ENVO_00000107</rdfs:seeAlso>
    </owl:Class>
    


    <!-- http://www.semanticweb.org/smarotta/ontologies/2022/4/silvanusOntology#Hectares -->

    <owl:Class rdf:about="http://www.semanticweb.org/smarotta/ontologies/2022/4/silvanusOntology#Hectares">
        <rdfs:subClassOf rdf:resource="http://www.semanticweb.org/smarotta/ontologies/2022/4/silvanusOntology#Spatial_entity"/>
    </owl:Class>
    


    <!-- http://www.semanticweb.org/smarotta/ontologies/2022/4/silvanusOntology#Heliport -->

    <owl:Class rdf:about="http://www.semanticweb.org/smarotta/ontologies/2022/4/silvanusOntology#Heliport">
        <rdfs:subClassOf rdf:resource="http://www.semanticweb.org/smarotta/ontologies/2022/4/silvanusOntology#Airport"/>
        <rdfs:comment rdf:datatype="http://www.w3.org/2001/XMLSchema#string">An Airport that is designed for launching, receiving, and housing Rotorcraft.</rdfs:comment>
        <rdfs:seeAlso>http://www.ontologylibrary.mil/CommonCore/Mid/ArtifactOntology#Heliport</rdfs:seeAlso>
    </owl:Class>
    


    <!-- http://www.semanticweb.org/smarotta/ontologies/2022/4/silvanusOntology#High-intensity_fire -->

    <owl:Class rdf:about="http://www.semanticweb.org/smarotta/ontologies/2022/4/silvanusOntology#High-intensity_fire">
        <rdfs:subClassOf rdf:resource="http://www.semanticweb.org/smarotta/ontologies/2022/4/silvanusOntology#Hazard-reduction_fire"/>
        <rdfs:comment>The high-intensity fires are set in order to clear a certain area, that is, to remove all fuel material.</rdfs:comment>
        <rdfs:seeAlso>http://cerrado.linkeddata.es/ecology/fire#HighIntensityFire</rdfs:seeAlso>
    </owl:Class>
    


    <!-- http://www.semanticweb.org/smarotta/ontologies/2022/4/silvanusOntology#High-severity_fire -->

    <owl:Class rdf:about="http://www.semanticweb.org/smarotta/ontologies/2022/4/silvanusOntology#High-severity_fire">
        <rdfs:subClassOf rdf:resource="http://www.semanticweb.org/smarotta/ontologies/2022/4/silvanusOntology#Uncontrolled_fire"/>
        <silvanusOntology:source>https://www.fs.fed.us/database/feis/glossary2.html</silvanusOntology:source>
        <rdfs:comment>May refer to either high soil burn severity, high vegetation burn severity, or replacement-severity fire. As used in LANDFIRE, refers only to replacement-severity fires, which kill or top-kill more than 75% of the upper canopy layer [9]. Also see discussion of fire severity.</rdfs:comment>
    </owl:Class>
    


    <!-- http://www.semanticweb.org/smarotta/ontologies/2022/4/silvanusOntology#High_priority_area -->

    <owl:Class rdf:about="http://www.semanticweb.org/smarotta/ontologies/2022/4/silvanusOntology#High_priority_area">
        <silvanusOntology:source>Greek pilot</silvanusOntology:source>
        <rdfs:comment>Area with high prority of intervention</rdfs:comment>
    </owl:Class>
    


    <!-- http://www.semanticweb.org/smarotta/ontologies/2022/4/silvanusOntology#Hospital -->

    <owl:Class rdf:about="http://www.semanticweb.org/smarotta/ontologies/2022/4/silvanusOntology#Hospital">
        <rdfs:subClassOf rdf:resource="http://www.semanticweb.org/smarotta/ontologies/2022/4/silvanusOntology#Infrastructure"/>
        <rdfs:subClassOf rdf:resource="http://www.semanticweb.org/smarotta/ontologies/2022/4/silvanusOntology#Medical_Facility"/>
        <rdfs:comment>Represents hospitals.</rdfs:comment>
        <rdfs:seeAlso>http://purl.obolibrary.org/obo/ENVO_00002173</rdfs:seeAlso>
        <rdfs:seeAlso>https://raw.githubusercontent.com/beAWARE-project/ontology/master/beAWARE_ontology#Hospital</rdfs:seeAlso>
    </owl:Class>
    


    <!-- http://www.semanticweb.org/smarotta/ontologies/2022/4/silvanusOntology#Hot_ashes -->

    <owl:Class rdf:about="http://www.semanticweb.org/smarotta/ontologies/2022/4/silvanusOntology#Hot_ashes">
        <rdfs:subClassOf rdf:resource="http://www.semanticweb.org/smarotta/ontologies/2022/4/silvanusOntology#Use_of_glowing_objects"/>
        <silvanusOntology:source>https://effis-gwis-cms.s3-eu-west-1.amazonaws.com/effis/reports-and-publications/effis-related-publications/lb-na-25-923-en-n.pdf (page 10)</silvanusOntology:source>
        <rdfs:comment>Wildfire caused by hot ash handling by people after a barbecue or a fire. This class is related to recreational activities. Hot ashes related to work are classified in the following class.</rdfs:comment>
    </owl:Class>
    


    <!-- http://www.semanticweb.org/smarotta/ontologies/2022/4/silvanusOntology#HousingEquipment -->

    <owl:Class rdf:about="http://www.semanticweb.org/smarotta/ontologies/2022/4/silvanusOntology#HousingEquipment">
        <rdfs:subClassOf rdf:resource="http://www.semanticweb.org/smarotta/ontologies/2022/4/silvanusOntology#ReliefItem"/>
        <rdfs:comment>Housing equipment items</rdfs:comment>
        <rdfs:seeAlso>http://www.semanticweb.org/earthquake#HousingEquipment</rdfs:seeAlso>
    </owl:Class>
    


    <!-- http://www.semanticweb.org/smarotta/ontologies/2022/4/silvanusOntology#Human -->

    <owl:Class rdf:about="http://www.semanticweb.org/smarotta/ontologies/2022/4/silvanusOntology#Human">
        <rdfs:subClassOf rdf:resource="http://www.semanticweb.org/smarotta/ontologies/2022/4/silvanusOntology#Living_being"/>
        <rdfs:comment>Represents human beings in danger.</rdfs:comment>
        <rdfs:seeAlso>https://raw.githubusercontent.com/beAWARE-project/ontology/master/beAWARE_ontology#Human</rdfs:seeAlso>
    </owl:Class>
    


    <!-- http://www.semanticweb.org/smarotta/ontologies/2022/4/silvanusOntology#HumanitarianAssistance -->

    <owl:Class rdf:about="http://www.semanticweb.org/smarotta/ontologies/2022/4/silvanusOntology#HumanitarianAssistance">
        <rdfs:subClassOf rdf:resource="http://www.semanticweb.org/smarotta/ontologies/2022/4/silvanusOntology#Response_procedure"/>
        <rdfs:comment>Humanitarian assistance</rdfs:comment>
        <rdfs:seeAlso>http://www.semanticweb.org/earthquake#HumanitarianAssistance</rdfs:seeAlso>
    </owl:Class>
    


    <!-- http://www.semanticweb.org/smarotta/ontologies/2022/4/silvanusOntology#Humidity -->

    <owl:Class rdf:about="http://www.semanticweb.org/smarotta/ontologies/2022/4/silvanusOntology#Humidity">
        <rdfs:subClassOf rdf:resource="http://www.semanticweb.org/smarotta/ontologies/2022/4/silvanusOntology#Climate_parameter"/>
        <rdfs:comment>Measure of the amount of moisture in the air.  It tells you how comfortable it is to be outside, and if there is enough moisture to create clouds and rain. Humidity may be absolute or relative. Absolute humidity is the amount of water vapor in a unit volume of air which is expressed in kilograms per cubic meter. It does not change according to the temperature of the air. When there is a high amount of water vapor in the air, absolute humidity will also be high.</rdfs:comment>
        <rdfs:seeAlso>https://bimerr.iot.linkeddata.es/def/weather#Humidity</rdfs:seeAlso>
    </owl:Class>
    


    <!-- http://www.semanticweb.org/smarotta/ontologies/2022/4/silvanusOntology#Humidity_sensor -->

    <owl:Class rdf:about="http://www.semanticweb.org/smarotta/ontologies/2022/4/silvanusOntology#Humidity_sensor">
        <rdfs:subClassOf rdf:resource="http://www.semanticweb.org/smarotta/ontologies/2022/4/silvanusOntology#IoT_sensor"/>
        <silvanusOntology:source>Most pilots</silvanusOntology:source>
        <rdfs:comment>A humidity sensor is a device that detects and measures water vapor.</rdfs:comment>
    </owl:Class>
    


    <!-- http://www.semanticweb.org/smarotta/ontologies/2022/4/silvanusOntology#Hydrant -->

    <owl:Class rdf:about="http://www.semanticweb.org/smarotta/ontologies/2022/4/silvanusOntology#Hydrant">
        <rdfs:subClassOf rdf:resource="http://www.semanticweb.org/smarotta/ontologies/2022/4/silvanusOntology#Response_resource"/>
        <silvanusOntology:source>Croatian pilot</silvanusOntology:source>
        <rdfs:comment>A fitting in a street or other public place with a nozzle by which a hose may be attached to a water main.</rdfs:comment>
    </owl:Class>
    


    <!-- http://www.semanticweb.org/smarotta/ontologies/2022/4/silvanusOntology#Hydrography -->

    <owl:Class rdf:about="http://www.semanticweb.org/smarotta/ontologies/2022/4/silvanusOntology#Hydrography">
        <rdfs:subClassOf rdf:resource="http://www.semanticweb.org/smarotta/ontologies/2022/4/silvanusOntology#Biodiversity_index"/>
        <silvanusOntology:source>Italian pilot</silvanusOntology:source>
        <rdfs:comment>Description of the physical features of oceans, seas, coastal areas, lakes and rivers, as well as with the prediction of their change over time</rdfs:comment>
    </owl:Class>
    


    <!-- http://www.semanticweb.org/smarotta/ontologies/2022/4/silvanusOntology#Ignition_probability_factor -->

    <owl:Class rdf:about="http://www.semanticweb.org/smarotta/ontologies/2022/4/silvanusOntology#Ignition_probability_factor">
        <rdfs:comment>Represents the factors that together affect the likelihood of a certain are to burn or to start a fire event.</rdfs:comment>
        <rdfs:seeAlso>http://cerrado.linkeddata.es/ecology/fire#IgnitionProbabilityFactor</rdfs:seeAlso>
    </owl:Class>
    


    <!-- http://www.semanticweb.org/smarotta/ontologies/2022/4/silvanusOntology#Image_analysis -->

    <owl:Class rdf:about="http://www.semanticweb.org/smarotta/ontologies/2022/4/silvanusOntology#Image_analysis">
        <rdfs:subClassOf rdf:resource="http://www.semanticweb.org/smarotta/ontologies/2022/4/silvanusOntology#Data_analysis"/>
        <rdfs:comment>Analysis of an image</rdfs:comment>
        <rdfs:seeAlso>https://raw.githubusercontent.com/beAWARE-project/ontology/master/beAWARE_ontology#ImageAnalysis</rdfs:seeAlso>
    </owl:Class>
    


    <!-- http://www.semanticweb.org/smarotta/ontologies/2022/4/silvanusOntology#Image_item -->

    <owl:Class rdf:about="http://www.semanticweb.org/smarotta/ontologies/2022/4/silvanusOntology#Image_item">
        <rdfs:subClassOf rdf:resource="http://www.semanticweb.org/smarotta/ontologies/2022/4/silvanusOntology#Media_item"/>
        <rdfs:comment>Represents an image item</rdfs:comment>
        <rdfs:seeAlso>https://raw.githubusercontent.com/beAWARE-project/ontology/master/beAWARE_ontology#ImageItem</rdfs:seeAlso>
    </owl:Class>
    


    <!-- http://www.semanticweb.org/smarotta/ontologies/2022/4/silvanusOntology#Impact -->

    <owl:Class rdf:about="http://www.semanticweb.org/smarotta/ontologies/2022/4/silvanusOntology#Impact">
        <rdfs:comment>Injuries, damage to properties etc.</rdfs:comment>
        <rdfs:seeAlso>https://raw.githubusercontent.com/beAWARE-project/ontology/master/beAWARE_ontology#Impact</rdfs:seeAlso>
    </owl:Class>
    


    <!-- http://www.semanticweb.org/smarotta/ontologies/2022/4/silvanusOntology#Incident -->

    <owl:Class rdf:about="http://www.semanticweb.org/smarotta/ontologies/2022/4/silvanusOntology#Incident">
        <rdfs:comment>Any collateral incident that can be caused by a fire damaging infrastructures and that affects  vulnerable objects</rdfs:comment>
        <rdfs:seeAlso>https://raw.githubusercontent.com/beAWARE-project/ontology/master/beAWARE_ontology#Incident</rdfs:seeAlso>
    </owl:Class>
    


    <!-- http://www.semanticweb.org/smarotta/ontologies/2022/4/silvanusOntology#IncidentCommander -->

    <owl:Class rdf:about="http://www.semanticweb.org/smarotta/ontologies/2022/4/silvanusOntology#IncidentCommander">
        <rdfs:subClassOf rdf:resource="http://www.semanticweb.org/smarotta/ontologies/2022/4/silvanusOntology#Responder"/>
        <rdfs:comment>The incident commander is the person responsible for all aspects of an emergency response; including quickly developing incident objectives, managing all incident operations, application of resources as well as responsibility for all persons involved. The incident commander sets priorities and defines the organization of the incident response teams and the overall incident action plan.</rdfs:comment>
        <rdfs:seeAlso>http://www.semanticweb.org/earthquake#IncidentCommander</rdfs:seeAlso>
    </owl:Class>
    


    <!-- http://www.semanticweb.org/smarotta/ontologies/2022/4/silvanusOntology#Incident_report -->

    <owl:Class rdf:about="http://www.semanticweb.org/smarotta/ontologies/2022/4/silvanusOntology#Incident_report">
        <rdfs:comment>Represents an incident report submitted to the Public Safety Answering Points (PSAP).</rdfs:comment>
        <rdfs:seeAlso>https://raw.githubusercontent.com/beAWARE-project/ontology/master/beAWARE_ontology#IncidentReport</rdfs:seeAlso>
    </owl:Class>
    


    <!-- http://www.semanticweb.org/smarotta/ontologies/2022/4/silvanusOntology#Industrial_building -->

    <owl:Class rdf:about="http://www.semanticweb.org/smarotta/ontologies/2022/4/silvanusOntology#Industrial_building">
        <rdfs:subClassOf rdf:resource="http://www.semanticweb.org/smarotta/ontologies/2022/4/silvanusOntology#Building"/>
        <rdfs:comment>An industrial building is a building within which goods are produced and, optionally, stored or within which services are rendered.</rdfs:comment>
        <rdfs:seeAlso>http://purl.obolibrary.org/obo/ENVO_00003861</rdfs:seeAlso>
    </owl:Class>
    


    <!-- http://www.semanticweb.org/smarotta/ontologies/2022/4/silvanusOntology#Infant -->

    <owl:Class rdf:about="http://www.semanticweb.org/smarotta/ontologies/2022/4/silvanusOntology#Infant">
        <rdfs:subClassOf rdf:resource="http://www.semanticweb.org/smarotta/ontologies/2022/4/silvanusOntology#Age_group"/>
        <rdfs:comment xml:lang="en">An infant is a child younger than one year of age</rdfs:comment>
        <rdfs:seeAlso>https://w3id.org/empathi/Infant</rdfs:seeAlso>
    </owl:Class>
    


    <!-- http://www.semanticweb.org/smarotta/ontologies/2022/4/silvanusOntology#Infantry_Fighting_Vehicle -->

    <owl:Class rdf:about="http://www.semanticweb.org/smarotta/ontologies/2022/4/silvanusOntology#Infantry_Fighting_Vehicle">
        <rdfs:subClassOf rdf:resource="http://www.semanticweb.org/smarotta/ontologies/2022/4/silvanusOntology#Ground_Motor_Vehicle"/>
        <rdfs:comment>An infantry fighting vehicle is a type of armoured fighting vehicle used to carry infantry into battle and provide direct-fire support</rdfs:comment>
        <rdfs:seeAlso>http://www.ontologylibrary.mil/CommonCore/Mid/ArtifactOntology#InfantryFightingVehicle</rdfs:seeAlso>
    </owl:Class>
    


    <!-- http://www.semanticweb.org/smarotta/ontologies/2022/4/silvanusOntology#Infrared_camera -->

    <owl:Class rdf:about="http://www.semanticweb.org/smarotta/ontologies/2022/4/silvanusOntology#Infrared_camera">
        <rdfs:subClassOf rdf:resource="http://www.semanticweb.org/smarotta/ontologies/2022/4/silvanusOntology#Camera"/>
        <silvanusOntology:source>Czech pilot</silvanusOntology:source>
        <rdfs:comment>A device that creates an image using infrared (IR) radiation, similar to a normal camera that forms an image using visible light.</rdfs:comment>
    </owl:Class>
    


    <!-- http://www.semanticweb.org/smarotta/ontologies/2022/4/silvanusOntology#Infrastructure -->

    <owl:Class rdf:about="http://www.semanticweb.org/smarotta/ontologies/2022/4/silvanusOntology#Infrastructure">
        <rdfs:subClassOf rdf:resource="http://www.semanticweb.org/smarotta/ontologies/2022/4/silvanusOntology#Asset"/>
        <rdfs:comment>Represents critical infrastructure that is in danger during a natural disaster.</rdfs:comment>
        <rdfs:seeAlso>http://www.semanticweb.org/earthquake#InfrastructureLoss</rdfs:seeAlso>
        <rdfs:seeAlso>https://raw.githubusercontent.com/beAWARE-project/ontology/master/beAWARE_ontology#Infrastructure</rdfs:seeAlso>
    </owl:Class>
    


    <!-- http://www.semanticweb.org/smarotta/ontologies/2022/4/silvanusOntology#Initial_spread_index -->

    <owl:Class rdf:about="http://www.semanticweb.org/smarotta/ontologies/2022/4/silvanusOntology#Initial_spread_index">
        <rdfs:subClassOf rdf:resource="http://www.semanticweb.org/smarotta/ontologies/2022/4/silvanusOntology#Fire_weather_index"/>
        <silvanusOntology:source>https://cwfis.cfs.nrcan.gc.ca/background/summary/fwi</silvanusOntology:source>
        <rdfs:comment>The Initial Spread Index (ISI) is a numeric rating of the expected rate of fire spread. It is based on wind speed and FFMC. Like the rest of the FWI system components, ISI does not take fuel type into account. Actual spread rates vary between fuel types at the same ISI.</rdfs:comment>
    </owl:Class>
    


    <!-- http://www.semanticweb.org/smarotta/ontologies/2022/4/silvanusOntology#Interest -->

    <owl:Class rdf:about="http://www.semanticweb.org/smarotta/ontologies/2022/4/silvanusOntology#Interest">
        <rdfs:subClassOf rdf:resource="http://www.semanticweb.org/smarotta/ontologies/2022/4/silvanusOntology#Responsible"/>
        <silvanusOntology:source>https://effis-gwis-cms.s3-eu-west-1.amazonaws.com/effis/reports-and-publications/effis-related-publications/lb-na-25-923-en-n.pdf (page 10)</silvanusOntology:source>
        <rdfs:comment>Wildfire set for profit, either directly for monetary gain or from a goal other than money: fraud, insurance, liquidate property, dissolve business, inventory, employment, parcel clearance, competition for agricultural, forestry, hunting and pastoral purposes to frighten wildlife, to get a job in the fire fighting area, to change land-uses or to get a better salary as fire-fighter, etc.</rdfs:comment>
    </owl:Class>
    


    <!-- http://www.semanticweb.org/smarotta/ontologies/2022/4/silvanusOntology#IoT_sensor -->

    <owl:Class rdf:about="http://www.semanticweb.org/smarotta/ontologies/2022/4/silvanusOntology#IoT_sensor">
        <rdfs:subClassOf rdf:resource="http://www.semanticweb.org/smarotta/ontologies/2022/4/silvanusOntology#Sensor"/>
        <silvanusOntology:source>Most pilots</silvanusOntology:source>
        <rdfs:comment>IoT devices are the nonstandard computing devices that connect wirelessly to a network and have the ability to transmit data, such as the many devices on the internet of things</rdfs:comment>
    </owl:Class>
    


    <!-- http://www.semanticweb.org/smarotta/ontologies/2022/4/silvanusOntology#Irresponsible -->

    <owl:Class rdf:about="http://www.semanticweb.org/smarotta/ontologies/2022/4/silvanusOntology#Irresponsible">
        <rdfs:subClassOf rdf:resource="http://www.semanticweb.org/smarotta/ontologies/2022/4/silvanusOntology#Deliberate"/>
        <owl:disjointWith rdf:resource="http://www.semanticweb.org/smarotta/ontologies/2022/4/silvanusOntology#Responsible"/>
        <silvanusOntology:source>https://effis-gwis-cms.s3-eu-west-1.amazonaws.com/effis/reports-and-publications/effis-related-publications/lb-na-25-923-en-n.pdf (page 10)</silvanusOntology:source>
        <rdfs:comment>Wildfire caused by people not responsible for their actions because under legal age or
mentally ill.</rdfs:comment>
    </owl:Class>
    


    <!-- http://www.semanticweb.org/smarotta/ontologies/2022/4/silvanusOntology#Irrigation -->

    <owl:Class rdf:about="http://www.semanticweb.org/smarotta/ontologies/2022/4/silvanusOntology#Irrigation">
        <rdfs:subClassOf rdf:resource="http://www.semanticweb.org/smarotta/ontologies/2022/4/silvanusOntology#Infrastructure"/>
        <rdfs:comment>Represents irrigation systems</rdfs:comment>
        <rdfs:seeAlso>http://www.semanticweb.org/earthquake#Irrigation</rdfs:seeAlso>
    </owl:Class>
    


    <!-- http://www.semanticweb.org/smarotta/ontologies/2022/4/silvanusOntology#Item -->

    <owl:Class rdf:about="http://www.semanticweb.org/smarotta/ontologies/2022/4/silvanusOntology#Item">
        <rdfs:subClassOf rdf:resource="http://www.semanticweb.org/smarotta/ontologies/2022/4/silvanusOntology#Response_resource"/>
        <rdfs:seeAlso>http://www.semanticweb.org/earthquake#Item</rdfs:seeAlso>
    </owl:Class>
    


    <!-- http://www.semanticweb.org/smarotta/ontologies/2022/4/silvanusOntology#Land_use -->

    <owl:Class rdf:about="http://www.semanticweb.org/smarotta/ontologies/2022/4/silvanusOntology#Land_use">
        <rdfs:subClassOf rdf:resource="http://www.semanticweb.org/smarotta/ontologies/2022/4/silvanusOntology#Biodiversity_index"/>
        <rdfs:comment>Use and occupation of the land</rdfs:comment>
        <rdfs:seeAlso>http://crossforest.eu/ilu/ontology/LandUse</rdfs:seeAlso>
    </owl:Class>
    


    <!-- http://www.semanticweb.org/smarotta/ontologies/2022/4/silvanusOntology#Leevee -->

    <owl:Class rdf:about="http://www.semanticweb.org/smarotta/ontologies/2022/4/silvanusOntology#Leevee">
        <rdfs:subClassOf rdf:resource="http://www.semanticweb.org/smarotta/ontologies/2022/4/silvanusOntology#Structure"/>
        <rdfs:comment>An embankment for preventing flooding.</rdfs:comment>
        <rdfs:seeAlso>https://raw.githubusercontent.com/beAWARE-project/ontology/master/beAWARE_ontology#Levee</rdfs:seeAlso>
    </owl:Class>
    


    <!-- http://www.semanticweb.org/smarotta/ontologies/2022/4/silvanusOntology#LeftBound -->

    <owl:Class rdf:about="http://www.semanticweb.org/smarotta/ontologies/2022/4/silvanusOntology#LeftBound">
        <rdfs:subClassOf rdf:resource="http://www.semanticweb.org/smarotta/ontologies/2022/4/silvanusOntology#Spatial_entity"/>
        <rdfs:comment>Left boundary of an area</rdfs:comment>
        <rdfs:seeAlso>http://crossforest.eu/position/ontology/LeftBound</rdfs:seeAlso>
    </owl:Class>
    


    <!-- http://www.semanticweb.org/smarotta/ontologies/2022/4/silvanusOntology#Lightning -->

    <owl:Class rdf:about="http://www.semanticweb.org/smarotta/ontologies/2022/4/silvanusOntology#Lightning">
        <rdfs:subClassOf rdf:resource="http://www.semanticweb.org/smarotta/ontologies/2022/4/silvanusOntology#Natural"/>
        <silvanusOntology:source>https://effis-gwis-cms.s3-eu-west-1.amazonaws.com/effis/reports-and-publications/effis-related-publications/lb-na-25-923-en-n.pdf (page 10)</silvanusOntology:source>
        <rdfs:comment>Wildfire caused directly or indirectly by lightning.</rdfs:comment>
    </owl:Class>
    


    <!-- http://www.semanticweb.org/smarotta/ontologies/2022/4/silvanusOntology#Living_being -->

    <owl:Class rdf:about="http://www.semanticweb.org/smarotta/ontologies/2022/4/silvanusOntology#Living_being">
        <rdfs:subClassOf rdf:resource="http://www.semanticweb.org/smarotta/ontologies/2022/4/silvanusOntology#Vulnerable_object"/>
        <rdfs:comment>Any living being that is in danger during a natural disaster.</rdfs:comment>
        <rdfs:seeAlso>https://raw.githubusercontent.com/beAWARE-project/ontology/master/beAWARE_ontology#LivingBeing</rdfs:seeAlso>
    </owl:Class>
    


    <!-- http://www.semanticweb.org/smarotta/ontologies/2022/4/silvanusOntology#Living_being_stat -->

    <owl:Class rdf:about="http://www.semanticweb.org/smarotta/ontologies/2022/4/silvanusOntology#Living_being_stat">
        <silvanusOntology:source>Indonesian pilot</silvanusOntology:source>
        <rdfs:comment>Statistics related to living beings</rdfs:comment>
    </owl:Class>
    


    <!-- http://www.semanticweb.org/smarotta/ontologies/2022/4/silvanusOntology#Location -->

    <owl:Class rdf:about="http://www.semanticweb.org/smarotta/ontologies/2022/4/silvanusOntology#Location">
        <rdfs:comment>Represents a location (point or area), indicated by latitude, longitude, and radius.</rdfs:comment>
        <rdfs:seeAlso>https://raw.githubusercontent.com/beAWARE-project/ontology/master/beAWARE_ontology#Location</rdfs:seeAlso>
    </owl:Class>
    


    <!-- http://www.semanticweb.org/smarotta/ontologies/2022/4/silvanusOntology#Locomotive -->

    <owl:Class rdf:about="http://www.semanticweb.org/smarotta/ontologies/2022/4/silvanusOntology#Locomotive">
        <rdfs:subClassOf rdf:resource="http://www.semanticweb.org/smarotta/ontologies/2022/4/silvanusOntology#Rail_Transport_Vehicle"/>
        <owl:disjointWith rdf:resource="http://www.semanticweb.org/smarotta/ontologies/2022/4/silvanusOntology#Train"/>
        <rdfs:comment>A self-propelled vehicle that runs on rails and is used for moving railroad cars</rdfs:comment>
        <rdfs:seeAlso>http://www.ontologylibrary.mil/CommonCore/Mid/ArtifactOntology#Locomotive</rdfs:seeAlso>
    </owl:Class>
    


    <!-- http://www.semanticweb.org/smarotta/ontologies/2022/4/silvanusOntology#LogisticChief -->

    <owl:Class rdf:about="http://www.semanticweb.org/smarotta/ontologies/2022/4/silvanusOntology#LogisticChief">
        <rdfs:subClassOf rdf:resource="http://www.semanticweb.org/smarotta/ontologies/2022/4/silvanusOntology#Responder"/>
        <rdfs:comment>The Logistics Section Chief Type 1 (LSC1) is responsible for managing, organizing, and supervising the Logistics section on wildland fire incidents and serves as a member of the Command and General Staff (C&amp;G) for the Incident Management Team (IMT). The LSC1 supervises the Service (Communications, Medical, and Food) (SVBD) and Support (Supply, Facilities, and Ground Support) Branch Directors (SUBD) of the Logistics functional area and reports to the Incident Commander (IC). The LSC1 works in the Logistics functional area.</rdfs:comment>
        <rdfs:seeAlso>http://www.semanticweb.org/earthquake#LogisticChief</rdfs:seeAlso>
    </owl:Class>
    


    <!-- http://www.semanticweb.org/smarotta/ontologies/2022/4/silvanusOntology#Low -->

    <owl:Class rdf:about="http://www.semanticweb.org/smarotta/ontologies/2022/4/silvanusOntology#Low">
        <rdfs:subClassOf rdf:resource="http://www.semanticweb.org/smarotta/ontologies/2022/4/silvanusOntology#Fire_severity"/>
        <silvanusOntology:source>https://www.fs.fed.us/database/feis/glossary2.html#LowSeverityFire</silvanusOntology:source>
        <rdfs:comment>A fire that has little effect on soil heating or on vegetation, especially the overstory vegetation</rdfs:comment>
    </owl:Class>
    


    <!-- http://www.semanticweb.org/smarotta/ontologies/2022/4/silvanusOntology#Low-severity_fire -->

    <owl:Class rdf:about="http://www.semanticweb.org/smarotta/ontologies/2022/4/silvanusOntology#Low-severity_fire">
        <rdfs:subClassOf rdf:resource="http://www.semanticweb.org/smarotta/ontologies/2022/4/silvanusOntology#Uncontrolled_fire"/>
        <silvanusOntology:source>https://www.fs.fed.us/database/feis/glossary2.html</silvanusOntology:source>
        <rdfs:comment>A fire that has little effect on soil heating or on vegetation, especially the overstory vegetation [121]. As used in LANDFIRE, a low-severity fire is a surface fire that replaces less than 26% of the upper canopy layer, thus maintaining the site in a given successional stage [9]. Similar to understory fire, but can refer to grasslands and shrublands as well as forests and woodlands. See discussion of fire severity.</rdfs:comment>
    </owl:Class>
    


    <!-- http://www.semanticweb.org/smarotta/ontologies/2022/4/silvanusOntology#LowerBound -->

    <owl:Class rdf:about="http://www.semanticweb.org/smarotta/ontologies/2022/4/silvanusOntology#LowerBound">
        <rdfs:subClassOf rdf:resource="http://www.semanticweb.org/smarotta/ontologies/2022/4/silvanusOntology#Spatial_entity"/>
        <rdfs:comment>Lower boundary of an area</rdfs:comment>
        <rdfs:seeAlso>http://crossforest.eu/position/ontology/LowerBound</rdfs:seeAlso>
    </owl:Class>
    


    <!-- http://www.semanticweb.org/smarotta/ontologies/2022/4/silvanusOntology#Major_socio-economic_region -->

    <owl:Class rdf:about="http://www.semanticweb.org/smarotta/ontologies/2022/4/silvanusOntology#Major_socio-economic_region">
        <rdfs:subClassOf rdf:resource="http://www.semanticweb.org/smarotta/ontologies/2022/4/silvanusOntology#NUTS_unit"/>
        <rdfs:comment>NUTS 1: major socio-economic regions</rdfs:comment>
        <rdfs:seeAlso>http://crossforest.eu/ifi/ontology/NUTS1</rdfs:seeAlso>
    </owl:Class>
    


    <!-- http://www.semanticweb.org/smarotta/ontologies/2022/4/silvanusOntology#Mangrove_Biome -->

    <owl:Class rdf:about="http://www.semanticweb.org/smarotta/ontologies/2022/4/silvanusOntology#Mangrove_Biome">
        <rdfs:subClassOf rdf:resource="http://www.semanticweb.org/smarotta/ontologies/2022/4/silvanusOntology#Terrestrial_Biome"/>
        <rdfs:comment>A mangrove biome is a terrestrial biome which includes, across its spatial extent, mangrove plants (Rhizophoraceae). Mangrove plants are able to withstand high levels of salinity as well as regions of anoxia and frequent tidal inundation. Mangrove biomes often occur near tropical and sub-tropical estuaries and depositional marine coastal environments where fine sediments (often with high organic content) collect in areas protected from high energy wave action.</rdfs:comment>
        <rdfs:seeAlso>http://purl.obolibrary.org/obo/ENVO_01000181</rdfs:seeAlso>
    </owl:Class>
    


    <!-- http://www.semanticweb.org/smarotta/ontologies/2022/4/silvanusOntology#Mean_height -->

    <owl:Class rdf:about="http://www.semanticweb.org/smarotta/ontologies/2022/4/silvanusOntology#Mean_height">
        <rdfs:subClassOf rdf:resource="http://www.semanticweb.org/smarotta/ontologies/2022/4/silvanusOntology#Vegetation_stat"/>
        <rdfs:comment>Mean height of the vegetation</rdfs:comment>
    </owl:Class>
    


    <!-- http://www.semanticweb.org/smarotta/ontologies/2022/4/silvanusOntology#Measurable_Entity -->

    <owl:Class rdf:about="http://www.semanticweb.org/smarotta/ontologies/2022/4/silvanusOntology#Measurable_Entity">
        <rdfs:comment xml:lang="en">Entity from which a measure or a number of measures is taken</rdfs:comment>
        <rdfs:seeAlso>http://crossforest.eu/measures/ontology/MeasurableEntity</rdfs:seeAlso>
    </owl:Class>
    


    <!-- http://www.semanticweb.org/smarotta/ontologies/2022/4/silvanusOntology#Measurable_Entity_in_Centimeters -->

    <owl:Class rdf:about="http://www.semanticweb.org/smarotta/ontologies/2022/4/silvanusOntology#Measurable_Entity_in_Centimeters">
        <owl:equivalentClass>
            <owl:Restriction>
                <owl:onProperty rdf:resource="http://www.semanticweb.org/smarotta/ontologies/2022/4/silvanusOntology#has_measure"/>
                <owl:someValuesFrom rdf:resource="http://www.semanticweb.org/smarotta/ontologies/2022/4/silvanusOntology#Measurable_Entity_in_Centimeters"/>
            </owl:Restriction>
        </owl:equivalentClass>
        <rdfs:subClassOf rdf:resource="http://www.semanticweb.org/smarotta/ontologies/2022/4/silvanusOntology#Measurable_Entity"/>
        <rdfs:seeAlso>http://crossforest.eu/measures/ontology/MeasurableEntityInCentimeters</rdfs:seeAlso>
    </owl:Class>
    


    <!-- http://www.semanticweb.org/smarotta/ontologies/2022/4/silvanusOntology#Measurable_Entity_in_Decimeters -->

    <owl:Class rdf:about="http://www.semanticweb.org/smarotta/ontologies/2022/4/silvanusOntology#Measurable_Entity_in_Decimeters">
        <owl:equivalentClass>
            <owl:Restriction>
                <owl:onProperty rdf:resource="http://www.semanticweb.org/smarotta/ontologies/2022/4/silvanusOntology#has_measure"/>
                <owl:someValuesFrom rdf:resource="http://www.semanticweb.org/smarotta/ontologies/2022/4/silvanusOntology#Measurable_Entity_in_Decimeters"/>
            </owl:Restriction>
        </owl:equivalentClass>
        <rdfs:subClassOf rdf:resource="http://www.semanticweb.org/smarotta/ontologies/2022/4/silvanusOntology#Measurable_Entity"/>
        <rdfs:seeAlso>http://crossforest.eu/measures/ontology/MeasurableEntityInDecimeters</rdfs:seeAlso>
    </owl:Class>
    


    <!-- http://www.semanticweb.org/smarotta/ontologies/2022/4/silvanusOntology#Measurable_Entity_in_Degrees -->

    <owl:Class rdf:about="http://www.semanticweb.org/smarotta/ontologies/2022/4/silvanusOntology#Measurable_Entity_in_Degrees">
        <owl:equivalentClass>
            <owl:Restriction>
                <owl:onProperty rdf:resource="http://www.semanticweb.org/smarotta/ontologies/2022/4/silvanusOntology#has_measure"/>
                <owl:someValuesFrom rdf:resource="http://www.semanticweb.org/smarotta/ontologies/2022/4/silvanusOntology#Measurable_Entity_in_Degrees"/>
            </owl:Restriction>
        </owl:equivalentClass>
        <rdfs:subClassOf rdf:resource="http://www.semanticweb.org/smarotta/ontologies/2022/4/silvanusOntology#Measurable_Entity"/>
        <rdfs:seeAlso>http://crossforest.eu/measures/ontology/MeasurableEntityInDegrees</rdfs:seeAlso>
    </owl:Class>
    


    <!-- http://www.semanticweb.org/smarotta/ontologies/2022/4/silvanusOntology#Measurable_Entity_in_Gradians -->

    <owl:Class rdf:about="http://www.semanticweb.org/smarotta/ontologies/2022/4/silvanusOntology#Measurable_Entity_in_Gradians">
        <owl:equivalentClass>
            <owl:Restriction>
                <owl:onProperty rdf:resource="http://www.semanticweb.org/smarotta/ontologies/2022/4/silvanusOntology#has_measure"/>
                <owl:someValuesFrom rdf:resource="http://www.semanticweb.org/smarotta/ontologies/2022/4/silvanusOntology#Measurable_Entity_in_Gradians"/>
            </owl:Restriction>
        </owl:equivalentClass>
        <rdfs:subClassOf rdf:resource="http://www.semanticweb.org/smarotta/ontologies/2022/4/silvanusOntology#Measurable_Entity"/>
        <rdfs:seeAlso>http://crossforest.eu/measures/ontology/MeasurableEntityInGradians</rdfs:seeAlso>
    </owl:Class>
    


    <!-- http://www.semanticweb.org/smarotta/ontologies/2022/4/silvanusOntology#Measurable_Entity_in_Hectares -->

    <owl:Class rdf:about="http://www.semanticweb.org/smarotta/ontologies/2022/4/silvanusOntology#Measurable_Entity_in_Hectares">
        <owl:equivalentClass>
            <owl:Restriction>
                <owl:onProperty rdf:resource="http://www.semanticweb.org/smarotta/ontologies/2022/4/silvanusOntology#has_measure"/>
                <owl:someValuesFrom rdf:resource="http://www.semanticweb.org/smarotta/ontologies/2022/4/silvanusOntology#Measurable_Entity_in_Hectares"/>
            </owl:Restriction>
        </owl:equivalentClass>
        <rdfs:subClassOf rdf:resource="http://www.semanticweb.org/smarotta/ontologies/2022/4/silvanusOntology#Measurable_Entity"/>
        <rdfs:seeAlso>http://crossforest.eu/measures/ontology/MeasurableEntityInHectares</rdfs:seeAlso>
    </owl:Class>
    


    <!-- http://www.semanticweb.org/smarotta/ontologies/2022/4/silvanusOntology#Measurable_Entity_in_Meters -->

    <owl:Class rdf:about="http://www.semanticweb.org/smarotta/ontologies/2022/4/silvanusOntology#Measurable_Entity_in_Meters">
        <owl:equivalentClass>
            <owl:Restriction>
                <owl:onProperty rdf:resource="http://www.semanticweb.org/smarotta/ontologies/2022/4/silvanusOntology#has_measure"/>
                <owl:someValuesFrom rdf:resource="http://www.semanticweb.org/smarotta/ontologies/2022/4/silvanusOntology#Measurable_Entity_in_Meters"/>
            </owl:Restriction>
        </owl:equivalentClass>
        <rdfs:subClassOf rdf:resource="http://www.semanticweb.org/smarotta/ontologies/2022/4/silvanusOntology#Measurable_Entity"/>
        <rdfs:seeAlso>http://crossforest.eu/measures/ontology/MeasurableEntityInMeters</rdfs:seeAlso>
    </owl:Class>
    


    <!-- http://www.semanticweb.org/smarotta/ontologies/2022/4/silvanusOntology#Measurable_Entity_in_Millimeters -->

    <owl:Class rdf:about="http://www.semanticweb.org/smarotta/ontologies/2022/4/silvanusOntology#Measurable_Entity_in_Millimeters">
        <owl:equivalentClass>
            <owl:Restriction>
                <owl:onProperty rdf:resource="http://www.semanticweb.org/smarotta/ontologies/2022/4/silvanusOntology#has_measure"/>
                <owl:someValuesFrom rdf:resource="http://www.semanticweb.org/smarotta/ontologies/2022/4/silvanusOntology#Measurable_Entity_in_Millimeters"/>
            </owl:Restriction>
        </owl:equivalentClass>
        <rdfs:subClassOf rdf:resource="http://www.semanticweb.org/smarotta/ontologies/2022/4/silvanusOntology#Measurable_Entity"/>
        <rdfs:seeAlso>http://crossforest.eu/measures/ontology/MeasurableEntityInMillimeters</rdfs:seeAlso>
    </owl:Class>
    


    <!-- http://www.semanticweb.org/smarotta/ontologies/2022/4/silvanusOntology#Measurable_Entity_in_Square_Meters -->

    <owl:Class rdf:about="http://www.semanticweb.org/smarotta/ontologies/2022/4/silvanusOntology#Measurable_Entity_in_Square_Meters">
        <owl:equivalentClass>
            <owl:Restriction>
                <owl:onProperty rdf:resource="http://www.semanticweb.org/smarotta/ontologies/2022/4/silvanusOntology#has_measure"/>
                <owl:someValuesFrom rdf:resource="http://www.semanticweb.org/smarotta/ontologies/2022/4/silvanusOntology#Measurable_Entity_in_Square_Meters"/>
            </owl:Restriction>
        </owl:equivalentClass>
        <rdfs:subClassOf rdf:resource="http://www.semanticweb.org/smarotta/ontologies/2022/4/silvanusOntology#Measurable_Entity"/>
        <rdfs:seeAlso>http://crossforest.eu/measures/ontology/MeasurableEntityInSquareMeters</rdfs:seeAlso>
    </owl:Class>
    


    <!-- http://www.semanticweb.org/smarotta/ontologies/2022/4/silvanusOntology#Measurable_Entity_in_Years -->

    <owl:Class rdf:about="http://www.semanticweb.org/smarotta/ontologies/2022/4/silvanusOntology#Measurable_Entity_in_Years">
        <owl:equivalentClass>
            <owl:Restriction>
                <owl:onProperty rdf:resource="http://www.semanticweb.org/smarotta/ontologies/2022/4/silvanusOntology#has_measure"/>
                <owl:someValuesFrom rdf:resource="http://www.semanticweb.org/smarotta/ontologies/2022/4/silvanusOntology#Measurable_Entity_in_Years"/>
            </owl:Restriction>
        </owl:equivalentClass>
        <rdfs:subClassOf rdf:resource="http://www.semanticweb.org/smarotta/ontologies/2022/4/silvanusOntology#Measurable_Entity"/>
        <rdfs:seeAlso>http://crossforest.eu/measures/ontology/MeasurableEntityInYears</rdfs:seeAlso>
    </owl:Class>
    


    <!-- http://www.semanticweb.org/smarotta/ontologies/2022/4/silvanusOntology#Measure -->

    <owl:Class rdf:about="http://www.semanticweb.org/smarotta/ontologies/2022/4/silvanusOntology#Measure">
        <rdfs:comment xml:lang="en">The measured value made over a property. It is also linked to the unit of measure in which the value is expressed and to the timestamp of the measurement.</rdfs:comment>
        <rdfs:seeAlso>http://crossforest.eu/measures/ontology/Measure</rdfs:seeAlso>
        <rdfs:seeAlso>https://saref.etsi.org/core/Measurement</rdfs:seeAlso>
    </owl:Class>
    


    <!-- http://www.semanticweb.org/smarotta/ontologies/2022/4/silvanusOntology#MeasureInUnities -->

    <owl:Class rdf:about="http://www.semanticweb.org/smarotta/ontologies/2022/4/silvanusOntology#MeasureInUnities">
        <rdfs:subClassOf rdf:resource="http://www.semanticweb.org/smarotta/ontologies/2022/4/silvanusOntology#Biodiversity_index"/>
        <rdfs:seeAlso>http://crossforest.eu/measures/ontology/MeasureInUnities</rdfs:seeAlso>
    </owl:Class>
    


    <!-- http://www.semanticweb.org/smarotta/ontologies/2022/4/silvanusOntology#Measure_In_Centimeters -->

    <owl:Class rdf:about="http://www.semanticweb.org/smarotta/ontologies/2022/4/silvanusOntology#Measure_In_Centimeters">
        <owl:equivalentClass>
            <owl:Restriction>
                <owl:onProperty rdf:resource="http://www.semanticweb.org/smarotta/ontologies/2022/4/silvanusOntology#has_unit"/>
                <owl:hasValue rdf:resource="http://www.semanticweb.org/smarotta/ontologies/2022/4/silvanusOntology#Centimeters"/>
            </owl:Restriction>
        </owl:equivalentClass>
        <rdfs:subClassOf rdf:resource="http://www.semanticweb.org/smarotta/ontologies/2022/4/silvanusOntology#Measure"/>
        <rdfs:seeAlso>http://crossforest.eu/measures/ontology/MeasureInCentimeters</rdfs:seeAlso>
    </owl:Class>
    


    <!-- http://www.semanticweb.org/smarotta/ontologies/2022/4/silvanusOntology#Measure_In_Decimeters -->

    <owl:Class rdf:about="http://www.semanticweb.org/smarotta/ontologies/2022/4/silvanusOntology#Measure_In_Decimeters">
        <owl:equivalentClass>
            <owl:Restriction>
                <owl:onProperty rdf:resource="http://www.semanticweb.org/smarotta/ontologies/2022/4/silvanusOntology#has_unit"/>
                <owl:hasValue rdf:resource="http://www.semanticweb.org/smarotta/ontologies/2022/4/silvanusOntology#Decimeters"/>
            </owl:Restriction>
        </owl:equivalentClass>
        <rdfs:subClassOf rdf:resource="http://www.semanticweb.org/smarotta/ontologies/2022/4/silvanusOntology#Measure"/>
        <rdfs:seeAlso>http://crossforest.eu/measures/ontology/MeasureInDecimeters</rdfs:seeAlso>
    </owl:Class>
    


    <!-- http://www.semanticweb.org/smarotta/ontologies/2022/4/silvanusOntology#Measure_In_Degrees -->

    <owl:Class rdf:about="http://www.semanticweb.org/smarotta/ontologies/2022/4/silvanusOntology#Measure_In_Degrees">
        <owl:equivalentClass>
            <owl:Restriction>
                <owl:onProperty rdf:resource="http://www.semanticweb.org/smarotta/ontologies/2022/4/silvanusOntology#has_unit"/>
                <owl:hasValue rdf:resource="http://www.semanticweb.org/smarotta/ontologies/2022/4/silvanusOntology#Degrees"/>
            </owl:Restriction>
        </owl:equivalentClass>
        <rdfs:subClassOf rdf:resource="http://www.semanticweb.org/smarotta/ontologies/2022/4/silvanusOntology#Measure"/>
        <rdfs:seeAlso>http://crossforest.eu/measures/ontology/MeasureInDegrees</rdfs:seeAlso>
    </owl:Class>
    


    <!-- http://www.semanticweb.org/smarotta/ontologies/2022/4/silvanusOntology#Measure_In_Gradians -->

    <owl:Class rdf:about="http://www.semanticweb.org/smarotta/ontologies/2022/4/silvanusOntology#Measure_In_Gradians">
        <owl:equivalentClass>
            <owl:Restriction>
                <owl:onProperty rdf:resource="http://www.semanticweb.org/smarotta/ontologies/2022/4/silvanusOntology#has_unit"/>
                <owl:hasValue rdf:resource="http://www.semanticweb.org/smarotta/ontologies/2022/4/silvanusOntology#Gradians"/>
            </owl:Restriction>
        </owl:equivalentClass>
        <rdfs:subClassOf rdf:resource="http://www.semanticweb.org/smarotta/ontologies/2022/4/silvanusOntology#Measure"/>
        <rdfs:seeAlso>http://crossforest.eu/measures/ontology/MeasureInGradians</rdfs:seeAlso>
    </owl:Class>
    


    <!-- http://www.semanticweb.org/smarotta/ontologies/2022/4/silvanusOntology#Measure_In_Hectares -->

    <owl:Class rdf:about="http://www.semanticweb.org/smarotta/ontologies/2022/4/silvanusOntology#Measure_In_Hectares">
        <owl:equivalentClass>
            <owl:Restriction>
                <owl:onProperty rdf:resource="http://www.semanticweb.org/smarotta/ontologies/2022/4/silvanusOntology#has_unit"/>
                <owl:hasValue rdf:resource="http://www.semanticweb.org/smarotta/ontologies/2022/4/silvanusOntology#Hectares"/>
            </owl:Restriction>
        </owl:equivalentClass>
        <rdfs:subClassOf rdf:resource="http://www.semanticweb.org/smarotta/ontologies/2022/4/silvanusOntology#Measure"/>
        <rdfs:seeAlso>http://crossforest.eu/measures/ontology/MeasureInHectares</rdfs:seeAlso>
    </owl:Class>
    


    <!-- http://www.semanticweb.org/smarotta/ontologies/2022/4/silvanusOntology#Measure_In_Meters -->

    <owl:Class rdf:about="http://www.semanticweb.org/smarotta/ontologies/2022/4/silvanusOntology#Measure_In_Meters">
        <owl:equivalentClass>
            <owl:Restriction>
                <owl:onProperty rdf:resource="http://www.semanticweb.org/smarotta/ontologies/2022/4/silvanusOntology#has_unit"/>
                <owl:hasValue rdf:resource="http://www.semanticweb.org/smarotta/ontologies/2022/4/silvanusOntology#Meters"/>
            </owl:Restriction>
        </owl:equivalentClass>
        <rdfs:subClassOf rdf:resource="http://www.semanticweb.org/smarotta/ontologies/2022/4/silvanusOntology#Measure"/>
        <rdfs:seeAlso>http://crossforest.eu/measures/ontology/MeasureInMeters</rdfs:seeAlso>
    </owl:Class>
    


    <!-- http://www.semanticweb.org/smarotta/ontologies/2022/4/silvanusOntology#Measure_In_Millimeters -->

    <owl:Class rdf:about="http://www.semanticweb.org/smarotta/ontologies/2022/4/silvanusOntology#Measure_In_Millimeters">
        <owl:equivalentClass>
            <owl:Restriction>
                <owl:onProperty rdf:resource="http://www.semanticweb.org/smarotta/ontologies/2022/4/silvanusOntology#has_unit"/>
                <owl:hasValue rdf:resource="http://www.semanticweb.org/smarotta/ontologies/2022/4/silvanusOntology#Millimeters"/>
            </owl:Restriction>
        </owl:equivalentClass>
        <rdfs:subClassOf rdf:resource="http://www.semanticweb.org/smarotta/ontologies/2022/4/silvanusOntology#Measure"/>
        <rdfs:seeAlso>http://crossforest.eu/measures/ontology/MeasureInMillimeters</rdfs:seeAlso>
    </owl:Class>
    


    <!-- http://www.semanticweb.org/smarotta/ontologies/2022/4/silvanusOntology#Measure_In_Percentage -->

    <owl:Class rdf:about="http://www.semanticweb.org/smarotta/ontologies/2022/4/silvanusOntology#Measure_In_Percentage">
        <owl:equivalentClass>
            <owl:Restriction>
                <owl:onProperty rdf:resource="http://www.semanticweb.org/smarotta/ontologies/2022/4/silvanusOntology#has_unit"/>
                <owl:hasValue rdf:resource="http://www.semanticweb.org/smarotta/ontologies/2022/4/silvanusOntology#Percentage"/>
            </owl:Restriction>
        </owl:equivalentClass>
        <rdfs:subClassOf rdf:resource="http://www.semanticweb.org/smarotta/ontologies/2022/4/silvanusOntology#Measure"/>
        <rdfs:seeAlso>http://crossforest.eu/measures/ontology/MeasureInPercentage</rdfs:seeAlso>
    </owl:Class>
    


    <!-- http://www.semanticweb.org/smarotta/ontologies/2022/4/silvanusOntology#Measure_In_SquareMeters -->

    <owl:Class rdf:about="http://www.semanticweb.org/smarotta/ontologies/2022/4/silvanusOntology#Measure_In_SquareMeters">
        <owl:equivalentClass>
            <owl:Restriction>
                <owl:onProperty rdf:resource="http://www.semanticweb.org/smarotta/ontologies/2022/4/silvanusOntology#has_unit"/>
                <owl:hasValue rdf:resource="http://www.semanticweb.org/smarotta/ontologies/2022/4/silvanusOntology#Square_Meters"/>
            </owl:Restriction>
        </owl:equivalentClass>
        <rdfs:subClassOf rdf:resource="http://www.semanticweb.org/smarotta/ontologies/2022/4/silvanusOntology#Measure"/>
        <rdfs:seeAlso>http://crossforest.eu/measures/ontology/MeasureInSquareMeters</rdfs:seeAlso>
    </owl:Class>
    


    <!-- http://www.semanticweb.org/smarotta/ontologies/2022/4/silvanusOntology#Measure_In_Unities -->

    <owl:Class rdf:about="http://www.semanticweb.org/smarotta/ontologies/2022/4/silvanusOntology#Measure_In_Unities">
        <owl:equivalentClass>
            <owl:Restriction>
                <owl:onProperty rdf:resource="http://www.semanticweb.org/smarotta/ontologies/2022/4/silvanusOntology#has_unit"/>
                <owl:hasValue rdf:resource="http://www.semanticweb.org/smarotta/ontologies/2022/4/silvanusOntology#Unities"/>
            </owl:Restriction>
        </owl:equivalentClass>
        <rdfs:subClassOf rdf:resource="http://www.semanticweb.org/smarotta/ontologies/2022/4/silvanusOntology#Measure"/>
        <rdfs:seeAlso>http://crossforest.eu/measures/ontology/MeasureInUnities</rdfs:seeAlso>
    </owl:Class>
    


    <!-- http://www.semanticweb.org/smarotta/ontologies/2022/4/silvanusOntology#Measure_In_Years -->

    <owl:Class rdf:about="http://www.semanticweb.org/smarotta/ontologies/2022/4/silvanusOntology#Measure_In_Years">
        <owl:equivalentClass>
            <owl:Restriction>
                <owl:onProperty rdf:resource="http://www.semanticweb.org/smarotta/ontologies/2022/4/silvanusOntology#has_unit"/>
                <owl:hasValue rdf:resource="http://www.semanticweb.org/smarotta/ontologies/2022/4/silvanusOntology#Years"/>
            </owl:Restriction>
        </owl:equivalentClass>
        <rdfs:subClassOf rdf:resource="http://www.semanticweb.org/smarotta/ontologies/2022/4/silvanusOntology#Measure"/>
        <rdfs:seeAlso>http://crossforest.eu/measures/ontology/MeasureInYears</rdfs:seeAlso>
    </owl:Class>
    


    <!-- http://www.semanticweb.org/smarotta/ontologies/2022/4/silvanusOntology#Media_item -->

    <owl:Class rdf:about="http://www.semanticweb.org/smarotta/ontologies/2022/4/silvanusOntology#Media_item">
        <rdfs:comment>Represents a generic media item. Subclasses include specific types of media items.</rdfs:comment>
        <rdfs:seeAlso>https://raw.githubusercontent.com/beAWARE-project/ontology/master/beAWARE_ontology#MediaItem</rdfs:seeAlso>
    </owl:Class>
    


    <!-- http://www.semanticweb.org/smarotta/ontologies/2022/4/silvanusOntology#MedicalItem -->

    <owl:Class rdf:about="http://www.semanticweb.org/smarotta/ontologies/2022/4/silvanusOntology#MedicalItem">
        <rdfs:subClassOf rdf:resource="http://www.semanticweb.org/smarotta/ontologies/2022/4/silvanusOntology#Item"/>
        <rdfs:comment>Drug or other medical items</rdfs:comment>
        <rdfs:seeAlso>http://www.semanticweb.org/earthquake#MedicalItem</rdfs:seeAlso>
    </owl:Class>
    


    <!-- http://www.semanticweb.org/smarotta/ontologies/2022/4/silvanusOntology#MedicalPlanningLeader -->

    <owl:Class rdf:about="http://www.semanticweb.org/smarotta/ontologies/2022/4/silvanusOntology#MedicalPlanningLeader">
        <rdfs:subClassOf rdf:resource="http://www.semanticweb.org/smarotta/ontologies/2022/4/silvanusOntology#Responder"/>
        <rdfs:comment>Person in charge of the medical planning</rdfs:comment>
        <rdfs:seeAlso>http://www.semanticweb.org/earthquake#MedicalPlanningLeader</rdfs:seeAlso>
    </owl:Class>
    


    <!-- http://www.semanticweb.org/smarotta/ontologies/2022/4/silvanusOntology#MedicalStaff -->

    <owl:Class rdf:about="http://www.semanticweb.org/smarotta/ontologies/2022/4/silvanusOntology#MedicalStaff">
        <rdfs:subClassOf rdf:resource="http://www.semanticweb.org/smarotta/ontologies/2022/4/silvanusOntology#Responder"/>
        <rdfs:comment>Medical staff</rdfs:comment>
        <rdfs:seeAlso>http://www.semanticweb.org/earthquake#MedicalStaff</rdfs:seeAlso>
    </owl:Class>
    


    <!-- http://www.semanticweb.org/smarotta/ontologies/2022/4/silvanusOntology#MedicalSupport -->

    <owl:Class rdf:about="http://www.semanticweb.org/smarotta/ontologies/2022/4/silvanusOntology#MedicalSupport">
        <rdfs:subClassOf rdf:resource="http://www.semanticweb.org/smarotta/ontologies/2022/4/silvanusOntology#Response_procedure"/>
        <rdfs:comment>Medical support</rdfs:comment>
        <rdfs:seeAlso>http://www.semanticweb.org/earthquake#MedicalSupport</rdfs:seeAlso>
    </owl:Class>
    


    <!-- http://www.semanticweb.org/smarotta/ontologies/2022/4/silvanusOntology#Medical_Facility -->

    <owl:Class rdf:about="http://www.semanticweb.org/smarotta/ontologies/2022/4/silvanusOntology#Medical_Facility">
        <rdfs:subClassOf rdf:resource="http://www.semanticweb.org/smarotta/ontologies/2022/4/silvanusOntology#Building"/>
        <rdfs:comment>A place where sick or injured people are given care or treatment (as a hospital, urgent care center, or a clinic).</rdfs:comment>
        <rdfs:seeAlso>http://www.ontologylibrary.mil/CommonCore/Mid/ArtifactOntology#HealthcareFacility</rdfs:seeAlso>
        <rdfs:seeAlso>http://www.semanticweb.org/earthquake#HospitalLoss</rdfs:seeAlso>
    </owl:Class>
    


    <!-- http://www.semanticweb.org/smarotta/ontologies/2022/4/silvanusOntology#Medical_equipment -->

    <owl:Class rdf:about="http://www.semanticweb.org/smarotta/ontologies/2022/4/silvanusOntology#Medical_equipment">
        <rdfs:subClassOf rdf:resource="http://www.semanticweb.org/smarotta/ontologies/2022/4/silvanusOntology#Response_resource"/>
        <silvanusOntology:source>Greek pilot</silvanusOntology:source>
        <rdfs:comment>Medical equipment to be used on the field</rdfs:comment>
    </owl:Class>
    


    <!-- http://www.semanticweb.org/smarotta/ontologies/2022/4/silvanusOntology#Mediterranean_Biome -->

    <owl:Class rdf:about="http://www.semanticweb.org/smarotta/ontologies/2022/4/silvanusOntology#Mediterranean_Biome">
        <rdfs:subClassOf rdf:resource="http://www.semanticweb.org/smarotta/ontologies/2022/4/silvanusOntology#Biome"/>
        <rdfs:comment>A biome which is subject to mediterranean climatic conditions.</rdfs:comment>
        <rdfs:seeAlso>http://purl.obolibrary.org/obo/ENVO_01001833</rdfs:seeAlso>
    </owl:Class>
    


    <!-- http://www.semanticweb.org/smarotta/ontologies/2022/4/silvanusOntology#Mediterranean_Savanna_Biome -->

    <owl:Class rdf:about="http://www.semanticweb.org/smarotta/ontologies/2022/4/silvanusOntology#Mediterranean_Savanna_Biome">
        <rdfs:subClassOf rdf:resource="http://www.semanticweb.org/smarotta/ontologies/2022/4/silvanusOntology#Mediterranean_Biome"/>
        <rdfs:comment>A savanna biome which is subject to mediterranean climate patterns.</rdfs:comment>
        <rdfs:seeAlso>http://purl.obolibrary.org/obo/ENVO_01000229</rdfs:seeAlso>
    </owl:Class>
    


    <!-- http://www.semanticweb.org/smarotta/ontologies/2022/4/silvanusOntology#Mediterranean_Sea_Biome -->

    <owl:Class rdf:about="http://www.semanticweb.org/smarotta/ontologies/2022/4/silvanusOntology#Mediterranean_Sea_Biome">
        <rdfs:subClassOf rdf:resource="http://www.semanticweb.org/smarotta/ontologies/2022/4/silvanusOntology#Mediterranean_Biome"/>
        <rdfs:comment>The mediterranean sea biome comprises mostly enclosed seas that have limited exchange of deep water with outer oceans and where the water circulation is dominated by salinity and temperature differences rather than winds.</rdfs:comment>
        <rdfs:seeAlso>http://purl.obolibrary.org/obo/ENVO_01000047</rdfs:seeAlso>
    </owl:Class>
    


    <!-- http://www.semanticweb.org/smarotta/ontologies/2022/4/silvanusOntology#Mediterranean_Shrubland_Biome -->

    <owl:Class rdf:about="http://www.semanticweb.org/smarotta/ontologies/2022/4/silvanusOntology#Mediterranean_Shrubland_Biome">
        <rdfs:subClassOf rdf:resource="http://www.semanticweb.org/smarotta/ontologies/2022/4/silvanusOntology#Mediterranean_Biome"/>
        <rdfs:comment>A mediterranean shrubland biome is a subtropical shrubland biome which includes communities adapted to hot to warm, dry summers, mild to cold, rainy winters, and the influence of large, usually marine, bodies of water.</rdfs:comment>
        <rdfs:seeAlso>http://purl.obolibrary.org/obo/ENVO_01000217</rdfs:seeAlso>
    </owl:Class>
    


    <!-- http://www.semanticweb.org/smarotta/ontologies/2022/4/silvanusOntology#Mediterranean_Woodland_Biome -->

    <owl:Class rdf:about="http://www.semanticweb.org/smarotta/ontologies/2022/4/silvanusOntology#Mediterranean_Woodland_Biome">
        <rdfs:subClassOf rdf:resource="http://www.semanticweb.org/smarotta/ontologies/2022/4/silvanusOntology#Mediterranean_Biome"/>
        <rdfs:comment>A subtropical woodland biome which includes communities adapted to hot to warm, dry summers, mild to cold, rainy winters, and the influence of large, usually marine, bodies of water.</rdfs:comment>
        <rdfs:seeAlso>http://purl.obolibrary.org/obo/ENVO_01000208</rdfs:seeAlso>
    </owl:Class>
    


    <!-- http://www.semanticweb.org/smarotta/ontologies/2022/4/silvanusOntology#Mental_illness -->

    <owl:Class rdf:about="http://www.semanticweb.org/smarotta/ontologies/2022/4/silvanusOntology#Mental_illness">
        <rdfs:subClassOf rdf:resource="http://www.semanticweb.org/smarotta/ontologies/2022/4/silvanusOntology#Irresponsible"/>
        <silvanusOntology:source>https://effis-gwis-cms.s3-eu-west-1.amazonaws.com/effis/reports-and-publications/effis-related-publications/lb-na-25-923-en-n.pdf (page 10)</silvanusOntology:source>
        <rdfs:comment>Wildfire caused by people in case of pyromania or other mental illnesses.</rdfs:comment>
    </owl:Class>
    


    <!-- http://www.semanticweb.org/smarotta/ontologies/2022/4/silvanusOntology#Military_Facility -->

    <owl:Class rdf:about="http://www.semanticweb.org/smarotta/ontologies/2022/4/silvanusOntology#Military_Facility">
        <rdfs:subClassOf rdf:resource="http://www.semanticweb.org/smarotta/ontologies/2022/4/silvanusOntology#Building"/>
        <rdfs:comment rdf:datatype="http://www.w3.org/2001/XMLSchema#string">A Facility that is designed to support forces that are authorized to use deadly force and weapons to support the interests of the state and some or all of its citizens.</rdfs:comment>
        <rdfs:seeAlso>http://www.ontologylibrary.mil/CommonCore/Mid/ArtifactOntology#MilitaryFacility</rdfs:seeAlso>
    </owl:Class>
    


    <!-- http://www.semanticweb.org/smarotta/ontologies/2022/4/silvanusOntology#Mission -->

    <owl:Class rdf:about="http://www.semanticweb.org/smarotta/ontologies/2022/4/silvanusOntology#Mission">
        <rdfs:comment>Represents a mission assigned to a rescue unit during a crisis.</rdfs:comment>
        <rdfs:seeAlso>https://raw.githubusercontent.com/beAWARE-project/ontology/master/beAWARE_ontology#Mission</rdfs:seeAlso>
    </owl:Class>
    


    <!-- http://www.semanticweb.org/smarotta/ontologies/2022/4/silvanusOntology#Mixed -->

    <owl:Class rdf:about="http://www.semanticweb.org/smarotta/ontologies/2022/4/silvanusOntology#Mixed">
        <rdfs:subClassOf rdf:resource="http://www.semanticweb.org/smarotta/ontologies/2022/4/silvanusOntology#Fire_severity"/>
        <silvanusOntology:source>https://www.fs.fed.us/database/feis/glossary2.html#MixedSeverityFire</silvanusOntology:source>
        <rdfs:comment>A fire that exhibits a wide range of fire severity as a result of surface fire in some patches, burning others with stand-replacement severity, and thinning the overstory in other patches. An equal proportion of low-, moderate-, and high-severity burning clearly fits into the mixed-severity fire class, but there is currently no standard by which to define what mix of fire severities should be classified as a mixed-severity fire</rdfs:comment>
    </owl:Class>
    


    <!-- http://www.semanticweb.org/smarotta/ontologies/2022/4/silvanusOntology#Moderate-severity_fire -->

    <owl:Class rdf:about="http://www.semanticweb.org/smarotta/ontologies/2022/4/silvanusOntology#Moderate-severity_fire">
        <rdfs:subClassOf rdf:resource="http://www.semanticweb.org/smarotta/ontologies/2022/4/silvanusOntology#Uncontrolled_fire"/>
        <silvanusOntology:source>https://www.fs.fed.us/database/feis/glossary2.html</silvanusOntology:source>
        <rdfs:comment>Fire that causes moderate soil heating. Occurs where litter is consumed and duff is charred or consumed, but the underlying mineral soil is not visibly altered [92,148]. Although thresholds are subjective, fire that kills from 30% to 70% of the upper canopy layer is generally considered moderate severity [121].</rdfs:comment>
    </owl:Class>
    


    <!-- http://www.semanticweb.org/smarotta/ontologies/2022/4/silvanusOntology#Moisture -->

    <owl:Class rdf:about="http://www.semanticweb.org/smarotta/ontologies/2022/4/silvanusOntology#Moisture">
        <rdfs:subClassOf rdf:resource="http://www.semanticweb.org/smarotta/ontologies/2022/4/silvanusOntology#Vegetation_stat"/>
        <silvanusOntology:source>https://www.fs.fed.us/database/feis/glossary2.html</silvanusOntology:source>
        <rdfs:comment>Moisture is associated with the water content in liquid phase present in any substance.

Aquic: A reducing regime in which the soil is nearly free of dissolved oxygen due to saturation by groundwater during periods when the soil temperature at 20 inches (50 cm) is &gt;41 °F (5 °C).
Udic: Soil is neither dry for as long as 90 cumulative days nor for as long as 60 consecutive days in the 90 days following summer solstice at periods when the soil temperature at 20 inches (50 cm) is &gt;41 °F (5 °C).
Ustic: A limited amount of water is available for plants but occurs at times when the soil temperature is optimum for plant growth.
Xeric: A limited amount of water is present but does not occur at optimum periods for plant growth; common in mediterranean climates with moist, cool winters and warm, dry summers.
Aridic: No water is available for plants for more than half the cumulative time that the soil temperature at 20 inches (50 cm) is &gt;41 °F (5 °C), and no period as long as 90 consecutive days when water is available for plants while soil temperature is continuously &gt;46 °F (8 °C) [125,134].</rdfs:comment>
    </owl:Class>
    


    <!-- http://www.semanticweb.org/smarotta/ontologies/2022/4/silvanusOntology#Moisture_sensor -->

    <owl:Class rdf:about="http://www.semanticweb.org/smarotta/ontologies/2022/4/silvanusOntology#Moisture_sensor">
        <rdfs:subClassOf rdf:resource="http://www.semanticweb.org/smarotta/ontologies/2022/4/silvanusOntology#IoT_sensor"/>
        <silvanusOntology:source>Most pilots</silvanusOntology:source>
        <rdfs:comment>A moisture sensor is a device that detects and measures water vapor.</rdfs:comment>
    </owl:Class>
    


    <!-- http://www.semanticweb.org/smarotta/ontologies/2022/4/silvanusOntology#Monitored_area -->

    <owl:Class rdf:about="http://www.semanticweb.org/smarotta/ontologies/2022/4/silvanusOntology#Monitored_area">
        <rdfs:comment>Area that is being monitored because is potentially susceptible to wildfires</rdfs:comment>
    </owl:Class>
    


    <!-- http://www.semanticweb.org/smarotta/ontologies/2022/4/silvanusOntology#Montane_Biome -->

    <owl:Class rdf:about="http://www.semanticweb.org/smarotta/ontologies/2022/4/silvanusOntology#Montane_Biome">
        <rdfs:subClassOf rdf:resource="http://www.semanticweb.org/smarotta/ontologies/2022/4/silvanusOntology#Biome"/>
        <rdfs:comment>A biome which is subject to montane altitudinal conditions.</rdfs:comment>
        <rdfs:seeAlso>http://purl.obolibrary.org/obo/ENVO_01001836</rdfs:seeAlso>
    </owl:Class>
    


    <!-- http://www.semanticweb.org/smarotta/ontologies/2022/4/silvanusOntology#Montane_Shrubland_Biome -->

    <owl:Class rdf:about="http://www.semanticweb.org/smarotta/ontologies/2022/4/silvanusOntology#Montane_Shrubland_Biome">
        <rdfs:subClassOf rdf:resource="http://www.semanticweb.org/smarotta/ontologies/2022/4/silvanusOntology#Shrubland_Biome"/>
        <rdfs:comment>A montane shrubland biome is a shrubland biome which occurs in regions elevated above sea level and which has community structure determined by elevation-dependent environmental conditions.</rdfs:comment>
        <rdfs:seeAlso>http://purl.obolibrary.org/obo/ENVO_01000216</rdfs:seeAlso>
    </owl:Class>
    


    <!-- http://www.semanticweb.org/smarotta/ontologies/2022/4/silvanusOntology#Monument -->

    <owl:Class rdf:about="http://www.semanticweb.org/smarotta/ontologies/2022/4/silvanusOntology#Monument">
        <rdfs:subClassOf rdf:resource="http://www.semanticweb.org/smarotta/ontologies/2022/4/silvanusOntology#Structure"/>
        <rdfs:comment>A structure or building that is built to honour a special person or event.</rdfs:comment>
        <rdfs:seeAlso>https://raw.githubusercontent.com/beAWARE-project/ontology/master/beAWARE_ontology#Monument</rdfs:seeAlso>
    </owl:Class>
    


    <!-- http://www.semanticweb.org/smarotta/ontologies/2022/4/silvanusOntology#Mortality_rate -->

    <owl:Class rdf:about="http://www.semanticweb.org/smarotta/ontologies/2022/4/silvanusOntology#Mortality_rate">
        <rdfs:subClassOf rdf:resource="http://www.semanticweb.org/smarotta/ontologies/2022/4/silvanusOntology#Living_being_stat"/>
        <silvanusOntology:source>Indonesian pilot</silvanusOntology:source>
        <rdfs:comment>Mortality rate of a species</rdfs:comment>
    </owl:Class>
    


    <!-- http://www.semanticweb.org/smarotta/ontologies/2022/4/silvanusOntology#Motorcycle -->

    <owl:Class rdf:about="http://www.semanticweb.org/smarotta/ontologies/2022/4/silvanusOntology#Motorcycle">
        <rdfs:subClassOf rdf:resource="http://www.semanticweb.org/smarotta/ontologies/2022/4/silvanusOntology#Ground_Motor_Vehicle"/>
        <rdfs:comment>A two-wheeled vehicle that is powered by a motor and has no pedals</rdfs:comment>
        <rdfs:seeAlso>http://www.ontologylibrary.mil/CommonCore/Mid/ArtifactOntology#Motorcycle</rdfs:seeAlso>
    </owl:Class>
    


    <!-- http://www.semanticweb.org/smarotta/ontologies/2022/4/silvanusOntology#NUTS_unit -->

    <owl:Class rdf:about="http://www.semanticweb.org/smarotta/ontologies/2022/4/silvanusOntology#NUTS_unit">
        <rdfs:subClassOf rdf:resource="http://www.semanticweb.org/smarotta/ontologies/2022/4/silvanusOntology#Spatial_entity"/>
        <rdfs:comment>The NUTS (Nomenclature of Territorial Units for Statistics) is a classification defined by the Eurostat office of the European Union.</rdfs:comment>
        <rdfs:seeAlso>http://crossforest.eu/ifi/ontology/NUTSUnit</rdfs:seeAlso>
    </owl:Class>
    


    <!-- http://www.semanticweb.org/smarotta/ontologies/2022/4/silvanusOntology#Natural -->

    <owl:Class rdf:about="http://www.semanticweb.org/smarotta/ontologies/2022/4/silvanusOntology#Natural">
        <rdfs:subClassOf rdf:resource="http://www.semanticweb.org/smarotta/ontologies/2022/4/silvanusOntology#Cause"/>
        <silvanusOntology:source>https://effis-gwis-cms.s3-eu-west-1.amazonaws.com/effis/reports-and-publications/effis-related-publications/lb-na-25-923-en-n.pdf (page 10)</silvanusOntology:source>
        <rdfs:comment>Any wildfire caused by natural origin, with no human involvement in any way</rdfs:comment>
    </owl:Class>
    


    <!-- http://www.semanticweb.org/smarotta/ontologies/2022/4/silvanusOntology#Natural_habitat -->

    <owl:Class rdf:about="http://www.semanticweb.org/smarotta/ontologies/2022/4/silvanusOntology#Natural_habitat">
        <rdfs:subClassOf rdf:resource="http://www.semanticweb.org/smarotta/ontologies/2022/4/silvanusOntology#Ecological_asset"/>
        <rdfs:comment>Represents natural habitats.</rdfs:comment>
        <rdfs:seeAlso>https://raw.githubusercontent.com/beAWARE-project/ontology/master/beAWARE_ontology#NaturalHabitat</rdfs:seeAlso>
    </owl:Class>
    


    <!-- http://www.semanticweb.org/smarotta/ontologies/2022/4/silvanusOntology#Nebulizer -->

    <owl:Class rdf:about="http://www.semanticweb.org/smarotta/ontologies/2022/4/silvanusOntology#Nebulizer">
        <rdfs:subClassOf rdf:resource="http://www.semanticweb.org/smarotta/ontologies/2022/4/silvanusOntology#Medical_equipment"/>
        <silvanusOntology:source>Greek pilot</silvanusOntology:source>
        <rdfs:comment>A nebulizer changes medication from a liquid to a mist so you can inhale it into your lungs.</rdfs:comment>
    </owl:Class>
    


    <!-- http://www.semanticweb.org/smarotta/ontologies/2022/4/silvanusOntology#Negligence -->

    <owl:Class rdf:about="http://www.semanticweb.org/smarotta/ontologies/2022/4/silvanusOntology#Negligence">
        <rdfs:subClassOf rdf:resource="http://www.semanticweb.org/smarotta/ontologies/2022/4/silvanusOntology#Cause"/>
        <silvanusOntology:source>https://effis-gwis-cms.s3-eu-west-1.amazonaws.com/effis/reports-and-publications/effis-related-publications/lb-na-25-923-en-n.pdf (page 10)</silvanusOntology:source>
        <rdfs:comment>Wildfire unintentionally caused by human using fire or glowing object, not connected to fatality</rdfs:comment>
    </owl:Class>
    


    <!-- http://www.semanticweb.org/smarotta/ontologies/2022/4/silvanusOntology#No_fire_effects -->

    <owl:Class rdf:about="http://www.semanticweb.org/smarotta/ontologies/2022/4/silvanusOntology#No_fire_effects">
        <rdfs:subClassOf rdf:resource="http://www.semanticweb.org/smarotta/ontologies/2022/4/silvanusOntology#Fire_severity"/>
        <silvanusOntology:source>https://www.fs.fed.us/database/feis/glossary2.html#FireSeverity</silvanusOntology:source>
        <rdfs:comment>A fire that has no effect on soil heating or on vegetation, especially the overstory vegetation</rdfs:comment>
    </owl:Class>
    


    <!-- http://www.semanticweb.org/smarotta/ontologies/2022/4/silvanusOntology#Non-resprouter -->

    <owl:Class rdf:about="http://www.semanticweb.org/smarotta/ontologies/2022/4/silvanusOntology#Non-resprouter">
        <rdfs:subClassOf rdf:resource="http://www.semanticweb.org/smarotta/ontologies/2022/4/silvanusOntology#Fire_strategy"/>
        <silvanusOntology:source>https://botany.one/2020/10/four-plant-strategies-to-deal-with-fire/</silvanusOntology:source>
        <rdfs:comment>Species die following a fire</rdfs:comment>
    </owl:Class>
    


    <!-- http://www.semanticweb.org/smarotta/ontologies/2022/4/silvanusOntology#Number_of_trees -->

    <owl:Class rdf:about="http://www.semanticweb.org/smarotta/ontologies/2022/4/silvanusOntology#Number_of_trees">
        <rdfs:subClassOf rdf:resource="http://www.semanticweb.org/smarotta/ontologies/2022/4/silvanusOntology#MeasureInUnities"/>
        <rdfs:comment>Number of trees in an area</rdfs:comment>
        <rdfs:seeAlso>http://crossforest.eu/ifi/ontology/NumberOfTrees</rdfs:seeAlso>
    </owl:Class>
    


    <!-- http://www.semanticweb.org/smarotta/ontologies/2022/4/silvanusOntology#Oasis -->

    <owl:Class rdf:about="http://www.semanticweb.org/smarotta/ontologies/2022/4/silvanusOntology#Oasis">
        <rdfs:subClassOf rdf:resource="http://www.semanticweb.org/smarotta/ontologies/2022/4/silvanusOntology#Vegetated_area"/>
        <rdfs:comment>An oasis is a vegetated area located in a desert, supplied with water from a water source which it surrounds, and surrounded by arid soil, sand, or rock.</rdfs:comment>
        <rdfs:seeAlso>http://purl.obolibrary.org/obo/ENVO_01001304</rdfs:seeAlso>
    </owl:Class>
    


    <!-- http://www.semanticweb.org/smarotta/ontologies/2022/4/silvanusOntology#Ocean_Biome -->

    <owl:Class rdf:about="http://www.semanticweb.org/smarotta/ontologies/2022/4/silvanusOntology#Ocean_Biome">
        <rdfs:subClassOf rdf:resource="http://www.semanticweb.org/smarotta/ontologies/2022/4/silvanusOntology#Biome"/>
        <rdfs:comment>A marine biome which is determined by an ocean.</rdfs:comment>
        <rdfs:seeAlso>http://purl.obolibrary.org/obo/ENVO_01000048</rdfs:seeAlso>
    </owl:Class>
    


    <!-- http://www.semanticweb.org/smarotta/ontologies/2022/4/silvanusOntology#Oil_pipeline_network -->

    <owl:Class rdf:about="http://www.semanticweb.org/smarotta/ontologies/2022/4/silvanusOntology#Oil_pipeline_network">
        <rdfs:subClassOf rdf:resource="http://www.semanticweb.org/smarotta/ontologies/2022/4/silvanusOntology#Pipeline_network"/>
        <rdfs:comment>A pipeline network which is used to transport oil to consumers.</rdfs:comment>
        <rdfs:seeAlso>http://purl.obolibrary.org/obo/ENVO_03600003</rdfs:seeAlso>
    </owl:Class>
    


    <!-- http://www.semanticweb.org/smarotta/ontologies/2022/4/silvanusOntology#OperationChief -->

    <owl:Class rdf:about="http://www.semanticweb.org/smarotta/ontologies/2022/4/silvanusOntology#OperationChief">
        <rdfs:subClassOf rdf:resource="http://www.semanticweb.org/smarotta/ontologies/2022/4/silvanusOntology#Responder"/>
        <rdfs:comment>The Operations Chief:
Is responsible to the Incident Commander for the direct management of all incident-related operational activities
Establishes tactical objectives for each operational period
Has direct involvement in the preparation of the Incident Action Plan
The Operations Section Chief may have one or more Deputies assigned. The assignment of Deputies from other agencies may be advantageous in the case of multijurisdictional incidents.</rdfs:comment>
        <rdfs:seeAlso>http://www.semanticweb.org/earthquake#OperationChief</rdfs:seeAlso>
    </owl:Class>
    


    <!-- http://www.semanticweb.org/smarotta/ontologies/2022/4/silvanusOntology#Other_accident -->

    <owl:Class rdf:about="http://www.semanticweb.org/smarotta/ontologies/2022/4/silvanusOntology#Other_accident">
        <rdfs:subClassOf rdf:resource="http://www.semanticweb.org/smarotta/ontologies/2022/4/silvanusOntology#Accident"/>
        <silvanusOntology:source>https://effis-gwis-cms.s3-eu-west-1.amazonaws.com/effis/reports-and-publications/effis-related-publications/lb-na-25-923-en-n.pdf (page 10)</silvanusOntology:source>
        <rdfs:comment>Wildfire caused by other accidental cause (Other technical incidents) than those previously defined. In this class are coded the wildfires due to “Sun” because the sun alone does not allow the ignition but needs an object like a piece of glass. Also included are causes such as “Glass”, “Friction energy”, “thermal reaction of chemicals” or “Self-ignition of coal”.</rdfs:comment>
    </owl:Class>
    


    <!-- http://www.semanticweb.org/smarotta/ontologies/2022/4/silvanusOntology#Other_negligent_use_of_fire -->

    <owl:Class rdf:about="http://www.semanticweb.org/smarotta/ontologies/2022/4/silvanusOntology#Other_negligent_use_of_fire">
        <rdfs:subClassOf rdf:resource="http://www.semanticweb.org/smarotta/ontologies/2022/4/silvanusOntology#Use_of_fire"/>
        <silvanusOntology:source>https://effis-gwis-cms.s3-eu-west-1.amazonaws.com/effis/reports-and-publications/effis-related-publications/lb-na-25-923-en-n.pdf (page 10)</silvanusOntology:source>
        <rdfs:comment>Wildfire caused by other use of fire than those previously defined. In this class are coded the wildfires due to “bonfires at work” “facility fires” and “Candles”.</rdfs:comment>
    </owl:Class>
    


    <!-- http://www.semanticweb.org/smarotta/ontologies/2022/4/silvanusOntology#Other_use_of_glowing_objects -->

    <owl:Class rdf:about="http://www.semanticweb.org/smarotta/ontologies/2022/4/silvanusOntology#Other_use_of_glowing_objects">
        <rdfs:subClassOf rdf:resource="http://www.semanticweb.org/smarotta/ontologies/2022/4/silvanusOntology#Use_of_glowing_objects"/>
        <silvanusOntology:source>https://effis-gwis-cms.s3-eu-west-1.amazonaws.com/effis/reports-and-publications/effis-related-publications/lb-na-25-923-en-n.pdf (page 10)</silvanusOntology:source>
        <rdfs:comment>Wildfire caused by other use of glowing object than those previously defined. In this class are coded wildfires due to working activities such as apiculture, fumigation or disinfection or due to glowing firebrands expulsed out of chimneys regardless of the building.</rdfs:comment>
    </owl:Class>
    


    <!-- http://www.semanticweb.org/smarotta/ontologies/2022/4/silvanusOntology#Overhead_lines -->

    <owl:Class rdf:about="http://www.semanticweb.org/smarotta/ontologies/2022/4/silvanusOntology#Overhead_lines">
        <rdfs:subClassOf rdf:resource="http://www.semanticweb.org/smarotta/ontologies/2022/4/silvanusOntology#Energy"/>
        <owl:disjointWith rdf:resource="http://www.semanticweb.org/smarotta/ontologies/2022/4/silvanusOntology#Substation"/>
        <silvanusOntology:source>Portuguese pilot</silvanusOntology:source>
        <rdfs:comment>An overhead power line is a structure used in electric power transmission and distribution to transmit electrical energy across large distances. It consists of one or more uninsulated electrical cables (commonly multiples of three for three-phase power) suspended by towers or poles.</rdfs:comment>
    </owl:Class>
    


    <!-- http://www.semanticweb.org/smarotta/ontologies/2022/4/silvanusOntology#Passive_crown_fire -->

    <owl:Class rdf:about="http://www.semanticweb.org/smarotta/ontologies/2022/4/silvanusOntology#Passive_crown_fire">
        <rdfs:subClassOf rdf:resource="http://www.semanticweb.org/smarotta/ontologies/2022/4/silvanusOntology#Crown_fire"/>
        <silvanusOntology:source>https://www.fs.fed.us/database/feis/glossary2.html</silvanusOntology:source>
        <rdfs:comment>A type of crown fire in which the crowns of individual trees or small groups of trees burn, but solid flaming in the canopy cannot be maintained except for short periods. Passive crown fire encompasses a wide range of crown fire behavior, from occasional torching of isolated trees to nearly active crown fire. Passive crown fire is also called torching or candling. A fire in the crowns of the trees in which trees or groups of trees torch, ignited by the passing front of the fire. The torching trees reinforce the spread rate, but these fires are not basically different from surface fires</rdfs:comment>
    </owl:Class>
    


    <!-- http://www.semanticweb.org/smarotta/ontologies/2022/4/silvanusOntology#Patrol -->

    <owl:Class rdf:about="http://www.semanticweb.org/smarotta/ontologies/2022/4/silvanusOntology#Patrol">
        <rdfs:subClassOf rdf:resource="http://www.semanticweb.org/smarotta/ontologies/2022/4/silvanusOntology#Responder"/>
        <silvanusOntology:source>Italian pilot</silvanusOntology:source>
        <rdfs:comment>An expedition to keep watch over an area, especially by guards or police walking or driving around at regular intervals.</rdfs:comment>
    </owl:Class>
    


    <!-- http://www.semanticweb.org/smarotta/ontologies/2022/4/silvanusOntology#Pier -->

    <owl:Class rdf:about="http://www.semanticweb.org/smarotta/ontologies/2022/4/silvanusOntology#Pier">
        <rdfs:subClassOf rdf:resource="http://www.semanticweb.org/smarotta/ontologies/2022/4/silvanusOntology#Transportation_Facility"/>
        <rdfs:comment rdf:datatype="http://www.w3.org/2001/XMLSchema#string">A Transportation Facility that is designed to partially enclose a harbor and form a landing place for Watercraft.</rdfs:comment>
        <rdfs:seeAlso>http://www.ontologylibrary.mil/CommonCore/Mid/ArtifactOntology#Pier</rdfs:seeAlso>
    </owl:Class>
    


    <!-- http://www.semanticweb.org/smarotta/ontologies/2022/4/silvanusOntology#Pipeline_network -->

    <owl:Class rdf:about="http://www.semanticweb.org/smarotta/ontologies/2022/4/silvanusOntology#Pipeline_network">
        <owl:equivalentClass rdf:resource="http://www.semanticweb.org/smarotta/ontologies/2022/4/silvanusOntology#Transmission_pipeline"/>
        <rdfs:subClassOf rdf:resource="http://www.semanticweb.org/smarotta/ontologies/2022/4/silvanusOntology#Infrastructure"/>
        <rdfs:comment>A human construction which is used to transport a material which is primarily composed of liquid or gas through a system of pipes.</rdfs:comment>
        <rdfs:seeAlso>http://purl.obolibrary.org/obo/ENVO_03600014</rdfs:seeAlso>
    </owl:Class>
    


    <!-- http://www.semanticweb.org/smarotta/ontologies/2022/4/silvanusOntology#PlanningChief -->

    <owl:Class rdf:about="http://www.semanticweb.org/smarotta/ontologies/2022/4/silvanusOntology#PlanningChief">
        <rdfs:subClassOf rdf:resource="http://www.semanticweb.org/smarotta/ontologies/2022/4/silvanusOntology#Responder"/>
        <rdfs:comment>The Planning Section Chief oversees incident-related data gathering and analysis regarding incident operations and assigned resources, facilitates incident action planning meetings and prepares the Incident Action Plan (IAP) for each operational period</rdfs:comment>
        <rdfs:seeAlso>http://www.semanticweb.org/earthquake#PlanningChief</rdfs:seeAlso>
    </owl:Class>
    


    <!-- http://www.semanticweb.org/smarotta/ontologies/2022/4/silvanusOntology#Plant -->

    <owl:Class rdf:about="http://www.semanticweb.org/smarotta/ontologies/2022/4/silvanusOntology#Plant">
        <rdfs:subClassOf rdf:resource="http://www.semanticweb.org/smarotta/ontologies/2022/4/silvanusOntology#Ecological_asset"/>
        <rdfs:comment>Represents the fauna.</rdfs:comment>
        <rdfs:seeAlso>https://raw.githubusercontent.com/beAWARE-project/ontology/master/beAWARE_ontology#Plant</rdfs:seeAlso>
    </owl:Class>
    


    <!-- http://www.semanticweb.org/smarotta/ontologies/2022/4/silvanusOntology#Plant_type -->

    <owl:Class rdf:about="http://www.semanticweb.org/smarotta/ontologies/2022/4/silvanusOntology#Plant_type">
        <rdfs:subClassOf rdf:resource="http://www.semanticweb.org/smarotta/ontologies/2022/4/silvanusOntology#Vegetation_type"/>
        <rdfs:comment>Type of plant</rdfs:comment>
    </owl:Class>
    


    <!-- http://www.semanticweb.org/smarotta/ontologies/2022/4/silvanusOntology#Polar_Biome -->

    <owl:Class rdf:about="http://www.semanticweb.org/smarotta/ontologies/2022/4/silvanusOntology#Polar_Biome">
        <rdfs:subClassOf rdf:resource="http://www.semanticweb.org/smarotta/ontologies/2022/4/silvanusOntology#Biome"/>
        <rdfs:comment>A biome which is subject to polar climatic conditions.</rdfs:comment>
        <rdfs:seeAlso>http://purl.obolibrary.org/obo/ENVO_01000339</rdfs:seeAlso>
    </owl:Class>
    


    <!-- http://www.semanticweb.org/smarotta/ontologies/2022/4/silvanusOntology#Police -->

    <owl:Class rdf:about="http://www.semanticweb.org/smarotta/ontologies/2022/4/silvanusOntology#Police">
        <rdfs:subClassOf rdf:resource="http://www.semanticweb.org/smarotta/ontologies/2022/4/silvanusOntology#Infrastructure"/>
        <rdfs:comment>Represents law enforcement infrastructure and services.</rdfs:comment>
        <rdfs:comment>http://www.semanticweb.org/earthquake#Police</rdfs:comment>
        <rdfs:seeAlso>https://raw.githubusercontent.com/beAWARE-project/ontology/master/beAWARE_ontology#Police</rdfs:seeAlso>
    </owl:Class>
    


    <!-- http://www.semanticweb.org/smarotta/ontologies/2022/4/silvanusOntology#Police_Station -->

    <owl:Class rdf:about="http://www.semanticweb.org/smarotta/ontologies/2022/4/silvanusOntology#Police_Station">
        <rdfs:subClassOf rdf:resource="http://www.semanticweb.org/smarotta/ontologies/2022/4/silvanusOntology#Public_Safety_Facility"/>
        <rdfs:comment rdf:datatype="http://www.w3.org/2001/XMLSchema#string">A Public Safety Facility that is designed for the professional and clerical processes of a local police force.</rdfs:comment>
        <rdfs:seeAlso>http://www.ontologylibrary.mil/CommonCore/Mid/ArtifactOntology#PoliceStation</rdfs:seeAlso>
    </owl:Class>
    


    <!-- http://www.semanticweb.org/smarotta/ontologies/2022/4/silvanusOntology#Polygon -->

    <owl:Class rdf:about="http://www.semanticweb.org/smarotta/ontologies/2022/4/silvanusOntology#Polygon">
        <rdfs:subClassOf rdf:resource="http://www.semanticweb.org/smarotta/ontologies/2022/4/silvanusOntology#Position"/>
        <rdfs:comment>A plane figure with at least three straight sides and angles, and typically five or more.</rdfs:comment>
        <rdfs:seeAlso>http://crossforest.eu/position/ontology/Polygon</rdfs:seeAlso>
    </owl:Class>
    


    <!-- http://www.semanticweb.org/smarotta/ontologies/2022/4/silvanusOntology#Population -->

    <owl:Class rdf:about="http://www.semanticweb.org/smarotta/ontologies/2022/4/silvanusOntology#Population">
        <rdfs:subClassOf rdf:resource="http://www.semanticweb.org/smarotta/ontologies/2022/4/silvanusOntology#Living_being_stat"/>
        <silvanusOntology:source>Indonesian pilot</silvanusOntology:source>
        <rdfs:comment>Population rate of a species</rdfs:comment>
    </owl:Class>
    


    <!-- http://www.semanticweb.org/smarotta/ontologies/2022/4/silvanusOntology#Population_index -->

    <owl:Class rdf:about="http://www.semanticweb.org/smarotta/ontologies/2022/4/silvanusOntology#Population_index">
        <rdfs:subClassOf rdf:resource="http://www.semanticweb.org/smarotta/ontologies/2022/4/silvanusOntology#Biodiversity_index"/>
        <silvanusOntology:source>https://www.fs.fed.us/database/feis/glossary2.html#PopulationIndex</silvanusOntology:source>
        <rdfs:comment>Any indicator of the size of a population (e.g., mountain bluebird nests/km2) [43].</rdfs:comment>
    </owl:Class>
    


    <!-- http://www.semanticweb.org/smarotta/ontologies/2022/4/silvanusOntology#Port -->

    <owl:Class rdf:about="http://www.semanticweb.org/smarotta/ontologies/2022/4/silvanusOntology#Port">
        <rdfs:subClassOf rdf:resource="http://www.semanticweb.org/smarotta/ontologies/2022/4/silvanusOntology#Transportation_Facility"/>
        <rdfs:comment rdf:datatype="http://www.w3.org/2001/XMLSchema#string">A Transportation Facility that is designed to contain harbors for docking Watercraft and for transfering people or cargo to and from land.</rdfs:comment>
        <rdfs:seeAlso>http://www.ontologylibrary.mil/CommonCore/Mid/ArtifactOntology#Port</rdfs:seeAlso>
        <rdfs:seeAlso>http://www.semanticweb.org/earthquake#PortLoss</rdfs:seeAlso>
    </owl:Class>
    


    <!-- http://www.semanticweb.org/smarotta/ontologies/2022/4/silvanusOntology#Position -->

    <owl:Class rdf:about="http://www.semanticweb.org/smarotta/ontologies/2022/4/silvanusOntology#Position">
        <rdfs:subClassOf rdf:resource="http://www.semanticweb.org/smarotta/ontologies/2022/4/silvanusOntology#Spatial_entity"/>
        <rdfs:comment>Position where a spatial entity can be located</rdfs:comment>
        <rdfs:seeAlso>http://crossforest.eu/position/ontology/Position</rdfs:seeAlso>
    </owl:Class>
    


    <!-- http://www.semanticweb.org/smarotta/ontologies/2022/4/silvanusOntology#Power_line -->

    <owl:Class rdf:about="http://www.semanticweb.org/smarotta/ontologies/2022/4/silvanusOntology#Power_line">
        <rdfs:subClassOf rdf:resource="http://www.semanticweb.org/smarotta/ontologies/2022/4/silvanusOntology#Response_resource"/>
        <silvanusOntology:source>Italian pilot</silvanusOntology:source>
        <rdfs:comment>Power line to use for equipment</rdfs:comment>
    </owl:Class>
    


    <!-- http://www.semanticweb.org/smarotta/ontologies/2022/4/silvanusOntology#Power_plant -->

    <owl:Class rdf:about="http://www.semanticweb.org/smarotta/ontologies/2022/4/silvanusOntology#Power_plant">
        <rdfs:subClassOf rdf:resource="http://www.semanticweb.org/smarotta/ontologies/2022/4/silvanusOntology#Industrial_building"/>
        <rdfs:comment>A power plant is a building which contains one or more generators which convert mechanical energy into electrical energy through the relative motion between a magnetic field and a conductor. The energy source harnessed to turn the generator varies widely.</rdfs:comment>
        <rdfs:seeAlso>http://purl.obolibrary.org/obo/ENVO_00002214</rdfs:seeAlso>
        <rdfs:seeAlso>http://www.semanticweb.org/earthquake#ElectricFacility</rdfs:seeAlso>
        <rdfs:seeAlso>https://w3id.org/empathi/Electricity</rdfs:seeAlso>
    </owl:Class>
    


    <!-- http://www.semanticweb.org/smarotta/ontologies/2022/4/silvanusOntology#Precipitation -->

    <owl:Class rdf:about="http://www.semanticweb.org/smarotta/ontologies/2022/4/silvanusOntology#Precipitation">
        <rdfs:subClassOf rdf:resource="http://www.semanticweb.org/smarotta/ontologies/2022/4/silvanusOntology#Climate_parameter"/>
        <rdfs:comment>Any product of the condensation of atmospheric water vapour that falls under gravity from clouds. The main forms of precipitation include drizzle, rain, sleet, snow, ice pellets, graupel and hail.</rdfs:comment>
        <rdfs:seeAlso>https://bimerr.iot.linkeddata.es/def/weather#Precipitation</rdfs:seeAlso>
    </owl:Class>
    


    <!-- http://www.semanticweb.org/smarotta/ontologies/2022/4/silvanusOntology#Preventive_procedure -->

    <owl:Class rdf:about="http://www.semanticweb.org/smarotta/ontologies/2022/4/silvanusOntology#Preventive_procedure">
        <silvanusOntology:source>Italian pilot</silvanusOntology:source>
        <rdfs:comment>Preventive interventions on the ground</rdfs:comment>
    </owl:Class>
    


    <!-- http://www.semanticweb.org/smarotta/ontologies/2022/4/silvanusOntology#Professional_unit -->

    <owl:Class rdf:about="http://www.semanticweb.org/smarotta/ontologies/2022/4/silvanusOntology#Professional_unit">
        <rdfs:subClassOf rdf:resource="http://www.semanticweb.org/smarotta/ontologies/2022/4/silvanusOntology#Firefighting_unit"/>
        <silvanusOntology:source>Czech pilot</silvanusOntology:source>
        <rdfs:comment>Professional firefighter</rdfs:comment>
    </owl:Class>
    


    <!-- http://www.semanticweb.org/smarotta/ontologies/2022/4/silvanusOntology#Property -->

    <owl:Class rdf:about="http://www.semanticweb.org/smarotta/ontologies/2022/4/silvanusOntology#Property">
        <rdfs:subClassOf rdf:resource="http://www.semanticweb.org/smarotta/ontologies/2022/4/silvanusOntology#Asset"/>
        <rdfs:comment>Represents any type of private property.</rdfs:comment>
        <rdfs:seeAlso>http://www.semanticweb.org/earthquake#PropertyLoss</rdfs:seeAlso>
        <rdfs:seeAlso>https://raw.githubusercontent.com/beAWARE-project/ontology/master/beAWARE_ontology#Property</rdfs:seeAlso>
    </owl:Class>
    


    <!-- http://www.semanticweb.org/smarotta/ontologies/2022/4/silvanusOntology#PublicInfoOfficer -->

    <owl:Class rdf:about="http://www.semanticweb.org/smarotta/ontologies/2022/4/silvanusOntology#PublicInfoOfficer">
        <rdfs:subClassOf rdf:resource="http://www.semanticweb.org/smarotta/ontologies/2022/4/silvanusOntology#Responder"/>
        <rdfs:comment>The PIO is the individual responsible for communicating with the public, media, and/or coordinating with other agencies, as necessary, with incident related information requirements.</rdfs:comment>
        <rdfs:seeAlso>http://www.semanticweb.org/earthquake#PublicInfoOfficer</rdfs:seeAlso>
    </owl:Class>
    


    <!-- http://www.semanticweb.org/smarotta/ontologies/2022/4/silvanusOntology#Public_Safety_Facility -->

    <owl:Class rdf:about="http://www.semanticweb.org/smarotta/ontologies/2022/4/silvanusOntology#Public_Safety_Facility">
        <rdfs:subClassOf rdf:resource="http://www.semanticweb.org/smarotta/ontologies/2022/4/silvanusOntology#Building"/>
        <rdfs:comment rdf:datatype="http://www.w3.org/2001/XMLSchema#string">A Facility that is designed for the prevention of and protection from events that could endanger, injure, or damage the general public.</rdfs:comment>
        <rdfs:seeAlso>http://www.ontologylibrary.mil/CommonCore/Mid/ArtifactOntology#PublicSafetyFacility</rdfs:seeAlso>
    </owl:Class>
    


    <!-- http://www.semanticweb.org/smarotta/ontologies/2022/4/silvanusOntology#Public_street -->

    <owl:Class rdf:about="http://www.semanticweb.org/smarotta/ontologies/2022/4/silvanusOntology#Public_street">
        <rdfs:subClassOf rdf:resource="http://www.semanticweb.org/smarotta/ontologies/2022/4/silvanusOntology#Street"/>
        <rdfs:comment>A road which is publically accessible.</rdfs:comment>
        <rdfs:seeAlso>http://purl.obolibrary.org/obo/ENVO_01000780</rdfs:seeAlso>
    </owl:Class>
    


    <!-- http://www.semanticweb.org/smarotta/ontologies/2022/4/silvanusOntology#Public_transport -->

    <owl:Class rdf:about="http://www.semanticweb.org/smarotta/ontologies/2022/4/silvanusOntology#Public_transport">
        <rdfs:subClassOf rdf:resource="http://www.semanticweb.org/smarotta/ontologies/2022/4/silvanusOntology#Transportation"/>
        <owl:disjointWith rdf:resource="http://www.semanticweb.org/smarotta/ontologies/2022/4/silvanusOntology#Street"/>
        <rdfs:comment>Represents public transportation services and infrastructure.</rdfs:comment>
        <rdfs:seeAlso>https://raw.githubusercontent.com/beAWARE-project/ontology/master/beAWARE_ontology#PublicTransportation</rdfs:seeAlso>
    </owl:Class>
    


    <!-- http://www.semanticweb.org/smarotta/ontologies/2022/4/silvanusOntology#Pumping_station -->

    <owl:Class rdf:about="http://www.semanticweb.org/smarotta/ontologies/2022/4/silvanusOntology#Pumping_station">
        <rdfs:subClassOf rdf:resource="http://www.semanticweb.org/smarotta/ontologies/2022/4/silvanusOntology#Water_supply"/>
        <silvanusOntology:source>Portuguese pilot</silvanusOntology:source>
        <rdfs:comment>Facilities containing pumps and equipment for pumping fluids from one place to another. They are used for a variety of infrastructure systems, such as the supply of water to canals, the drainage of low-lying land, and the removal of sewage to processing sites.</rdfs:comment>
    </owl:Class>
    


    <!-- http://www.semanticweb.org/smarotta/ontologies/2022/4/silvanusOntology#Rail_Facility -->

    <owl:Class rdf:about="http://www.semanticweb.org/smarotta/ontologies/2022/4/silvanusOntology#Rail_Facility">
        <rdfs:subClassOf rdf:resource="http://www.semanticweb.org/smarotta/ontologies/2022/4/silvanusOntology#Building"/>
        <rdfs:comment rdf:datatype="http://www.w3.org/2001/XMLSchema#string">A Transportation Facility that is designed for transferring people or cargo to and from Trains.</rdfs:comment>
        <rdfs:seeAlso>http://www.ontologylibrary.mil/CommonCore/Mid/ArtifactOntology#RailFacility</rdfs:seeAlso>
        <rdfs:seeAlso>http://www.semanticweb.org/earthquake#RailwayLoss</rdfs:seeAlso>
    </owl:Class>
    


    <!-- http://www.semanticweb.org/smarotta/ontologies/2022/4/silvanusOntology#Rail_Transport_Vehicle -->

    <owl:Class rdf:about="http://www.semanticweb.org/smarotta/ontologies/2022/4/silvanusOntology#Rail_Transport_Vehicle">
        <rdfs:subClassOf rdf:resource="http://www.semanticweb.org/smarotta/ontologies/2022/4/silvanusOntology#Ground_Vehicle"/>
        <rdfs:comment>A vehicle used for the carrying of cargo or passengers on a rail transport system (a railroad/railway). Such cars, when coupled together and hauled by one or more locomotives, form a train.</rdfs:comment>
        <rdfs:seeAlso>http://www.ontologylibrary.mil/CommonCore/Mid/ArtifactOntology#RailTransportVehicle</rdfs:seeAlso>
    </owl:Class>
    


    <!-- http://www.semanticweb.org/smarotta/ontologies/2022/4/silvanusOntology#Railroads -->

    <owl:Class rdf:about="http://www.semanticweb.org/smarotta/ontologies/2022/4/silvanusOntology#Railroads">
        <rdfs:subClassOf rdf:resource="http://www.semanticweb.org/smarotta/ontologies/2022/4/silvanusOntology#Accident"/>
        <silvanusOntology:source>https://effis-gwis-cms.s3-eu-west-1.amazonaws.com/effis/reports-and-publications/effis-related-publications/lb-na-25-923-en-n.pdf (page 10)</silvanusOntology:source>
        <rdfs:comment>Wildfire caused by sparks emitted by train brakes or fall of catenaries. It has to be linked with the operation of trains. Fires lit intentionally or not by passengers or railway employees (by smoking, managing vegetation, etc.) are not classified in this category and must be classified in the category corresponding to “what these persons did” to set the fire (and not to “where they were”).</rdfs:comment>
    </owl:Class>
    


    <!-- http://www.semanticweb.org/smarotta/ontologies/2022/4/silvanusOntology#Rangeland_Biome -->

    <owl:Class rdf:about="http://www.semanticweb.org/smarotta/ontologies/2022/4/silvanusOntology#Rangeland_Biome">
        <rdfs:subClassOf rdf:resource="http://www.semanticweb.org/smarotta/ontologies/2022/4/silvanusOntology#Anthropogenic_Terrestrial_Biome"/>
        <rdfs:comment>A rangeland biome is an anthropogenic terrestrial biome which is primarily used for the rearing and grazing of livestock.</rdfs:comment>
        <rdfs:seeAlso>http://purl.obolibrary.org/obo/ENVO_01000247</rdfs:seeAlso>
    </owl:Class>
    


    <!-- http://www.semanticweb.org/smarotta/ontologies/2022/4/silvanusOntology#Recreation -->

    <owl:Class rdf:about="http://www.semanticweb.org/smarotta/ontologies/2022/4/silvanusOntology#Recreation">
        <rdfs:subClassOf rdf:resource="http://www.semanticweb.org/smarotta/ontologies/2022/4/silvanusOntology#Use_of_fire"/>
        <silvanusOntology:source>https://effis-gwis-cms.s3-eu-west-1.amazonaws.com/effis/reports-and-publications/effis-related-publications/lb-na-25-923-en-n.pdf (page 10)</silvanusOntology:source>
        <rdfs:comment>Wildfire caused by people engaged in a recreational activity (vacationing, fishing, picnicking, non-commercial berry picking, hiking, and hunting) setting barbecues, bonfires and campfires of any kind (for cooking, heating, etc).</rdfs:comment>
    </owl:Class>
    


    <!-- http://www.semanticweb.org/smarotta/ontologies/2022/4/silvanusOntology#Reference_Position -->

    <owl:Class rdf:about="http://www.semanticweb.org/smarotta/ontologies/2022/4/silvanusOntology#Reference_Position">
        <rdfs:subClassOf rdf:resource="http://www.semanticweb.org/smarotta/ontologies/2022/4/silvanusOntology#Position"/>
        <rdfs:comment xml:lang="en">Position taken as reference for the position of other spatial entities</rdfs:comment>
        <rdfs:seeAlso>http://crossforest.eu/position/ontology/ReferencePosition</rdfs:seeAlso>
    </owl:Class>
    


    <!-- http://www.semanticweb.org/smarotta/ontologies/2022/4/silvanusOntology#RehabilitationAndRecovery -->

    <owl:Class rdf:about="http://www.semanticweb.org/smarotta/ontologies/2022/4/silvanusOntology#RehabilitationAndRecovery">
        <rdfs:subClassOf rdf:resource="http://www.semanticweb.org/smarotta/ontologies/2022/4/silvanusOntology#Response_procedure"/>
        <rdfs:comment>Restoration of the environment</rdfs:comment>
        <rdfs:seeAlso>http://www.semanticweb.org/earthquake#RehabilitationAndRecovery</rdfs:seeAlso>
    </owl:Class>
    


    <!-- http://www.semanticweb.org/smarotta/ontologies/2022/4/silvanusOntology#Rekindle -->

    <owl:Class rdf:about="http://www.semanticweb.org/smarotta/ontologies/2022/4/silvanusOntology#Rekindle">
        <rdfs:subClassOf rdf:resource="http://www.semanticweb.org/smarotta/ontologies/2022/4/silvanusOntology#Cause"/>
        <silvanusOntology:source>https://effis-gwis-cms.s3-eu-west-1.amazonaws.com/effis/reports-and-publications/effis-related-publications/lb-na-25-923-en-n.pdf (page 10)</silvanusOntology:source>
        <rdfs:comment>Wildfire caused by re-ignition of a previous fire, due to latent heat or embers.</rdfs:comment>
    </owl:Class>
    


    <!-- http://www.semanticweb.org/smarotta/ontologies/2022/4/silvanusOntology#Relative_humidity -->

    <owl:Class rdf:about="http://www.semanticweb.org/smarotta/ontologies/2022/4/silvanusOntology#Relative_humidity">
        <rdfs:subClassOf rdf:resource="http://www.semanticweb.org/smarotta/ontologies/2022/4/silvanusOntology#Climate_parameter"/>
        <silvanusOntology:source>&quot;https://cwfis.cfs.nrcan.gc.ca/background/summary/fwi</silvanusOntology:source>
        <rdfs:comment>Humidity is associated with the water content in gaseous phase present in the air.Relative humidity is the percentage or ratio of the amount of water vapor in a volume of air at a given temperature and the amount that it can hold at that given temperature. An amount of water vapor in warm air will result to a lower relative humidity than in cool air.</rdfs:comment>
    </owl:Class>
    


    <!-- http://www.semanticweb.org/smarotta/ontologies/2022/4/silvanusOntology#Reliability -->

    <owl:Class rdf:about="http://www.semanticweb.org/smarotta/ontologies/2022/4/silvanusOntology#Reliability">
        <rdfs:comment xml:lang="en">Reliability of the measurement</rdfs:comment>
        <rdfs:seeAlso>http://crossforest.eu/measures/ontology/Reliability</rdfs:seeAlso>
    </owl:Class>
    


    <!-- http://www.semanticweb.org/smarotta/ontologies/2022/4/silvanusOntology#ReliefItem -->

    <owl:Class rdf:about="http://www.semanticweb.org/smarotta/ontologies/2022/4/silvanusOntology#ReliefItem">
        <rdfs:subClassOf rdf:resource="http://www.semanticweb.org/smarotta/ontologies/2022/4/silvanusOntology#Item"/>
        <rdfs:comment>Relief items for people affected by fire</rdfs:comment>
        <rdfs:seeAlso>http://www.semanticweb.org/earthquake#ReliefItem</rdfs:seeAlso>
    </owl:Class>
    


    <!-- http://www.semanticweb.org/smarotta/ontologies/2022/4/silvanusOntology#Replacement -->

    <owl:Class rdf:about="http://www.semanticweb.org/smarotta/ontologies/2022/4/silvanusOntology#Replacement">
        <rdfs:subClassOf rdf:resource="http://www.semanticweb.org/smarotta/ontologies/2022/4/silvanusOntology#Fire_severity"/>
        <silvanusOntology:source>https://www.fs.fed.us/database/feis/glossary2.html#ReplacementSeverityFire</silvanusOntology:source>
        <rdfs:comment>A fire that causes &gt;75% kill or top-kill of the upper canopy layer (&gt;80%, according to Smith&apos;s [122] definition of stand-replacing fire), reverting vegetation to an earlier successional stage. Can be applied to all vegetation formations (forests, woodlands, shrublands, and grasslands). Replacement-severity fire may kill or only top-kill the plants in the upper canopy layer. LANDFIRE documentation states explicitly that replacement of the upper canopy can occur in any vegetation formation: &quot;replacement fire in grassland removes the leaves, but leaves sprout from the basal crown, whereas replacement fire in most conifers causes mortality of the plant&quot;</rdfs:comment>
    </owl:Class>
    


    <!-- http://www.semanticweb.org/smarotta/ontologies/2022/4/silvanusOntology#Replacement-severity_fire -->

    <owl:Class rdf:about="http://www.semanticweb.org/smarotta/ontologies/2022/4/silvanusOntology#Replacement-severity_fire">
        <rdfs:subClassOf rdf:resource="http://www.semanticweb.org/smarotta/ontologies/2022/4/silvanusOntology#Uncontrolled_fire"/>
        <silvanusOntology:source>https://www.fs.fed.us/database/feis/glossary2.html</silvanusOntology:source>
        <rdfs:comment>A fire that causes &gt;75% kill or top-kill of the upper canopy layer (&gt;80%, according to Smith&apos;s [122] definition of stand-replacing fire), reverting vegetation to an earlier successional stage. Can be applied to all vegetation formations (forests, woodlands, shrublands, and grasslands). Replacement-severity fire may kill or only top-kill the plants in the upper canopy layer. LANDFIRE documentation states explicitly that replacement of the upper canopy can occur in any vegetation formation: &quot;replacement fire in grassland removes the leaves, but leaves sprout from the basal crown, whereas replacement fire in most conifers causes mortality of the plant&quot; [9]. See stand-replacement fire and fire severity.</rdfs:comment>
    </owl:Class>
    


    <!-- http://www.semanticweb.org/smarotta/ontologies/2022/4/silvanusOntology#RescueTeam -->

    <owl:Class rdf:about="http://www.semanticweb.org/smarotta/ontologies/2022/4/silvanusOntology#RescueTeam">
        <rdfs:subClassOf rdf:resource="http://www.semanticweb.org/smarotta/ontologies/2022/4/silvanusOntology#Response_resource"/>
        <rdfs:comment>Rescue team</rdfs:comment>
        <rdfs:seeAlso>http://www.semanticweb.org/earthquake#RescueTeam</rdfs:seeAlso>
    </owl:Class>
    


    <!-- http://www.semanticweb.org/smarotta/ontologies/2022/4/silvanusOntology#Reservoir -->

    <owl:Class rdf:about="http://www.semanticweb.org/smarotta/ontologies/2022/4/silvanusOntology#Reservoir">
        <rdfs:subClassOf rdf:resource="http://www.semanticweb.org/smarotta/ontologies/2022/4/silvanusOntology#Water_supply"/>
        <silvanusOntology:source>Portuguese pilot</silvanusOntology:source>
        <rdfs:comment>Water reservoirs locations for airborne firefighting water tanks refilling. Include only the possible locations.</rdfs:comment>
    </owl:Class>
    


    <!-- http://www.semanticweb.org/smarotta/ontologies/2022/4/silvanusOntology#ResourceUnitLeader -->

    <owl:Class rdf:about="http://www.semanticweb.org/smarotta/ontologies/2022/4/silvanusOntology#ResourceUnitLeader">
        <rdfs:subClassOf rdf:resource="http://www.semanticweb.org/smarotta/ontologies/2022/4/silvanusOntology#Responder"/>
        <rdfs:comment>The Resources Unit Leader (RESL) establishes all incident check-in activities including preparing and processing resource status information and maintaining a master list of resources assigned to the incident and their assignment at the incident. The RESL supervises the Status/Check-in Recorder (SCKN) and reports to the Planning Section Chief (PSC). The RESL works in the Planning functional area.</rdfs:comment>
        <rdfs:seeAlso>http://www.semanticweb.org/earthquake#ResourceUnitLeader</rdfs:seeAlso>
    </owl:Class>
    


    <!-- http://www.semanticweb.org/smarotta/ontologies/2022/4/silvanusOntology#Responder -->

    <owl:Class rdf:about="http://www.semanticweb.org/smarotta/ontologies/2022/4/silvanusOntology#Responder">
        <rdfs:subClassOf rdf:resource="http://www.semanticweb.org/smarotta/ontologies/2022/4/silvanusOntology#Response_resource"/>
        <rdfs:comment>Represents a first responder unit.</rdfs:comment>
        <rdfs:seeAlso>http://www.semanticweb.org/earthquake#FirstResponder</rdfs:seeAlso>
        <rdfs:seeAlso>https://raw.githubusercontent.com/beAWARE-project/ontology/master/beAWARE_ontology#Responder</rdfs:seeAlso>
    </owl:Class>
    


    <!-- http://www.semanticweb.org/smarotta/ontologies/2022/4/silvanusOntology#Response_procedure -->

    <owl:Class rdf:about="http://www.semanticweb.org/smarotta/ontologies/2022/4/silvanusOntology#Response_procedure">
        <rdfs:subClassOf rdf:resource="http://www.semanticweb.org/smarotta/ontologies/2022/4/silvanusOntology#Response_resource"/>
        <rdfs:comment>Response procedure</rdfs:comment>
        <rdfs:seeAlso>http://www.semanticweb.org/earthquake#Emergency_Response</rdfs:seeAlso>
    </owl:Class>
    


    <!-- http://www.semanticweb.org/smarotta/ontologies/2022/4/silvanusOntology#Response_resource -->

    <owl:Class rdf:about="http://www.semanticweb.org/smarotta/ontologies/2022/4/silvanusOntology#Response_resource">
        <rdfs:comment>Assets for fighting the fire</rdfs:comment>
        <rdfs:seeAlso>http://www.semanticweb.org/earthquake#Resources</rdfs:seeAlso>
    </owl:Class>
    


    <!-- http://www.semanticweb.org/smarotta/ontologies/2022/4/silvanusOntology#Response_vehicle -->

    <owl:Class rdf:about="http://www.semanticweb.org/smarotta/ontologies/2022/4/silvanusOntology#Response_vehicle">
        <rdfs:subClassOf rdf:resource="http://www.semanticweb.org/smarotta/ontologies/2022/4/silvanusOntology#Response_resource"/>
        <rdfs:comment>Vehicle for emergency response</rdfs:comment>
    </owl:Class>
    


    <!-- http://www.semanticweb.org/smarotta/ontologies/2022/4/silvanusOntology#Responsible -->

    <owl:Class rdf:about="http://www.semanticweb.org/smarotta/ontologies/2022/4/silvanusOntology#Responsible">
        <rdfs:subClassOf rdf:resource="http://www.semanticweb.org/smarotta/ontologies/2022/4/silvanusOntology#Deliberate"/>
        <silvanusOntology:source>https://effis-gwis-cms.s3-eu-west-1.amazonaws.com/effis/reports-and-publications/effis-related-publications/lb-na-25-923-en-n.pdf (page 10)</silvanusOntology:source>
        <rdfs:comment>Wildfire wilfully ignited by people over the legal age, which burns or spreads to vegetation or property without consent of the owner.</rdfs:comment>
    </owl:Class>
    


    <!-- http://www.semanticweb.org/smarotta/ontologies/2022/4/silvanusOntology#Resprouer -->

    <owl:Class rdf:about="http://www.semanticweb.org/smarotta/ontologies/2022/4/silvanusOntology#Resprouer">
        <rdfs:subClassOf rdf:resource="http://www.semanticweb.org/smarotta/ontologies/2022/4/silvanusOntology#Fire_strategy"/>
        <owl:disjointWith rdf:resource="http://www.semanticweb.org/smarotta/ontologies/2022/4/silvanusOntology#Serotinous"/>
        <silvanusOntology:source>https://botany.one/2020/10/four-plant-strategies-to-deal-with-fire/</silvanusOntology:source>
        <rdfs:comment>Species can survive fires and resprout</rdfs:comment>
    </owl:Class>
    


    <!-- http://www.semanticweb.org/smarotta/ontologies/2022/4/silvanusOntology#RightBound -->

    <owl:Class rdf:about="http://www.semanticweb.org/smarotta/ontologies/2022/4/silvanusOntology#RightBound">
        <rdfs:subClassOf rdf:resource="http://www.semanticweb.org/smarotta/ontologies/2022/4/silvanusOntology#Spatial_entity"/>
        <rdfs:comment>Right boundary of an area</rdfs:comment>
        <rdfs:seeAlso>http://crossforest.eu/position/ontology/RightBound</rdfs:seeAlso>
    </owl:Class>
    


    <!-- http://www.semanticweb.org/smarotta/ontologies/2022/4/silvanusOntology#River -->

    <owl:Class rdf:about="http://www.semanticweb.org/smarotta/ontologies/2022/4/silvanusOntology#River">
        <rdfs:subClassOf rdf:resource="http://www.semanticweb.org/smarotta/ontologies/2022/4/silvanusOntology#Ecological_asset"/>
        <rdfs:comment>Represents rivers.</rdfs:comment>
        <rdfs:seeAlso>https://raw.githubusercontent.com/beAWARE-project/ontology/master/beAWARE_ontology#River</rdfs:seeAlso>
    </owl:Class>
    


    <!-- http://www.semanticweb.org/smarotta/ontologies/2022/4/silvanusOntology#Rreaction_intensity -->

    <owl:Class rdf:about="http://www.semanticweb.org/smarotta/ontologies/2022/4/silvanusOntology#Rreaction_intensity">
        <rdfs:subClassOf rdf:resource="http://www.semanticweb.org/smarotta/ontologies/2022/4/silvanusOntology#Fire_characteristic"/>
        <silvanusOntology:source>https://www.fs.fed.us/database/feis/glossary2.html#ReactionIntensity</silvanusOntology:source>
        <rdfs:comment>The energy release rate of the fire front. The energy is released when burning gases are released from combustable organic matter in fuels; therefore, fuel parameters including particle size, bulk density, moisture, and chemical composition are factors determining reation intensity. Expressed as the amount of heat released/unit area2 [115].</rdfs:comment>
    </owl:Class>
    


    <!-- http://www.semanticweb.org/smarotta/ontologies/2022/4/silvanusOntology#SafetyOfficer -->

    <owl:Class rdf:about="http://www.semanticweb.org/smarotta/ontologies/2022/4/silvanusOntology#SafetyOfficer">
        <rdfs:subClassOf rdf:resource="http://www.semanticweb.org/smarotta/ontologies/2022/4/silvanusOntology#Responder"/>
        <rdfs:comment>Safety officers will be responsible for the following:

Identifying safety issues
Starting corrective action
Maintaining safe systems of work;
Ensuring people are wearing appropriate personal protection equipment
Observing the working environment
Monitoring physical condition of crews
Regular reviews
Recording an analytical risk assessment
Updating the incident commander when circumstances change

This is not an exhaustive list.</rdfs:comment>
        <rdfs:seeAlso>http://www.semanticweb.org/earthquake#SafetyOfficer</rdfs:seeAlso>
    </owl:Class>
    


    <!-- http://www.semanticweb.org/smarotta/ontologies/2022/4/silvanusOntology#SanitaryEquipment -->

    <owl:Class rdf:about="http://www.semanticweb.org/smarotta/ontologies/2022/4/silvanusOntology#SanitaryEquipment">
        <rdfs:subClassOf rdf:resource="http://www.semanticweb.org/smarotta/ontologies/2022/4/silvanusOntology#ReliefItem"/>
        <rdfs:comment>Sanitary equipment items</rdfs:comment>
        <rdfs:seeAlso>http://www.semanticweb.org/earthquake#SanitaryEquipment</rdfs:seeAlso>
    </owl:Class>
    


    <!-- http://www.semanticweb.org/smarotta/ontologies/2022/4/silvanusOntology#Satellite -->

    <owl:Class rdf:about="http://www.semanticweb.org/smarotta/ontologies/2022/4/silvanusOntology#Satellite">
        <rdfs:subClassOf rdf:resource="http://www.semanticweb.org/smarotta/ontologies/2022/4/silvanusOntology#Sensor"/>
        <silvanusOntology:source>Most pilots</silvanusOntology:source>
        <rdfs:comment>An artificial body placed in orbit round the earth or moon or another planet in order to collect information or for communication.</rdfs:comment>
    </owl:Class>
    


    <!-- http://www.semanticweb.org/smarotta/ontologies/2022/4/silvanusOntology#Savanna -->

    <owl:Class rdf:about="http://www.semanticweb.org/smarotta/ontologies/2022/4/silvanusOntology#Savanna">
        <rdfs:subClassOf rdf:resource="http://www.semanticweb.org/smarotta/ontologies/2022/4/silvanusOntology#Biodiversity_index"/>
        <silvanusOntology:source>https://www.fs.fed.us/database/feis/glossary2.html#savanna</silvanusOntology:source>
        <rdfs:comment>A formation in which the overstory is dominated by woody vegetation growing as scattered individuals or clusters. The dominant life form may be trees (i.e., tree savanna; dominants are &gt;6.5 feet (2 m) tall) or shrubs (i.e., shrub savanna; dominants are ≤6.5 feet (2 m) tall) [112]. The understory is composed of grass; shrubs are sparse to absent [113,120]. When describing savannas, use of a hyphen indicates about equal cover of dominant overstory and understory species (e.g., Oregon white oak-California brome savanna). Compare with grassland, shrubland woodland, wooded shrubland, forest.</rdfs:comment>
    </owl:Class>
    


    <!-- http://www.semanticweb.org/smarotta/ontologies/2022/4/silvanusOntology#Sawmill -->

    <owl:Class rdf:about="http://www.semanticweb.org/smarotta/ontologies/2022/4/silvanusOntology#Sawmill">
        <rdfs:subClassOf rdf:resource="http://www.semanticweb.org/smarotta/ontologies/2022/4/silvanusOntology#Industrial_building"/>
        <rdfs:comment>A building within which logs are cut into lumber products.</rdfs:comment>
        <rdfs:seeAlso>http://purl.obolibrary.org/obo/ENVO_00004638</rdfs:seeAlso>
    </owl:Class>
    


    <!-- http://www.semanticweb.org/smarotta/ontologies/2022/4/silvanusOntology#Scrub_fire -->

    <owl:Class rdf:about="http://www.semanticweb.org/smarotta/ontologies/2022/4/silvanusOntology#Scrub_fire">
        <rdfs:subClassOf rdf:resource="http://www.semanticweb.org/smarotta/ontologies/2022/4/silvanusOntology#Fire"/>
        <rdfs:comment>A fire in scrubby trees.</rdfs:comment>
        <rdfs:seeAlso>http://cerrado.linkeddata.es/ecology/fire#ScrubFire</rdfs:seeAlso>
    </owl:Class>
    


    <!-- http://www.semanticweb.org/smarotta/ontologies/2022/4/silvanusOntology#Scrubland_Area -->

    <owl:Class rdf:about="http://www.semanticweb.org/smarotta/ontologies/2022/4/silvanusOntology#Scrubland_Area">
        <rdfs:subClassOf rdf:resource="http://www.semanticweb.org/smarotta/ontologies/2022/4/silvanusOntology#Vegetated_area"/>
        <rdfs:comment>Area covered with low-growing or stunted perennial vegetation and usually not mixed with trees.</rdfs:comment>
        <rdfs:seeAlso>http://purl.obolibrary.org/obo/ENVO_00000300</rdfs:seeAlso>
    </owl:Class>
    


    <!-- http://www.semanticweb.org/smarotta/ontologies/2022/4/silvanusOntology#SearchAndRescue -->

    <owl:Class rdf:about="http://www.semanticweb.org/smarotta/ontologies/2022/4/silvanusOntology#SearchAndRescue">
        <rdfs:subClassOf rdf:resource="http://www.semanticweb.org/smarotta/ontologies/2022/4/silvanusOntology#Response_procedure"/>
        <rdfs:comment>Search and rescue operations</rdfs:comment>
        <rdfs:seeAlso>http://www.semanticweb.org/earthquake#SearchAndRescue</rdfs:seeAlso>
    </owl:Class>
    


    <!-- http://www.semanticweb.org/smarotta/ontologies/2022/4/silvanusOntology#Season -->

    <owl:Class rdf:about="http://www.semanticweb.org/smarotta/ontologies/2022/4/silvanusOntology#Season">
        <rdfs:subClassOf rdf:resource="http://www.semanticweb.org/smarotta/ontologies/2022/4/silvanusOntology#Climate_parameter"/>
        <rdfs:comment>Season of the year</rdfs:comment>
        <rdfs:seeAlso>https://bimerr.iot.linkeddata.es/def/weather#Season</rdfs:seeAlso>
    </owl:Class>
    


    <!-- http://www.semanticweb.org/smarotta/ontologies/2022/4/silvanusOntology#Self-ignition -->

    <owl:Class rdf:about="http://www.semanticweb.org/smarotta/ontologies/2022/4/silvanusOntology#Self-ignition">
        <rdfs:subClassOf rdf:resource="http://www.semanticweb.org/smarotta/ontologies/2022/4/silvanusOntology#Accident"/>
        <silvanusOntology:source>https://effis-gwis-cms.s3-eu-west-1.amazonaws.com/effis/reports-and-publications/effis-related-publications/lb-na-25-923-en-n.pdf (page 10)</silvanusOntology:source>
        <rdfs:comment>Wildfire caused by self-ignition of vegetation wastes and other products left in piles.</rdfs:comment>
    </owl:Class>
    


    <!-- http://www.semanticweb.org/smarotta/ontologies/2022/4/silvanusOntology#Sensor -->

    <owl:Class rdf:about="http://www.semanticweb.org/smarotta/ontologies/2022/4/silvanusOntology#Sensor">
        <rdfs:comment>A Sensor is an instrument that observes a property or phenomenon with the goal of producing an estimate of the value of a parameter.</rdfs:comment>
        <rdfs:seeAlso>http://www.semanticweb.org/earthquake#Instruments</rdfs:seeAlso>
        <rdfs:seeAlso>http://www.w3.org/ns/sosa/Sensor</rdfs:seeAlso>
        <rdfs:seeAlso>https://raw.githubusercontent.com/beAWARE-project/ontology/master/beAWARE_ontology#Sensor</rdfs:seeAlso>
    </owl:Class>
    


    <!-- http://www.semanticweb.org/smarotta/ontologies/2022/4/silvanusOntology#Serotinous -->

    <owl:Class rdf:about="http://www.semanticweb.org/smarotta/ontologies/2022/4/silvanusOntology#Serotinous">
        <rdfs:subClassOf rdf:resource="http://www.semanticweb.org/smarotta/ontologies/2022/4/silvanusOntology#Fire_strategy"/>
        <silvanusOntology:source>https://botany.one/2020/10/four-plant-strategies-to-deal-with-fire/</silvanusOntology:source>
        <rdfs:comment>Species disperse seeds postfires</rdfs:comment>
    </owl:Class>
    


    <!-- http://www.semanticweb.org/smarotta/ontologies/2022/4/silvanusOntology#Sewer -->

    <owl:Class rdf:about="http://www.semanticweb.org/smarotta/ontologies/2022/4/silvanusOntology#Sewer">
        <rdfs:subClassOf rdf:resource="http://www.semanticweb.org/smarotta/ontologies/2022/4/silvanusOntology#Infrastructure"/>
        <rdfs:comment>Represents sewage infrastructure.</rdfs:comment>
        <rdfs:seeAlso>http://www.semanticweb.org/earthquake#SewageSystem</rdfs:seeAlso>
        <rdfs:seeAlso>https://raw.githubusercontent.com/beAWARE-project/ontology/master/beAWARE_ontology#Sewer</rdfs:seeAlso>
    </owl:Class>
    


    <!-- http://www.semanticweb.org/smarotta/ontologies/2022/4/silvanusOntology#Shrubland -->

    <owl:Class rdf:about="http://www.semanticweb.org/smarotta/ontologies/2022/4/silvanusOntology#Shrubland">
        <rdfs:subClassOf rdf:resource="http://www.semanticweb.org/smarotta/ontologies/2022/4/silvanusOntology#Biodiversity_index"/>
        <silvanusOntology:source>https://www.fs.fed.us/database/feis/glossary2.html#shrubland</silvanusOntology:source>
        <rdfs:comment>A formation in which the overstory is dominated by shrubs 1.6 to 16 feet (0.5-5 m) tall, and trees have &lt;5% total cover [75]. Compare with grassland, woodland, wooded shrubland, savanna, forest.</rdfs:comment>
    </owl:Class>
    


    <!-- http://www.semanticweb.org/smarotta/ontologies/2022/4/silvanusOntology#Shrubland_Biome -->

    <owl:Class rdf:about="http://www.semanticweb.org/smarotta/ontologies/2022/4/silvanusOntology#Shrubland_Biome">
        <rdfs:subClassOf rdf:resource="http://www.semanticweb.org/smarotta/ontologies/2022/4/silvanusOntology#Terrestrial_Biome"/>
        <rdfs:comment>A shrubland biome is a terrestrial biome which includes, across its entire spatial extent, dense groups of shrubs.</rdfs:comment>
        <rdfs:seeAlso>http://purl.obolibrary.org/obo/ENVO_01000176</rdfs:seeAlso>
    </owl:Class>
    


    <!-- http://www.semanticweb.org/smarotta/ontologies/2022/4/silvanusOntology#Silvanus_module -->

    <owl:Class rdf:about="http://www.semanticweb.org/smarotta/ontologies/2022/4/silvanusOntology#Silvanus_module">
        <rdfs:comment>A task that has to do with analyzing or processing items.</rdfs:comment>
        <rdfs:seeAlso>https://raw.githubusercontent.com/beAWARE-project/ontology/master/beAWARE_ontology#Task</rdfs:seeAlso>
    </owl:Class>
    


    <!-- http://www.semanticweb.org/smarotta/ontologies/2022/4/silvanusOntology#Sky_Cover -->

    <owl:Class rdf:about="http://www.semanticweb.org/smarotta/ontologies/2022/4/silvanusOntology#Sky_Cover">
        <rdfs:subClassOf rdf:resource="http://www.semanticweb.org/smarotta/ontologies/2022/4/silvanusOntology#Climate_parameter"/>
        <rdfs:comment xml:lang="en">The extent to which the sky is obscured by clouds.</rdfs:comment>
        <rdfs:seeAlso>https://bimerr.iot.linkeddata.es/def/weather#SkyCover</rdfs:seeAlso>
    </owl:Class>
    


    <!-- http://www.semanticweb.org/smarotta/ontologies/2022/4/silvanusOntology#Small_region_for_specific_diagnoses -->

    <owl:Class rdf:about="http://www.semanticweb.org/smarotta/ontologies/2022/4/silvanusOntology#Small_region_for_specific_diagnoses">
        <rdfs:subClassOf rdf:resource="http://www.semanticweb.org/smarotta/ontologies/2022/4/silvanusOntology#NUTS_unit"/>
        <rdfs:comment>NUTS 3: as small regions for specific diagnoses</rdfs:comment>
        <rdfs:seeAlso>http://crossforest.eu/ifi/ontology/NUTS3</rdfs:seeAlso>
    </owl:Class>
    


    <!-- http://www.semanticweb.org/smarotta/ontologies/2022/4/silvanusOntology#Smoke_amount -->

    <owl:Class rdf:about="http://www.semanticweb.org/smarotta/ontologies/2022/4/silvanusOntology#Smoke_amount">
        <rdfs:subClassOf rdf:resource="http://www.semanticweb.org/smarotta/ontologies/2022/4/silvanusOntology#Fire_characteristic"/>
        <silvanusOntology:source>French pilot</silvanusOntology:source>
        <rdfs:comment>Amount of smoke in the air</rdfs:comment>
    </owl:Class>
    


    <!-- http://www.semanticweb.org/smarotta/ontologies/2022/4/silvanusOntology#Smoke_detector -->

    <owl:Class rdf:about="http://www.semanticweb.org/smarotta/ontologies/2022/4/silvanusOntology#Smoke_detector">
        <rdfs:subClassOf rdf:resource="http://www.semanticweb.org/smarotta/ontologies/2022/4/silvanusOntology#Chemical_sensor"/>
        <silvanusOntology:source>French pilot</silvanusOntology:source>
        <rdfs:comment>A smoke detector is a device that senses smoke, typically as an indicator of fire.</rdfs:comment>
    </owl:Class>
    


    <!-- http://www.semanticweb.org/smarotta/ontologies/2022/4/silvanusOntology#Soil -->

    <owl:Class rdf:about="http://www.semanticweb.org/smarotta/ontologies/2022/4/silvanusOntology#Soil">
        <rdfs:subClassOf rdf:resource="http://www.semanticweb.org/smarotta/ontologies/2022/4/silvanusOntology#Evnironment_index"/>
        <rdfs:comment>Ground properties where the measures are made.</rdfs:comment>
        <rdfs:seeAlso>https://bimerr.iot.linkeddata.es/def/weather#Ground</rdfs:seeAlso>
    </owl:Class>
    


    <!-- http://www.semanticweb.org/smarotta/ontologies/2022/4/silvanusOntology#Soil_pH -->

    <owl:Class rdf:about="http://www.semanticweb.org/smarotta/ontologies/2022/4/silvanusOntology#Soil_pH">
        <rdfs:subClassOf rdf:resource="http://www.semanticweb.org/smarotta/ontologies/2022/4/silvanusOntology#Evnironment_index"/>
        <silvanusOntology:source>Indonesian pilot</silvanusOntology:source>
        <rdfs:comment>Soil pH is a measure of the acidity or basicity (alkalinity) of a soil. Soil pH is a key characteristic that can be used to make informative analysis both qualitative and quantitatively regarding soil characteristics.</rdfs:comment>
    </owl:Class>
    


    <!-- http://www.semanticweb.org/smarotta/ontologies/2022/4/silvanusOntology#Soil_structure -->

    <owl:Class rdf:about="http://www.semanticweb.org/smarotta/ontologies/2022/4/silvanusOntology#Soil_structure">
        <rdfs:subClassOf rdf:resource="http://www.semanticweb.org/smarotta/ontologies/2022/4/silvanusOntology#Evnironment_index"/>
        <silvanusOntology:source>Indonesian pilot</silvanusOntology:source>
        <rdfs:comment>Soil structure describes the arrangement of the solid parts of the soil and of the pore spaces located between them (Marshall &amp; Holmes, 1979).</rdfs:comment>
    </owl:Class>
    


    <!-- http://www.semanticweb.org/smarotta/ontologies/2022/4/silvanusOntology#Soil_type -->

    <owl:Class rdf:about="http://www.semanticweb.org/smarotta/ontologies/2022/4/silvanusOntology#Soil_type">
        <rdfs:subClassOf rdf:resource="http://www.semanticweb.org/smarotta/ontologies/2022/4/silvanusOntology#Evnironment_index"/>
        <silvanusOntology:source>Indonesian pilot</silvanusOntology:source>
        <rdfs:comment>A soil type is a taxonomic unit in soil science. All soils that share a certain set of well-defined properties form a distinctive soil type.[1] Soil type is a technical term of soil classification, the science that deals with the systematic categorization of soils. Every soil of the world belongs to a certain soil type. Soil type is an abstract term. In nature, you will not find soil types. You will find soils that belong to a certain soil type.</rdfs:comment>
    </owl:Class>
    


    <!-- http://www.semanticweb.org/smarotta/ontologies/2022/4/silvanusOntology#Spatial_entity -->

    <owl:Class rdf:about="http://www.semanticweb.org/smarotta/ontologies/2022/4/silvanusOntology#Spatial_entity">
        <rdfs:comment>It&apos;s the entity used to describe the spatial reations between entities or other elements.</rdfs:comment>
        <rdfs:seeAlso>http://ecoinformatics.org/oboe/oboe.1.0/oboe-spatial.owl#SpatialEntity</rdfs:seeAlso>
        <rdfs:seeAlso>http://www.w3.org/2003/01/geo/wgs84_pos#SpatialThing</rdfs:seeAlso>
    </owl:Class>
    


    <!-- http://www.semanticweb.org/smarotta/ontologies/2022/4/silvanusOntology#Species_richness -->

    <owl:Class rdf:about="http://www.semanticweb.org/smarotta/ontologies/2022/4/silvanusOntology#Species_richness">
        <rdfs:subClassOf rdf:resource="http://www.semanticweb.org/smarotta/ontologies/2022/4/silvanusOntology#Biodiversity_index"/>
        <silvanusOntology:source>https://www.fs.fed.us/database/feis/glossary2.html</silvanusOntology:source>
        <rdfs:comment>The number of different species represented in an ecological community, landscape or region [26].</rdfs:comment>
    </owl:Class>
    


    <!-- http://www.semanticweb.org/smarotta/ontologies/2022/4/silvanusOntology#Spirometer -->

    <owl:Class rdf:about="http://www.semanticweb.org/smarotta/ontologies/2022/4/silvanusOntology#Spirometer">
        <rdfs:subClassOf rdf:resource="http://www.semanticweb.org/smarotta/ontologies/2022/4/silvanusOntology#Health_sensor"/>
        <silvanusOntology:source>AHEPA</silvanusOntology:source>
        <rdfs:comment>A spirometer is an apparatus for measuring the volume of air inspired and expired by the lungs. A spirometer measures ventilation, the movement of air into and out of the lungs. The spirogram will identify two different types of abnormal ventilation patterns, obstructive and restrictive.</rdfs:comment>
    </owl:Class>
    


    <!-- http://www.semanticweb.org/smarotta/ontologies/2022/4/silvanusOntology#Square -->

    <owl:Class rdf:about="http://www.semanticweb.org/smarotta/ontologies/2022/4/silvanusOntology#Square">
        <rdfs:subClassOf rdf:resource="http://www.semanticweb.org/smarotta/ontologies/2022/4/silvanusOntology#Structure"/>
        <rdfs:comment>Represents squares in danger during an environmental crisis.</rdfs:comment>
        <rdfs:seeAlso>https://raw.githubusercontent.com/beAWARE-project/ontology/master/beAWARE_ontology#Square</rdfs:seeAlso>
    </owl:Class>
    


    <!-- http://www.semanticweb.org/smarotta/ontologies/2022/4/silvanusOntology#Starting_point -->

    <owl:Class rdf:about="http://www.semanticweb.org/smarotta/ontologies/2022/4/silvanusOntology#Starting_point">
        <rdfs:subClassOf rdf:resource="http://www.semanticweb.org/smarotta/ontologies/2022/4/silvanusOntology#Spatial_entity"/>
        <rdfs:comment>Starting point of a space</rdfs:comment>
        <rdfs:seeAlso>http://cerrado.linkeddata.es/ecology/fire#StartingPoint</rdfs:seeAlso>
    </owl:Class>
    


    <!-- http://www.semanticweb.org/smarotta/ontologies/2022/4/silvanusOntology#Starting_time -->

    <owl:Class rdf:about="http://www.semanticweb.org/smarotta/ontologies/2022/4/silvanusOntology#Starting_time">
        <rdfs:subClassOf rdf:resource="http://www.semanticweb.org/smarotta/ontologies/2022/4/silvanusOntology#Temporal_entity"/>
        <rdfs:comment>Starting timestamp of an event</rdfs:comment>
        <rdfs:seeAlso>http://cerrado.linkeddata.es/ecology/fire#StartingTime</rdfs:seeAlso>
    </owl:Class>
    


    <!-- http://www.semanticweb.org/smarotta/ontologies/2022/4/silvanusOntology#Static_camera -->

    <owl:Class rdf:about="http://www.semanticweb.org/smarotta/ontologies/2022/4/silvanusOntology#Static_camera">
        <rdfs:subClassOf rdf:resource="http://www.semanticweb.org/smarotta/ontologies/2022/4/silvanusOntology#Camera"/>
        <silvanusOntology:source>Italian pilot</silvanusOntology:source>
        <rdfs:comment>Static Camera means a Body type or Non-PTZ camera installed in a fixed position at a fixed field of view. Static Cameras may have variable zoom capabilities.</rdfs:comment>
    </owl:Class>
    


    <!-- http://www.semanticweb.org/smarotta/ontologies/2022/4/silvanusOntology#Street -->

    <owl:Class rdf:about="http://www.semanticweb.org/smarotta/ontologies/2022/4/silvanusOntology#Street">
        <rdfs:subClassOf rdf:resource="http://www.semanticweb.org/smarotta/ontologies/2022/4/silvanusOntology#Transportation"/>
        <rdfs:comment>Represents the road network infrastructure.</rdfs:comment>
        <rdfs:seeAlso>http://purl.obolibrary.org/obo/ENVO_00000064</rdfs:seeAlso>
        <rdfs:seeAlso>http://www.semanticweb.org/earthquake#RoadLoss</rdfs:seeAlso>
        <rdfs:seeAlso>https://raw.githubusercontent.com/beAWARE-project/ontology/master/beAWARE_ontology#Street</rdfs:seeAlso>
    </owl:Class>
    


    <!-- http://www.semanticweb.org/smarotta/ontologies/2022/4/silvanusOntology#Structure -->

    <owl:Class rdf:about="http://www.semanticweb.org/smarotta/ontologies/2022/4/silvanusOntology#Structure">
        <rdfs:subClassOf rdf:resource="http://www.semanticweb.org/smarotta/ontologies/2022/4/silvanusOntology#Asset"/>
        <silvanusOntology:output>Building Infrastructure characterized and displayed on map</silvanusOntology:output>
        <rdfs:comment>Represents various structures and buildings.</rdfs:comment>
        <rdfs:seeAlso>http://purl.obolibrary.org/obo/ENVO_00000070</rdfs:seeAlso>
        <rdfs:seeAlso>https://raw.githubusercontent.com/beAWARE-project/ontology/master/beAWARE_ontology#Structure</rdfs:seeAlso>
    </owl:Class>
    


    <!-- http://www.semanticweb.org/smarotta/ontologies/2022/4/silvanusOntology#Subalpine_Biome -->

    <owl:Class rdf:about="http://www.semanticweb.org/smarotta/ontologies/2022/4/silvanusOntology#Subalpine_Biome">
        <rdfs:subClassOf rdf:resource="http://www.semanticweb.org/smarotta/ontologies/2022/4/silvanusOntology#Biome"/>
        <rdfs:comment>A biome which is subject to subapline altitudinal conditions.</rdfs:comment>
        <rdfs:seeAlso>http://purl.obolibrary.org/obo/ENVO_01001837</rdfs:seeAlso>
    </owl:Class>
    


    <!-- http://www.semanticweb.org/smarotta/ontologies/2022/4/silvanusOntology#Subpolar_Biome -->

    <owl:Class rdf:about="http://www.semanticweb.org/smarotta/ontologies/2022/4/silvanusOntology#Subpolar_Biome">
        <rdfs:subClassOf rdf:resource="http://www.semanticweb.org/smarotta/ontologies/2022/4/silvanusOntology#Biome"/>
        <rdfs:comment>A biome which is subject to subpolar climatic conditions.</rdfs:comment>
        <rdfs:seeAlso>http://purl.obolibrary.org/obo/ENVO_01001834</rdfs:seeAlso>
    </owl:Class>
    


    <!-- http://www.semanticweb.org/smarotta/ontologies/2022/4/silvanusOntology#Substation -->

    <owl:Class rdf:about="http://www.semanticweb.org/smarotta/ontologies/2022/4/silvanusOntology#Substation">
        <rdfs:subClassOf rdf:resource="http://www.semanticweb.org/smarotta/ontologies/2022/4/silvanusOntology#Energy"/>
        <silvanusOntology:source>Portuguese pilot</silvanusOntology:source>
        <rdfs:comment>A substation is a part of an electrical generation, transmission, and distribution system. Substations transform voltage from high to low, or the reverse, or perform any of several other important functions. Between the generating station and consumer, electric power may flow through several substations at different voltage levels. A substation may include transformers to change voltage levels between high transmission voltages and lower distribution voltages, or at the interconnection of two different transmission voltages.</rdfs:comment>
    </owl:Class>
    


    <!-- http://www.semanticweb.org/smarotta/ontologies/2022/4/silvanusOntology#Subtropical_Biome -->

    <owl:Class rdf:about="http://www.semanticweb.org/smarotta/ontologies/2022/4/silvanusOntology#Subtropical_Biome">
        <rdfs:subClassOf rdf:resource="http://www.semanticweb.org/smarotta/ontologies/2022/4/silvanusOntology#Biome"/>
        <rdfs:comment>A biome which is subject to subtropical climatic conditions.</rdfs:comment>
        <rdfs:seeAlso>http://purl.obolibrary.org/obo/ENVO_01001832</rdfs:seeAlso>
    </owl:Class>
    


    <!-- http://www.semanticweb.org/smarotta/ontologies/2022/4/silvanusOntology#Subtropical_Shrubland_Biome -->

    <owl:Class rdf:about="http://www.semanticweb.org/smarotta/ontologies/2022/4/silvanusOntology#Subtropical_Shrubland_Biome">
        <rdfs:subClassOf rdf:resource="http://www.semanticweb.org/smarotta/ontologies/2022/4/silvanusOntology#Shrubland_Biome"/>
        <rdfs:comment>A shrubland biome which is subject to subtropical climate patterns.</rdfs:comment>
        <rdfs:seeAlso>http://purl.obolibrary.org/obo/ENVO_01000213</rdfs:seeAlso>
    </owl:Class>
    


    <!-- http://www.semanticweb.org/smarotta/ontologies/2022/4/silvanusOntology#Summer_camp -->

    <owl:Class rdf:about="http://www.semanticweb.org/smarotta/ontologies/2022/4/silvanusOntology#Summer_camp">
        <rdfs:subClassOf rdf:resource="http://www.semanticweb.org/smarotta/ontologies/2022/4/silvanusOntology#Building"/>
        <rdfs:comment>A camp providing recreational and sporting facilities for children during the summer holiday period.</rdfs:comment>
    </owl:Class>
    


    <!-- http://www.semanticweb.org/smarotta/ontologies/2022/4/silvanusOntology#SupplyGood -->

    <owl:Class rdf:about="http://www.semanticweb.org/smarotta/ontologies/2022/4/silvanusOntology#SupplyGood">
        <rdfs:subClassOf rdf:resource="http://www.semanticweb.org/smarotta/ontologies/2022/4/silvanusOntology#Item"/>
        <rdfs:comment>Materials</rdfs:comment>
        <rdfs:seeAlso>http://www.semanticweb.org/earthquake#SupplyGood</rdfs:seeAlso>
    </owl:Class>
    


    <!-- http://www.semanticweb.org/smarotta/ontologies/2022/4/silvanusOntology#SupplyGoodSupport -->

    <owl:Class rdf:about="http://www.semanticweb.org/smarotta/ontologies/2022/4/silvanusOntology#SupplyGoodSupport">
        <rdfs:subClassOf rdf:resource="http://www.semanticweb.org/smarotta/ontologies/2022/4/silvanusOntology#Response_procedure"/>
        <rdfs:comment>Support to the supply of goods</rdfs:comment>
        <rdfs:seeAlso>http://www.semanticweb.org/earthquake#SupplyGoodSupport</rdfs:seeAlso>
    </owl:Class>
    


    <!-- http://www.semanticweb.org/smarotta/ontologies/2022/4/silvanusOntology#SupplyLeader -->

    <owl:Class rdf:about="http://www.semanticweb.org/smarotta/ontologies/2022/4/silvanusOntology#SupplyLeader">
        <rdfs:subClassOf rdf:resource="http://www.semanticweb.org/smarotta/ontologies/2022/4/silvanusOntology#Responder"/>
        <rdfs:comment>The Supply  Leader (SPUL) is primarily responsible for ordering personnel, equipment, and supplies for wildland fire incidents. The SPUL is responsible for overseeing and supervising the ordering and receiving process and determining the right size inventory for the incident.</rdfs:comment>
        <rdfs:seeAlso>http://www.semanticweb.org/earthquake#SupplyLeader</rdfs:seeAlso>
    </owl:Class>
    


    <!-- http://www.semanticweb.org/smarotta/ontologies/2022/4/silvanusOntology#Tank -->

    <owl:Class rdf:about="http://www.semanticweb.org/smarotta/ontologies/2022/4/silvanusOntology#Tank">
        <rdfs:subClassOf rdf:resource="http://www.semanticweb.org/smarotta/ontologies/2022/4/silvanusOntology#Ground_Motor_Vehicle"/>
        <rdfs:comment>An enclosed heavily armed and armored combat vehicle that moves on tracks</rdfs:comment>
        <rdfs:seeAlso>http://www.ontologylibrary.mil/CommonCore/Mid/ArtifactOntology#Tank</rdfs:seeAlso>
    </owl:Class>
    


    <!-- http://www.semanticweb.org/smarotta/ontologies/2022/4/silvanusOntology#TaskForceSectorLeader -->

    <owl:Class rdf:about="http://www.semanticweb.org/smarotta/ontologies/2022/4/silvanusOntology#TaskForceSectorLeader">
        <rdfs:subClassOf rdf:resource="http://www.semanticweb.org/smarotta/ontologies/2022/4/silvanusOntology#Responder"/>
        <rdfs:comment>The Task Force Leader (TFLD) directs any combination of personnel, crews and different types of Incident Command System (ICS) equipment in performing tactical missions on a division or segment of a division, on wildland fire incidents. The TFLD reports to a Division/Group Supervisor (DIVS), Incident Commander (IC), or other assigned supervisor. The TFLD works in the Operations functional area.</rdfs:comment>
        <rdfs:seeAlso>http://www.semanticweb.org/earthquake#TaskForceSectorLeader</rdfs:seeAlso>
    </owl:Class>
    


    <!-- http://www.semanticweb.org/smarotta/ontologies/2022/4/silvanusOntology#Temperate_Biome -->

    <owl:Class rdf:about="http://www.semanticweb.org/smarotta/ontologies/2022/4/silvanusOntology#Temperate_Biome">
        <rdfs:subClassOf rdf:resource="http://www.semanticweb.org/smarotta/ontologies/2022/4/silvanusOntology#Biome"/>
        <rdfs:comment>A biome which is subject to temperate climatic conditions.</rdfs:comment>
        <rdfs:seeAlso>http://purl.obolibrary.org/obo/ENVO_01001831</rdfs:seeAlso>
    </owl:Class>
    


    <!-- http://www.semanticweb.org/smarotta/ontologies/2022/4/silvanusOntology#Temperate_Shrubland_Biome -->

    <owl:Class rdf:about="http://www.semanticweb.org/smarotta/ontologies/2022/4/silvanusOntology#Temperate_Shrubland_Biome">
        <rdfs:subClassOf rdf:resource="http://www.semanticweb.org/smarotta/ontologies/2022/4/silvanusOntology#Shrubland_Biome"/>
        <rdfs:comment>A shrubland biome which is subject to temperate climate patterns.</rdfs:comment>
        <rdfs:seeAlso>http://purl.obolibrary.org/obo/ENVO_01000215</rdfs:seeAlso>
    </owl:Class>
    


    <!-- http://www.semanticweb.org/smarotta/ontologies/2022/4/silvanusOntology#Temperature -->

    <owl:Class rdf:about="http://www.semanticweb.org/smarotta/ontologies/2022/4/silvanusOntology#Temperature">
        <rdfs:subClassOf rdf:resource="http://www.semanticweb.org/smarotta/ontologies/2022/4/silvanusOntology#Climate_parameter"/>
        <silvanusOntology:source>https://cwfis.cfs.nrcan.gc.ca/background/summary/fwi</silvanusOntology:source>
        <rdfs:comment>Temperature in a given area at a given time</rdfs:comment>
        <rdfs:seeAlso>https://bimerr.iot.linkeddata.es/def/weather#Temperature</rdfs:seeAlso>
    </owl:Class>
    


    <!-- http://www.semanticweb.org/smarotta/ontologies/2022/4/silvanusOntology#Temporal_entity -->

    <owl:Class rdf:about="http://www.semanticweb.org/smarotta/ontologies/2022/4/silvanusOntology#Temporal_entity">
        <rdfs:comment>It&apos;s the entity used to describe the temporal relationships between entities or other elements.</rdfs:comment>
        <rdfs:seeAlso>http://ecoinformatics.org/oboe/oboe.1.0/oboe-temporal.owl#TemporalEntity</rdfs:seeAlso>
    </owl:Class>
    


    <!-- http://www.semanticweb.org/smarotta/ontologies/2022/4/silvanusOntology#Terrestrial_Biome -->

    <owl:Class rdf:about="http://www.semanticweb.org/smarotta/ontologies/2022/4/silvanusOntology#Terrestrial_Biome">
        <rdfs:subClassOf rdf:resource="http://www.semanticweb.org/smarotta/ontologies/2022/4/silvanusOntology#Biome"/>
        <rdfs:comment>A biome which is primarily or completely situated on a landmass.</rdfs:comment>
        <rdfs:seeAlso>http://purl.obolibrary.org/obo/ENVO_00000446</rdfs:seeAlso>
    </owl:Class>
    


    <!-- http://www.semanticweb.org/smarotta/ontologies/2022/4/silvanusOntology#Text_analysis -->

    <owl:Class rdf:about="http://www.semanticweb.org/smarotta/ontologies/2022/4/silvanusOntology#Text_analysis">
        <rdfs:subClassOf rdf:resource="http://www.semanticweb.org/smarotta/ontologies/2022/4/silvanusOntology#Data_analysis"/>
        <rdfs:comment>Analysis of a text</rdfs:comment>
        <rdfs:seeAlso>https://raw.githubusercontent.com/beAWARE-project/ontology/master/beAWARE_ontology#TextAnalysis</rdfs:seeAlso>
    </owl:Class>
    


    <!-- http://www.semanticweb.org/smarotta/ontologies/2022/4/silvanusOntology#Text_item -->

    <owl:Class rdf:about="http://www.semanticweb.org/smarotta/ontologies/2022/4/silvanusOntology#Text_item">
        <rdfs:subClassOf rdf:resource="http://www.semanticweb.org/smarotta/ontologies/2022/4/silvanusOntology#Media_item"/>
        <rdfs:comment>Represents a text item</rdfs:comment>
        <rdfs:seeAlso>https://raw.githubusercontent.com/beAWARE-project/ontology/master/beAWARE_ontology#TextItem</rdfs:seeAlso>
    </owl:Class>
    


    <!-- http://www.semanticweb.org/smarotta/ontologies/2022/4/silvanusOntology#Thermometer -->

    <owl:Class rdf:about="http://www.semanticweb.org/smarotta/ontologies/2022/4/silvanusOntology#Thermometer">
        <rdfs:subClassOf rdf:resource="http://www.semanticweb.org/smarotta/ontologies/2022/4/silvanusOntology#IoT_sensor"/>
        <silvanusOntology:source>Most pilots</silvanusOntology:source>
        <rdfs:comment>An instrument for measuring and indicating temperature</rdfs:comment>
    </owl:Class>
    


    <!-- http://www.semanticweb.org/smarotta/ontologies/2022/4/silvanusOntology#Thickness_of_Dead_Layer -->

    <owl:Class rdf:about="http://www.semanticweb.org/smarotta/ontologies/2022/4/silvanusOntology#Thickness_of_Dead_Layer">
        <rdfs:subClassOf rdf:resource="http://www.semanticweb.org/smarotta/ontologies/2022/4/silvanusOntology#Biodiversity_index"/>
        <rdfs:comment>Thickness of Dead Layer</rdfs:comment>
        <rdfs:seeAlso>http://crossforest.eu/ifi/ontology/DeadLayer</rdfs:seeAlso>
    </owl:Class>
    


    <!-- http://www.semanticweb.org/smarotta/ontologies/2022/4/silvanusOntology#Tidal_Mangrove_Shrubland -->

    <owl:Class rdf:about="http://www.semanticweb.org/smarotta/ontologies/2022/4/silvanusOntology#Tidal_Mangrove_Shrubland">
        <rdfs:subClassOf rdf:resource="http://www.semanticweb.org/smarotta/ontologies/2022/4/silvanusOntology#Shrubland_Biome"/>
        <rdfs:comment>A shrubland biome which is densely vegetated by dwarf or short mangroves (and associates) that are generally less than 6 meters in height, is tidally influenced, is located in tropical or subtropical areas.</rdfs:comment>
        <rdfs:seeAlso>http://purl.obolibrary.org/obo/ENVO_01001369</rdfs:seeAlso>
    </owl:Class>
    


    <!-- http://www.semanticweb.org/smarotta/ontologies/2022/4/silvanusOntology#Time_since_last_precipitation -->

    <owl:Class rdf:about="http://www.semanticweb.org/smarotta/ontologies/2022/4/silvanusOntology#Time_since_last_precipitation">
        <rdfs:subClassOf rdf:resource="http://www.semanticweb.org/smarotta/ontologies/2022/4/silvanusOntology#Climate_parameter"/>
        <silvanusOntology:source>Croatian pilot</silvanusOntology:source>
        <rdfs:comment>Period without precipitations in a given area</rdfs:comment>
    </owl:Class>
    


    <!-- http://www.semanticweb.org/smarotta/ontologies/2022/4/silvanusOntology#Topography -->

    <owl:Class rdf:about="http://www.semanticweb.org/smarotta/ontologies/2022/4/silvanusOntology#Topography">
        <rdfs:subClassOf rdf:resource="http://www.semanticweb.org/smarotta/ontologies/2022/4/silvanusOntology#Biodiversity_index"/>
        <silvanusOntology:output>Topography layer available on map.</silvanusOntology:output>
        <silvanusOntology:source>Italian pilot</silvanusOntology:source>
        <silvanusOntology:source>Portuguese pilot</silvanusOntology:source>
        <rdfs:comment>Topography of the terrain, as it is important for the modelling of the fire spread behaviour, as well as for the coordination of firefighting crews.</rdfs:comment>
    </owl:Class>
    


    <!-- http://www.semanticweb.org/smarotta/ontologies/2022/4/silvanusOntology#Total_heat_release -->

    <owl:Class rdf:about="http://www.semanticweb.org/smarotta/ontologies/2022/4/silvanusOntology#Total_heat_release">
        <rdfs:subClassOf rdf:resource="http://www.semanticweb.org/smarotta/ontologies/2022/4/silvanusOntology#Fire_characteristic"/>
        <silvanusOntology:source>https://www.fs.fed.us/database/feis/glossary2.html</silvanusOntology:source>
        <rdfs:comment>The heat released by combustion during burnout of all fuels, expressed in BTU/foot2 or Kcal/meter2 [20].</rdfs:comment>
    </owl:Class>
    


    <!-- http://www.semanticweb.org/smarotta/ontologies/2022/4/silvanusOntology#Tourist_flow_sensor -->

    <owl:Class rdf:about="http://www.semanticweb.org/smarotta/ontologies/2022/4/silvanusOntology#Tourist_flow_sensor">
        <rdfs:subClassOf rdf:resource="http://www.semanticweb.org/smarotta/ontologies/2022/4/silvanusOntology#Sensor"/>
        <silvanusOntology:source>Romanian pilot</silvanusOntology:source>
        <rdfs:comment>A people counter is an electronic device that is used to measure the number of people traversing a certain passage or entrance. Examples include simple manual clickers, smart-flooring technologies, infrared beams, thermal imaging systems, WiFi trackers and video counters using advanced machine learning algorithms.</rdfs:comment>
    </owl:Class>
    


    <!-- http://www.semanticweb.org/smarotta/ontologies/2022/4/silvanusOntology#Touristic_route -->

    <owl:Class rdf:about="http://www.semanticweb.org/smarotta/ontologies/2022/4/silvanusOntology#Touristic_route">
        <rdfs:subClassOf rdf:resource="http://www.semanticweb.org/smarotta/ontologies/2022/4/silvanusOntology#Transportation"/>
        <silvanusOntology:source>Slovak pilot</silvanusOntology:source>
        <rdfs:comment>An established or selected course for travel consisting, typically, of secondary roads with significant scenic, cultural, historic, geological or natural features and including vistas, rest areas, and interpretive sites matching the scenic characteristics of the course.</rdfs:comment>
    </owl:Class>
    


    <!-- http://www.semanticweb.org/smarotta/ontologies/2022/4/silvanusOntology#Track -->

    <owl:Class rdf:about="http://www.semanticweb.org/smarotta/ontologies/2022/4/silvanusOntology#Track">
        <rdfs:subClassOf rdf:resource="http://www.semanticweb.org/smarotta/ontologies/2022/4/silvanusOntology#Street"/>
        <rdfs:comment>A small road, generally not paved.</rdfs:comment>
        <rdfs:seeAlso>http://purl.obolibrary.org/obo/ENVO_00000122</rdfs:seeAlso>
    </owl:Class>
    


    <!-- http://www.semanticweb.org/smarotta/ontologies/2022/4/silvanusOntology#Train -->

    <owl:Class rdf:about="http://www.semanticweb.org/smarotta/ontologies/2022/4/silvanusOntology#Train">
        <rdfs:subClassOf rdf:resource="http://www.semanticweb.org/smarotta/ontologies/2022/4/silvanusOntology#Rail_Transport_Vehicle"/>
        <rdfs:comment>A connected line of railroad cars with or without a locomotive</rdfs:comment>
        <rdfs:seeAlso>http://www.ontologylibrary.mil/CommonCore/Mid/ArtifactOntology#Train</rdfs:seeAlso>
    </owl:Class>
    


    <!-- http://www.semanticweb.org/smarotta/ontologies/2022/4/silvanusOntology#Transmission_pipeline -->

    <owl:Class rdf:about="http://www.semanticweb.org/smarotta/ontologies/2022/4/silvanusOntology#Transmission_pipeline">
        <rdfs:subClassOf rdf:resource="http://www.semanticweb.org/smarotta/ontologies/2022/4/silvanusOntology#Water_supply"/>
        <silvanusOntology:source>Portuguese pilot</silvanusOntology:source>
        <rdfs:comment>A human construction which is used to transport a material which is primarily composed of liquid or gas through a system of pipes.</rdfs:comment>
        <rdfs:seeAlso>http://purl.obolibrary.org/obo/ENVO_03600014</rdfs:seeAlso>
    </owl:Class>
    


    <!-- http://www.semanticweb.org/smarotta/ontologies/2022/4/silvanusOntology#Transmission_tower -->

    <owl:Class rdf:about="http://www.semanticweb.org/smarotta/ontologies/2022/4/silvanusOntology#Transmission_tower">
        <rdfs:subClassOf rdf:resource="http://www.semanticweb.org/smarotta/ontologies/2022/4/silvanusOntology#Energy"/>
        <silvanusOntology:source>Portuguese pilot</silvanusOntology:source>
        <rdfs:comment>A transmission tower is a tall structure, usually a steel lattice tower, used to support an overhead power line.</rdfs:comment>
    </owl:Class>
    


    <!-- http://www.semanticweb.org/smarotta/ontologies/2022/4/silvanusOntology#Transportation -->

    <owl:Class rdf:about="http://www.semanticweb.org/smarotta/ontologies/2022/4/silvanusOntology#Transportation">
        <rdfs:subClassOf rdf:resource="http://www.semanticweb.org/smarotta/ontologies/2022/4/silvanusOntology#Infrastructure"/>
        <rdfs:comment>Represents transportation services and infrastructure.</rdfs:comment>
        <rdfs:seeAlso>https://raw.githubusercontent.com/beAWARE-project/ontology/master/beAWARE_ontology#Transportation</rdfs:seeAlso>
    </owl:Class>
    


    <!-- http://www.semanticweb.org/smarotta/ontologies/2022/4/silvanusOntology#Transportation_Facility -->

    <owl:Class rdf:about="http://www.semanticweb.org/smarotta/ontologies/2022/4/silvanusOntology#Transportation_Facility">
        <rdfs:subClassOf rdf:resource="http://www.semanticweb.org/smarotta/ontologies/2022/4/silvanusOntology#Building"/>
        <rdfs:comment rdf:datatype="http://www.w3.org/2001/XMLSchema#string">A Facility that is designed for commencing or concluding the transportation of transportation artifacts, or for housing transportation artifacts.</rdfs:comment>
        <rdfs:seeAlso>http://www.ontologylibrary.mil/CommonCore/Mid/ArtifactOntology#TransportationFacility</rdfs:seeAlso>
    </owl:Class>
    


    <!-- http://www.semanticweb.org/smarotta/ontologies/2022/4/silvanusOntology#Tree_type -->

    <owl:Class rdf:about="http://www.semanticweb.org/smarotta/ontologies/2022/4/silvanusOntology#Tree_type">
        <rdfs:subClassOf rdf:resource="http://www.semanticweb.org/smarotta/ontologies/2022/4/silvanusOntology#Vegetation_type"/>
        <rdfs:comment>Type of tree</rdfs:comment>
    </owl:Class>
    


    <!-- http://www.semanticweb.org/smarotta/ontologies/2022/4/silvanusOntology#Tropical_Biome -->

    <owl:Class rdf:about="http://www.semanticweb.org/smarotta/ontologies/2022/4/silvanusOntology#Tropical_Biome">
        <rdfs:subClassOf rdf:resource="http://www.semanticweb.org/smarotta/ontologies/2022/4/silvanusOntology#Biome"/>
        <rdfs:comment>A biome which is subject to tropical climatic conditions.</rdfs:comment>
        <rdfs:seeAlso>http://purl.obolibrary.org/obo/ENVO_01001830</rdfs:seeAlso>
    </owl:Class>
    


    <!-- http://www.semanticweb.org/smarotta/ontologies/2022/4/silvanusOntology#Tropical_Marginal_Sea_Biome -->

    <owl:Class rdf:about="http://www.semanticweb.org/smarotta/ontologies/2022/4/silvanusOntology#Tropical_Marginal_Sea_Biome">
        <rdfs:subClassOf rdf:resource="http://www.semanticweb.org/smarotta/ontologies/2022/4/silvanusOntology#Tropical_Biome"/>
        <rdfs:comment>A marginal sea biome which is located in a region with a tropical climate.</rdfs:comment>
        <rdfs:seeAlso>http://purl.obolibrary.org/obo/ENVO_01001230</rdfs:seeAlso>
    </owl:Class>
    


    <!-- http://www.semanticweb.org/smarotta/ontologies/2022/4/silvanusOntology#Tropical_Marine_Coral_Reef_Biome -->

    <owl:Class rdf:about="http://www.semanticweb.org/smarotta/ontologies/2022/4/silvanusOntology#Tropical_Marine_Coral_Reef_Biome">
        <rdfs:subClassOf rdf:resource="http://www.semanticweb.org/smarotta/ontologies/2022/4/silvanusOntology#Tropical_Biome"/>
        <rdfs:comment>A marine coral reef biome which is located in a region with a tropical climate.</rdfs:comment>
        <rdfs:seeAlso>http://purl.obolibrary.org/obo/ENVO_01000854</rdfs:seeAlso>
    </owl:Class>
    


    <!-- http://www.semanticweb.org/smarotta/ontologies/2022/4/silvanusOntology#Tropical_Marine_Upwelling_Biome -->

    <owl:Class rdf:about="http://www.semanticweb.org/smarotta/ontologies/2022/4/silvanusOntology#Tropical_Marine_Upwelling_Biome">
        <rdfs:subClassOf rdf:resource="http://www.semanticweb.org/smarotta/ontologies/2022/4/silvanusOntology#Tropical_Biome"/>
        <rdfs:comment>A marine upwelling biome which is subject to tropical climate patterns.</rdfs:comment>
        <rdfs:seeAlso>http://purl.obolibrary.org/obo/ENVO_01000859</rdfs:seeAlso>
    </owl:Class>
    


    <!-- http://www.semanticweb.org/smarotta/ontologies/2022/4/silvanusOntology#Tropical_Savanna_Biome -->

    <owl:Class rdf:about="http://www.semanticweb.org/smarotta/ontologies/2022/4/silvanusOntology#Tropical_Savanna_Biome">
        <rdfs:subClassOf rdf:resource="http://www.semanticweb.org/smarotta/ontologies/2022/4/silvanusOntology#Tropical_Biome"/>
        <rdfs:comment>A savanna biome which is located in a region with a tropical climate.</rdfs:comment>
        <rdfs:seeAlso>http://purl.obolibrary.org/obo/ENVO_01000188</rdfs:seeAlso>
    </owl:Class>
    


    <!-- http://www.semanticweb.org/smarotta/ontologies/2022/4/silvanusOntology#Tropical_Shrubland_Biome -->

    <owl:Class rdf:about="http://www.semanticweb.org/smarotta/ontologies/2022/4/silvanusOntology#Tropical_Shrubland_Biome">
        <rdfs:subClassOf rdf:resource="http://www.semanticweb.org/smarotta/ontologies/2022/4/silvanusOntology#Shrubland_Biome"/>
        <rdfs:subClassOf rdf:resource="http://www.semanticweb.org/smarotta/ontologies/2022/4/silvanusOntology#Tropical_Biome"/>
        <rdfs:comment>A shrubland biome which is subject to tropical climate patterns.</rdfs:comment>
        <rdfs:seeAlso>http://purl.obolibrary.org/obo/ENVO_01000214</rdfs:seeAlso>
    </owl:Class>
    


    <!-- http://www.semanticweb.org/smarotta/ontologies/2022/4/silvanusOntology#Tropical_Woodland_Biome -->

    <owl:Class rdf:about="http://www.semanticweb.org/smarotta/ontologies/2022/4/silvanusOntology#Tropical_Woodland_Biome">
        <rdfs:subClassOf rdf:resource="http://www.semanticweb.org/smarotta/ontologies/2022/4/silvanusOntology#Tropical_Biome"/>
        <rdfs:comment>A woodland biome which is located in a region with a tropical climate.</rdfs:comment>
        <rdfs:seeAlso>http://purl.obolibrary.org/obo/ENVO_01000220</rdfs:seeAlso>
    </owl:Class>
    


    <!-- http://www.semanticweb.org/smarotta/ontologies/2022/4/silvanusOntology#Truck -->

    <owl:Class rdf:about="http://www.semanticweb.org/smarotta/ontologies/2022/4/silvanusOntology#Truck">
        <rdfs:subClassOf rdf:resource="http://www.semanticweb.org/smarotta/ontologies/2022/4/silvanusOntology#Ground_Motor_Vehicle"/>
        <rdfs:comment>A wheeled vehicle for moving heavy articles</rdfs:comment>
        <rdfs:seeAlso>http://www.ontologylibrary.mil/CommonCore/Mid/ArtifactOntology#Truck</rdfs:seeAlso>
    </owl:Class>
    


    <!-- http://www.semanticweb.org/smarotta/ontologies/2022/4/silvanusOntology#Tundra_Biome -->

    <owl:Class rdf:about="http://www.semanticweb.org/smarotta/ontologies/2022/4/silvanusOntology#Tundra_Biome">
        <rdfs:subClassOf rdf:resource="http://www.semanticweb.org/smarotta/ontologies/2022/4/silvanusOntology#Terrestrial_Biome"/>
        <rdfs:comment>A terrestrial biome which comprises a tundra ecosystem that has reached its climax community.</rdfs:comment>
        <rdfs:seeAlso>http://purl.obolibrary.org/obo/ENVO_01000180</rdfs:seeAlso>
    </owl:Class>
    


    <!-- http://www.semanticweb.org/smarotta/ontologies/2022/4/silvanusOntology#UAV -->

    <owl:Class rdf:about="http://www.semanticweb.org/smarotta/ontologies/2022/4/silvanusOntology#UAV">
        <rdfs:subClassOf rdf:resource="http://www.semanticweb.org/smarotta/ontologies/2022/4/silvanusOntology#IoT_sensor"/>
        <silvanusOntology:source>Most pilots</silvanusOntology:source>
        <rdfs:comment>An unmanned aerial vehicle (UAV), commonly known as a drone, is an aircraft without any human pilot, crew, or passengers on board.</rdfs:comment>
    </owl:Class>
    


    <!-- http://www.semanticweb.org/smarotta/ontologies/2022/4/silvanusOntology#UGV -->

    <owl:Class rdf:about="http://www.semanticweb.org/smarotta/ontologies/2022/4/silvanusOntology#UGV">
        <rdfs:subClassOf rdf:resource="http://www.semanticweb.org/smarotta/ontologies/2022/4/silvanusOntology#IoT_sensor"/>
        <silvanusOntology:source>Most pilots</silvanusOntology:source>
        <rdfs:comment>An unmanned ground vehicle (UGV) is a vehicle that operates while in contact with the ground and without an onboard human presence.</rdfs:comment>
    </owl:Class>
    


    <!-- http://www.semanticweb.org/smarotta/ontologies/2022/4/silvanusOntology#Uncontrolled_fire -->

    <owl:Class rdf:about="http://www.semanticweb.org/smarotta/ontologies/2022/4/silvanusOntology#Uncontrolled_fire">
        <rdfs:subClassOf rdf:resource="http://www.semanticweb.org/smarotta/ontologies/2022/4/silvanusOntology#Fire"/>
        <rdfs:comment>Fires that were not planned, but were started by arson, accident or lightning and burn out-of-control.</rdfs:comment>
        <rdfs:seeAlso>http://cerrado.linkeddata.es/ecology/fire#UncontrolledFire</rdfs:seeAlso>
    </owl:Class>
    


    <!-- http://www.semanticweb.org/smarotta/ontologies/2022/4/silvanusOntology#Unit -->

    <owl:Class rdf:about="http://www.semanticweb.org/smarotta/ontologies/2022/4/silvanusOntology#Unit">
        <rdfs:comment xml:lang="en">Unit in which a measure is taken</rdfs:comment>
        <rdfs:seeAlso>http://crossforest.eu/measures/ontology/Unit</rdfs:seeAlso>
        <rdfs:seeAlso>https://w3id.org/saref#UnitOfMeasure</rdfs:seeAlso>
    </owl:Class>
    


    <!-- http://www.semanticweb.org/smarotta/ontologies/2022/4/silvanusOntology#Unknown -->

    <owl:Class rdf:about="http://www.semanticweb.org/smarotta/ontologies/2022/4/silvanusOntology#Unknown">
        <rdfs:subClassOf rdf:resource="http://www.semanticweb.org/smarotta/ontologies/2022/4/silvanusOntology#Cause"/>
        <silvanusOntology:source>https://effis-gwis-cms.s3-eu-west-1.amazonaws.com/effis/reports-and-publications/effis-related-publications/lb-na-25-923-en-n.pdf (page 10)</silvanusOntology:source>
        <rdfs:comment>Wildfire with no cause found</rdfs:comment>
    </owl:Class>
    


    <!-- http://www.semanticweb.org/smarotta/ontologies/2022/4/silvanusOntology#UpperBound -->

    <owl:Class rdf:about="http://www.semanticweb.org/smarotta/ontologies/2022/4/silvanusOntology#UpperBound">
        <rdfs:subClassOf rdf:resource="http://www.semanticweb.org/smarotta/ontologies/2022/4/silvanusOntology#Spatial_entity"/>
        <rdfs:comment>Upper boundary of an area</rdfs:comment>
        <rdfs:seeAlso>http://crossforest.eu/position/ontology/UpperBound</rdfs:seeAlso>
    </owl:Class>
    


    <!-- http://www.semanticweb.org/smarotta/ontologies/2022/4/silvanusOntology#Use_of_fire -->

    <owl:Class rdf:about="http://www.semanticweb.org/smarotta/ontologies/2022/4/silvanusOntology#Use_of_fire">
        <rdfs:subClassOf rdf:resource="http://www.semanticweb.org/smarotta/ontologies/2022/4/silvanusOntology#Negligence"/>
        <owl:disjointWith rdf:resource="http://www.semanticweb.org/smarotta/ontologies/2022/4/silvanusOntology#Use_of_glowing_objects"/>
        <silvanusOntology:source>https://effis-gwis-cms.s3-eu-west-1.amazonaws.com/effis/reports-and-publications/effis-related-publications/lb-na-25-923-en-n.pdf (page 10)</silvanusOntology:source>
        <rdfs:comment>Wildfire unintentionally set by people making fire especially for cleaning or recreation. The difference between “deliberate” and this category is that the fire is initially voluntarily set for a specific purpose and not in order to destroy the natural area. To be classified in this category, the fire has to escape and get out of control.</rdfs:comment>
    </owl:Class>
    


    <!-- http://www.semanticweb.org/smarotta/ontologies/2022/4/silvanusOntology#Use_of_glowing_objects -->

    <owl:Class rdf:about="http://www.semanticweb.org/smarotta/ontologies/2022/4/silvanusOntology#Use_of_glowing_objects">
        <rdfs:subClassOf rdf:resource="http://www.semanticweb.org/smarotta/ontologies/2022/4/silvanusOntology#Negligence"/>
        <silvanusOntology:source>https://effis-gwis-cms.s3-eu-west-1.amazonaws.com/effis/reports-and-publications/effis-related-publications/lb-na-25-923-en-n.pdf (page 10)</silvanusOntology:source>
        <rdfs:comment>Wildfire unintentionally set by people using glowing objects such as (i) fireworks, (ii) cigarettes, (iii) hot ash handling by residents or (iv) during working activities such as apiculture, fumigation or disinfection or when expulsion of firebrands out of chimney.</rdfs:comment>
    </owl:Class>
    


    <!-- http://www.semanticweb.org/smarotta/ontologies/2022/4/silvanusOntology#Vandalism -->

    <owl:Class rdf:about="http://www.semanticweb.org/smarotta/ontologies/2022/4/silvanusOntology#Vandalism">
        <rdfs:subClassOf rdf:resource="http://www.semanticweb.org/smarotta/ontologies/2022/4/silvanusOntology#Responsible"/>
        <silvanusOntology:source>https://effis-gwis-cms.s3-eu-west-1.amazonaws.com/effis/reports-and-publications/effis-related-publications/lb-na-25-923-en-n.pdf (page 10)</silvanusOntology:source>
        <rdfs:comment>Malicious or mischievous fire setting that results in damage to property: wilful and malicious mischief or peer group pressure</rdfs:comment>
    </owl:Class>
    


    <!-- http://www.semanticweb.org/smarotta/ontologies/2022/4/silvanusOntology#Vegetated_area -->

    <owl:Class rdf:about="http://www.semanticweb.org/smarotta/ontologies/2022/4/silvanusOntology#Vegetated_area">
        <rdfs:subClassOf rdf:resource="http://www.semanticweb.org/smarotta/ontologies/2022/4/silvanusOntology#Biodiversity_index"/>
        <rdfs:comment>A vegetated area is a geographic feature which has ground cover dominated by plant communities.</rdfs:comment>
        <rdfs:seeAlso>http://purl.obolibrary.org/obo/ENVO_01001305</rdfs:seeAlso>
    </owl:Class>
    


    <!-- http://www.semanticweb.org/smarotta/ontologies/2022/4/silvanusOntology#Vegetation_growth -->

    <owl:Class rdf:about="http://www.semanticweb.org/smarotta/ontologies/2022/4/silvanusOntology#Vegetation_growth">
        <rdfs:subClassOf rdf:resource="http://www.semanticweb.org/smarotta/ontologies/2022/4/silvanusOntology#Biodiversity_index"/>
        <silvanusOntology:input>Earth Observations, UAV/optical sensing, LIDAR sensing, Weather, Soil data, Soil water content, in-situ sensors (cameras)</silvanusOntology:input>
        <silvanusOntology:output>Date prediction of when the clearing will be necessary.</silvanusOntology:output>
        <silvanusOntology:source>Portuguese pilot</silvanusOntology:source>
        <rdfs:comment>Estimation in the temporal dimension of when the vegetation or biomass, will reach a predetermined size or density, through the development of a vegetation growth rate. This will optimize the clearing interventions.</rdfs:comment>
    </owl:Class>
    


    <!-- http://www.semanticweb.org/smarotta/ontologies/2022/4/silvanusOntology#Vegetation_index -->

    <owl:Class rdf:about="http://www.semanticweb.org/smarotta/ontologies/2022/4/silvanusOntology#Vegetation_index">
        <rdfs:subClassOf rdf:resource="http://www.semanticweb.org/smarotta/ontologies/2022/4/silvanusOntology#Biodiversity_index"/>
        <silvanusOntology:source>Portugues pilot</silvanusOntology:source>
    </owl:Class>
    


    <!-- http://www.semanticweb.org/smarotta/ontologies/2022/4/silvanusOntology#Vegetation_management -->

    <owl:Class rdf:about="http://www.semanticweb.org/smarotta/ontologies/2022/4/silvanusOntology#Vegetation_management">
        <rdfs:subClassOf rdf:resource="http://www.semanticweb.org/smarotta/ontologies/2022/4/silvanusOntology#Use_of_fire"/>
        <silvanusOntology:source>https://effis-gwis-cms.s3-eu-west-1.amazonaws.com/effis/reports-and-publications/effis-related-publications/lb-na-25-923-en-n.pdf (page 10)</silvanusOntology:source>
        <rdfs:comment>Wildfire caused by any kind of vegetation burnings for private, forestry, pastoral (pasture regeneration) purposes including prescribed burnings, burning of slashes or of piles of vegetal waste but except for agricultural purposes.</rdfs:comment>
    </owl:Class>
    


    <!-- http://www.semanticweb.org/smarotta/ontologies/2022/4/silvanusOntology#Vegetation_quantity -->

    <owl:Class rdf:about="http://www.semanticweb.org/smarotta/ontologies/2022/4/silvanusOntology#Vegetation_quantity">
        <rdfs:subClassOf rdf:resource="http://www.semanticweb.org/smarotta/ontologies/2022/4/silvanusOntology#Biodiversity_index"/>
        <silvanusOntology:source>Croatian pilot</silvanusOntology:source>
        <rdfs:comment>Quantity of vegetation</rdfs:comment>
    </owl:Class>
    


    <!-- http://www.semanticweb.org/smarotta/ontologies/2022/4/silvanusOntology#Vegetation_stat -->

    <owl:Class rdf:about="http://www.semanticweb.org/smarotta/ontologies/2022/4/silvanusOntology#Vegetation_stat">
        <silvanusOntology:source>Indonesian pilot</silvanusOntology:source>
        <rdfs:comment>Statistics related to vegetation</rdfs:comment>
    </owl:Class>
    


    <!-- http://www.semanticweb.org/smarotta/ontologies/2022/4/silvanusOntology#Vegetation_type -->

    <owl:Class rdf:about="http://www.semanticweb.org/smarotta/ontologies/2022/4/silvanusOntology#Vegetation_type">
        <rdfs:subClassOf rdf:resource="http://www.semanticweb.org/smarotta/ontologies/2022/4/silvanusOntology#Biodiversity_index"/>
        <silvanusOntology:source>Croatian pilot</silvanusOntology:source>
        <rdfs:comment>Type of vegetation</rdfs:comment>
    </owl:Class>
    


    <!-- http://www.semanticweb.org/smarotta/ontologies/2022/4/silvanusOntology#Vegetation_vertical_structure -->

    <owl:Class rdf:about="http://www.semanticweb.org/smarotta/ontologies/2022/4/silvanusOntology#Vegetation_vertical_structure">
        <rdfs:subClassOf rdf:resource="http://www.semanticweb.org/smarotta/ontologies/2022/4/silvanusOntology#Biodiversity_index"/>
        <silvanusOntology:input>Earth Observations, UAV sensing, LIDAR</silvanusOntology:input>
        <silvanusOntology:output>Maps with indicators of understory biomass (e.g., understory biomass volume per unit area)</silvanusOntology:output>
        <silvanusOntology:source>Portugues pilot</silvanusOntology:source>
        <rdfs:comment>Forest understory growth can greatly contribute to the spread and to severe canopy forest fires. Vegetation management may be required, including the use of livestock grazing coupled (or not) with mechanized interventions. Identification of areas with dense and continuous undergrowth is needed to guide management and plan interventions.</rdfs:comment>
    </owl:Class>
    


    <!-- http://www.semanticweb.org/smarotta/ontologies/2022/4/silvanusOntology#Vehicle -->

    <owl:Class rdf:about="http://www.semanticweb.org/smarotta/ontologies/2022/4/silvanusOntology#Vehicle">
        <rdfs:subClassOf rdf:resource="http://www.semanticweb.org/smarotta/ontologies/2022/4/silvanusOntology#Property"/>
        <rdfs:comment>Represents any type of vehicle.</rdfs:comment>
        <rdfs:seeAlso>https://raw.githubusercontent.com/beAWARE-project/ontology/master/beAWARE_ontology#Vehicle</rdfs:seeAlso>
    </owl:Class>
    


    <!-- http://www.semanticweb.org/smarotta/ontologies/2022/4/silvanusOntology#Vehicles -->

    <owl:Class rdf:about="http://www.semanticweb.org/smarotta/ontologies/2022/4/silvanusOntology#Vehicles">
        <rdfs:subClassOf rdf:resource="http://www.semanticweb.org/smarotta/ontologies/2022/4/silvanusOntology#Accident"/>
        <silvanusOntology:source>https://effis-gwis-cms.s3-eu-west-1.amazonaws.com/effis/reports-and-publications/effis-related-publications/lb-na-25-923-en-n.pdf (page 10)</silvanusOntology:source>
        <rdfs:comment>Wildfire caused by exhausts (expulsion of glowing carbon deposits, hot catalytic converter) and brakes of vehicles travelling along the road, or by road incidents (Burning motor for example) or traffic accidents</rdfs:comment>
    </owl:Class>
    


    <!-- http://www.semanticweb.org/smarotta/ontologies/2022/4/silvanusOntology#Video_analysis -->

    <owl:Class rdf:about="http://www.semanticweb.org/smarotta/ontologies/2022/4/silvanusOntology#Video_analysis">
        <rdfs:subClassOf rdf:resource="http://www.semanticweb.org/smarotta/ontologies/2022/4/silvanusOntology#Data_analysis"/>
        <rdfs:comment>Analysis of a video</rdfs:comment>
        <rdfs:seeAlso>https://raw.githubusercontent.com/beAWARE-project/ontology/master/beAWARE_ontology#VideoAnalysis</rdfs:seeAlso>
    </owl:Class>
    


    <!-- http://www.semanticweb.org/smarotta/ontologies/2022/4/silvanusOntology#Video_item -->

    <owl:Class rdf:about="http://www.semanticweb.org/smarotta/ontologies/2022/4/silvanusOntology#Video_item">
        <rdfs:subClassOf rdf:resource="http://www.semanticweb.org/smarotta/ontologies/2022/4/silvanusOntology#Media_item"/>
        <rdfs:comment>Represents a video item</rdfs:comment>
        <rdfs:seeAlso>https://raw.githubusercontent.com/beAWARE-project/ontology/master/beAWARE_ontology#VideoItem</rdfs:seeAlso>
    </owl:Class>
    


    <!-- http://www.semanticweb.org/smarotta/ontologies/2022/4/silvanusOntology#Village_Biome -->

    <owl:Class rdf:about="http://www.semanticweb.org/smarotta/ontologies/2022/4/silvanusOntology#Village_Biome">
        <rdfs:subClassOf rdf:resource="http://www.semanticweb.org/smarotta/ontologies/2022/4/silvanusOntology#Anthropogenic_Terrestrial_Biome"/>
        <rdfs:comment>A village biome is an anthropogenic terrestrial biome which contains settlements such as villages, towns, and/or small cities and which is primarily used for agricultural activity.</rdfs:comment>
        <rdfs:seeAlso>http://purl.obolibrary.org/obo/ENVO_01000246</rdfs:seeAlso>
    </owl:Class>
    


    <!-- http://www.semanticweb.org/smarotta/ontologies/2022/4/silvanusOntology#Volcanism -->

    <owl:Class rdf:about="http://www.semanticweb.org/smarotta/ontologies/2022/4/silvanusOntology#Volcanism">
        <rdfs:subClassOf rdf:resource="http://www.semanticweb.org/smarotta/ontologies/2022/4/silvanusOntology#Natural"/>
        <silvanusOntology:source>https://effis-gwis-cms.s3-eu-west-1.amazonaws.com/effis/reports-and-publications/effis-related-publications/lb-na-25-923-en-n.pdf (page 10)</silvanusOntology:source>
        <rdfs:comment>Wildfire caused by volcanism.</rdfs:comment>
    </owl:Class>
    


    <!-- http://www.semanticweb.org/smarotta/ontologies/2022/4/silvanusOntology#Volume_with_bark -->

    <owl:Class rdf:about="http://www.semanticweb.org/smarotta/ontologies/2022/4/silvanusOntology#Volume_with_bark">
        <rdfs:subClassOf rdf:resource="http://www.semanticweb.org/smarotta/ontologies/2022/4/silvanusOntology#Measure"/>
        <rdfs:comment>Volume of the tree including the bark</rdfs:comment>
        <rdfs:seeAlso>http://crossforest.eu/ifi/ontology/VolumeWithBark</rdfs:seeAlso>
    </owl:Class>
    


    <!-- http://www.semanticweb.org/smarotta/ontologies/2022/4/silvanusOntology#Volunteer_unit -->

    <owl:Class rdf:about="http://www.semanticweb.org/smarotta/ontologies/2022/4/silvanusOntology#Volunteer_unit">
        <rdfs:subClassOf rdf:resource="http://www.semanticweb.org/smarotta/ontologies/2022/4/silvanusOntology#Firefighting_unit"/>
        <silvanusOntology:source>Czech pilot</silvanusOntology:source>
        <rdfs:comment>Volunteer  firefighter</rdfs:comment>
        <rdfs:seeAlso>http://www.semanticweb.org/earthquake#Volunteer</rdfs:seeAlso>
    </owl:Class>
    


    <!-- http://www.semanticweb.org/smarotta/ontologies/2022/4/silvanusOntology#Vulnerable_object -->

    <owl:Class rdf:about="http://www.semanticweb.org/smarotta/ontologies/2022/4/silvanusOntology#Vulnerable_object">
        <rdfs:comment>Any living being or object that needs to be protected from hazards.</rdfs:comment>
        <rdfs:seeAlso>http://www.semanticweb.org/earthquake#Loss</rdfs:seeAlso>
        <rdfs:seeAlso>https://raw.githubusercontent.com/beAWARE-project/ontology/master/beAWARE_ontology#VulnerableObject</rdfs:seeAlso>
    </owl:Class>
    


    <!-- http://www.semanticweb.org/smarotta/ontologies/2022/4/silvanusOntology#Wall -->

    <owl:Class rdf:about="http://www.semanticweb.org/smarotta/ontologies/2022/4/silvanusOntology#Wall">
        <rdfs:subClassOf rdf:resource="http://www.semanticweb.org/smarotta/ontologies/2022/4/silvanusOntology#Structure"/>
        <rdfs:comment>A vertical structure often made of stone or brick that divides or surrounds something.</rdfs:comment>
        <rdfs:seeAlso>https://raw.githubusercontent.com/beAWARE-project/ontology/master/beAWARE_ontology#Wall</rdfs:seeAlso>
    </owl:Class>
    


    <!-- http://www.semanticweb.org/smarotta/ontologies/2022/4/silvanusOntology#Waste_management -->

    <owl:Class rdf:about="http://www.semanticweb.org/smarotta/ontologies/2022/4/silvanusOntology#Waste_management">
        <rdfs:subClassOf rdf:resource="http://www.semanticweb.org/smarotta/ontologies/2022/4/silvanusOntology#Use_of_fire"/>
        <silvanusOntology:source>https://effis-gwis-cms.s3-eu-west-1.amazonaws.com/effis/reports-and-publications/effis-related-publications/lb-na-25-923-en-n.pdf (page 10)</silvanusOntology:source>
        <rdfs:comment>Wildfire caused by garbage burnings in official or illegal dumps (dunghill) including</rdfs:comment>
    </owl:Class>
    


    <!-- http://www.semanticweb.org/smarotta/ontologies/2022/4/silvanusOntology#Waste_treatment_plant -->

    <owl:Class rdf:about="http://www.semanticweb.org/smarotta/ontologies/2022/4/silvanusOntology#Waste_treatment_plant">
        <rdfs:subClassOf rdf:resource="http://www.semanticweb.org/smarotta/ontologies/2022/4/silvanusOntology#Industrial_building"/>
        <rdfs:comment>Building for waste treatment</rdfs:comment>
        <rdfs:seeAlso>http://purl.obolibrary.org/obo/ENVO_00002272</rdfs:seeAlso>
    </owl:Class>
    


    <!-- http://www.semanticweb.org/smarotta/ontologies/2022/4/silvanusOntology#WaterFacility -->

    <owl:Class rdf:about="http://www.semanticweb.org/smarotta/ontologies/2022/4/silvanusOntology#WaterFacility">
        <rdfs:subClassOf rdf:resource="http://www.semanticweb.org/smarotta/ontologies/2022/4/silvanusOntology#Building"/>
        <rdfs:comment>Any plants, structures and other real and personal property acquired, rehabilitated or constructed or planned for the purpose of accumulating, supplying, transmitting, treating or distributing water, including but not limited to surface or groundwater reservoirs, basins, dams, canals, aqueducts, aqueduct taps, standpipes, conduits, pipelines, mains, pumping stations, pumps, water distribution systems, compensating reservoirs, intake stations, waterworks or sources of water supply, wells and purification.</rdfs:comment>
        <rdfs:seeAlso>http://www.semanticweb.org/earthquake#WaterFacility</rdfs:seeAlso>
        <rdfs:seeAlso>https://w3id.org/empathi/Water</rdfs:seeAlso>
    </owl:Class>
    


    <!-- http://www.semanticweb.org/smarotta/ontologies/2022/4/silvanusOntology#Water_infrastructures_criticality -->

    <owl:Class rdf:about="http://www.semanticweb.org/smarotta/ontologies/2022/4/silvanusOntology#Water_infrastructures_criticality">
        <rdfs:subClassOf rdf:resource="http://www.semanticweb.org/smarotta/ontologies/2022/4/silvanusOntology#Infrastructure"/>
        <silvanusOntology:output>Water  Infrastructures Criticallity  displayed on map</silvanusOntology:output>
        <silvanusOntology:source>Portuguese pilot</silvanusOntology:source>
        <rdfs:comment>Criticallity, based on the design flow and system´s redundancy characteristics</rdfs:comment>
    </owl:Class>
    


    <!-- http://www.semanticweb.org/smarotta/ontologies/2022/4/silvanusOntology#Water_source -->

    <owl:Class rdf:about="http://www.semanticweb.org/smarotta/ontologies/2022/4/silvanusOntology#Water_source">
        <rdfs:subClassOf rdf:resource="http://www.semanticweb.org/smarotta/ontologies/2022/4/silvanusOntology#Response_resource"/>
        <silvanusOntology:source>Portuguese pilot</silvanusOntology:source>
        <rdfs:comment>Refers to bodies of water (such as rivers, streams, lakes, reservoirs, springs, and ground water) that provide water to public drinking-water supplies and private wells. Water sources can include: Surface water (for example, a lake, river, or reservoir) Ground water (for example, an aquifer</rdfs:comment>
    </owl:Class>
    


    <!-- http://www.semanticweb.org/smarotta/ontologies/2022/4/silvanusOntology#Water_supply -->

    <owl:Class rdf:about="http://www.semanticweb.org/smarotta/ontologies/2022/4/silvanusOntology#Water_supply">
        <rdfs:subClassOf rdf:resource="http://www.semanticweb.org/smarotta/ontologies/2022/4/silvanusOntology#Infrastructure"/>
        <rdfs:comment>Water  Infrastructures typology  displayed on map</rdfs:comment>
        <rdfs:seeAlso>http://www.semanticweb.org/earthquake#WaterSupply</rdfs:seeAlso>
        <rdfs:seeAlso>https://raw.githubusercontent.com/beAWARE-project/ontology/master/beAWARE_ontology#WaterSupply</rdfs:seeAlso>
    </owl:Class>
    


    <!-- http://www.semanticweb.org/smarotta/ontologies/2022/4/silvanusOntology#Watercraft -->

    <owl:Class rdf:about="http://www.semanticweb.org/smarotta/ontologies/2022/4/silvanusOntology#Watercraft">
        <rdfs:subClassOf rdf:resource="http://www.semanticweb.org/smarotta/ontologies/2022/4/silvanusOntology#Response_vehicle"/>
        <rdfs:comment>Craft for water transport</rdfs:comment>
        <rdfs:seeAlso>http://www.ontologylibrary.mil/CommonCore/Mid/ArtifactOntology#Watercraft</rdfs:seeAlso>
    </owl:Class>
    


    <!-- http://www.semanticweb.org/smarotta/ontologies/2022/4/silvanusOntology#Weapons -->

    <owl:Class rdf:about="http://www.semanticweb.org/smarotta/ontologies/2022/4/silvanusOntology#Weapons">
        <rdfs:subClassOf rdf:resource="http://www.semanticweb.org/smarotta/ontologies/2022/4/silvanusOntology#Accident"/>
        <silvanusOntology:source>https://effis-gwis-cms.s3-eu-west-1.amazonaws.com/effis/reports-and-publications/effis-related-publications/lb-na-25-923-en-n.pdf (page 10)</silvanusOntology:source>
        <rdfs:comment>Wildfire caused either by military exercises (firing, explosions) or by citizens using firearms (in hunting activities for instance) or explosion due to explosives during works. This class takes also into account the fires set after explosions due to ammunitions from I and II World Wars buried underground.</rdfs:comment>
    </owl:Class>
    


    <!-- http://www.semanticweb.org/smarotta/ontologies/2022/4/silvanusOntology#Weather_station -->

    <owl:Class rdf:about="http://www.semanticweb.org/smarotta/ontologies/2022/4/silvanusOntology#Weather_station">
        <rdfs:subClassOf rdf:resource="http://www.semanticweb.org/smarotta/ontologies/2022/4/silvanusOntology#Sensor"/>
        <rdfs:comment>A weather station is a facility, either on land or sea, with instruments and equipment for measuring atmospheric conditions to provide information for weather forecasts and to study the weather and climate. The measurements taken include temperature, atmospheric pressure, humidity, wind speed, wind direction, and precipitation amounts.</rdfs:comment>
    </owl:Class>
    


    <!-- http://www.semanticweb.org/smarotta/ontologies/2022/4/silvanusOntology#Wetland_Area -->

    <owl:Class rdf:about="http://www.semanticweb.org/smarotta/ontologies/2022/4/silvanusOntology#Wetland_Area">
        <rdfs:subClassOf rdf:resource="http://www.semanticweb.org/smarotta/ontologies/2022/4/silvanusOntology#Vegetated_area"/>
        <rdfs:comment>A vegetated area which overlaps a wetland ecosystem.</rdfs:comment>
        <rdfs:seeAlso>http://purl.obolibrary.org/obo/ENVO_00000043</rdfs:seeAlso>
    </owl:Class>
    


    <!-- http://www.semanticweb.org/smarotta/ontologies/2022/4/silvanusOntology#Wildfire -->

    <owl:Class rdf:about="http://www.semanticweb.org/smarotta/ontologies/2022/4/silvanusOntology#Wildfire">
        <rdfs:subClassOf rdf:resource="http://www.semanticweb.org/smarotta/ontologies/2022/4/silvanusOntology#Uncontrolled_fire"/>
        <rdfs:comment>A fire burning in wildland fuel.</rdfs:comment>
        <rdfs:seeAlso>http://cerrado.linkeddata.es/ecology/fire#Wildfire</rdfs:seeAlso>
        <rdfs:seeAlso>http://www.semanticweb.org/earthquake#WildFire</rdfs:seeAlso>
    </owl:Class>
    


    <!-- http://www.semanticweb.org/smarotta/ontologies/2022/4/silvanusOntology#Wind_condition -->

    <owl:Class rdf:about="http://www.semanticweb.org/smarotta/ontologies/2022/4/silvanusOntology#Wind_condition">
        <rdfs:subClassOf rdf:resource="http://www.semanticweb.org/smarotta/ontologies/2022/4/silvanusOntology#Climate_parameter"/>
        <silvanusOntology:source>https://cwfis.cfs.nrcan.gc.ca/background/summary/fwi</silvanusOntology:source>
        <rdfs:comment>The perceptible natural movement of the air, especially in the form of a current of air blowing from a particular direction.</rdfs:comment>
        <rdfs:seeAlso>https://bimerr.iot.linkeddata.es/def/weather#Wind</rdfs:seeAlso>
    </owl:Class>
    


    <!-- http://www.semanticweb.org/smarotta/ontologies/2022/4/silvanusOntology#Wind_direction -->

    <owl:Class rdf:about="http://www.semanticweb.org/smarotta/ontologies/2022/4/silvanusOntology#Wind_direction">
        <rdfs:subClassOf rdf:resource="http://www.semanticweb.org/smarotta/ontologies/2022/4/silvanusOntology#Wind_condition"/>
        <silvanusOntology:source>https://cwfis.cfs.nrcan.gc.ca/background/summary/fwi</silvanusOntology:source>
        <rdfs:comment>Wind direction</rdfs:comment>
    </owl:Class>
    


    <!-- http://www.semanticweb.org/smarotta/ontologies/2022/4/silvanusOntology#Wind_speed -->

    <owl:Class rdf:about="http://www.semanticweb.org/smarotta/ontologies/2022/4/silvanusOntology#Wind_speed">
        <rdfs:subClassOf rdf:resource="http://www.semanticweb.org/smarotta/ontologies/2022/4/silvanusOntology#Wind_condition"/>
        <silvanusOntology:source>https://cwfis.cfs.nrcan.gc.ca/background/summary/fwi</silvanusOntology:source>
        <rdfs:comment>Wind speed</rdfs:comment>
    </owl:Class>
    


    <!-- http://www.semanticweb.org/smarotta/ontologies/2022/4/silvanusOntology#Wooded_shrubland -->

    <owl:Class rdf:about="http://www.semanticweb.org/smarotta/ontologies/2022/4/silvanusOntology#Wooded_shrubland">
        <rdfs:subClassOf rdf:resource="http://www.semanticweb.org/smarotta/ontologies/2022/4/silvanusOntology#Biodiversity_index"/>
        <silvanusOntology:source>https://www.fs.fed.us/database/feis/glossary2.html#WoodedShrubland</silvanusOntology:source>
        <rdfs:comment>A formation dominated by woody species, in which the proportion of shrubs is generally greater than the proportion of trees [112]. Grass and bare ground are usually present but not required for defining this formation. Compare with grassland, shrubland, wooded shrubland, savanna, forest.</rdfs:comment>
    </owl:Class>
    


    <!-- http://www.semanticweb.org/smarotta/ontologies/2022/4/silvanusOntology#Woodland -->

    <owl:Class rdf:about="http://www.semanticweb.org/smarotta/ontologies/2022/4/silvanusOntology#Woodland">
        <rdfs:subClassOf rdf:resource="http://www.semanticweb.org/smarotta/ontologies/2022/4/silvanusOntology#Biodiversity_index"/>
        <silvanusOntology:source>https://www.fs.fed.us/database/feis/glossary2.html#woodland</silvanusOntology:source>
        <rdfs:comment>A formation in which tree cover is greater than shrub cover, but the canopy is not closed [112]. Generally, overstory trees are &gt;16 feet (5 m) tall and have 25% to 60% cover [75]. When describing woodlands, use of a dash indicates an overstory/understory relationship (e.g., bur oak/big bluestem woodland). Compare with grassland, shrubland, wooded shrubland, savanna, forest.</rdfs:comment>
    </owl:Class>
    


    <!-- http://www.semanticweb.org/smarotta/ontologies/2022/4/silvanusOntology#Woodland_Area -->

    <owl:Class rdf:about="http://www.semanticweb.org/smarotta/ontologies/2022/4/silvanusOntology#Woodland_Area">
        <rdfs:subClassOf rdf:resource="http://www.semanticweb.org/smarotta/ontologies/2022/4/silvanusOntology#Vegetated_area"/>
        <rdfs:comment>Land having a cover of trees, shrubs, or both.</rdfs:comment>
        <rdfs:seeAlso>http://purl.obolibrary.org/obo/ENVO_00000109</rdfs:seeAlso>
    </owl:Class>
    


    <!-- http://www.semanticweb.org/smarotta/ontologies/2022/4/silvanusOntology#Woodland_Biome -->

    <owl:Class rdf:about="http://www.semanticweb.org/smarotta/ontologies/2022/4/silvanusOntology#Woodland_Biome">
        <rdfs:subClassOf rdf:resource="http://www.semanticweb.org/smarotta/ontologies/2022/4/silvanusOntology#Terrestrial_Biome"/>
        <rdfs:comment>A woodland biome is a terrestrial biome which includes, across its entire spatial extent, woody plants spaced sufficiently far apart to allow light penetration to support communities of herbaceous plants or shrubs living closer to the woodland floor.</rdfs:comment>
        <rdfs:seeAlso>http://purl.obolibrary.org/obo/ENVO_01000175</rdfs:seeAlso>
    </owl:Class>
    


    <!-- http://www.semanticweb.org/smarotta/ontologies/2022/4/silvanusOntology#Works -->

    <owl:Class rdf:about="http://www.semanticweb.org/smarotta/ontologies/2022/4/silvanusOntology#Works">
        <rdfs:subClassOf rdf:resource="http://www.semanticweb.org/smarotta/ontologies/2022/4/silvanusOntology#Accident"/>
        <silvanusOntology:source>https://effis-gwis-cms.s3-eu-west-1.amazonaws.com/effis/reports-and-publications/effis-related-publications/lb-na-25-923-en-n.pdf (page 10)</silvanusOntology:source>
        <rdfs:comment>Wildfire caused by sparks emitted by engines and machinery (such as chainsaw) in industry, forestry and agriculture or people at work (explosions, welding, grinding, smoldering) or by ignition of flammables and vapors during works in industrial activities.</rdfs:comment>
    </owl:Class>
    


    <!-- http://www.semanticweb.org/smarotta/ontologies/2022/4/silvanusOntology#Xeric_Shrubland_Biome -->

    <owl:Class rdf:about="http://www.semanticweb.org/smarotta/ontologies/2022/4/silvanusOntology#Xeric_Shrubland_Biome">
        <rdfs:subClassOf rdf:resource="http://www.semanticweb.org/smarotta/ontologies/2022/4/silvanusOntology#Shrubland_Biome"/>
        <rdfs:comment>A shrubland biome which is subject to xeric climate patterns.</rdfs:comment>
        <rdfs:seeAlso>http://purl.obolibrary.org/obo/ENVO_01000218</rdfs:seeAlso>
    </owl:Class>
    


    <!-- http://www.semanticweb.org/smarotta/ontologies/2022/4/silvanusOntology#Years -->

    <owl:Class rdf:about="http://www.semanticweb.org/smarotta/ontologies/2022/4/silvanusOntology#Years"/>
    


    <!-- http://www.semanticweb.org/smarotta/ontologies/2022/4/silvanusOntology#food_processing_building -->

    <owl:Class rdf:about="http://www.semanticweb.org/smarotta/ontologies/2022/4/silvanusOntology#food_processing_building">
        <rdfs:subClassOf rdf:resource="http://www.semanticweb.org/smarotta/ontologies/2022/4/silvanusOntology#Industrial_building"/>
        <rdfs:comment>A food processing building is a building in which materials that contain or consist of essential body nutrients - such as carbohydrates, fats, proteins, vitamins, or minerals - and may be ingested and assimilated by an organism to produce energy, stimulate growth, and maintain life are converted alternative forms.</rdfs:comment>
        <rdfs:seeAlso>http://purl.obolibrary.org/obo/ENVO_00003863</rdfs:seeAlso>
    </owl:Class>
    


    <!-- http://www.semanticweb.org/smarotta/ontologies/2022/4/silvanusOntology#ford -->

    <owl:Class rdf:about="http://www.semanticweb.org/smarotta/ontologies/2022/4/silvanusOntology#ford">
        <rdfs:subClassOf rdf:resource="http://www.semanticweb.org/smarotta/ontologies/2022/4/silvanusOntology#Transportation"/>
        <rdfs:comment>The shallow part of a stream which can be easily crossed.</rdfs:comment>
        <rdfs:seeAlso>http://purl.obolibrary.org/obo/ENVO_00000411</rdfs:seeAlso>
    </owl:Class>
    


    <!-- http://www.semanticweb.org/smarotta/ontologies/2022/4/silvanusOntology#lock -->

    <owl:Class rdf:about="http://www.semanticweb.org/smarotta/ontologies/2022/4/silvanusOntology#lock">
        <rdfs:subClassOf rdf:resource="http://www.semanticweb.org/smarotta/ontologies/2022/4/silvanusOntology#Transportation"/>
        <rdfs:comment>A device for raising and lowering boats between stretches of water of different levels on river and canal waterways.</rdfs:comment>
        <rdfs:seeAlso>http://purl.obolibrary.org/obo/ENVO_00000357</rdfs:seeAlso>
    </owl:Class>
    


    <!-- http://www.semanticweb.org/smarotta/ontologies/2022/4/silvanusOntology#pier -->

    <owl:Class rdf:about="http://www.semanticweb.org/smarotta/ontologies/2022/4/silvanusOntology#pier">
        <rdfs:subClassOf rdf:resource="http://www.semanticweb.org/smarotta/ontologies/2022/4/silvanusOntology#Transportation"/>
        <rdfs:comment>A raised walkway over water, supported by piles or pillars.</rdfs:comment>
        <rdfs:seeAlso>http://purl.obolibrary.org/obo/ENVO_00000563</rdfs:seeAlso>
    </owl:Class>
    


    <!-- http://www.semanticweb.org/smarotta/ontologies/2022/4/silvanusOntology#railway -->

    <owl:Class rdf:about="http://www.semanticweb.org/smarotta/ontologies/2022/4/silvanusOntology#railway">
        <rdfs:subClassOf rdf:resource="http://www.semanticweb.org/smarotta/ontologies/2022/4/silvanusOntology#Transportation"/>
        <rdfs:comment>A permanent way having one or more rails which provides a track for cars.</rdfs:comment>
        <rdfs:seeAlso>http://purl.obolibrary.org/obo/ENVO_00000065</rdfs:seeAlso>
    </owl:Class>
    


    <!-- http://www.semanticweb.org/smarotta/ontologies/2022/4/silvanusOntology#university_campus -->

    <owl:Class rdf:about="http://www.semanticweb.org/smarotta/ontologies/2022/4/silvanusOntology#university_campus">
        <rdfs:subClassOf rdf:resource="http://www.semanticweb.org/smarotta/ontologies/2022/4/silvanusOntology#Building"/>
        <rdfs:comment>An area of land on which a college or university and related institutional buildings are situated.</rdfs:comment>
        <rdfs:seeAlso>http://purl.obolibrary.org/obo/ENVO_00000467</rdfs:seeAlso>
    </owl:Class>
    


    <!-- http://www.semanticweb.org/smarotta/ontologies/2022/4/silvanusOntology#water_intake -->

    <owl:Class rdf:about="http://www.semanticweb.org/smarotta/ontologies/2022/4/silvanusOntology#water_intake">
        <rdfs:subClassOf rdf:resource="http://www.semanticweb.org/smarotta/ontologies/2022/4/silvanusOntology#Building"/>
        <rdfs:comment>A hydraulic-engineering installation which transports water - in specified amounts, of a specified quality, and in accordance with a water-consumption plan - from a source of supply into a conduit.</rdfs:comment>
        <rdfs:seeAlso>http://purl.obolibrary.org/obo/ENVO_01000968</rdfs:seeAlso>
    </owl:Class>
    


    <!-- http://www.semanticweb.org/smarotta/ontologies/2022/4/silvanusOntology#1-hour_timelag_fuels -->

    <owl:Class rdf:about="http://www.semanticweb.org/smarotta/ontologies/2022/4/silvanusOntology#1-hour_timelag_fuels">
        <rdfs:subClassOf rdf:resource="http://www.semanticweb.org/smarotta/ontologies/2022/4/silvanusOntology#Fuel_class"/>
        <silvanusOntology:source>https://www.fs.fed.us/database/feis/glossary2.html#FuelClass</silvanusOntology:source>
        <rdfs:comment>1-hour timelag fuels: Dead fuels comprised of herbaceous plants or woody plants less than about 0.25 inch (6.4 mm) in diameter and the surface layer of litter on the forest floor.</rdfs:comment>
    </owl:Class>
    


    <!-- http://www.semanticweb.org/smarotta/ontologies/2022/4/silvanusOntology#10-hour_timelag_fuels -->

    <owl:Class rdf:about="http://www.semanticweb.org/smarotta/ontologies/2022/4/silvanusOntology#10-hour_timelag_fuels">
        <rdfs:subClassOf rdf:resource="http://www.semanticweb.org/smarotta/ontologies/2022/4/silvanusOntology#Fuel_class"/>
        <silvanusOntology:source>https://www.fs.fed.us/database/feis/glossary2.html#FuelClass</silvanusOntology:source>
        <rdfs:comment>10-hour timelag fuels: Dead fuels comprised of wood from 0.25 to 1 inch (0.6-2.5 cm) in diameter and the litter from just beneath the surface to around 0.75 inch (1.9 cm) below ground.</rdfs:comment>
    </owl:Class>
    


    <!-- http://www.semanticweb.org/smarotta/ontologies/2022/4/silvanusOntology#100-hour_timelag_fuels -->

    <owl:Class rdf:about="http://www.semanticweb.org/smarotta/ontologies/2022/4/silvanusOntology#100-hour_timelag_fuels">
        <rdfs:subClassOf rdf:resource="http://www.semanticweb.org/smarotta/ontologies/2022/4/silvanusOntology#Fuel_class"/>
        <silvanusOntology:source>https://www.fs.fed.us/database/feis/glossary2.html#FuelClass</silvanusOntology:source>
        <rdfs:comment>100-hour timelag fuels: Dead fuels comprised of wood from 1 to 3 inches (2.5-7.6 cm) in diameter and litter from around 0.75 to about 4 inches (1.9-10 cm) below ground.</rdfs:comment>
    </owl:Class>
    


    <!-- http://www.semanticweb.org/smarotta/ontologies/2022/4/silvanusOntology#1000-hour_timelag_fuels -->

    <owl:Class rdf:about="http://www.semanticweb.org/smarotta/ontologies/2022/4/silvanusOntology#1000-hour_timelag_fuels">
        <rdfs:subClassOf rdf:resource="http://www.semanticweb.org/smarotta/ontologies/2022/4/silvanusOntology#Fuel_class"/>
        <silvanusOntology:source>https://www.fs.fed.us/database/feis/glossary2.html#FuelClass</silvanusOntology:source>
        <rdfs:comment>1,000-hour timelag fuels: Dead fuels comprised of wood from 3 to 8 inches (7.6-20.3) in diameter and the forest floor layer &gt;4 inches (10 cm) below ground.</rdfs:comment>
    </owl:Class>
    


    <!-- http://www.semanticweb.org/smarotta/ontologies/2022/4/silvanusOntology#24h_precipitation -->

    <owl:Class rdf:about="http://www.semanticweb.org/smarotta/ontologies/2022/4/silvanusOntology#24h_precipitation">
        <rdfs:subClassOf rdf:resource="http://www.semanticweb.org/smarotta/ontologies/2022/4/silvanusOntology#Precipitation"/>
        <silvanusOntology:source>https://cwfis.cfs.nrcan.gc.ca/background/summary/fwi</silvanusOntology:source>
        <rdfs:comment>Precipitations in the last 24h</rdfs:comment>
    </owl:Class>
    


    <!-- http://www.semanticweb.org/smarotta/ontologies/2022/4/silvanusOntology#Fireworks,_firecrackers,_distress_flares -->

    <owl:Class rdf:about="http://www.semanticweb.org/smarotta/ontologies/2022/4/silvanusOntology#Fireworks,_firecrackers,_distress_flares">
        <rdfs:subClassOf rdf:resource="http://www.semanticweb.org/smarotta/ontologies/2022/4/silvanusOntology#Use_of_glowing_objects"/>
        <silvanusOntology:source>https://effis-gwis-cms.s3-eu-west-1.amazonaws.com/effis/reports-and-publications/effis-related-publications/lb-na-25-923-en-n.pdf (page 10)</silvanusOntology:source>
        <rdfs:comment>Wildfire caused by fireworks with or without preventive measures, by firecrackers and by distress flares regardless of who lit it.</rdfs:comment>
    </owl:Class>
    


    <!-- 
    ///////////////////////////////////////////////////////////////////////////////////////
    //
    // Individuals
    //
    ///////////////////////////////////////////////////////////////////////////////////////
     -->

    


    <!-- http://www.semanticweb.org/smarotta/ontologies/2022/4/silvanusOntology#Aquic -->

    <owl:NamedIndividual rdf:about="http://www.semanticweb.org/smarotta/ontologies/2022/4/silvanusOntology#Aquic">
        <rdf:type rdf:resource="http://www.semanticweb.org/smarotta/ontologies/2022/4/silvanusOntology#Moisture"/>
    </owl:NamedIndividual>
    


    <!-- http://www.semanticweb.org/smarotta/ontologies/2022/4/silvanusOntology#Aridic -->

    <owl:NamedIndividual rdf:about="http://www.semanticweb.org/smarotta/ontologies/2022/4/silvanusOntology#Aridic">
        <rdf:type rdf:resource="http://www.semanticweb.org/smarotta/ontologies/2022/4/silvanusOntology#Moisture"/>
    </owl:NamedIndividual>
    


    <!-- http://www.semanticweb.org/smarotta/ontologies/2022/4/silvanusOntology#Centimeters -->

    <owl:NamedIndividual rdf:about="http://www.semanticweb.org/smarotta/ontologies/2022/4/silvanusOntology#Centimeters">
        <rdf:type rdf:resource="http://www.semanticweb.org/smarotta/ontologies/2022/4/silvanusOntology#Unit"/>
    </owl:NamedIndividual>
    


    <!-- http://www.semanticweb.org/smarotta/ontologies/2022/4/silvanusOntology#Codominant -->

    <owl:NamedIndividual rdf:about="http://www.semanticweb.org/smarotta/ontologies/2022/4/silvanusOntology#Codominant">
        <rdf:type rdf:resource="http://www.semanticweb.org/smarotta/ontologies/2022/4/silvanusOntology#Crown_class"/>
    </owl:NamedIndividual>
    


    <!-- http://www.semanticweb.org/smarotta/ontologies/2022/4/silvanusOntology#Cubic_Meters_by_Hectare -->

    <owl:NamedIndividual rdf:about="http://www.semanticweb.org/smarotta/ontologies/2022/4/silvanusOntology#Cubic_Meters_by_Hectare">
        <rdf:type rdf:resource="http://www.semanticweb.org/smarotta/ontologies/2022/4/silvanusOntology#Unit"/>
    </owl:NamedIndividual>
    


    <!-- http://www.semanticweb.org/smarotta/ontologies/2022/4/silvanusOntology#Decimeters -->

    <owl:NamedIndividual rdf:about="http://www.semanticweb.org/smarotta/ontologies/2022/4/silvanusOntology#Decimeters">
        <rdf:type rdf:resource="http://www.semanticweb.org/smarotta/ontologies/2022/4/silvanusOntology#Unit"/>
    </owl:NamedIndividual>
    


    <!-- http://www.semanticweb.org/smarotta/ontologies/2022/4/silvanusOntology#Degrees -->

    <owl:NamedIndividual rdf:about="http://www.semanticweb.org/smarotta/ontologies/2022/4/silvanusOntology#Degrees">
        <rdf:type rdf:resource="http://www.semanticweb.org/smarotta/ontologies/2022/4/silvanusOntology#Unit"/>
    </owl:NamedIndividual>
    


    <!-- http://www.semanticweb.org/smarotta/ontologies/2022/4/silvanusOntology#Dominant -->

    <owl:NamedIndividual rdf:about="http://www.semanticweb.org/smarotta/ontologies/2022/4/silvanusOntology#Dominant">
        <rdf:type rdf:resource="http://www.semanticweb.org/smarotta/ontologies/2022/4/silvanusOntology#Crown_class"/>
    </owl:NamedIndividual>
    


    <!-- http://www.semanticweb.org/smarotta/ontologies/2022/4/silvanusOntology#Emergent -->

    <owl:NamedIndividual rdf:about="http://www.semanticweb.org/smarotta/ontologies/2022/4/silvanusOntology#Emergent">
        <rdf:type rdf:resource="http://www.semanticweb.org/smarotta/ontologies/2022/4/silvanusOntology#Crown_class"/>
    </owl:NamedIndividual>
    


    <!-- http://www.semanticweb.org/smarotta/ontologies/2022/4/silvanusOntology#Gradians -->

    <owl:NamedIndividual rdf:about="http://www.semanticweb.org/smarotta/ontologies/2022/4/silvanusOntology#Gradians">
        <rdf:type rdf:resource="http://www.semanticweb.org/smarotta/ontologies/2022/4/silvanusOntology#Unit"/>
    </owl:NamedIndividual>
    


    <!-- http://www.semanticweb.org/smarotta/ontologies/2022/4/silvanusOntology#Hectares -->

    <owl:NamedIndividual rdf:about="http://www.semanticweb.org/smarotta/ontologies/2022/4/silvanusOntology#Hectares">
        <rdf:type rdf:resource="http://www.semanticweb.org/smarotta/ontologies/2022/4/silvanusOntology#Unit"/>
    </owl:NamedIndividual>
    


    <!-- http://www.semanticweb.org/smarotta/ontologies/2022/4/silvanusOntology#Intermediate -->

    <owl:NamedIndividual rdf:about="http://www.semanticweb.org/smarotta/ontologies/2022/4/silvanusOntology#Intermediate"/>
    


    <!-- http://www.semanticweb.org/smarotta/ontologies/2022/4/silvanusOntology#Meters -->

    <owl:NamedIndividual rdf:about="http://www.semanticweb.org/smarotta/ontologies/2022/4/silvanusOntology#Meters">
        <rdf:type rdf:resource="http://www.semanticweb.org/smarotta/ontologies/2022/4/silvanusOntology#Unit"/>
    </owl:NamedIndividual>
    


    <!-- http://www.semanticweb.org/smarotta/ontologies/2022/4/silvanusOntology#Millimeters -->

    <owl:NamedIndividual rdf:about="http://www.semanticweb.org/smarotta/ontologies/2022/4/silvanusOntology#Millimeters">
        <rdf:type rdf:resource="http://www.semanticweb.org/smarotta/ontologies/2022/4/silvanusOntology#Unit"/>
    </owl:NamedIndividual>
    


    <!-- http://www.semanticweb.org/smarotta/ontologies/2022/4/silvanusOntology#Overtopped -->

    <owl:NamedIndividual rdf:about="http://www.semanticweb.org/smarotta/ontologies/2022/4/silvanusOntology#Overtopped">
        <rdf:type rdf:resource="http://www.semanticweb.org/smarotta/ontologies/2022/4/silvanusOntology#Crown_class"/>
    </owl:NamedIndividual>
    


    <!-- http://www.semanticweb.org/smarotta/ontologies/2022/4/silvanusOntology#Percentage -->

    <owl:NamedIndividual rdf:about="http://www.semanticweb.org/smarotta/ontologies/2022/4/silvanusOntology#Percentage">
        <rdf:type rdf:resource="http://www.semanticweb.org/smarotta/ontologies/2022/4/silvanusOntology#Unit"/>
    </owl:NamedIndividual>
    


    <!-- http://www.semanticweb.org/smarotta/ontologies/2022/4/silvanusOntology#Seedling -->

    <owl:NamedIndividual rdf:about="http://www.semanticweb.org/smarotta/ontologies/2022/4/silvanusOntology#Seedling">
        <rdf:type rdf:resource="http://www.semanticweb.org/smarotta/ontologies/2022/4/silvanusOntology#Crown_class"/>
    </owl:NamedIndividual>
    


    <!-- http://www.semanticweb.org/smarotta/ontologies/2022/4/silvanusOntology#Square_Meters -->

    <owl:NamedIndividual rdf:about="http://www.semanticweb.org/smarotta/ontologies/2022/4/silvanusOntology#Square_Meters">
        <rdf:type rdf:resource="http://www.semanticweb.org/smarotta/ontologies/2022/4/silvanusOntology#Unit"/>
    </owl:NamedIndividual>
    


    <!-- http://www.semanticweb.org/smarotta/ontologies/2022/4/silvanusOntology#Square_Meters_by_Hectare -->

    <owl:NamedIndividual rdf:about="http://www.semanticweb.org/smarotta/ontologies/2022/4/silvanusOntology#Square_Meters_by_Hectare">
        <rdf:type rdf:resource="http://www.semanticweb.org/smarotta/ontologies/2022/4/silvanusOntology#Unit"/>
    </owl:NamedIndividual>
    


    <!-- http://www.semanticweb.org/smarotta/ontologies/2022/4/silvanusOntology#Udic -->

    <owl:NamedIndividual rdf:about="http://www.semanticweb.org/smarotta/ontologies/2022/4/silvanusOntology#Udic">
        <rdf:type rdf:resource="http://www.semanticweb.org/smarotta/ontologies/2022/4/silvanusOntology#Moisture"/>
    </owl:NamedIndividual>
    


    <!-- http://www.semanticweb.org/smarotta/ontologies/2022/4/silvanusOntology#Unities -->

    <owl:NamedIndividual rdf:about="http://www.semanticweb.org/smarotta/ontologies/2022/4/silvanusOntology#Unities">
        <rdf:type rdf:resource="http://www.semanticweb.org/smarotta/ontologies/2022/4/silvanusOntology#Unit"/>
    </owl:NamedIndividual>
    


    <!-- http://www.semanticweb.org/smarotta/ontologies/2022/4/silvanusOntology#Units_by_Hectare -->

    <owl:NamedIndividual rdf:about="http://www.semanticweb.org/smarotta/ontologies/2022/4/silvanusOntology#Units_by_Hectare">
        <rdf:type rdf:resource="http://www.semanticweb.org/smarotta/ontologies/2022/4/silvanusOntology#Unit"/>
    </owl:NamedIndividual>
    


    <!-- http://www.semanticweb.org/smarotta/ontologies/2022/4/silvanusOntology#Ustic -->

    <owl:NamedIndividual rdf:about="http://www.semanticweb.org/smarotta/ontologies/2022/4/silvanusOntology#Ustic">
        <rdf:type rdf:resource="http://www.semanticweb.org/smarotta/ontologies/2022/4/silvanusOntology#Moisture"/>
    </owl:NamedIndividual>
    


    <!-- http://www.semanticweb.org/smarotta/ontologies/2022/4/silvanusOntology#Xeric -->

    <owl:NamedIndividual rdf:about="http://www.semanticweb.org/smarotta/ontologies/2022/4/silvanusOntology#Xeric">
        <rdf:type rdf:resource="http://www.semanticweb.org/smarotta/ontologies/2022/4/silvanusOntology#Moisture"/>
    </owl:NamedIndividual>
    


    <!-- http://www.semanticweb.org/smarotta/ontologies/2022/4/silvanusOntology#Years -->

    <owl:NamedIndividual rdf:about="http://www.semanticweb.org/smarotta/ontologies/2022/4/silvanusOntology#Years">
        <rdf:type rdf:resource="http://www.semanticweb.org/smarotta/ontologies/2022/4/silvanusOntology#Unit"/>
    </owl:NamedIndividual>
    


    <!-- 
    ///////////////////////////////////////////////////////////////////////////////////////
    //
    // Annotations
    //
    ///////////////////////////////////////////////////////////////////////////////////////
     -->

    <rdf:Description rdf:about="http://www.semanticweb.org/smarotta/ontologies/2022/4/silvanusOntology#Hectares">
        <rdfs:seeAlso>http://crossforest.eu/measures/ontology/Hectares</rdfs:seeAlso>
        <rdfs:comment>The hectare is a non-SI metric unit of area equal to a square with 100-metre sides (1 hm2), or 10,000 m2, and is primarily used in the measurement of land.</rdfs:comment>
    </rdf:Description>
    <rdf:Description rdf:about="http://www.semanticweb.org/smarotta/ontologies/2022/4/silvanusOntology#Years">
        <rdfs:seeAlso>http://crossforest.eu/measures/ontology/Years</rdfs:seeAlso>
        <rdfs:comment>Time measured in years</rdfs:comment>
    </rdf:Description>
    


    <!-- 
    ///////////////////////////////////////////////////////////////////////////////////////
    //
    // General axioms
    //
    ///////////////////////////////////////////////////////////////////////////////////////
     -->

    <rdf:Description>
        <rdf:type rdf:resource="http://www.w3.org/2002/07/owl#AllDisjointClasses"/>
        <owl:members rdf:parseType="Collection">
            <rdf:Description rdf:about="http://www.semanticweb.org/smarotta/ontologies/2022/4/silvanusOntology#Accident"/>
            <rdf:Description rdf:about="http://www.semanticweb.org/smarotta/ontologies/2022/4/silvanusOntology#Deliberate"/>
            <rdf:Description rdf:about="http://www.semanticweb.org/smarotta/ontologies/2022/4/silvanusOntology#Natural"/>
            <rdf:Description rdf:about="http://www.semanticweb.org/smarotta/ontologies/2022/4/silvanusOntology#Negligence"/>
            <rdf:Description rdf:about="http://www.semanticweb.org/smarotta/ontologies/2022/4/silvanusOntology#Rekindle"/>
            <rdf:Description rdf:about="http://www.semanticweb.org/smarotta/ontologies/2022/4/silvanusOntology#Unknown"/>
        </owl:members>
    </rdf:Description>
    <rdf:Description>
        <rdf:type rdf:resource="http://www.w3.org/2002/07/owl#AllDisjointClasses"/>
        <owl:members rdf:parseType="Collection">
            <rdf:Description rdf:about="http://www.semanticweb.org/smarotta/ontologies/2022/4/silvanusOntology#Adolescent"/>
            <rdf:Description rdf:about="http://www.semanticweb.org/smarotta/ontologies/2022/4/silvanusOntology#Adult"/>
            <rdf:Description rdf:about="http://www.semanticweb.org/smarotta/ontologies/2022/4/silvanusOntology#Child"/>
            <rdf:Description rdf:about="http://www.semanticweb.org/smarotta/ontologies/2022/4/silvanusOntology#Infant"/>
        </owl:members>
    </rdf:Description>
    <rdf:Description>
        <rdf:type rdf:resource="http://www.w3.org/2002/07/owl#AllDisjointClasses"/>
        <owl:members rdf:parseType="Collection">
            <rdf:Description rdf:about="http://www.semanticweb.org/smarotta/ontologies/2022/4/silvanusOntology#Agricultural_management"/>
            <rdf:Description rdf:about="http://www.semanticweb.org/smarotta/ontologies/2022/4/silvanusOntology#Other_negligent_use_of_fire"/>
            <rdf:Description rdf:about="http://www.semanticweb.org/smarotta/ontologies/2022/4/silvanusOntology#Recreation"/>
            <rdf:Description rdf:about="http://www.semanticweb.org/smarotta/ontologies/2022/4/silvanusOntology#Vegetation_management"/>
            <rdf:Description rdf:about="http://www.semanticweb.org/smarotta/ontologies/2022/4/silvanusOntology#Waste_management"/>
        </owl:members>
    </rdf:Description>
    <rdf:Description>
        <rdf:type rdf:resource="http://www.w3.org/2002/07/owl#AllDisjointClasses"/>
        <owl:members rdf:parseType="Collection">
            <rdf:Description rdf:about="http://www.semanticweb.org/smarotta/ontologies/2022/4/silvanusOntology#Agriculture"/>
            <rdf:Description rdf:about="http://www.semanticweb.org/smarotta/ontologies/2022/4/silvanusOntology#Dunes"/>
            <rdf:Description rdf:about="http://www.semanticweb.org/smarotta/ontologies/2022/4/silvanusOntology#Natural_habitat"/>
            <rdf:Description rdf:about="http://www.semanticweb.org/smarotta/ontologies/2022/4/silvanusOntology#Plant"/>
            <rdf:Description rdf:about="http://www.semanticweb.org/smarotta/ontologies/2022/4/silvanusOntology#River"/>
        </owl:members>
    </rdf:Description>
    <rdf:Description>
        <rdf:type rdf:resource="http://www.w3.org/2002/07/owl#AllDisjointClasses"/>
        <owl:members rdf:parseType="Collection">
            <rdf:Description rdf:about="http://www.semanticweb.org/smarotta/ontologies/2022/4/silvanusOntology#Aircraft"/>
            <rdf:Description rdf:about="http://www.semanticweb.org/smarotta/ontologies/2022/4/silvanusOntology#Ground_Vehicle"/>
            <rdf:Description rdf:about="http://www.semanticweb.org/smarotta/ontologies/2022/4/silvanusOntology#Watercraft"/>
        </owl:members>
    </rdf:Description>
    <rdf:Description>
        <rdf:type rdf:resource="http://www.w3.org/2002/07/owl#AllDisjointClasses"/>
        <owl:members rdf:parseType="Collection">
            <rdf:Description rdf:about="http://www.semanticweb.org/smarotta/ontologies/2022/4/silvanusOntology#Airport"/>
            <rdf:Description rdf:about="http://www.semanticweb.org/smarotta/ontologies/2022/4/silvanusOntology#Pier"/>
            <rdf:Description rdf:about="http://www.semanticweb.org/smarotta/ontologies/2022/4/silvanusOntology#Port"/>
        </owl:members>
    </rdf:Description>
    <rdf:Description>
        <rdf:type rdf:resource="http://www.w3.org/2002/07/owl#AllDisjointClasses"/>
        <owl:members rdf:parseType="Collection">
            <rdf:Description rdf:about="http://www.semanticweb.org/smarotta/ontologies/2022/4/silvanusOntology#All_season_road"/>
            <rdf:Description rdf:about="http://www.semanticweb.org/smarotta/ontologies/2022/4/silvanusOntology#Asphalt_road"/>
            <rdf:Description rdf:about="http://www.semanticweb.org/smarotta/ontologies/2022/4/silvanusOntology#Concrete_road"/>
            <rdf:Description rdf:about="http://www.semanticweb.org/smarotta/ontologies/2022/4/silvanusOntology#Driveway"/>
            <rdf:Description rdf:about="http://www.semanticweb.org/smarotta/ontologies/2022/4/silvanusOntology#Public_street"/>
            <rdf:Description rdf:about="http://www.semanticweb.org/smarotta/ontologies/2022/4/silvanusOntology#Track"/>
        </owl:members>
    </rdf:Description>
    <rdf:Description>
        <rdf:type rdf:resource="http://www.w3.org/2002/07/owl#AllDisjointClasses"/>
        <owl:members rdf:parseType="Collection">
            <rdf:Description rdf:about="http://www.semanticweb.org/smarotta/ontologies/2022/4/silvanusOntology#Allocentric_Position"/>
            <rdf:Description rdf:about="http://www.semanticweb.org/smarotta/ontologies/2022/4/silvanusOntology#Egocentric_Position"/>
            <rdf:Description rdf:about="http://www.semanticweb.org/smarotta/ontologies/2022/4/silvanusOntology#Geocentric_Position"/>
            <rdf:Description rdf:about="http://www.semanticweb.org/smarotta/ontologies/2022/4/silvanusOntology#Polygon"/>
            <rdf:Description rdf:about="http://www.semanticweb.org/smarotta/ontologies/2022/4/silvanusOntology#Reference_Position"/>
        </owl:members>
    </rdf:Description>
    <rdf:Description>
        <rdf:type rdf:resource="http://www.w3.org/2002/07/owl#AllDisjointClasses"/>
        <owl:members rdf:parseType="Collection">
            <rdf:Description rdf:about="http://www.semanticweb.org/smarotta/ontologies/2022/4/silvanusOntology#Alpine_Biome"/>
            <rdf:Description rdf:about="http://www.semanticweb.org/smarotta/ontologies/2022/4/silvanusOntology#Aquatic_Biome"/>
            <rdf:Description rdf:about="http://www.semanticweb.org/smarotta/ontologies/2022/4/silvanusOntology#Arid_Biome"/>
            <rdf:Description rdf:about="http://www.semanticweb.org/smarotta/ontologies/2022/4/silvanusOntology#Mediterranean_Biome"/>
            <rdf:Description rdf:about="http://www.semanticweb.org/smarotta/ontologies/2022/4/silvanusOntology#Montane_Biome"/>
            <rdf:Description rdf:about="http://www.semanticweb.org/smarotta/ontologies/2022/4/silvanusOntology#Ocean_Biome"/>
            <rdf:Description rdf:about="http://www.semanticweb.org/smarotta/ontologies/2022/4/silvanusOntology#Polar_Biome"/>
            <rdf:Description rdf:about="http://www.semanticweb.org/smarotta/ontologies/2022/4/silvanusOntology#Subalpine_Biome"/>
            <rdf:Description rdf:about="http://www.semanticweb.org/smarotta/ontologies/2022/4/silvanusOntology#Subpolar_Biome"/>
            <rdf:Description rdf:about="http://www.semanticweb.org/smarotta/ontologies/2022/4/silvanusOntology#Subtropical_Biome"/>
            <rdf:Description rdf:about="http://www.semanticweb.org/smarotta/ontologies/2022/4/silvanusOntology#Temperate_Biome"/>
            <rdf:Description rdf:about="http://www.semanticweb.org/smarotta/ontologies/2022/4/silvanusOntology#Terrestrial_Biome"/>
            <rdf:Description rdf:about="http://www.semanticweb.org/smarotta/ontologies/2022/4/silvanusOntology#Tropical_Biome"/>
        </owl:members>
    </rdf:Description>
    <rdf:Description>
        <rdf:type rdf:resource="http://www.w3.org/2002/07/owl#AllDisjointClasses"/>
        <owl:members rdf:parseType="Collection">
            <rdf:Description rdf:about="http://www.semanticweb.org/smarotta/ontologies/2022/4/silvanusOntology#Animal"/>
            <rdf:Description rdf:about="http://www.semanticweb.org/smarotta/ontologies/2022/4/silvanusOntology#Biome"/>
            <rdf:Description rdf:about="http://www.semanticweb.org/smarotta/ontologies/2022/4/silvanusOntology#Damage_quantification"/>
            <rdf:Description rdf:about="http://www.semanticweb.org/smarotta/ontologies/2022/4/silvanusOntology#Diametric_class"/>
            <rdf:Description rdf:about="http://www.semanticweb.org/smarotta/ontologies/2022/4/silvanusOntology#Dominant_formation"/>
            <rdf:Description rdf:about="http://www.semanticweb.org/smarotta/ontologies/2022/4/silvanusOntology#Erosion"/>
            <rdf:Description rdf:about="http://www.semanticweb.org/smarotta/ontologies/2022/4/silvanusOntology#Evnironment_index"/>
            <rdf:Description rdf:about="http://www.semanticweb.org/smarotta/ontologies/2022/4/silvanusOntology#Fuel"/>
            <rdf:Description rdf:about="http://www.semanticweb.org/smarotta/ontologies/2022/4/silvanusOntology#Geology"/>
            <rdf:Description rdf:about="http://www.semanticweb.org/smarotta/ontologies/2022/4/silvanusOntology#Grazing_activity"/>
            <rdf:Description rdf:about="http://www.semanticweb.org/smarotta/ontologies/2022/4/silvanusOntology#Hydrography"/>
            <rdf:Description rdf:about="http://www.semanticweb.org/smarotta/ontologies/2022/4/silvanusOntology#Land_use"/>
            <rdf:Description rdf:about="http://www.semanticweb.org/smarotta/ontologies/2022/4/silvanusOntology#Measure"/>
            <rdf:Description rdf:about="http://www.semanticweb.org/smarotta/ontologies/2022/4/silvanusOntology#MeasureInUnities"/>
            <rdf:Description rdf:about="http://www.semanticweb.org/smarotta/ontologies/2022/4/silvanusOntology#Topography"/>
            <rdf:Description rdf:about="http://www.semanticweb.org/smarotta/ontologies/2022/4/silvanusOntology#Vegetated_area"/>
            <rdf:Description rdf:about="http://www.semanticweb.org/smarotta/ontologies/2022/4/silvanusOntology#Vegetation_growth"/>
            <rdf:Description rdf:about="http://www.semanticweb.org/smarotta/ontologies/2022/4/silvanusOntology#Vegetation_index"/>
        </owl:members>
    </rdf:Description>
    <rdf:Description>
        <rdf:type rdf:resource="http://www.w3.org/2002/07/owl#AllDisjointClasses"/>
        <owl:members rdf:parseType="Collection">
            <rdf:Description rdf:about="http://www.semanticweb.org/smarotta/ontologies/2022/4/silvanusOntology#Animal"/>
            <rdf:Description rdf:about="http://www.semanticweb.org/smarotta/ontologies/2022/4/silvanusOntology#Biome"/>
            <rdf:Description rdf:about="http://www.semanticweb.org/smarotta/ontologies/2022/4/silvanusOntology#Damage_quantification"/>
            <rdf:Description rdf:about="http://www.semanticweb.org/smarotta/ontologies/2022/4/silvanusOntology#Evnironment_index"/>
            <rdf:Description rdf:about="http://www.semanticweb.org/smarotta/ontologies/2022/4/silvanusOntology#Fuel"/>
            <rdf:Description rdf:about="http://www.semanticweb.org/smarotta/ontologies/2022/4/silvanusOntology#Geology"/>
            <rdf:Description rdf:about="http://www.semanticweb.org/smarotta/ontologies/2022/4/silvanusOntology#Grazing_activity"/>
            <rdf:Description rdf:about="http://www.semanticweb.org/smarotta/ontologies/2022/4/silvanusOntology#Hydrography"/>
            <rdf:Description rdf:about="http://www.semanticweb.org/smarotta/ontologies/2022/4/silvanusOntology#Land_use"/>
            <rdf:Description rdf:about="http://www.semanticweb.org/smarotta/ontologies/2022/4/silvanusOntology#Topography"/>
            <rdf:Description rdf:about="http://www.semanticweb.org/smarotta/ontologies/2022/4/silvanusOntology#Vegetated_area"/>
            <rdf:Description rdf:about="http://www.semanticweb.org/smarotta/ontologies/2022/4/silvanusOntology#Vegetation_growth"/>
            <rdf:Description rdf:about="http://www.semanticweb.org/smarotta/ontologies/2022/4/silvanusOntology#Vegetation_index"/>
        </owl:members>
    </rdf:Description>
    <rdf:Description>
        <rdf:type rdf:resource="http://www.w3.org/2002/07/owl#AllDisjointClasses"/>
        <owl:members rdf:parseType="Collection">
            <rdf:Description rdf:about="http://www.semanticweb.org/smarotta/ontologies/2022/4/silvanusOntology#Anthropogenic_Terrestrial_Biome"/>
            <rdf:Description rdf:about="http://www.semanticweb.org/smarotta/ontologies/2022/4/silvanusOntology#Mangrove_Biome"/>
            <rdf:Description rdf:about="http://www.semanticweb.org/smarotta/ontologies/2022/4/silvanusOntology#Shrubland_Biome"/>
            <rdf:Description rdf:about="http://www.semanticweb.org/smarotta/ontologies/2022/4/silvanusOntology#Tundra_Biome"/>
            <rdf:Description rdf:about="http://www.semanticweb.org/smarotta/ontologies/2022/4/silvanusOntology#Woodland_Biome"/>
        </owl:members>
    </rdf:Description>
    <rdf:Description>
        <rdf:type rdf:resource="http://www.w3.org/2002/07/owl#AllDisjointClasses"/>
        <owl:members rdf:parseType="Collection">
            <rdf:Description rdf:about="http://www.semanticweb.org/smarotta/ontologies/2022/4/silvanusOntology#Area_Of_Cropland"/>
            <rdf:Description rdf:about="http://www.semanticweb.org/smarotta/ontologies/2022/4/silvanusOntology#Area_Of_Evergreen_Forest"/>
            <rdf:Description rdf:about="http://www.semanticweb.org/smarotta/ontologies/2022/4/silvanusOntology#Area_Of_Lichen-dominated_Vegetation"/>
            <rdf:Description rdf:about="http://www.semanticweb.org/smarotta/ontologies/2022/4/silvanusOntology#Area_Of_Mixed_Forest"/>
            <rdf:Description rdf:about="http://www.semanticweb.org/smarotta/ontologies/2022/4/silvanusOntology#Area_Of_Moss-dominated_Vegetation"/>
            <rdf:Description rdf:about="http://www.semanticweb.org/smarotta/ontologies/2022/4/silvanusOntology#Area_Of_Sedge-_And_Forb-dominated_Herbaceous_Vegetation"/>
            <rdf:Description rdf:about="http://www.semanticweb.org/smarotta/ontologies/2022/4/silvanusOntology#Area_Of_Tundra"/>
            <rdf:Description rdf:about="http://www.semanticweb.org/smarotta/ontologies/2022/4/silvanusOntology#Area_Of_Woody_Wetland"/>
            <rdf:Description rdf:about="http://www.semanticweb.org/smarotta/ontologies/2022/4/silvanusOntology#Bush_Area"/>
            <rdf:Description rdf:about="http://www.semanticweb.org/smarotta/ontologies/2022/4/silvanusOntology#Flower_Strip"/>
            <rdf:Description rdf:about="http://www.semanticweb.org/smarotta/ontologies/2022/4/silvanusOntology#Grassland_Area"/>
            <rdf:Description rdf:about="http://www.semanticweb.org/smarotta/ontologies/2022/4/silvanusOntology#Heath"/>
            <rdf:Description rdf:about="http://www.semanticweb.org/smarotta/ontologies/2022/4/silvanusOntology#Oasis"/>
            <rdf:Description rdf:about="http://www.semanticweb.org/smarotta/ontologies/2022/4/silvanusOntology#Scrubland_Area"/>
            <rdf:Description rdf:about="http://www.semanticweb.org/smarotta/ontologies/2022/4/silvanusOntology#Wetland_Area"/>
            <rdf:Description rdf:about="http://www.semanticweb.org/smarotta/ontologies/2022/4/silvanusOntology#Woodland_Area"/>
        </owl:members>
    </rdf:Description>
    <rdf:Description>
        <rdf:type rdf:resource="http://www.w3.org/2002/07/owl#AllDisjointClasses"/>
        <owl:members rdf:parseType="Collection">
            <rdf:Description rdf:about="http://www.semanticweb.org/smarotta/ontologies/2022/4/silvanusOntology#Armored_Personnel_Carrier"/>
            <rdf:Description rdf:about="http://www.semanticweb.org/smarotta/ontologies/2022/4/silvanusOntology#Automobile"/>
            <rdf:Description rdf:about="http://www.semanticweb.org/smarotta/ontologies/2022/4/silvanusOntology#Bus"/>
            <rdf:Description rdf:about="http://www.semanticweb.org/smarotta/ontologies/2022/4/silvanusOntology#Infantry_Fighting_Vehicle"/>
            <rdf:Description rdf:about="http://www.semanticweb.org/smarotta/ontologies/2022/4/silvanusOntology#Motorcycle"/>
            <rdf:Description rdf:about="http://www.semanticweb.org/smarotta/ontologies/2022/4/silvanusOntology#Tank"/>
            <rdf:Description rdf:about="http://www.semanticweb.org/smarotta/ontologies/2022/4/silvanusOntology#Truck"/>
        </owl:members>
    </rdf:Description>
    <rdf:Description>
        <rdf:type rdf:resource="http://www.w3.org/2002/07/owl#AllDisjointClasses"/>
        <owl:members rdf:parseType="Collection">
            <rdf:Description rdf:about="http://www.semanticweb.org/smarotta/ontologies/2022/4/silvanusOntology#Basal_Area"/>
            <rdf:Description rdf:about="http://www.semanticweb.org/smarotta/ontologies/2022/4/silvanusOntology#Measure_In_Centimeters"/>
            <rdf:Description rdf:about="http://www.semanticweb.org/smarotta/ontologies/2022/4/silvanusOntology#Measure_In_Decimeters"/>
            <rdf:Description rdf:about="http://www.semanticweb.org/smarotta/ontologies/2022/4/silvanusOntology#Measure_In_Degrees"/>
            <rdf:Description rdf:about="http://www.semanticweb.org/smarotta/ontologies/2022/4/silvanusOntology#Measure_In_Gradians"/>
            <rdf:Description rdf:about="http://www.semanticweb.org/smarotta/ontologies/2022/4/silvanusOntology#Measure_In_Hectares"/>
            <rdf:Description rdf:about="http://www.semanticweb.org/smarotta/ontologies/2022/4/silvanusOntology#Measure_In_Meters"/>
            <rdf:Description rdf:about="http://www.semanticweb.org/smarotta/ontologies/2022/4/silvanusOntology#Measure_In_Millimeters"/>
            <rdf:Description rdf:about="http://www.semanticweb.org/smarotta/ontologies/2022/4/silvanusOntology#Measure_In_Percentage"/>
            <rdf:Description rdf:about="http://www.semanticweb.org/smarotta/ontologies/2022/4/silvanusOntology#Measure_In_SquareMeters"/>
            <rdf:Description rdf:about="http://www.semanticweb.org/smarotta/ontologies/2022/4/silvanusOntology#Measure_In_Unities"/>
            <rdf:Description rdf:about="http://www.semanticweb.org/smarotta/ontologies/2022/4/silvanusOntology#Measure_In_Years"/>
            <rdf:Description rdf:about="http://www.semanticweb.org/smarotta/ontologies/2022/4/silvanusOntology#Volume_with_bark"/>
        </owl:members>
    </rdf:Description>
    <rdf:Description>
        <rdf:type rdf:resource="http://www.w3.org/2002/07/owl#AllDisjointClasses"/>
        <owl:members rdf:parseType="Collection">
            <rdf:Description rdf:about="http://www.semanticweb.org/smarotta/ontologies/2022/4/silvanusOntology#Basic_region_for_the_application_of_regional_policies"/>
            <rdf:Description rdf:about="http://www.semanticweb.org/smarotta/ontologies/2022/4/silvanusOntology#Major_socio-economic_region"/>
            <rdf:Description rdf:about="http://www.semanticweb.org/smarotta/ontologies/2022/4/silvanusOntology#Small_region_for_specific_diagnoses"/>
        </owl:members>
    </rdf:Description>
    <rdf:Description>
        <rdf:type rdf:resource="http://www.w3.org/2002/07/owl#AllDisjointClasses"/>
        <owl:members rdf:parseType="Collection">
            <rdf:Description rdf:about="http://www.semanticweb.org/smarotta/ontologies/2022/4/silvanusOntology#Bicycle"/>
            <rdf:Description rdf:about="http://www.semanticweb.org/smarotta/ontologies/2022/4/silvanusOntology#Ground_Motor_Vehicle"/>
            <rdf:Description rdf:about="http://www.semanticweb.org/smarotta/ontologies/2022/4/silvanusOntology#Rail_Transport_Vehicle"/>
        </owl:members>
    </rdf:Description>
    <rdf:Description>
        <rdf:type rdf:resource="http://www.w3.org/2002/07/owl#AllDisjointClasses"/>
        <owl:members rdf:parseType="Collection">
            <rdf:Description rdf:about="http://www.semanticweb.org/smarotta/ontologies/2022/4/silvanusOntology#Bridge"/>
            <rdf:Description rdf:about="http://www.semanticweb.org/smarotta/ontologies/2022/4/silvanusOntology#Building"/>
            <rdf:Description rdf:about="http://www.semanticweb.org/smarotta/ontologies/2022/4/silvanusOntology#Church"/>
            <rdf:Description rdf:about="http://www.semanticweb.org/smarotta/ontologies/2022/4/silvanusOntology#Collection_point"/>
            <rdf:Description rdf:about="http://www.semanticweb.org/smarotta/ontologies/2022/4/silvanusOntology#Constructed_barrier"/>
            <rdf:Description rdf:about="http://www.semanticweb.org/smarotta/ontologies/2022/4/silvanusOntology#Cycling_route"/>
            <rdf:Description rdf:about="http://www.semanticweb.org/smarotta/ontologies/2022/4/silvanusOntology#Leevee"/>
            <rdf:Description rdf:about="http://www.semanticweb.org/smarotta/ontologies/2022/4/silvanusOntology#Monument"/>
            <rdf:Description rdf:about="http://www.semanticweb.org/smarotta/ontologies/2022/4/silvanusOntology#Square"/>
            <rdf:Description rdf:about="http://www.semanticweb.org/smarotta/ontologies/2022/4/silvanusOntology#Summer_camp"/>
            <rdf:Description rdf:about="http://www.semanticweb.org/smarotta/ontologies/2022/4/silvanusOntology#Touristic_route"/>
            <rdf:Description rdf:about="http://www.semanticweb.org/smarotta/ontologies/2022/4/silvanusOntology#Wall"/>
            <rdf:Description rdf:about="http://www.semanticweb.org/smarotta/ontologies/2022/4/silvanusOntology#university_campus"/>
            <rdf:Description rdf:about="http://www.semanticweb.org/smarotta/ontologies/2022/4/silvanusOntology#water_intake"/>
        </owl:members>
    </rdf:Description>
    <rdf:Description>
        <rdf:type rdf:resource="http://www.w3.org/2002/07/owl#AllDisjointClasses"/>
        <owl:members rdf:parseType="Collection">
            <rdf:Description rdf:about="http://www.semanticweb.org/smarotta/ontologies/2022/4/silvanusOntology#Bridge"/>
            <rdf:Description rdf:about="http://www.semanticweb.org/smarotta/ontologies/2022/4/silvanusOntology#Causeway"/>
            <rdf:Description rdf:about="http://www.semanticweb.org/smarotta/ontologies/2022/4/silvanusOntology#Public_transport"/>
            <rdf:Description rdf:about="http://www.semanticweb.org/smarotta/ontologies/2022/4/silvanusOntology#Street"/>
            <rdf:Description rdf:about="http://www.semanticweb.org/smarotta/ontologies/2022/4/silvanusOntology#ford"/>
            <rdf:Description rdf:about="http://www.semanticweb.org/smarotta/ontologies/2022/4/silvanusOntology#lock"/>
            <rdf:Description rdf:about="http://www.semanticweb.org/smarotta/ontologies/2022/4/silvanusOntology#pier"/>
            <rdf:Description rdf:about="http://www.semanticweb.org/smarotta/ontologies/2022/4/silvanusOntology#railway"/>
        </owl:members>
    </rdf:Description>
    <rdf:Description>
        <rdf:type rdf:resource="http://www.w3.org/2002/07/owl#AllDisjointClasses"/>
        <owl:members rdf:parseType="Collection">
            <rdf:Description rdf:about="http://www.semanticweb.org/smarotta/ontologies/2022/4/silvanusOntology#Cigarettes"/>
            <rdf:Description rdf:about="http://www.semanticweb.org/smarotta/ontologies/2022/4/silvanusOntology#Hot_ashes"/>
            <rdf:Description rdf:about="http://www.semanticweb.org/smarotta/ontologies/2022/4/silvanusOntology#Other_use_of_glowing_objects"/>
            <rdf:Description rdf:about="http://www.semanticweb.org/smarotta/ontologies/2022/4/silvanusOntology#Fireworks,_firecrackers,_distress_flares"/>
        </owl:members>
    </rdf:Description>
    <rdf:Description>
        <rdf:type rdf:resource="http://www.w3.org/2002/07/owl#AllDisjointClasses"/>
        <owl:members rdf:parseType="Collection">
            <rdf:Description rdf:about="http://www.semanticweb.org/smarotta/ontologies/2022/4/silvanusOntology#Clothing"/>
            <rdf:Description rdf:about="http://www.semanticweb.org/smarotta/ontologies/2022/4/silvanusOntology#DryFood"/>
            <rdf:Description rdf:about="http://www.semanticweb.org/smarotta/ontologies/2022/4/silvanusOntology#First_Aid_Kit"/>
            <rdf:Description rdf:about="http://www.semanticweb.org/smarotta/ontologies/2022/4/silvanusOntology#HousingEquipment"/>
            <rdf:Description rdf:about="http://www.semanticweb.org/smarotta/ontologies/2022/4/silvanusOntology#SanitaryEquipment"/>
        </owl:members>
    </rdf:Description>
    <rdf:Description>
        <rdf:type rdf:resource="http://www.w3.org/2002/07/owl#AllDisjointClasses"/>
        <owl:members rdf:parseType="Collection">
            <rdf:Description rdf:about="http://www.semanticweb.org/smarotta/ontologies/2022/4/silvanusOntology#Communication"/>
            <rdf:Description rdf:about="http://www.semanticweb.org/smarotta/ontologies/2022/4/silvanusOntology#Educational_facility"/>
            <rdf:Description rdf:about="http://www.semanticweb.org/smarotta/ontologies/2022/4/silvanusOntology#Energy"/>
            <rdf:Description rdf:about="http://www.semanticweb.org/smarotta/ontologies/2022/4/silvanusOntology#Fire_department"/>
            <rdf:Description rdf:about="http://www.semanticweb.org/smarotta/ontologies/2022/4/silvanusOntology#Garbage_collection"/>
            <rdf:Description rdf:about="http://www.semanticweb.org/smarotta/ontologies/2022/4/silvanusOntology#Hospital"/>
            <rdf:Description rdf:about="http://www.semanticweb.org/smarotta/ontologies/2022/4/silvanusOntology#Police"/>
            <rdf:Description rdf:about="http://www.semanticweb.org/smarotta/ontologies/2022/4/silvanusOntology#Sewer"/>
            <rdf:Description rdf:about="http://www.semanticweb.org/smarotta/ontologies/2022/4/silvanusOntology#Transportation"/>
            <rdf:Description rdf:about="http://www.semanticweb.org/smarotta/ontologies/2022/4/silvanusOntology#Water_supply"/>
        </owl:members>
    </rdf:Description>
    <rdf:Description>
        <rdf:type rdf:resource="http://www.w3.org/2002/07/owl#AllDisjointClasses"/>
        <owl:members rdf:parseType="Collection">
            <rdf:Description rdf:about="http://www.semanticweb.org/smarotta/ontologies/2022/4/silvanusOntology#Conflict"/>
            <rdf:Description rdf:about="http://www.semanticweb.org/smarotta/ontologies/2022/4/silvanusOntology#Crime_concealment"/>
            <rdf:Description rdf:about="http://www.semanticweb.org/smarotta/ontologies/2022/4/silvanusOntology#Excitement"/>
            <rdf:Description rdf:about="http://www.semanticweb.org/smarotta/ontologies/2022/4/silvanusOntology#Extremist"/>
            <rdf:Description rdf:about="http://www.semanticweb.org/smarotta/ontologies/2022/4/silvanusOntology#Interest"/>
            <rdf:Description rdf:about="http://www.semanticweb.org/smarotta/ontologies/2022/4/silvanusOntology#Vandalism"/>
        </owl:members>
    </rdf:Description>
    <rdf:Description>
        <rdf:type rdf:resource="http://www.w3.org/2002/07/owl#AllDisjointClasses"/>
        <owl:members rdf:parseType="Collection">
            <rdf:Description rdf:about="http://www.semanticweb.org/smarotta/ontologies/2022/4/silvanusOntology#Dense_Settlement_Biome"/>
            <rdf:Description rdf:about="http://www.semanticweb.org/smarotta/ontologies/2022/4/silvanusOntology#Rangeland_Biome"/>
            <rdf:Description rdf:about="http://www.semanticweb.org/smarotta/ontologies/2022/4/silvanusOntology#Village_Biome"/>
        </owl:members>
    </rdf:Description>
    <rdf:Description>
        <rdf:type rdf:resource="http://www.w3.org/2002/07/owl#AllDisjointClasses"/>
        <owl:members rdf:parseType="Collection">
            <rdf:Description rdf:about="http://www.semanticweb.org/smarotta/ontologies/2022/4/silvanusOntology#Ecological_asset"/>
            <rdf:Description rdf:about="http://www.semanticweb.org/smarotta/ontologies/2022/4/silvanusOntology#Infrastructure"/>
            <rdf:Description rdf:about="http://www.semanticweb.org/smarotta/ontologies/2022/4/silvanusOntology#Property"/>
        </owl:members>
    </rdf:Description>
    <rdf:Description>
        <rdf:type rdf:resource="http://www.w3.org/2002/07/owl#AllDisjointClasses"/>
        <owl:members rdf:parseType="Collection">
            <rdf:Description rdf:about="http://www.semanticweb.org/smarotta/ontologies/2022/4/silvanusOntology#Ecological_asset"/>
            <rdf:Description rdf:about="http://www.semanticweb.org/smarotta/ontologies/2022/4/silvanusOntology#Infrastructure"/>
            <rdf:Description rdf:about="http://www.semanticweb.org/smarotta/ontologies/2022/4/silvanusOntology#Property"/>
            <rdf:Description rdf:about="http://www.semanticweb.org/smarotta/ontologies/2022/4/silvanusOntology#Structure"/>
        </owl:members>
    </rdf:Description>
    <rdf:Description>
        <rdf:type rdf:resource="http://www.w3.org/2002/07/owl#AllDisjointClasses"/>
        <owl:members rdf:parseType="Collection">
            <rdf:Description rdf:about="http://www.semanticweb.org/smarotta/ontologies/2022/4/silvanusOntology#Electrical_power"/>
            <rdf:Description rdf:about="http://www.semanticweb.org/smarotta/ontologies/2022/4/silvanusOntology#Other_accident"/>
            <rdf:Description rdf:about="http://www.semanticweb.org/smarotta/ontologies/2022/4/silvanusOntology#Railroads"/>
            <rdf:Description rdf:about="http://www.semanticweb.org/smarotta/ontologies/2022/4/silvanusOntology#Self-ignition"/>
            <rdf:Description rdf:about="http://www.semanticweb.org/smarotta/ontologies/2022/4/silvanusOntology#Vehicles"/>
            <rdf:Description rdf:about="http://www.semanticweb.org/smarotta/ontologies/2022/4/silvanusOntology#Weapons"/>
            <rdf:Description rdf:about="http://www.semanticweb.org/smarotta/ontologies/2022/4/silvanusOntology#Works"/>
        </owl:members>
    </rdf:Description>
    <rdf:Description>
        <rdf:type rdf:resource="http://www.w3.org/2002/07/owl#AllDisjointClasses"/>
        <owl:members rdf:parseType="Collection">
            <rdf:Description rdf:about="http://www.semanticweb.org/smarotta/ontologies/2022/4/silvanusOntology#Firefighting_unit"/>
            <rdf:Description rdf:about="http://www.semanticweb.org/smarotta/ontologies/2022/4/silvanusOntology#IncidentCommander"/>
            <rdf:Description rdf:about="http://www.semanticweb.org/smarotta/ontologies/2022/4/silvanusOntology#LogisticChief"/>
            <rdf:Description rdf:about="http://www.semanticweb.org/smarotta/ontologies/2022/4/silvanusOntology#MedicalPlanningLeader"/>
            <rdf:Description rdf:about="http://www.semanticweb.org/smarotta/ontologies/2022/4/silvanusOntology#OperationChief"/>
            <rdf:Description rdf:about="http://www.semanticweb.org/smarotta/ontologies/2022/4/silvanusOntology#Patrol"/>
            <rdf:Description rdf:about="http://www.semanticweb.org/smarotta/ontologies/2022/4/silvanusOntology#PlanningChief"/>
            <rdf:Description rdf:about="http://www.semanticweb.org/smarotta/ontologies/2022/4/silvanusOntology#PublicInfoOfficer"/>
            <rdf:Description rdf:about="http://www.semanticweb.org/smarotta/ontologies/2022/4/silvanusOntology#ResourceUnitLeader"/>
            <rdf:Description rdf:about="http://www.semanticweb.org/smarotta/ontologies/2022/4/silvanusOntology#SafetyOfficer"/>
            <rdf:Description rdf:about="http://www.semanticweb.org/smarotta/ontologies/2022/4/silvanusOntology#SupplyLeader"/>
            <rdf:Description rdf:about="http://www.semanticweb.org/smarotta/ontologies/2022/4/silvanusOntology#TaskForceSectorLeader"/>
        </owl:members>
    </rdf:Description>
    <rdf:Description>
        <rdf:type rdf:resource="http://www.w3.org/2002/07/owl#AllDisjointClasses"/>
        <owl:members rdf:parseType="Collection">
            <rdf:Description rdf:about="http://www.semanticweb.org/smarotta/ontologies/2022/4/silvanusOntology#Gas_emission"/>
            <rdf:Description rdf:about="http://www.semanticweb.org/smarotta/ontologies/2022/4/silvanusOntology#Lightning"/>
            <rdf:Description rdf:about="http://www.semanticweb.org/smarotta/ontologies/2022/4/silvanusOntology#Volcanism"/>
        </owl:members>
    </rdf:Description>
    <rdf:Description>
        <rdf:type rdf:resource="http://www.w3.org/2002/07/owl#AllDisjointClasses"/>
        <owl:members rdf:parseType="Collection">
            <rdf:Description rdf:about="http://www.semanticweb.org/smarotta/ontologies/2022/4/silvanusOntology#Measurable_Entity_in_Centimeters"/>
            <rdf:Description rdf:about="http://www.semanticweb.org/smarotta/ontologies/2022/4/silvanusOntology#Measurable_Entity_in_Decimeters"/>
            <rdf:Description rdf:about="http://www.semanticweb.org/smarotta/ontologies/2022/4/silvanusOntology#Measurable_Entity_in_Degrees"/>
            <rdf:Description rdf:about="http://www.semanticweb.org/smarotta/ontologies/2022/4/silvanusOntology#Measurable_Entity_in_Gradians"/>
            <rdf:Description rdf:about="http://www.semanticweb.org/smarotta/ontologies/2022/4/silvanusOntology#Measurable_Entity_in_Hectares"/>
            <rdf:Description rdf:about="http://www.semanticweb.org/smarotta/ontologies/2022/4/silvanusOntology#Measurable_Entity_in_Meters"/>
            <rdf:Description rdf:about="http://www.semanticweb.org/smarotta/ontologies/2022/4/silvanusOntology#Measurable_Entity_in_Millimeters"/>
            <rdf:Description rdf:about="http://www.semanticweb.org/smarotta/ontologies/2022/4/silvanusOntology#Measurable_Entity_in_Square_Meters"/>
            <rdf:Description rdf:about="http://www.semanticweb.org/smarotta/ontologies/2022/4/silvanusOntology#Measurable_Entity_in_Years"/>
        </owl:members>
    </rdf:Description>
    <rdf:Description>
        <rdf:type rdf:resource="http://www.w3.org/2002/07/owl#AllDisjointClasses"/>
        <owl:members rdf:parseType="Collection">
            <rdf:Description rdf:about="http://www.semanticweb.org/smarotta/ontologies/2022/4/silvanusOntology#MedicalItem"/>
            <rdf:Description rdf:about="http://www.semanticweb.org/smarotta/ontologies/2022/4/silvanusOntology#ReliefItem"/>
            <rdf:Description rdf:about="http://www.semanticweb.org/smarotta/ontologies/2022/4/silvanusOntology#SupplyGood"/>
        </owl:members>
    </rdf:Description>
    <rdf:Description>
        <rdf:type rdf:resource="http://www.w3.org/2002/07/owl#AllDisjointClasses"/>
        <owl:members rdf:parseType="Collection">
            <rdf:Description rdf:about="http://www.semanticweb.org/smarotta/ontologies/2022/4/silvanusOntology#Mediterranean_Savanna_Biome"/>
            <rdf:Description rdf:about="http://www.semanticweb.org/smarotta/ontologies/2022/4/silvanusOntology#Mediterranean_Sea_Biome"/>
            <rdf:Description rdf:about="http://www.semanticweb.org/smarotta/ontologies/2022/4/silvanusOntology#Mediterranean_Shrubland_Biome"/>
            <rdf:Description rdf:about="http://www.semanticweb.org/smarotta/ontologies/2022/4/silvanusOntology#Mediterranean_Woodland_Biome"/>
        </owl:members>
    </rdf:Description>
    <rdf:Description>
        <rdf:type rdf:resource="http://www.w3.org/2002/07/owl#AllDisjointClasses"/>
        <owl:members rdf:parseType="Collection">
            <rdf:Description rdf:about="http://www.semanticweb.org/smarotta/ontologies/2022/4/silvanusOntology#Montane_Shrubland_Biome"/>
            <rdf:Description rdf:about="http://www.semanticweb.org/smarotta/ontologies/2022/4/silvanusOntology#Subtropical_Shrubland_Biome"/>
            <rdf:Description rdf:about="http://www.semanticweb.org/smarotta/ontologies/2022/4/silvanusOntology#Temperate_Shrubland_Biome"/>
            <rdf:Description rdf:about="http://www.semanticweb.org/smarotta/ontologies/2022/4/silvanusOntology#Tidal_Mangrove_Shrubland"/>
            <rdf:Description rdf:about="http://www.semanticweb.org/smarotta/ontologies/2022/4/silvanusOntology#Tropical_Shrubland_Biome"/>
            <rdf:Description rdf:about="http://www.semanticweb.org/smarotta/ontologies/2022/4/silvanusOntology#Xeric_Shrubland_Biome"/>
        </owl:members>
    </rdf:Description>
    <rdf:Description>
        <rdf:type rdf:resource="http://www.w3.org/2002/07/owl#AllDisjointClasses"/>
        <owl:members rdf:parseType="Collection">
            <rdf:Description rdf:about="http://www.semanticweb.org/smarotta/ontologies/2022/4/silvanusOntology#Tropical_Marginal_Sea_Biome"/>
            <rdf:Description rdf:about="http://www.semanticweb.org/smarotta/ontologies/2022/4/silvanusOntology#Tropical_Marine_Coral_Reef_Biome"/>
            <rdf:Description rdf:about="http://www.semanticweb.org/smarotta/ontologies/2022/4/silvanusOntology#Tropical_Marine_Upwelling_Biome"/>
            <rdf:Description rdf:about="http://www.semanticweb.org/smarotta/ontologies/2022/4/silvanusOntology#Tropical_Savanna_Biome"/>
            <rdf:Description rdf:about="http://www.semanticweb.org/smarotta/ontologies/2022/4/silvanusOntology#Tropical_Shrubland_Biome"/>
            <rdf:Description rdf:about="http://www.semanticweb.org/smarotta/ontologies/2022/4/silvanusOntology#Tropical_Woodland_Biome"/>
        </owl:members>
    </rdf:Description>
</rdf:RDF>



<!-- Generated by the OWL API (version 4.5.9.2019-02-01T07:24:44Z) https://github.com/owlcs/owlapi -->

